<?xml version="1.0"?>
<rdf:RDF xmlns="http://www.wageneder.at/ontology/bpmn2.0"
     xml:base="http://www.wageneder.at/ontology/bpmn2.0"
     xmlns:rdf="http://www.w3.org/1999/02/22-rdf-syntax-ns#"
     xmlns:owl="http://www.w3.org/2002/07/owl#"
     xmlns:xml="http://www.w3.org/XML/1998/namespace"
     xmlns:xsd="http://www.w3.org/2001/XMLSchema#"
     xmlns:rdfs="http://www.w3.org/2000/01/rdf-schema#"
     xmlns:bpmn2="http://www.wageneder.at/ontology/bpmn2.0#"
     xmlns:dc="http://purl.org/dc/elements/1.1/">
    <owl:Ontology rdf:about="http://www.wageneder.at/ontology/bpmn2.0">
        <bpmn2:developer rdf:datatype="http://www.w3.org/2001/XMLSchema#string">Fortmüller Vanessa, Hribernig Nikolaus, Plank Patrick, Stangl Michaela</bpmn2:developer>
        <rdfs:comment rdf:datatype="http://www.w3.org/2001/XMLSchema#string">BPMN 2.0 Ontology

created as part of the 2nd Bachelor Thesis &quot;Ontological Analysis of BPMN 2.0&quot; at the Bachelor Degree Course &quot;Information Management&quot; at the University of Applied Sciences in Graz, Austria.</rdfs:comment>
        <dc:creator rdf:datatype="http://www.w3.org/2001/XMLSchema#string">Maximilian Wageneder</dc:creator>
    </owl:Ontology>
    


    <!-- 
    ///////////////////////////////////////////////////////////////////////////////////////
    //
    // Annotation properties
    //
    ///////////////////////////////////////////////////////////////////////////////////////
     -->

    


    <!-- http://purl.org/dc/elements/1.1/creator -->

    <owl:AnnotationProperty rdf:about="http://purl.org/dc/elements/1.1/creator"/>
    


    <!-- http://www.wageneder.at/ontology/bpmn2.0#developer -->

    <owl:AnnotationProperty rdf:about="http://www.wageneder.at/ontology/bpmn2.0#developer"/>
    


    <!-- 
    ///////////////////////////////////////////////////////////////////////////////////////
    //
    // Object Properties
    //
    ///////////////////////////////////////////////////////////////////////////////////////
     -->

    


    <!-- http://www.w3.org/2002/07/owl#topObjectProperty -->

    <rdf:Description rdf:about="http://www.w3.org/2002/07/owl#topObjectProperty">
        <rdfs:comment>Specifies an optional transformation Expression. The actual scope of accessible data for that Expression is defined by the source and target of the specific Data Association types.</rdfs:comment>
    </rdf:Description>
    


    <!-- http://www.wageneder.at/ontology/bpmn2.0#hasActivationCondition -->

    <owl:ObjectProperty rdf:about="http://www.wageneder.at/ontology/bpmn2.0#hasActivationCondition">
        <rdfs:comment>Determines which combination of incoming tokens will be synchronized for activation of the Gateway.</rdfs:comment>
    </owl:ObjectProperty>
    


    <!-- http://www.wageneder.at/ontology/bpmn2.0#hasActivity -->

    <owl:ObjectProperty rdf:about="http://www.wageneder.at/ontology/bpmn2.0#hasActivity"/>
    


    <!-- http://www.wageneder.at/ontology/bpmn2.0#hasActivityRef -->

    <owl:ObjectProperty rdf:about="http://www.wageneder.at/ontology/bpmn2.0#hasActivityRef">
        <rdfs:comment>For a Start Event:
This Event “catches” the compensation for an Event Sub-Process. No further
information is REQUIRED. The Event Sub-Process will provide the Id necessary
to match the Compensation Event with the Event that threw the compensation,
or the compensation will have been a broadcast.
For an End Event:
The Activity to be compensated MAY be supplied. If an Activity is not supplied,
then the compensation is broadcast to all completed Activities in the current Sub-
Process (if present), or the entire Process instance (if at the global level).
For an Intermediate Event within normal flow:
The Activity to be compensated MAY be supplied. If an Activity is not supplied,
then the compensation is broadcast to all completed Activities in the current Sub-
Process (if present), or the entire Process instance (if at the global level). This
“throws” the compensation.
For an Intermediate Event attached to the boundary of an Activity:
This Event “catches” the compensation. No further information is REQUIRED. The
Activity the Event is attached to will provide the Id necessary to match the
Compensation Event with the Event that threw the compensation, or the
compensation will have been a broadcast.</rdfs:comment>
    </owl:ObjectProperty>
    


    <!-- http://www.wageneder.at/ontology/bpmn2.0#hasArtifact -->

    <owl:ObjectProperty rdf:about="http://www.wageneder.at/ontology/bpmn2.0#hasArtifact"/>
    


    <!-- http://www.wageneder.at/ontology/bpmn2.0#hasArtifacts -->

    <owl:ObjectProperty rdf:about="http://www.wageneder.at/ontology/bpmn2.0#hasArtifacts">
        <rdfs:comment>This attribute provides the list of Artifacts that are contained within the Collaboration.</rdfs:comment>
    </owl:ObjectProperty>
    


    <!-- http://www.wageneder.at/ontology/bpmn2.0#hasAssignment -->

    <owl:ObjectProperty rdf:about="http://www.wageneder.at/ontology/bpmn2.0#hasAssignment">
        <rdfs:subPropertyOf rdf:resource="http://www.w3.org/2002/07/owl#topObjectProperty"/>
        <rdfs:comment>Specifies one or more data elements Assignments. By using an Assignment, single data structure elements can be assigned from the source structure to the target structure.</rdfs:comment>
    </owl:ObjectProperty>
    


    <!-- http://www.wageneder.at/ontology/bpmn2.0#hasAssociationDirection -->

    <owl:ObjectProperty rdf:about="http://www.wageneder.at/ontology/bpmn2.0#hasAssociationDirection">
        <rdfs:comment>associationDirection is an attribute that defines whether or not the Association shows any directionality with an arrowhead. The default is None (no arrowhead). A value of One means that the arrowhead SHALL be at the Target Object. A value of Both means that there SHALL be an arrowhead at both ends of the Association line.</rdfs:comment>
    </owl:ObjectProperty>
    


    <!-- http://www.wageneder.at/ontology/bpmn2.0#hasAttachedToRef -->

    <owl:ObjectProperty rdf:about="http://www.wageneder.at/ontology/bpmn2.0#hasAttachedToRef"/>
    


    <!-- http://www.wageneder.at/ontology/bpmn2.0#hasAuditing -->

    <owl:ObjectProperty rdf:about="http://www.wageneder.at/ontology/bpmn2.0#hasAuditing">
        <rdfs:subPropertyOf rdf:resource="http://www.w3.org/2002/07/owl#topObjectProperty"/>
        <rdfs:comment>A hook for specifying audit related properties. Auditing can only be defined for a Process.</rdfs:comment>
    </owl:ObjectProperty>
    


    <!-- http://www.wageneder.at/ontology/bpmn2.0#hasBehaviour -->

    <owl:ObjectProperty rdf:about="http://www.wageneder.at/ontology/bpmn2.0#hasBehaviour">
        <rdfs:comment>The attribute behavior acts as a shortcut for specifying when events
SHALL be thrown from an Activity instance that is about to complete. It
can assume values of None, One, All, and Complex, resulting in the
following behavior:
• None: the EventDefinition which is associated through the
noneEvent association will be thrown for each instance completing.
• One: the EventDefinition referenced through the oneEvent
association will be thrown upon the first instance completing.
• All: no Event is ever thrown; a token is produced after completion of all
instances.
• Complex: the complexBehaviorDefinitions are consulted to
determine if and which Events to throw.
For the behaviors of none and one, a default SignalEventDefinition
will be thrown which automatically carries the current runtime
attributes of the MI Activity.
Any thrown Events can be caught by boundary Events on the Multi-
Instance Activity.</rdfs:comment>
    </owl:ObjectProperty>
    


    <!-- http://www.wageneder.at/ontology/bpmn2.0#hasBody -->

    <owl:ObjectProperty rdf:about="http://www.wageneder.at/ontology/bpmn2.0#hasBody">
        <rdfs:subPropertyOf rdf:resource="http://www.w3.org/2002/07/owl#topObjectProperty"/>
        <rdfs:comment>The body of the Expression.
Note that this attribute is not relevant when the XML Schema is used for interchange. Instead, the FormalExpression complex type supports mixed content. The body of the Expression would be specified as element content. 

For example:

&lt;formalExpression id=“ID_2&quot;&gt;
   count(../dataObject[id=&quot;CustomerRecord_1&quot;]/emailAddress) &gt; 0
   &lt;evaluatesToType id=&quot;ID_3&quot; typeRef=“xsd:boolean&quot;/&gt;
&lt;/formalExpression&gt;</rdfs:comment>
    </owl:ObjectProperty>
    


    <!-- http://www.wageneder.at/ontology/bpmn2.0#hasBoundaryEventRefs -->

    <owl:ObjectProperty rdf:about="http://www.wageneder.at/ontology/bpmn2.0#hasBoundaryEventRefs">
        <rdfs:comment>This references the Intermediate Events that are attached to the boundary of the Activity.</rdfs:comment>
    </owl:ObjectProperty>
    


    <!-- http://www.wageneder.at/ontology/bpmn2.0#hasCallConversation -->

    <owl:ObjectProperty rdf:about="http://www.wageneder.at/ontology/bpmn2.0#hasCallConversation"/>
    


    <!-- http://www.wageneder.at/ontology/bpmn2.0#hasCallableElements -->

    <owl:ObjectProperty rdf:about="http://www.wageneder.at/ontology/bpmn2.0#hasCallableElements">
        <rdfs:comment>The CallableElements that use this Interface.</rdfs:comment>
    </owl:ObjectProperty>
    


    <!-- http://www.wageneder.at/ontology/bpmn2.0#hasCalledCollaborationRef -->

    <owl:ObjectProperty rdf:about="http://www.wageneder.at/ontology/bpmn2.0#hasCalledCollaborationRef">
        <rdfs:comment>The element to be called, which MAY be either a Collaboration or a GlobalConversation. The called element MUST NOT be a Choreography or a GlobalChoreographyTask (which are subtypes of Collaboration)</rdfs:comment>
    </owl:ObjectProperty>
    


    <!-- http://www.wageneder.at/ontology/bpmn2.0#hasCalledElement -->

    <owl:ObjectProperty rdf:about="http://www.wageneder.at/ontology/bpmn2.0#hasCalledElement">
        <rdfs:comment>The element to be called, which will be either a Process or a GlobalTask. Other CallableElements, such as Choreography, GlobalChoreographyTask, Conversation, and GlobalCommunication MUST NOT be called by the Call Conversation element.</rdfs:comment>
    </owl:ObjectProperty>
    


    <!-- http://www.wageneder.at/ontology/bpmn2.0#hasCategorizedFlowElements -->

    <owl:ObjectProperty rdf:about="http://www.wageneder.at/ontology/bpmn2.0#hasCategorizedFlowElements">
        <rdfs:subPropertyOf rdf:resource="http://www.w3.org/2002/07/owl#topObjectProperty"/>
        <rdfs:comment>The FlowElements attribute identifies all of the elements (e.g., Events, Activities, Gateways, and Artifacts) that are within the boundaries of the Group.</rdfs:comment>
    </owl:ObjectProperty>
    


    <!-- http://www.wageneder.at/ontology/bpmn2.0#hasCategory -->

    <owl:ObjectProperty rdf:about="http://www.wageneder.at/ontology/bpmn2.0#hasCategory">
        <rdfs:subPropertyOf rdf:resource="http://www.w3.org/2002/07/owl#topObjectProperty"/>
        <rdfs:comment>The category attribute specifies the Category representing the Category as such and contains the CategoryValue (Further details about the definition of a Category can be found on page 70).</rdfs:comment>
    </owl:ObjectProperty>
    


    <!-- http://www.wageneder.at/ontology/bpmn2.0#hasCategoryValue -->

    <owl:ObjectProperty rdf:about="http://www.wageneder.at/ontology/bpmn2.0#hasCategoryValue">
        <rdfs:subPropertyOf rdf:resource="http://www.w3.org/2002/07/owl#topObjectProperty"/>
        <rdfs:comment>The categoryValue attribute specifies one or more values of the Category. For example, the Category is “Region” then this Category could specify values like “North,” “South,” “West,” and “East.”</rdfs:comment>
    </owl:ObjectProperty>
    


    <!-- http://www.wageneder.at/ontology/bpmn2.0#hasCategoryValueRef -->

    <owl:ObjectProperty rdf:about="http://www.wageneder.at/ontology/bpmn2.0#hasCategoryValueRef">
        <rdfs:comment>The categoryValueRef attribute specifies the CategoryValue that the Group represents. (Further details about the definition of a Category and CategoryValue can be found on page 70.) The name of the Category and the value of the CategoryValue separated by delineator &quot;.&quot; provides the label for the Group. The graphical elements within the boundaries of the Group will be assigned the CategoryValue.</rdfs:comment>
    </owl:ObjectProperty>
    


    <!-- http://www.wageneder.at/ontology/bpmn2.0#hasChildLaneSet -->

    <owl:ObjectProperty rdf:about="http://www.wageneder.at/ontology/bpmn2.0#hasChildLaneSet">
        <rdfs:comment>A reference to a LaneSet element for embedded Lanes.</rdfs:comment>
    </owl:ObjectProperty>
    


    <!-- http://www.wageneder.at/ontology/bpmn2.0#hasChoreographyRef -->

    <owl:ObjectProperty rdf:about="http://www.wageneder.at/ontology/bpmn2.0#hasChoreographyRef">
        <rdfs:comment>The choreographyRef model association defines the Choreographies that
can be shown between the Pools of the Collaboration.</rdfs:comment>
    </owl:ObjectProperty>
    


    <!-- http://www.wageneder.at/ontology/bpmn2.0#hasCollaboration -->

    <owl:ObjectProperty rdf:about="http://www.wageneder.at/ontology/bpmn2.0#hasCollaboration"/>
    


    <!-- http://www.wageneder.at/ontology/bpmn2.0#hasCompletionCondition -->

    <owl:ObjectProperty rdf:about="http://www.wageneder.at/ontology/bpmn2.0#hasCompletionCondition">
        <rdfs:comment>This attribute defines a boolean Expression that when evaluated to true, cancels the remaining Activity instances and produces a token.</rdfs:comment>
    </owl:ObjectProperty>
    


    <!-- http://www.wageneder.at/ontology/bpmn2.0#hasComplexBehaviourDefinition -->

    <owl:ObjectProperty rdf:about="http://www.wageneder.at/ontology/bpmn2.0#hasComplexBehaviourDefinition">
        <rdfs:comment>Controls when and which Events are thrown in case behavior is set to complex.</rdfs:comment>
    </owl:ObjectProperty>
    


    <!-- http://www.wageneder.at/ontology/bpmn2.0#hasComplexGateway -->

    <owl:ObjectProperty rdf:about="http://www.wageneder.at/ontology/bpmn2.0#hasComplexGateway"/>
    


    <!-- http://www.wageneder.at/ontology/bpmn2.0#hasCondition -->

    <owl:ObjectProperty rdf:about="http://www.wageneder.at/ontology/bpmn2.0#hasCondition">
        <rdfs:comment>This attribute defines a boolean Expression that when evaluated to true, cancels the remaining Activity instances and produces a token.</rdfs:comment>
    </owl:ObjectProperty>
    


    <!-- http://www.wageneder.at/ontology/bpmn2.0#hasConditionExpression -->

    <owl:ObjectProperty rdf:about="http://www.wageneder.at/ontology/bpmn2.0#hasConditionExpression">
        <rdfs:comment>An optional boolean Expression that acts as a gating condition. A token will only be placed on this Sequence Flow if this conditionExpression evaluates to true.</rdfs:comment>
    </owl:ObjectProperty>
    


    <!-- http://www.wageneder.at/ontology/bpmn2.0#hasContainer -->

    <owl:ObjectProperty rdf:about="http://www.wageneder.at/ontology/bpmn2.0#hasContainer"/>
    


    <!-- http://www.wageneder.at/ontology/bpmn2.0#hasConversationAssociation -->

    <owl:ObjectProperty rdf:about="http://www.wageneder.at/ontology/bpmn2.0#hasConversationAssociation"/>
    


    <!-- http://www.wageneder.at/ontology/bpmn2.0#hasConversationAssociations -->

    <owl:ObjectProperty rdf:about="http://www.wageneder.at/ontology/bpmn2.0#hasConversationAssociations">
        <rdfs:comment>This attribute provides a list of mappings from the Conversations of a referenced Collaboration to the Conversations of another Collaboration.
It is used when:
• When a Choreography is referenced by a Collaboration.</rdfs:comment>
    </owl:ObjectProperty>
    


    <!-- http://www.wageneder.at/ontology/bpmn2.0#hasConversationLinks -->

    <owl:ObjectProperty rdf:about="http://www.wageneder.at/ontology/bpmn2.0#hasConversationLinks">
        <rdfs:comment>This provides the Conversation Links that are used in the Collaboration.</rdfs:comment>
    </owl:ObjectProperty>
    


    <!-- http://www.wageneder.at/ontology/bpmn2.0#hasConversationNode -->

    <owl:ObjectProperty rdf:about="http://www.wageneder.at/ontology/bpmn2.0#hasConversationNode"/>
    


    <!-- http://www.wageneder.at/ontology/bpmn2.0#hasConversationNodes -->

    <owl:ObjectProperty rdf:about="http://www.wageneder.at/ontology/bpmn2.0#hasConversationNodes">
        <rdfs:comment>The ConversationNodes model aggregation relationship allows a Sub- Conversation to contain other ConversationNodes, in order to group Message Flows of the Sub-Conversation and associate correlation information.</rdfs:comment>
    </owl:ObjectProperty>
    


    <!-- http://www.wageneder.at/ontology/bpmn2.0#hasConversations -->

    <owl:ObjectProperty rdf:about="http://www.wageneder.at/ontology/bpmn2.0#hasConversations">
        <rdfs:comment>The conversations model aggregation relationship allows a Collaboration to contain Conversation elements, in order to group Message Flows of the Collaboration and associate correlation information, as is REQUIRED for the definitional Collaboration of a Process model. The Conversation elements will be visualized if the Collaboration is a Collaboration, but not for a Choreography.</rdfs:comment>
    </owl:ObjectProperty>
    


    <!-- http://www.wageneder.at/ontology/bpmn2.0#hasCorrelationKeyRef -->

    <owl:ObjectProperty rdf:about="http://www.wageneder.at/ontology/bpmn2.0#hasCorrelationKeyRef">
        <rdfs:comment>The CorrelationKey this CorrelationSubscription refers to.</rdfs:comment>
    </owl:ObjectProperty>
    


    <!-- http://www.wageneder.at/ontology/bpmn2.0#hasCorrelationKeys -->

    <owl:ObjectProperty rdf:about="http://www.wageneder.at/ontology/bpmn2.0#hasCorrelationKeys">
        <rdfs:comment>This is a list of the ConversationNode’s CorrelationKeys, which are used to
group Message Flows for the ConversationNode</rdfs:comment>
    </owl:ObjectProperty>
    


    <!-- http://www.wageneder.at/ontology/bpmn2.0#hasCorrelationProperty -->

    <owl:ObjectProperty rdf:about="http://www.wageneder.at/ontology/bpmn2.0#hasCorrelationProperty"/>
    


    <!-- http://www.wageneder.at/ontology/bpmn2.0#hasCorrelationPropertyBinding -->

    <owl:ObjectProperty rdf:about="http://www.wageneder.at/ontology/bpmn2.0#hasCorrelationPropertyBinding">
        <rdfs:comment>The bindings to specific CorrelationProperties and FormalExpressions (extraction rules atop the Process context).</rdfs:comment>
    </owl:ObjectProperty>
    


    <!-- http://www.wageneder.at/ontology/bpmn2.0#hasCorrelationPropertyRef -->

    <owl:ObjectProperty rdf:about="http://www.wageneder.at/ontology/bpmn2.0#hasCorrelationPropertyRef">
        <rdfs:comment>The CorrelationProperties, representing the partial keys of this
CorrelationKey.</rdfs:comment>
    </owl:ObjectProperty>
    


    <!-- http://www.wageneder.at/ontology/bpmn2.0#hasCorrelationPropertyRetrievalExpression -->

    <owl:ObjectProperty rdf:about="http://www.wageneder.at/ontology/bpmn2.0#hasCorrelationPropertyRetrievalExpression">
        <rdfs:comment>The CorrelationPropertyRetrievalExpressions for this CorrelationProperty, representing the associations of FormalExpressions (extraction paths) to specific Messages occurring in this Conversation.</rdfs:comment>
    </owl:ObjectProperty>
    


    <!-- http://www.wageneder.at/ontology/bpmn2.0#hasCorrelationSet -->

    <owl:ObjectProperty rdf:about="http://www.wageneder.at/ontology/bpmn2.0#hasCorrelationSet"/>
    


    <!-- http://www.wageneder.at/ontology/bpmn2.0#hasCorrelationSubscriptions -->

    <owl:ObjectProperty rdf:about="http://www.wageneder.at/ontology/bpmn2.0#hasCorrelationSubscriptions">
        <rdfs:comment>correlationSubscriptions are a feature of context-based correlation
(cf. sub clause 8.3.3). CorrelationSubscriptions are used to correlate incoming Messages against data in the Process context. A Process MAY contain several correlationSubscriptions.</rdfs:comment>
    </owl:ObjectProperty>
    


    <!-- http://www.wageneder.at/ontology/bpmn2.0#hasDataInputAssociations -->

    <owl:ObjectProperty rdf:about="http://www.wageneder.at/ontology/bpmn2.0#hasDataInputAssociations">
        <rdfs:comment>An optional reference to the DataInputAssociations. A DataInputAssociation defines how the DataInput of the Activity’s InputOutputSpecification will be populated.</rdfs:comment>
    </owl:ObjectProperty>
    


    <!-- http://www.wageneder.at/ontology/bpmn2.0#hasDataInputRefs -->

    <owl:ObjectProperty rdf:about="http://www.wageneder.at/ontology/bpmn2.0#hasDataInputRefs">
        <rdfs:comment>The DataInput elements that collectively make up this data requirement.</rdfs:comment>
    </owl:ObjectProperty>
    


    <!-- http://www.wageneder.at/ontology/bpmn2.0#hasDataInputs -->

    <owl:ObjectProperty rdf:about="http://www.wageneder.at/ontology/bpmn2.0#hasDataInputs">
        <rdfs:comment>The Data Inputs for the throw Event. This is an ordered set.</rdfs:comment>
    </owl:ObjectProperty>
    


    <!-- http://www.wageneder.at/ontology/bpmn2.0#hasDataObjectRef -->

    <owl:ObjectProperty rdf:about="http://www.wageneder.at/ontology/bpmn2.0#hasDataObjectRef">
        <rdfs:comment>The Data Object referenced by the Data Object Reference.</rdfs:comment>
    </owl:ObjectProperty>
    


    <!-- http://www.wageneder.at/ontology/bpmn2.0#hasDataOutputAssociations -->

    <owl:ObjectProperty rdf:about="http://www.wageneder.at/ontology/bpmn2.0#hasDataOutputAssociations">
        <rdfs:comment>An optional reference to the DataOutputAssociations.</rdfs:comment>
    </owl:ObjectProperty>
    


    <!-- http://www.wageneder.at/ontology/bpmn2.0#hasDataOutputRefs -->

    <owl:ObjectProperty rdf:about="http://www.wageneder.at/ontology/bpmn2.0#hasDataOutputRefs">
        <rdfs:comment>The DataOutput elements that MAY collectively be outputted.</rdfs:comment>
    </owl:ObjectProperty>
    


    <!-- http://www.wageneder.at/ontology/bpmn2.0#hasDataOutputs -->

    <owl:ObjectProperty rdf:about="http://www.wageneder.at/ontology/bpmn2.0#hasDataOutputs">
        <rdfs:comment>The Data Outputs for the catch Event. This is an ordered set.</rdfs:comment>
    </owl:ObjectProperty>
    


    <!-- http://www.wageneder.at/ontology/bpmn2.0#hasDataPath -->

    <owl:ObjectProperty rdf:about="http://www.wageneder.at/ontology/bpmn2.0#hasDataPath">
        <rdfs:comment>The FormalExpression that defines the extraction rule atop the Process context.</rdfs:comment>
    </owl:ObjectProperty>
    


    <!-- http://www.wageneder.at/ontology/bpmn2.0#hasDataState -->

    <owl:ObjectProperty rdf:about="http://www.wageneder.at/ontology/bpmn2.0#hasDataState">
        <rdfs:comment>A reference to the DataState, which defines certain states for the data contained in the Item.</rdfs:comment>
    </owl:ObjectProperty>
    


    <!-- http://www.wageneder.at/ontology/bpmn2.0#hasDataStoreRef -->

    <owl:ObjectProperty rdf:about="http://www.wageneder.at/ontology/bpmn2.0#hasDataStoreRef">
        <rdfs:comment>Provides the reference to a global DataStore.</rdfs:comment>
    </owl:ObjectProperty>
    


    <!-- http://www.wageneder.at/ontology/bpmn2.0#hasDefault -->

    <owl:ObjectProperty rdf:about="http://www.wageneder.at/ontology/bpmn2.0#hasDefault">
        <rdfs:comment>The Sequence Flow that will receive a token when none of the conditionExpressions on other outgoing Sequence Flows evalu- ate to true. The default Sequence Flow should not have a conditionExpression. Any such Expression SHALL be ignored.</rdfs:comment>
    </owl:ObjectProperty>
    


    <!-- http://www.wageneder.at/ontology/bpmn2.0#hasDefinition -->

    <owl:ObjectProperty rdf:about="http://www.wageneder.at/ontology/bpmn2.0#hasDefinition">
        <rdfs:subPropertyOf rdf:resource="http://www.w3.org/2002/07/owl#topObjectProperty"/>
        <rdfs:domain rdf:resource="http://www.wageneder.at/ontology/bpmn2.0#Extension"/>
        <rdfs:comment>Defines the content of the extension.
Note that in the XML schema, this definition is provided by an external XML schema file and is simply referenced by QName.</rdfs:comment>
    </owl:ObjectProperty>
    


    <!-- http://www.wageneder.at/ontology/bpmn2.0#hasDefinitionalCollaborationRef -->

    <owl:ObjectProperty rdf:about="http://www.wageneder.at/ontology/bpmn2.0#hasDefinitionalCollaborationRef">
        <rdfs:comment>For Processes that interact with other Participants, a definitional Collaboration can be referenced by the Process. The definitional Collaboration specifies the Participants the Process interacts with, and more specifically, which individual service, Send or Receive Task, or Message Event, is connected to which Participant through Message Flows. The definitional Collaboration need not be displayed.
Additionally, the definitional Collaboration can be used to include Conversation information within a Process.</rdfs:comment>
    </owl:ObjectProperty>
    


    <!-- http://www.wageneder.at/ontology/bpmn2.0#hasDiagrams -->

    <owl:ObjectProperty rdf:about="http://www.wageneder.at/ontology/bpmn2.0#hasDiagrams">
        <rdfs:subPropertyOf rdf:resource="http://www.w3.org/2002/07/owl#topObjectProperty"/>
        <rdfs:comment>This attribute lists the BPMNDiagrams that are contained within this Definitions (see page 367 for more information on BPMNDiagrams).</rdfs:comment>
    </owl:ObjectProperty>
    


    <!-- http://www.wageneder.at/ontology/bpmn2.0#hasDirection -->

    <owl:ObjectProperty rdf:about="http://www.wageneder.at/ontology/bpmn2.0#hasDirection">
        <rdfs:comment>This attribute specifies the direction of the relationship.</rdfs:comment>
    </owl:ObjectProperty>
    


    <!-- http://www.wageneder.at/ontology/bpmn2.0#hasDocumentation -->

    <owl:ObjectProperty rdf:about="http://www.wageneder.at/ontology/bpmn2.0#hasDocumentation">
        <rdfs:domain rdf:resource="http://www.wageneder.at/ontology/bpmn2.0#BaseElement"/>
        <rdfs:comment>This attribute is used to annotate the BPMN element, such as descriptions and other documentation.</rdfs:comment>
    </owl:ObjectProperty>
    


    <!-- http://www.wageneder.at/ontology/bpmn2.0#hasEndPointRefs -->

    <owl:ObjectProperty rdf:about="http://www.wageneder.at/ontology/bpmn2.0#hasEndPointRefs">
        <rdfs:comment>This attribute is used to specify the address (or endpoint reference) of concrete services realizing the Participant.</rdfs:comment>
    </owl:ObjectProperty>
    


    <!-- http://www.wageneder.at/ontology/bpmn2.0#hasError -->

    <owl:ObjectProperty rdf:about="http://www.wageneder.at/ontology/bpmn2.0#hasError">
        <rdfs:comment>If the trigger is an Error, then an Error payload MAY be provided.</rdfs:comment>
    </owl:ObjectProperty>
    


    <!-- http://www.wageneder.at/ontology/bpmn2.0#hasErrorRef -->

    <owl:ObjectProperty rdf:about="http://www.wageneder.at/ontology/bpmn2.0#hasErrorRef">
        <rdfs:comment>This attribute specifies errors that the Operation may return. An Operation MAY refer to zero or more Error elements.</rdfs:comment>
    </owl:ObjectProperty>
    


    <!-- http://www.wageneder.at/ontology/bpmn2.0#hasEscalationRef -->

    <owl:ObjectProperty rdf:about="http://www.wageneder.at/ontology/bpmn2.0#hasEscalationRef">
        <rdfs:comment>If the trigger is an Escalation, then an Escalation payload MAY be provided.</rdfs:comment>
    </owl:ObjectProperty>
    


    <!-- http://www.wageneder.at/ontology/bpmn2.0#hasEvaluatesToTypeRef -->

    <owl:ObjectProperty rdf:about="http://www.wageneder.at/ontology/bpmn2.0#hasEvaluatesToTypeRef">
        <rdfs:subPropertyOf rdf:resource="http://www.w3.org/2002/07/owl#topObjectProperty"/>
        <rdfs:comment>The type of object that this Expression returns when evaluated. For example, conditional Expressions evaluate to a boolean.</rdfs:comment>
    </owl:ObjectProperty>
    


    <!-- http://www.wageneder.at/ontology/bpmn2.0#hasEvent -->

    <owl:ObjectProperty rdf:about="http://www.wageneder.at/ontology/bpmn2.0#hasEvent"/>
    


    <!-- http://www.wageneder.at/ontology/bpmn2.0#hasEventDefinitionRefs -->

    <owl:ObjectProperty rdf:about="http://www.wageneder.at/ontology/bpmn2.0#hasEventDefinitionRefs">
        <rdfs:comment>References the reusable EventDefinitions that are triggers
expected for a catch Event. Reusable EventDefinitions are
defined as top-level elements. These EventDefinitions can be
shared by different catch and throw Events.
• If there is no EventDefinition defined, then this is
considered a catch None Event and the Event will not have
an internal marker (see Figure 10.91).
• If there is more than one EventDefinition defined, this is
considered a Catch Multiple Event and the Event will have
the pentagon internal marker (see Figure 10.90).
This is an ordered set.</rdfs:comment>
    </owl:ObjectProperty>
    


    <!-- http://www.wageneder.at/ontology/bpmn2.0#hasEventDefinitions -->

    <owl:ObjectProperty rdf:about="http://www.wageneder.at/ontology/bpmn2.0#hasEventDefinitions">
        <rdfs:comment>Defines the event EventDefinitions that are triggers expected
for a catch Event. These EventDefinitions are only valid inside
the current Event.
• If there is no EventDefinition defined, then this is
considered a catch None Event and the Event will not have an
internal marker (see Figure 10.91).
• If there is more than one EventDefinition defined, this is
considered a catch Multiple Event and the Event will have the
pentagon internal marker (see Figure 10.90).
This is an ordered set.</rdfs:comment>
    </owl:ObjectProperty>
    


    <!-- http://www.wageneder.at/ontology/bpmn2.0#hasEventGatewayType -->

    <owl:ObjectProperty rdf:about="http://www.wageneder.at/ontology/bpmn2.0#hasEventGatewayType">
        <rdfs:comment>The eventGatewayType determines the behavior of the Gateway when used to instantiate a Process (as described above).
The attribute can only be set to parallel when the instantiate attribute is set to true.</rdfs:comment>
    </owl:ObjectProperty>
    


    <!-- http://www.wageneder.at/ontology/bpmn2.0#hasExclusiceGateway -->

    <owl:ObjectProperty rdf:about="http://www.wageneder.at/ontology/bpmn2.0#hasExclusiceGateway"/>
    


    <!-- http://www.wageneder.at/ontology/bpmn2.0#hasExpression -->

    <owl:ObjectProperty rdf:about="http://www.wageneder.at/ontology/bpmn2.0#hasExpression">
        <rdfs:comment>The element ResourceAssignmentExpression MUST contain an Expression which is used at runtime to assign resource(s) to a ResourceRole element.</rdfs:comment>
    </owl:ObjectProperty>
    


    <!-- http://www.wageneder.at/ontology/bpmn2.0#hasExtensionAttributeDefinition -->

    <owl:ObjectProperty rdf:about="http://www.wageneder.at/ontology/bpmn2.0#hasExtensionAttributeDefinition">
        <rdfs:comment>Defines the extension attribute for which this value is being provided.</rdfs:comment>
    </owl:ObjectProperty>
    


    <!-- http://www.wageneder.at/ontology/bpmn2.0#hasExtensionAttributeDefinitions -->

    <owl:ObjectProperty rdf:about="http://www.wageneder.at/ontology/bpmn2.0#hasExtensionAttributeDefinitions">
        <rdfs:subPropertyOf rdf:resource="http://www.w3.org/2002/07/owl#topObjectProperty"/>
        <rdfs:domain rdf:resource="http://www.wageneder.at/ontology/bpmn2.0#ExtensionDefinition"/>
        <rdfs:comment>The specific attributes that make up the extension.</rdfs:comment>
    </owl:ObjectProperty>
    


    <!-- http://www.wageneder.at/ontology/bpmn2.0#hasExtensionDefinitions -->

    <owl:ObjectProperty rdf:about="http://www.wageneder.at/ontology/bpmn2.0#hasExtensionDefinitions">
        <rdfs:subPropertyOf rdf:resource="http://www.w3.org/2002/07/owl#topObjectProperty"/>
        <rdfs:domain rdf:resource="http://www.wageneder.at/ontology/bpmn2.0#BaseElement"/>
        <rdfs:comment>This attribute is used to attach additional attributes and associations to any BaseElement. This association is not applicable when the XML schema interchange is used, since the XSD mechanisms for supporting anyAttribute and any element already satisfy this requirement. See page 57 for additional information on extensibility.</rdfs:comment>
    </owl:ObjectProperty>
    


    <!-- http://www.wageneder.at/ontology/bpmn2.0#hasExtensionValues -->

    <owl:ObjectProperty rdf:about="http://www.wageneder.at/ontology/bpmn2.0#hasExtensionValues">
        <rdfs:subPropertyOf rdf:resource="http://www.w3.org/2002/07/owl#topObjectProperty"/>
        <rdfs:domain rdf:resource="http://www.wageneder.at/ontology/bpmn2.0#BaseElement"/>
        <rdfs:comment>This attribute is used to provide values for extended attributes and model associations. This association is not applicable when the XML schema interchange is used, since the XSD mechanisms for supporting anyAttribute and any element already satisfy this requirement. See page 57 for additional information on extensibility.</rdfs:comment>
    </owl:ObjectProperty>
    


    <!-- http://www.wageneder.at/ontology/bpmn2.0#hasExtensions -->

    <owl:ObjectProperty rdf:about="http://www.wageneder.at/ontology/bpmn2.0#hasExtensions">
        <rdfs:subPropertyOf rdf:resource="http://www.w3.org/2002/07/owl#topObjectProperty"/>
        <rdfs:comment>This attribute identifies extensions beyond the attributes and model associations in the base BPMN specification. See page 57 for additional information on extensibility.</rdfs:comment>
    </owl:ObjectProperty>
    


    <!-- http://www.wageneder.at/ontology/bpmn2.0#hasFlowElements -->

    <owl:ObjectProperty rdf:about="http://www.wageneder.at/ontology/bpmn2.0#hasFlowElements">
        <rdfs:comment>This association specifies the particular flow elements contained in a FlowElementContainer. Flow elements are Events, Gateways, Sequence Flows, Activities, Data Objects, Data Associations, and Choreography Activities.
Note that:
• ChoreographyActivitiesMUSTNOTbeincludedasaflowElementfora Process.
• Activities, Data Associations, and Data Objects MUST NOT be included as a flowElement for a Choreography.</rdfs:comment>
    </owl:ObjectProperty>
    


    <!-- http://www.wageneder.at/ontology/bpmn2.0#hasFlowElementsContainer -->

    <owl:ObjectProperty rdf:about="http://www.wageneder.at/ontology/bpmn2.0#hasFlowElementsContainer"/>
    


    <!-- http://www.wageneder.at/ontology/bpmn2.0#hasFlowNodeRefs -->

    <owl:ObjectProperty rdf:about="http://www.wageneder.at/ontology/bpmn2.0#hasFlowNodeRefs">
        <rdfs:comment>The list of FlowNodes partitioned into this Lane according to the partitionElement defined as part of the Lane element.</rdfs:comment>
    </owl:ObjectProperty>
    


    <!-- http://www.wageneder.at/ontology/bpmn2.0#hasFrom -->

    <owl:ObjectProperty rdf:about="http://www.wageneder.at/ontology/bpmn2.0#hasFrom">
        <rdfs:comment>The Expression that evaluates the source of the Assignment.</rdfs:comment>
    </owl:ObjectProperty>
    


    <!-- http://www.wageneder.at/ontology/bpmn2.0#hasGatewayDirection -->

    <owl:ObjectProperty rdf:about="http://www.wageneder.at/ontology/bpmn2.0#hasGatewayDirection">
        <rdfs:comment>An attribute that adds constraints on how the Gateway MAY be used.</rdfs:comment>
    </owl:ObjectProperty>
    


    <!-- http://www.wageneder.at/ontology/bpmn2.0#hasIOBinding -->

    <owl:ObjectProperty rdf:about="http://www.wageneder.at/ontology/bpmn2.0#hasIOBinding">
        <rdfs:comment>The InputOutputBinding defines a combination of one InputSet and one OutputSet in order to bind this to an operation defined in an interface.</rdfs:comment>
    </owl:ObjectProperty>
    


    <!-- http://www.wageneder.at/ontology/bpmn2.0#hasIOSpecification -->

    <owl:ObjectProperty rdf:about="http://www.wageneder.at/ontology/bpmn2.0#hasIOSpecification">
        <rdfs:comment>The InputOutputSpecification defines the inputs and outputs and the InputSets and OutputSets for the Activity. See page 211 for more information on the InputOutputSpecification.</rdfs:comment>
    </owl:ObjectProperty>
    


    <!-- http://www.wageneder.at/ontology/bpmn2.0#hasImplementationRef -->

    <owl:ObjectProperty rdf:about="http://www.wageneder.at/ontology/bpmn2.0#hasImplementationRef">
        <rdfs:comment>This attribute allows to reference a concrete artifact in the underlying implementation technology representing that operation, such as a WSDL operation.</rdfs:comment>
    </owl:ObjectProperty>
    


    <!-- http://www.wageneder.at/ontology/bpmn2.0#hasImport -->

    <owl:ObjectProperty rdf:about="http://www.wageneder.at/ontology/bpmn2.0#hasImport">
        <rdfs:comment>Identifies the location of the data structure and its format. If the importType attribute is left unspecified, the typeLanguage specified in the Definitions that contains this ItemDefinition is assumed.</rdfs:comment>
    </owl:ObjectProperty>
    


    <!-- http://www.wageneder.at/ontology/bpmn2.0#hasImports -->

    <owl:ObjectProperty rdf:about="http://www.wageneder.at/ontology/bpmn2.0#hasImports">
        <rdfs:subPropertyOf rdf:resource="http://www.w3.org/2002/07/owl#topObjectProperty"/>
        <rdfs:comment>This attribute is used to import externally defined elements and make them available for use by elements within this Definitions.</rdfs:comment>
    </owl:ObjectProperty>
    


    <!-- http://www.wageneder.at/ontology/bpmn2.0#hasInMessageRef -->

    <owl:ObjectProperty rdf:about="http://www.wageneder.at/ontology/bpmn2.0#hasInMessageRef">
        <rdfs:comment>This attribute specifies the input Message of the Operation. An Operation has exactly one input Message.</rdfs:comment>
    </owl:ObjectProperty>
    


    <!-- http://www.wageneder.at/ontology/bpmn2.0#hasInclusiveGateway -->

    <owl:ObjectProperty rdf:about="http://www.wageneder.at/ontology/bpmn2.0#hasInclusiveGateway"/>
    


    <!-- http://www.wageneder.at/ontology/bpmn2.0#hasIncoming -->

    <owl:ObjectProperty rdf:about="http://www.wageneder.at/ontology/bpmn2.0#hasIncoming">
        <rdfs:comment>This attribute identifies the incoming Sequence Flow of the FlowNode.</rdfs:comment>
    </owl:ObjectProperty>
    


    <!-- http://www.wageneder.at/ontology/bpmn2.0#hasIncomingConversationLinks -->

    <owl:ObjectProperty rdf:about="http://www.wageneder.at/ontology/bpmn2.0#hasIncomingConversationLinks"/>
    


    <!-- http://www.wageneder.at/ontology/bpmn2.0#hasInnerConversationNodeRef -->

    <owl:ObjectProperty rdf:about="http://www.wageneder.at/ontology/bpmn2.0#hasInnerConversationNodeRef">
        <rdfs:comment>This attribute defines the ConversationNodes of the referenced element (e.g., a Choreography to be used in a Collaboration) that will be mapped to the parent element (e.g., the Collaboration).</rdfs:comment>
    </owl:ObjectProperty>
    


    <!-- http://www.wageneder.at/ontology/bpmn2.0#hasInnerMessageFlowRef -->

    <owl:ObjectProperty rdf:about="http://www.wageneder.at/ontology/bpmn2.0#hasInnerMessageFlowRef">
        <rdfs:comment>This attribute defines the Message Flow of the referenced element (e.g., a Choreography to be used in a Collaboration) that will be mapped to the parent element (e.g., the Collaboration).</rdfs:comment>
    </owl:ObjectProperty>
    


    <!-- http://www.wageneder.at/ontology/bpmn2.0#hasInnerParticipantRef -->

    <owl:ObjectProperty rdf:about="http://www.wageneder.at/ontology/bpmn2.0#hasInnerParticipantRef">
        <rdfs:comment>This attribute defines the Participant of the referenced element (e.g., a Choreography to be used in a Collaboration) that will be mapped to the parent element (e.g., the Collaboration).</rdfs:comment>
    </owl:ObjectProperty>
    


    <!-- http://www.wageneder.at/ontology/bpmn2.0#hasInputDataItem -->

    <owl:ObjectProperty rdf:about="http://www.wageneder.at/ontology/bpmn2.0#hasInputDataItem">
        <rdfs:comment>A Data Input, representing for every Activity instance the single item of the collection stored in the loopDataInput. This Data Input can be the source of DataInputAssociation to a data input of the Activity’s InputOutputSpecification. The type of this Data Input MUST the scalar of the type defined for the loopDataInput.</rdfs:comment>
    </owl:ObjectProperty>
    


    <!-- http://www.wageneder.at/ontology/bpmn2.0#hasInputDataRef -->

    <owl:ObjectProperty rdf:about="http://www.wageneder.at/ontology/bpmn2.0#hasInputDataRef">
        <rdfs:comment>A reference to one specific DataInput defined as part of the InputOutputSpecification of the Activity.</rdfs:comment>
    </owl:ObjectProperty>
    


    <!-- http://www.wageneder.at/ontology/bpmn2.0#hasInputSet -->

    <owl:ObjectProperty rdf:about="http://www.wageneder.at/ontology/bpmn2.0#hasInputSet">
        <rdfs:comment>The InputSet for the throw Event.</rdfs:comment>
    </owl:ObjectProperty>
    


    <!-- http://www.wageneder.at/ontology/bpmn2.0#hasInputSetRefs -->

    <owl:ObjectProperty rdf:about="http://www.wageneder.at/ontology/bpmn2.0#hasInputSetRefs">
        <rdfs:comment>A DataInput is used in one or more InputSets. This attribute is derived from the InputSets.</rdfs:comment>
    </owl:ObjectProperty>
    


    <!-- http://www.wageneder.at/ontology/bpmn2.0#hasInputSetWithOptional -->

    <owl:ObjectProperty rdf:about="http://www.wageneder.at/ontology/bpmn2.0#hasInputSetWithOptional">
        <rdfs:comment>Each InputSet that uses this DataInput can determine if the Activity can start executing with this DataInput state in “unavailable.” This attribute lists those InputSets.</rdfs:comment>
    </owl:ObjectProperty>
    


    <!-- http://www.wageneder.at/ontology/bpmn2.0#hasInputSetWithWhileExecuting -->

    <owl:ObjectProperty rdf:about="http://www.wageneder.at/ontology/bpmn2.0#hasInputSetWithWhileExecuting">
        <rdfs:comment>Each InputSet that uses this DataInput can determine if the Activity can evaluate this DataInput while executing. This attribute lists those InputSets.</rdfs:comment>
    </owl:ObjectProperty>
    


    <!-- http://www.wageneder.at/ontology/bpmn2.0#hasInputSets -->

    <owl:ObjectProperty rdf:about="http://www.wageneder.at/ontology/bpmn2.0#hasInputSets">
        <rdfs:comment>A reference to the InputSets defined by the InputOutputSpecification. Every InputOutputSpecification MUST define at least one InputSet.</rdfs:comment>
    </owl:ObjectProperty>
    


    <!-- http://www.wageneder.at/ontology/bpmn2.0#hasInterfaceRef -->

    <owl:ObjectProperty rdf:about="http://www.wageneder.at/ontology/bpmn2.0#hasInterfaceRef">
        <rdfs:comment>This association defines Interfaces that a Participant supports. The
definition of Interfaces is provided on page 102.</rdfs:comment>
    </owl:ObjectProperty>
    


    <!-- http://www.wageneder.at/ontology/bpmn2.0#hasItemKind -->

    <owl:ObjectProperty rdf:about="http://www.wageneder.at/ontology/bpmn2.0#hasItemKind">
        <rdfs:comment>This defines the nature of the Item. Possible values are physical or information. The default value is information.</rdfs:comment>
    </owl:ObjectProperty>
    


    <!-- http://www.wageneder.at/ontology/bpmn2.0#hasItemRef -->

    <owl:ObjectProperty rdf:about="http://www.wageneder.at/ontology/bpmn2.0#hasItemRef">
        <rdfs:comment>An ItemDefinition is used to define the “payload” of the Message.</rdfs:comment>
    </owl:ObjectProperty>
    


    <!-- http://www.wageneder.at/ontology/bpmn2.0#hasItemSubjectRef -->

    <owl:ObjectProperty rdf:about="http://www.wageneder.at/ontology/bpmn2.0#hasItemSubjectRef">
        <rdfs:comment>Specification of the items that are stored or conveyed by the ItemAwareElement.</rdfs:comment>
    </owl:ObjectProperty>
    


    <!-- http://www.wageneder.at/ontology/bpmn2.0#hasLaneSet -->

    <owl:ObjectProperty rdf:about="http://www.wageneder.at/ontology/bpmn2.0#hasLaneSet"/>
    


    <!-- http://www.wageneder.at/ontology/bpmn2.0#hasLaneSets -->

    <owl:ObjectProperty rdf:about="http://www.wageneder.at/ontology/bpmn2.0#hasLaneSets">
        <rdfs:comment>This attribute defines the list of LaneSets used in the FlowElementsContainer LaneSets are not used for Choreographies or Sub-Choreographies.</rdfs:comment>
    </owl:ObjectProperty>
    


    <!-- http://www.wageneder.at/ontology/bpmn2.0#hasLanes -->

    <owl:ObjectProperty rdf:about="http://www.wageneder.at/ontology/bpmn2.0#hasLanes">
        <rdfs:comment>One or more Lane elements, which define a specific partition in the LaneSet.</rdfs:comment>
    </owl:ObjectProperty>
    


    <!-- http://www.wageneder.at/ontology/bpmn2.0#hasLoopCardinality -->

    <owl:ObjectProperty rdf:about="http://www.wageneder.at/ontology/bpmn2.0#hasLoopCardinality">
        <rdfs:comment>A numeric Expression that controls the number of Activity instances that will be created. This Expression MUST evaluate to an integer. This MAY be underspecified, meaning that the modeler MAY simply document the condition. In such a case the loop cannot be formally executed.
In order to initialize a valid multi-instance, either the loopCardinality Expression or the loopDataInput MUST be specified.</rdfs:comment>
    </owl:ObjectProperty>
    


    <!-- http://www.wageneder.at/ontology/bpmn2.0#hasLoopCharacteristics -->

    <owl:ObjectProperty rdf:about="http://www.wageneder.at/ontology/bpmn2.0#hasLoopCharacteristics">
        <rdfs:comment>An Activity MAY be performed once or MAY be repeated. If repeated, the Activity MUST have loopCharacteristics that define the repe- tition criteria (if the isExecutable attribute of the Process is set to true).</rdfs:comment>
    </owl:ObjectProperty>
    


    <!-- http://www.wageneder.at/ontology/bpmn2.0#hasLoopCondition -->

    <owl:ObjectProperty rdf:about="http://www.wageneder.at/ontology/bpmn2.0#hasLoopCondition">
        <rdfs:comment>A boolean Expression that controls the loop. The Activity will only loop as long as this condition is true. The looping behavior MAY be underspecified, meaning that the modeler can simply document the condition, in which case the loop cannot be formally executed.</rdfs:comment>
    </owl:ObjectProperty>
    


    <!-- http://www.wageneder.at/ontology/bpmn2.0#hasLoopDataInputRef -->

    <owl:ObjectProperty rdf:about="http://www.wageneder.at/ontology/bpmn2.0#hasLoopDataInputRef">
        <rdfs:comment>This ItemAwareElement is used to determine the number of Activity instances, one Activity instance per item in the collection of data stored in that ItemAwareElement element.
For Tasks it is a reference to a Data Input which is part of the Activity’s InputOutputSpecification.
For Sub-Processes it is a reference to a collection-valued Data Object in the context that is visible to the Sub-Processes.
In order to initialize a valid multi-instance, either the loopCardinality Expression or the loopDataInput MUST be specified.</rdfs:comment>
    </owl:ObjectProperty>
    


    <!-- http://www.wageneder.at/ontology/bpmn2.0#hasLoopDataOutputRef -->

    <owl:ObjectProperty rdf:about="http://www.wageneder.at/ontology/bpmn2.0#hasLoopDataOutputRef">
        <rdfs:comment>This ItemAwareElement specifies the collection of data, which will be produced by the multi-instance.
For Tasks it is a reference to a Data Output which is part of the Activity’s InputOutputSpecification.
For Sub-Processes it is a reference to a collection-valued Data Object in the context that is visible to the Sub-Processes.</rdfs:comment>
    </owl:ObjectProperty>
    


    <!-- http://www.wageneder.at/ontology/bpmn2.0#hasMessage -->

    <owl:ObjectProperty rdf:about="http://www.wageneder.at/ontology/bpmn2.0#hasMessage"/>
    


    <!-- http://www.wageneder.at/ontology/bpmn2.0#hasMessageFlow -->

    <owl:ObjectProperty rdf:about="http://www.wageneder.at/ontology/bpmn2.0#hasMessageFlow">
        <rdfs:comment>This provides the list of Message Flows that are used in the Collaboration. Message Flows are visualized in Collaboration (as dashed line) and hidden in Choreography.</rdfs:comment>
    </owl:ObjectProperty>
    


    <!-- http://www.wageneder.at/ontology/bpmn2.0#hasMessageFlowAssociation -->

    <owl:ObjectProperty rdf:about="http://www.wageneder.at/ontology/bpmn2.0#hasMessageFlowAssociation"/>
    


    <!-- http://www.wageneder.at/ontology/bpmn2.0#hasMessageFlowAssociations -->

    <owl:ObjectProperty rdf:about="http://www.wageneder.at/ontology/bpmn2.0#hasMessageFlowAssociations">
        <rdfs:comment>This attribute provides a list of mappings for the Message Flows of the Collaboration to Message Flows of a referenced model. It is used in the following situation:
• When a Choreography is referenced by a Collaboration. This allows the &quot;wiring up&quot; of the Collaboration Message Flows to the appropriate Choreography Activities.</rdfs:comment>
    </owl:ObjectProperty>
    


    <!-- http://www.wageneder.at/ontology/bpmn2.0#hasMessageFlowRefs -->

    <owl:ObjectProperty rdf:about="http://www.wageneder.at/ontology/bpmn2.0#hasMessageFlowRefs">
        <rdfs:comment>A reference to all Message Flows (and consequently Messages) grouped by a
Conversation element.</rdfs:comment>
    </owl:ObjectProperty>
    


    <!-- http://www.wageneder.at/ontology/bpmn2.0#hasMessagePath -->

    <owl:ObjectProperty rdf:about="http://www.wageneder.at/ontology/bpmn2.0#hasMessagePath">
        <rdfs:comment>The FormalExpression that defines how to extract a CorrelationProperty from the Message payload.</rdfs:comment>
    </owl:ObjectProperty>
    


    <!-- http://www.wageneder.at/ontology/bpmn2.0#hasMessageRef -->

    <owl:ObjectProperty rdf:about="http://www.wageneder.at/ontology/bpmn2.0#hasMessageRef">
        <rdfs:comment>A Message for the messageRef attribute MAY be entered. 
This indicates that the Message will be sent by the Task. 
The Message in this context is equivalent to an out-only message pattern (Web service). 
One or more corresponding outgoing Message Flows MAY be shown on the diagram. 
However, the display of the Message Flows is NOT REQUIRED. 
The Message is applied to all outgoing Message Flows and the Message will be sent down all outgoing Message Flows at the completion of a single instance of the Task.</rdfs:comment>
    </owl:ObjectProperty>
    


    <!-- http://www.wageneder.at/ontology/bpmn2.0#hasMethod -->

    <owl:ObjectProperty rdf:about="http://www.wageneder.at/ontology/bpmn2.0#hasMethod">
        <rdfs:comment>The method is an attribute that defines the Transaction method used to
commit or cancel a Transaction. For executable Processes, it SHOULD be
set to a technology specific URI, e.g., http://schemas.xmlsoap.org/
ws/2004/10/wsat for WS-AtomicTransaction, or http://
docs.oasis-open.org/ws-tx/wsba/2006/06/AtomicOutcome for
WS-BusinessActivity. For compatibility with BPMN 1.1, it can also be set to
&quot;##compensate,&quot; &quot;##store,&quot; or &quot;##image.&quot;</rdfs:comment>
    </owl:ObjectProperty>
    


    <!-- http://www.wageneder.at/ontology/bpmn2.0#hasMonitoring -->

    <owl:ObjectProperty rdf:about="http://www.wageneder.at/ontology/bpmn2.0#hasMonitoring">
        <rdfs:subPropertyOf rdf:resource="http://www.w3.org/2002/07/owl#topObjectProperty"/>
        <rdfs:comment>A hook for specifying monitoring related properties. Monitoring can only be defined for a Process.</rdfs:comment>
    </owl:ObjectProperty>
    


    <!-- http://www.wageneder.at/ontology/bpmn2.0#hasNoneBehaviourEventRef -->

    <owl:ObjectProperty rdf:about="http://www.wageneder.at/ontology/bpmn2.0#hasNoneBehaviourEventRef">
        <rdfs:comment>The EventDefinition which is thrown when the behavior is set to none and an internal Activity instance has completed.</rdfs:comment>
    </owl:ObjectProperty>
    


    <!-- http://www.wageneder.at/ontology/bpmn2.0#hasOneBehaviourEventRef -->

    <owl:ObjectProperty rdf:about="http://www.wageneder.at/ontology/bpmn2.0#hasOneBehaviourEventRef">
        <rdfs:comment>The EventDefinition which is thrown when behavior is set to one and the first internal Activity instance has completed.</rdfs:comment>
    </owl:ObjectProperty>
    


    <!-- http://www.wageneder.at/ontology/bpmn2.0#hasOperationRef -->

    <owl:ObjectProperty rdf:about="http://www.wageneder.at/ontology/bpmn2.0#hasOperationRef">
        <rdfs:comment>This attribute specifies the operation that is invoked by the Service/Send Task.</rdfs:comment>
    </owl:ObjectProperty>
    


    <!-- http://www.wageneder.at/ontology/bpmn2.0#hasOperations -->

    <owl:ObjectProperty rdf:about="http://www.wageneder.at/ontology/bpmn2.0#hasOperations">
        <rdfs:comment>This attribute specifies operations that are defined as part of the
Interface. An Interface has at least one Operation.</rdfs:comment>
    </owl:ObjectProperty>
    


    <!-- http://www.wageneder.at/ontology/bpmn2.0#hasOptionalInputRefs -->

    <owl:ObjectProperty rdf:about="http://www.wageneder.at/ontology/bpmn2.0#hasOptionalInputRefs">
        <rdfs:comment>The DataInput elements that are a part of the InputSet that can be in the state of “unavailable” when the Activity starts executing. This association MUST NOT reference a DataInput that is not listed in the dataInputRefs.</rdfs:comment>
    </owl:ObjectProperty>
    


    <!-- http://www.wageneder.at/ontology/bpmn2.0#hasOptionalOutputRefs -->

    <owl:ObjectProperty rdf:about="http://www.wageneder.at/ontology/bpmn2.0#hasOptionalOutputRefs">
        <rdfs:comment>The DataOutput elements that are a part of the OutputSet that do not have to be produced when the Activity completes executing. This association MUST NOT reference a DataOutput that is not listed in the dataOutputRefs.</rdfs:comment>
    </owl:ObjectProperty>
    


    <!-- http://www.wageneder.at/ontology/bpmn2.0#hasOrdering -->

    <owl:ObjectProperty rdf:about="http://www.wageneder.at/ontology/bpmn2.0#hasOrdering">
        <rdfs:comment>This attribute defines if the Activities within the Process can be performed in
parallel or MUST be performed sequentially. The default setting is parallel
and the setting of sequential is a restriction on the performance that can be
needed due to shared resources. When the setting is sequential, then only
one Activity can be performed at a time. When the setting is parallel, then
zero (0) to all the Activities of the Sub-Process can be performed in parallel.</rdfs:comment>
    </owl:ObjectProperty>
    


    <!-- http://www.wageneder.at/ontology/bpmn2.0#hasOutMessageRef -->

    <owl:ObjectProperty rdf:about="http://www.wageneder.at/ontology/bpmn2.0#hasOutMessageRef">
        <rdfs:comment>This attribute specifies the output Message of the Operation. An Operation has at most one input Message.</rdfs:comment>
    </owl:ObjectProperty>
    


    <!-- http://www.wageneder.at/ontology/bpmn2.0#hasOuterConversationNodeRef -->

    <owl:ObjectProperty rdf:about="http://www.wageneder.at/ontology/bpmn2.0#hasOuterConversationNodeRef">
        <rdfs:comment>This attribute defines the ConversationNodes of the parent element (e.g., a Collaboration references a Choreography) that will be mapped to the referenced element (e.g., the Choreography).</rdfs:comment>
    </owl:ObjectProperty>
    


    <!-- http://www.wageneder.at/ontology/bpmn2.0#hasOuterMessageFlowRef -->

    <owl:ObjectProperty rdf:about="http://www.wageneder.at/ontology/bpmn2.0#hasOuterMessageFlowRef">
        <rdfs:comment>This attribute defines the Message Flow of the parent element (e.g., a Collaboration references a Choreography) that will be mapped to the referenced element (e.g., the Choreography).</rdfs:comment>
    </owl:ObjectProperty>
    


    <!-- http://www.wageneder.at/ontology/bpmn2.0#hasOuterParticipantRef -->

    <owl:ObjectProperty rdf:about="http://www.wageneder.at/ontology/bpmn2.0#hasOuterParticipantRef">
        <rdfs:comment>This attribute defines the Participant of the parent element (e.g., a Collaboration references a Choreography) that will be mapped to the referenced element (e.g., the Choreography).</rdfs:comment>
    </owl:ObjectProperty>
    


    <!-- http://www.wageneder.at/ontology/bpmn2.0#hasOutgoing -->

    <owl:ObjectProperty rdf:about="http://www.wageneder.at/ontology/bpmn2.0#hasOutgoing">
        <rdfs:comment>This attribute identifies the outgoing Sequence Flow of the FlowNode. This is an ordered collection.</rdfs:comment>
    </owl:ObjectProperty>
    


    <!-- http://www.wageneder.at/ontology/bpmn2.0#hasOutgoingConversationLinks -->

    <owl:ObjectProperty rdf:about="http://www.wageneder.at/ontology/bpmn2.0#hasOutgoingConversationLinks"/>
    


    <!-- http://www.wageneder.at/ontology/bpmn2.0#hasOutputDataItem -->

    <owl:ObjectProperty rdf:about="http://www.wageneder.at/ontology/bpmn2.0#hasOutputDataItem">
        <rdfs:comment>A Data Output, representing for every Activity instance the single item of the collection stored in the loopDataOutput. This Data Output can be the target of DataOutputAssociation to a data output of the Activity’s InputOutputSpecification. The type of this Data Output MUST the scalar of the type defined for the loopDataOutput.</rdfs:comment>
    </owl:ObjectProperty>
    


    <!-- http://www.wageneder.at/ontology/bpmn2.0#hasOutputDataRef -->

    <owl:ObjectProperty rdf:about="http://www.wageneder.at/ontology/bpmn2.0#hasOutputDataRef">
        <rdfs:comment>outputDataRef: DataOutput A reference to one specific DataOutput defined as part of the InputOutputSpecification of the Activity.</rdfs:comment>
    </owl:ObjectProperty>
    


    <!-- http://www.wageneder.at/ontology/bpmn2.0#hasOutputSet -->

    <owl:ObjectProperty rdf:about="http://www.wageneder.at/ontology/bpmn2.0#hasOutputSet">
        <rdfs:comment>The OutputSet for the catch Event.</rdfs:comment>
    </owl:ObjectProperty>
    


    <!-- http://www.wageneder.at/ontology/bpmn2.0#hasOutputSetRefs -->

    <owl:ObjectProperty rdf:about="http://www.wageneder.at/ontology/bpmn2.0#hasOutputSetRefs">
        <rdfs:comment>A DataOutput is used in one or more OutputSets. This attribute is derived from the OutputSets.</rdfs:comment>
    </owl:ObjectProperty>
    


    <!-- http://www.wageneder.at/ontology/bpmn2.0#hasOutputSetWithOptional -->

    <owl:ObjectProperty rdf:about="http://www.wageneder.at/ontology/bpmn2.0#hasOutputSetWithOptional">
        <rdfs:comment>Each OutputSet that uses this DataOutput can determine if the Activity can complete executing without producing this DataInput. This attribute lists those OutputSets.</rdfs:comment>
    </owl:ObjectProperty>
    


    <!-- http://www.wageneder.at/ontology/bpmn2.0#hasOutputSetWithWhileExecuting -->

    <owl:ObjectProperty rdf:about="http://www.wageneder.at/ontology/bpmn2.0#hasOutputSetWithWhileExecuting">
        <rdfs:comment>Each OutputSet that uses this DataInput can determine if the Activity can produce this DataOutput while executing. This attribute lists those OutputSets.</rdfs:comment>
    </owl:ObjectProperty>
    


    <!-- http://www.wageneder.at/ontology/bpmn2.0#hasOutputSets -->

    <owl:ObjectProperty rdf:about="http://www.wageneder.at/ontology/bpmn2.0#hasOutputSets">
        <rdfs:comment>A reference to the OutputSets defined by the InputOutputSpecification. Every Data Interface MUST define at least one OutputSet.</rdfs:comment>
    </owl:ObjectProperty>
    


    <!-- http://www.wageneder.at/ontology/bpmn2.0#hasParameterRef -->

    <owl:ObjectProperty rdf:about="http://www.wageneder.at/ontology/bpmn2.0#hasParameterRef">
        <rdfs:comment>Reference to the parameter defined by the Resource.</rdfs:comment>
    </owl:ObjectProperty>
    


    <!-- http://www.wageneder.at/ontology/bpmn2.0#hasParentLane -->

    <owl:ObjectProperty rdf:about="http://www.wageneder.at/ontology/bpmn2.0#hasParentLane">
        <rdfs:comment>The reference to a Lane element which is the parent of this LaneSet.</rdfs:comment>
    </owl:ObjectProperty>
    


    <!-- http://www.wageneder.at/ontology/bpmn2.0#hasParticipant -->

    <owl:ObjectProperty rdf:about="http://www.wageneder.at/ontology/bpmn2.0#hasParticipant"/>
    


    <!-- http://www.wageneder.at/ontology/bpmn2.0#hasParticipantAssociation -->

    <owl:ObjectProperty rdf:about="http://www.wageneder.at/ontology/bpmn2.0#hasParticipantAssociation"/>
    


    <!-- http://www.wageneder.at/ontology/bpmn2.0#hasParticipantAssociations -->

    <owl:ObjectProperty rdf:about="http://www.wageneder.at/ontology/bpmn2.0#hasParticipantAssociations">
        <rdfs:comment>This attribute provides a list of mappings from the Participants of a referenced Collaboration to the Participants of another Collaboration. It is used in the following situations
• When a Choreography is referenced by the Collaboration.
• When a definitional Collaboration for a Process is referenced through a Call Activity (and mapped to definitional Collaboration of the calling Process).</rdfs:comment>
    </owl:ObjectProperty>
    


    <!-- http://www.wageneder.at/ontology/bpmn2.0#hasParticipantMultiplicity -->

    <owl:ObjectProperty rdf:about="http://www.wageneder.at/ontology/bpmn2.0#hasParticipantMultiplicity">
        <rdfs:comment>The participantMultiplicityRef model association is used to define Participants that represent more than one (1) instance of the Participant for a given interaction. See the next sub clause for more details on ParticipantMultiplicity.</rdfs:comment>
    </owl:ObjectProperty>
    


    <!-- http://www.wageneder.at/ontology/bpmn2.0#hasParticipantRef -->

    <owl:ObjectProperty rdf:about="http://www.wageneder.at/ontology/bpmn2.0#hasParticipantRef">
        <rdfs:comment>Specifies how the PartnerEntity/ParticipantEntity participates in Collaborations and 
Choreographies.</rdfs:comment>
    </owl:ObjectProperty>
    


    <!-- http://www.wageneder.at/ontology/bpmn2.0#hasParticipantRefs -->

    <owl:ObjectProperty rdf:about="http://www.wageneder.at/ontology/bpmn2.0#hasParticipantRefs">
        <rdfs:comment>This provides the list of Participants that are used in the ConversationNode from the list provided by the ConversationNode’s parent Conversation. This reference is visualized through a Conversation Link (see page 131).</rdfs:comment>
    </owl:ObjectProperty>
    


    <!-- http://www.wageneder.at/ontology/bpmn2.0#hasParticipants -->

    <owl:ObjectProperty rdf:about="http://www.wageneder.at/ontology/bpmn2.0#hasParticipants">
        <rdfs:comment>This provides the list of Participants that are used in the Collaboration. Participants are visualized as Pools in a Collaboration and as Participant Bands in Choreography Activities in a Choreography.</rdfs:comment>
    </owl:ObjectProperty>
    


    <!-- http://www.wageneder.at/ontology/bpmn2.0#hasPartitionElement -->

    <owl:ObjectProperty rdf:about="http://www.wageneder.at/ontology/bpmn2.0#hasPartitionElement">
        <rdfs:comment>A reference to a BaseElement that specifies the partition value and partition type. Using this partition element a BPMN compliant tool can determine the FlowElements that have to be partitioned in this Lane.</rdfs:comment>
    </owl:ObjectProperty>
    


    <!-- http://www.wageneder.at/ontology/bpmn2.0#hasPartitionElementRef -->

    <owl:ObjectProperty rdf:about="http://www.wageneder.at/ontology/bpmn2.0#hasPartitionElementRef">
        <rdfs:comment>A reference to a BaseElement that specifies the partition value and partition type. Using this partition element a BPMN compliant tool can determine the FlowElements that have to be partitioned in this Lane.</rdfs:comment>
    </owl:ObjectProperty>
    


    <!-- http://www.wageneder.at/ontology/bpmn2.0#hasPartnerEntityRef -->

    <owl:ObjectProperty rdf:about="http://www.wageneder.at/ontology/bpmn2.0#hasPartnerEntityRef">
        <rdfs:comment>The partnerEntityRef attribute identifies a PartnerEntity that the Participant plays in the Collaboration. Both a PartnerRole and a PartnerEntity MAY be defined for the Participant.This attribute is derived from the participantRefs of PartnerEntity.</rdfs:comment>
    </owl:ObjectProperty>
    


    <!-- http://www.wageneder.at/ontology/bpmn2.0#hasPartnerRoleRef -->

    <owl:ObjectProperty rdf:about="http://www.wageneder.at/ontology/bpmn2.0#hasPartnerRoleRef">
        <rdfs:comment>The partnerRoleRef attribute identifies a PartnerRole that the Participant plays in the Collaboration. Both a PartnerRole and a PartnerEntity MAY be defined for the Participant. This attribute is derived from the participantRefs of PartnerRole.</rdfs:comment>
    </owl:ObjectProperty>
    


    <!-- http://www.wageneder.at/ontology/bpmn2.0#hasProcess -->

    <owl:ObjectProperty rdf:about="http://www.wageneder.at/ontology/bpmn2.0#hasProcess">
        <rdfs:comment>The Process owning the LaneSet</rdfs:comment>
    </owl:ObjectProperty>
    


    <!-- http://www.wageneder.at/ontology/bpmn2.0#hasProcessRef -->

    <owl:ObjectProperty rdf:about="http://www.wageneder.at/ontology/bpmn2.0#hasProcessRef">
        <rdfs:comment>The processRef attribute identifies the Process that the Participant uses in the Collaboration. The Process will be displayed within the Participant’s Pool.</rdfs:comment>
    </owl:ObjectProperty>
    


    <!-- http://www.wageneder.at/ontology/bpmn2.0#hasProcessType -->

    <owl:ObjectProperty rdf:about="http://www.wageneder.at/ontology/bpmn2.0#hasProcessType">
        <rdfs:comment>The processType attribute Provides additional information about the level of abstraction modeled by this Process. A public Process shows only those flow elements that are relevant to external consumers. Internal details are not modeled. These Processes are publicly visible and can be used within a Collaboration. Note that the public processType was named abstract in BPMN 1.2. A private Process is one that is internal to a specific organization. By default, the processType is “none,” meaning undefined.</rdfs:comment>
    </owl:ObjectProperty>
    


    <!-- http://www.wageneder.at/ontology/bpmn2.0#hasProperties -->

    <owl:ObjectProperty rdf:about="http://www.wageneder.at/ontology/bpmn2.0#hasProperties">
        <rdfs:comment>Modeler-defined properties MAY be added to an Activity. These properties are contained within the Activity.</rdfs:comment>
    </owl:ObjectProperty>
    


    <!-- http://www.wageneder.at/ontology/bpmn2.0#hasRelationships -->

    <owl:ObjectProperty rdf:about="http://www.wageneder.at/ontology/bpmn2.0#hasRelationships">
        <rdfs:comment>This attribute enables the extension and integration of BPMN models into larger system/development Processes.</rdfs:comment>
    </owl:ObjectProperty>
    


    <!-- http://www.wageneder.at/ontology/bpmn2.0#hasRenderings -->

    <owl:ObjectProperty rdf:about="http://www.wageneder.at/ontology/bpmn2.0#hasRenderings">
        <rdfs:comment>This attributes acts as a hook which allows BPMN adopters to specify task rendering attributes by using the BPMN Extension mechanism.</rdfs:comment>
    </owl:ObjectProperty>
    


    <!-- http://www.wageneder.at/ontology/bpmn2.0#hasResourceAssignmentExpression -->

    <owl:ObjectProperty rdf:about="http://www.wageneder.at/ontology/bpmn2.0#hasResourceAssignmentExpression">
        <rdfs:comment>This defines the Expression used for the Resource assignment (see below). Should not be specified when a resourceRef is provided.</rdfs:comment>
    </owl:ObjectProperty>
    


    <!-- http://www.wageneder.at/ontology/bpmn2.0#hasResourceParameterBindings -->

    <owl:ObjectProperty rdf:about="http://www.wageneder.at/ontology/bpmn2.0#hasResourceParameterBindings">
        <rdfs:comment>This defines the Parameter bindings used for the Resource assignment (see below). Is only applicable if a resourceRef is specified.</rdfs:comment>
    </owl:ObjectProperty>
    


    <!-- http://www.wageneder.at/ontology/bpmn2.0#hasResourceParameters -->

    <owl:ObjectProperty rdf:about="http://www.wageneder.at/ontology/bpmn2.0#hasResourceParameters">
        <rdfs:comment>This model association specifies the definition of the parameters needed at runtime to resolve the Resource.</rdfs:comment>
    </owl:ObjectProperty>
    


    <!-- http://www.wageneder.at/ontology/bpmn2.0#hasResourceRef -->

    <owl:ObjectProperty rdf:about="http://www.wageneder.at/ontology/bpmn2.0#hasResourceRef">
        <rdfs:comment>The Resource that is associated with Activity. Should not be specified when resourceAssignmentExpression is provided.</rdfs:comment>
    </owl:ObjectProperty>
    


    <!-- http://www.wageneder.at/ontology/bpmn2.0#hasResources -->

    <owl:ObjectProperty rdf:about="http://www.wageneder.at/ontology/bpmn2.0#hasResources">
        <rdfs:comment>Defines the resource that will perform or will be responsible for the Activity. The resource, e.g., a performer, can be specified in the form of a specific individual, a group, an organization role or position, or an orga- nization.</rdfs:comment>
    </owl:ObjectProperty>
    


    <!-- http://www.wageneder.at/ontology/bpmn2.0#hasRootElements -->

    <owl:ObjectProperty rdf:about="http://www.wageneder.at/ontology/bpmn2.0#hasRootElements">
        <rdfs:comment>This attribute lists the root elements that are at the root of this Definitions. These elements can be referenced within this Definitions and are visible to other Definitions.</rdfs:comment>
    </owl:ObjectProperty>
    


    <!-- http://www.wageneder.at/ontology/bpmn2.0#hasSignalRef -->

    <owl:ObjectProperty rdf:about="http://www.wageneder.at/ontology/bpmn2.0#hasSignalRef">
        <rdfs:comment>If the trigger is a Signal, then a Signal is provided.</rdfs:comment>
    </owl:ObjectProperty>
    


    <!-- http://www.wageneder.at/ontology/bpmn2.0#hasSourceRef -->

    <owl:ObjectProperty rdf:about="http://www.wageneder.at/ontology/bpmn2.0#hasSourceRef">
        <rdfs:comment>The BaseElement that the Association is connecting from.</rdfs:comment>
    </owl:ObjectProperty>
    


    <!-- http://www.wageneder.at/ontology/bpmn2.0#hasSources -->

    <owl:ObjectProperty rdf:about="http://www.wageneder.at/ontology/bpmn2.0#hasSources">
        <rdfs:comment>This association defines artifacts that are augmented by the relationship.</rdfs:comment>
    </owl:ObjectProperty>
    


    <!-- http://www.wageneder.at/ontology/bpmn2.0#hasStructureRef -->

    <owl:ObjectProperty rdf:about="http://www.wageneder.at/ontology/bpmn2.0#hasStructureRef">
        <rdfs:comment>1. Error: An ItemDefinition is used to define the “payload” of the Error.

2. Escalation: An ItemDefinition is used to define the “payload” of the Escalation.</rdfs:comment>
    </owl:ObjectProperty>
    


    <!-- http://www.wageneder.at/ontology/bpmn2.0#hasSubConversation -->

    <owl:ObjectProperty rdf:about="http://www.wageneder.at/ontology/bpmn2.0#hasSubConversation"/>
    


    <!-- http://www.wageneder.at/ontology/bpmn2.0#hasSupportedInterfaceRefs -->

    <owl:ObjectProperty rdf:about="http://www.wageneder.at/ontology/bpmn2.0#hasSupportedInterfaceRefs">
        <rdfs:comment>The Interfaces describing the external behavior provided by this element.</rdfs:comment>
    </owl:ObjectProperty>
    


    <!-- http://www.wageneder.at/ontology/bpmn2.0#hasSupports -->

    <owl:ObjectProperty rdf:about="http://www.wageneder.at/ontology/bpmn2.0#hasSupports">
        <rdfs:comment>Modelers can declare that they intend all executions or performances of one Process to also be valid for another Process. This means they expect all the executions or performances of the first Processes to also follow the steps laid out in the second Process</rdfs:comment>
    </owl:ObjectProperty>
    


    <!-- http://www.wageneder.at/ontology/bpmn2.0#hasTarget -->

    <owl:ObjectProperty rdf:about="http://www.wageneder.at/ontology/bpmn2.0#hasTarget">
        <rdfs:comment>Used to reference the corresponding &apos;throw&apos; or &apos;source&apos; LinkEventDefinition, when this LinkEventDefinition represents a &apos;catch&apos; or &apos;target&apos; LinkEventDefinition.</rdfs:comment>
    </owl:ObjectProperty>
    


    <!-- http://www.wageneder.at/ontology/bpmn2.0#hasTargetRef -->

    <owl:ObjectProperty rdf:about="http://www.wageneder.at/ontology/bpmn2.0#hasTargetRef">
        <rdfs:comment>The BaseElement that the Association is connecting to.</rdfs:comment>
    </owl:ObjectProperty>
    


    <!-- http://www.wageneder.at/ontology/bpmn2.0#hasTargets -->

    <owl:ObjectProperty rdf:about="http://www.wageneder.at/ontology/bpmn2.0#hasTargets">
        <rdfs:comment>This association defines artifacts used to extend the semantics of the source element(s).</rdfs:comment>
    </owl:ObjectProperty>
    


    <!-- http://www.wageneder.at/ontology/bpmn2.0#hasTimeCycle -->

    <owl:ObjectProperty rdf:about="http://www.wageneder.at/ontology/bpmn2.0#hasTimeCycle">
        <rdfs:comment>If the trigger is a Timer, then a timeCycle MAY be entered. Timer attributes are
mutually exclusive and if any of the other Timer attributes is set, timeCycle MUST
NOT be set (if the isExecutable attribute of the Process is set to true). The
return type of the attribute timeCycle MUST conform to the ISO-8601 format for
recurring time interval representations.</rdfs:comment>
    </owl:ObjectProperty>
    


    <!-- http://www.wageneder.at/ontology/bpmn2.0#hasTimeDate -->

    <owl:ObjectProperty rdf:about="http://www.wageneder.at/ontology/bpmn2.0#hasTimeDate">
        <rdfs:comment>If the trigger is a Timer, then a timeDate MAY be entered. Timer attributes are
mutually exclusive and if any of the other Timer attributes is set, timeDate MUST
NOT be set (if the isExecutable attribute of the Process is set to true). The
return type of the attribute timeDate MUST conform to the ISO-8601 format for date
and time representations.</rdfs:comment>
    </owl:ObjectProperty>
    


    <!-- http://www.wageneder.at/ontology/bpmn2.0#hasTimeDuration -->

    <owl:ObjectProperty rdf:about="http://www.wageneder.at/ontology/bpmn2.0#hasTimeDuration">
        <rdfs:comment>If the trigger is a Timer, then a timeDuration MAY be entered. Timer attributes
are mutually exclusive and if any of the other Timer attributes is set, timeDuration
MUST NOT be set (if the isExecutable attribute of the Process is set to true).
The return type of the attribute timeDuration MUST conform to the ISO-8601
format for time interval representations.</rdfs:comment>
    </owl:ObjectProperty>
    


    <!-- http://www.wageneder.at/ontology/bpmn2.0#hasTo -->

    <owl:ObjectProperty rdf:about="http://www.wageneder.at/ontology/bpmn2.0#hasTo">
        <rdfs:comment>The Expression that defines the actual Assignment operation and the target data element.</rdfs:comment>
    </owl:ObjectProperty>
    


    <!-- http://www.wageneder.at/ontology/bpmn2.0#hasTransformation -->

    <owl:ObjectProperty rdf:about="http://www.wageneder.at/ontology/bpmn2.0#hasTransformation"/>
    


    <!-- http://www.wageneder.at/ontology/bpmn2.0#hasType -->

    <owl:ObjectProperty rdf:about="http://www.wageneder.at/ontology/bpmn2.0#hasType">
        <rdfs:comment>Specifies the type of the query parameter.</rdfs:comment>
    </owl:ObjectProperty>
    


    <!-- http://www.wageneder.at/ontology/bpmn2.0#hasUserTask -->

    <owl:ObjectProperty rdf:about="http://www.wageneder.at/ontology/bpmn2.0#hasUserTask"/>
    


    <!-- http://www.wageneder.at/ontology/bpmn2.0#hasValue -->

    <owl:ObjectProperty rdf:about="http://www.wageneder.at/ontology/bpmn2.0#hasValue">
        <rdfs:comment>The contained attribute value, used when the associated ExtensionAttributeDefinition.isReference is false.
The type of this Element MUST conform to the type specified in the associated ExtensionAttributeDefinition.</rdfs:comment>
    </owl:ObjectProperty>
    


    <!-- http://www.wageneder.at/ontology/bpmn2.0#hasValueRef -->

    <owl:ObjectProperty rdf:about="http://www.wageneder.at/ontology/bpmn2.0#hasValueRef">
        <rdfs:comment>The referenced attribute value, used when the associated ExtensionAttributeDefinition.isReference is true. The type of this Element MUST conform to the type specified in the associated ExtensionAttributeDefinition.</rdfs:comment>
    </owl:ObjectProperty>
    


    <!-- http://www.wageneder.at/ontology/bpmn2.0#hasWhileExecutingInputRefs -->

    <owl:ObjectProperty rdf:about="http://www.wageneder.at/ontology/bpmn2.0#hasWhileExecutingInputRefs">
        <rdfs:comment>The DataInput elements that are a part of the InputSet that can be evaluated while the Activity is executing. This association MUST NOT reference a DataInput that is not listed in the dataInputRefs.</rdfs:comment>
    </owl:ObjectProperty>
    


    <!-- http://www.wageneder.at/ontology/bpmn2.0#hasWhileExecutingOutputRefs -->

    <owl:ObjectProperty rdf:about="http://www.wageneder.at/ontology/bpmn2.0#hasWhileExecutingOutputRefs">
        <rdfs:comment>The DataOutput elements that are a part of the OutputSet that can be produced while the Activity is executing. This association MUST NOT reference a DataOutput that is not listed in the dataOutputRefs.</rdfs:comment>
    </owl:ObjectProperty>
    


    <!-- 
    ///////////////////////////////////////////////////////////////////////////////////////
    //
    // Data properties
    //
    ///////////////////////////////////////////////////////////////////////////////////////
     -->

    


    <!-- http://www.wageneder.at/ontology/bpmn2.0#activationCount -->

    <owl:DatatypeProperty rdf:about="http://www.wageneder.at/ontology/bpmn2.0#activationCount"/>
    


    <!-- http://www.wageneder.at/ontology/bpmn2.0#actualOwner -->

    <owl:DatatypeProperty rdf:about="http://www.wageneder.at/ontology/bpmn2.0#actualOwner"/>
    


    <!-- http://www.wageneder.at/ontology/bpmn2.0#cancelActivity -->

    <owl:DatatypeProperty rdf:about="http://www.wageneder.at/ontology/bpmn2.0#cancelActivity"/>
    


    <!-- http://www.wageneder.at/ontology/bpmn2.0#cancelRemainingInstances -->

    <owl:DatatypeProperty rdf:about="http://www.wageneder.at/ontology/bpmn2.0#cancelRemainingInstances"/>
    


    <!-- http://www.wageneder.at/ontology/bpmn2.0#capacity -->

    <owl:DatatypeProperty rdf:about="http://www.wageneder.at/ontology/bpmn2.0#capacity"/>
    


    <!-- http://www.wageneder.at/ontology/bpmn2.0#completionQuantity -->

    <owl:DatatypeProperty rdf:about="http://www.wageneder.at/ontology/bpmn2.0#completionQuantity">
        <rdfs:comment>The default value is 1. The value MUST NOT be less than 1. This attribute defines the number of tokens that MUST be generated from the Activity. This number of tokens will be sent done any outgoing Sequence Flow (assuming any Sequence Flow conditions are satis- fied). Note that any value for the attribute that is greater than 1 is an advanced type of modeling and should be used with caution.</rdfs:comment>
    </owl:DatatypeProperty>
    


    <!-- http://www.wageneder.at/ontology/bpmn2.0#errorCode -->

    <owl:DatatypeProperty rdf:about="http://www.wageneder.at/ontology/bpmn2.0#errorCode">
        <rdfs:comment>For an End Event:
If the result is an Error, then the errorCode MUST be supplied (if the processType attribute of the Process is set to execut- able) This “throws” the Error.

For an Intermediate Event within normal flow:
If the trigger is an Error, then the errorCode MUST be entered
(if the processType attribute of the Process is set to execut-
able). This “throws” the Error.

For an Intermediate Event attached to the boundary of an Activity:
If the trigger is an Error, then the errorCode MAY be entered. This Event “catches” the Error. If there is no errorCode, then any error SHALL trigger the Event. If there is an errorCode, then only an Error that matches the errorCode SHALL trigger the Event.</rdfs:comment>
    </owl:DatatypeProperty>
    


    <!-- http://www.wageneder.at/ontology/bpmn2.0#escalationCode -->

    <owl:DatatypeProperty rdf:about="http://www.wageneder.at/ontology/bpmn2.0#escalationCode">
        <rdfs:comment>For an End Event:
If the Result is an Escalation, then the escalationCode
MUST be supplied (if the processType attribute of the Process is set to executable). This “throws” the Escalation.

For an Intermediate Event within normal flow:
If the trigger is an Escalation, then the escalationCode
MUST be entered (if the processType attribute of the Process is
set to executable). This “throws” the Escalation.

For an Intermediate Event attached to the boundary of an Activity:
If the trigger is an Escalation, then the escalationCode MAY be entered. This Event “catches” the Escalation. If there is no escalationCode, then any Escalation SHALL trigger the Event. If there is an escalationCode, then only an Escala- tion that matches the escalationCode SHALL trigger the Event.</rdfs:comment>
    </owl:DatatypeProperty>
    


    <!-- http://www.wageneder.at/ontology/bpmn2.0#exporter -->

    <owl:DatatypeProperty rdf:about="http://www.wageneder.at/ontology/bpmn2.0#exporter">
        <rdfs:subPropertyOf rdf:resource="http://www.w3.org/2002/07/owl#topDataProperty"/>
        <rdfs:comment>This attribute identifies the tool that is exporting the bpmn model file.</rdfs:comment>
    </owl:DatatypeProperty>
    


    <!-- http://www.wageneder.at/ontology/bpmn2.0#exporterVersion -->

    <owl:DatatypeProperty rdf:about="http://www.wageneder.at/ontology/bpmn2.0#exporterVersion">
        <rdfs:subPropertyOf rdf:resource="http://www.w3.org/2002/07/owl#topDataProperty"/>
        <rdfs:comment>This attribute identifies the version of the tool that is exporting the bpmn model file.</rdfs:comment>
    </owl:DatatypeProperty>
    


    <!-- http://www.wageneder.at/ontology/bpmn2.0#expressionLanguage -->

    <owl:DatatypeProperty rdf:about="http://www.wageneder.at/ontology/bpmn2.0#expressionLanguage">
        <rdfs:subPropertyOf rdf:resource="http://www.w3.org/2002/07/owl#topDataProperty"/>
        <rdfs:comment>This attribute identifies the formal Expression language used in Expressions within the elements of this Definition. The Default is “http://www.w3.org/1999/XPath”. This value MAY be overridden on each individual formal Expression. The language MUST be specified in a URI format.</rdfs:comment>
    </owl:DatatypeProperty>
    


    <!-- http://www.wageneder.at/ontology/bpmn2.0#extensionDefinitions -->

    <owl:DatatypeProperty rdf:about="http://www.wageneder.at/ontology/bpmn2.0#extensionDefinitions">
        <rdfs:subPropertyOf rdf:resource="http://www.w3.org/2002/07/owl#topDataProperty"/>
        <rdfs:domain rdf:resource="http://www.wageneder.at/ontology/bpmn2.0#BaseElement"/>
        <rdfs:comment>This attribute is used to attach additional attributes and associations to any BaseElement. This association is not applicable when the XML schema interchange is used, since the XSD mechanisms for supporting anyAttribute and any element already satisfy this requirement. See page 57 for additional information on extensibility.</rdfs:comment>
    </owl:DatatypeProperty>
    


    <!-- http://www.wageneder.at/ontology/bpmn2.0#extensionValues -->

    <owl:DatatypeProperty rdf:about="http://www.wageneder.at/ontology/bpmn2.0#extensionValues">
        <rdfs:subPropertyOf rdf:resource="http://www.w3.org/2002/07/owl#topDataProperty"/>
        <rdfs:domain rdf:resource="http://www.wageneder.at/ontology/bpmn2.0#BaseElement"/>
        <rdfs:comment>This attribute is used to provide values for extended attributes and model associations. This association is not applicable when the XML schema interchange is used, since the XSD mechanisms for supporting anyAttribute and any element already satisfy this requirement. See page 57 for additional information on extensibility.</rdfs:comment>
    </owl:DatatypeProperty>
    


    <!-- http://www.wageneder.at/ontology/bpmn2.0#id -->

    <owl:DatatypeProperty rdf:about="http://www.wageneder.at/ontology/bpmn2.0#id">
        <rdfs:comment>This attribute is used to uniquely identify BPMN elements. The id is REQUIRED if this element is referenced or intended to be referenced by something else. If the element is not currently referenced and is never intended to be referenced, the id MAY be omitted.</rdfs:comment>
    </owl:DatatypeProperty>
    


    <!-- http://www.wageneder.at/ontology/bpmn2.0#implementation -->

    <owl:DatatypeProperty rdf:about="http://www.wageneder.at/ontology/bpmn2.0#implementation">
        <rdfs:comment>This attribute specifies the technology that will be used to send and receive the Messages. Valid values are &quot;##unspec- ified&quot; for leaving the implementation technology open, &quot;##WebService&quot; for the Web service technology or a URI identifying any other technology or coordination protocol. A Web service is the default technology.</rdfs:comment>
    </owl:DatatypeProperty>
    


    <!-- http://www.wageneder.at/ontology/bpmn2.0#importType -->

    <owl:DatatypeProperty rdf:about="http://www.wageneder.at/ontology/bpmn2.0#importType">
        <rdfs:subPropertyOf rdf:resource="http://www.w3.org/2002/07/owl#topDataProperty"/>
        <rdfs:comment>Identifies the type of document being imported by providing an absolute URI that identifies the encoding language used in the document.The value of the importType attribute MUST be set to http://www.w3.org/2001/XMLSchema when importing XML Schema 1.0 documents, to http://www.w3.org/TR/wsdl20/ when importing WSDL 2.0 documents, and http://www.omg.org/spec/BPMN/20100524/MODEL when importing BPMN 2.0 documents. Other types of documents MAY be supported. Importing Xml Schema 1.0, WSDL 2.0 and BPMN 2.0 types MUST be supported.</rdfs:comment>
    </owl:DatatypeProperty>
    


    <!-- http://www.wageneder.at/ontology/bpmn2.0#instantiate -->

    <owl:DatatypeProperty rdf:about="http://www.wageneder.at/ontology/bpmn2.0#instantiate">
        <rdfs:comment>Receive Tasks can be defined as the instantiation mechanism for the Process with the instantiate attribute. This attribute MAY be set to true if the Task is the first Activity (i.e., there are no incoming Sequence Flows). Multiple Tasks MAY have this attribute set to true.</rdfs:comment>
    </owl:DatatypeProperty>
    


    <!-- http://www.wageneder.at/ontology/bpmn2.0#isClosed -->

    <owl:DatatypeProperty rdf:about="http://www.wageneder.at/ontology/bpmn2.0#isClosed"/>
    


    <!-- http://www.wageneder.at/ontology/bpmn2.0#isCollection -->

    <owl:DatatypeProperty rdf:about="http://www.wageneder.at/ontology/bpmn2.0#isCollection">
        <rdfs:comment>Setting this flag to true indicates that the actual data type is a collection.</rdfs:comment>
    </owl:DatatypeProperty>
    


    <!-- http://www.wageneder.at/ontology/bpmn2.0#isExecutable -->

    <owl:DatatypeProperty rdf:about="http://www.wageneder.at/ontology/bpmn2.0#isExecutable"/>
    


    <!-- http://www.wageneder.at/ontology/bpmn2.0#isForCompensation -->

    <owl:DatatypeProperty rdf:about="http://www.wageneder.at/ontology/bpmn2.0#isForCompensation">
        <rdfs:comment>A flag that identifies whether this Activity is intended for the purposes of compensation.
If false, then this Activity executes as a result of normal execution flow. If true, this Activity is only activated when a Compensation Event is detected and initiated under Compensation Event visibility scope (see page 281 for more information on scopes).</rdfs:comment>
    </owl:DatatypeProperty>
    


    <!-- http://www.wageneder.at/ontology/bpmn2.0#isImmediate -->

    <owl:DatatypeProperty rdf:about="http://www.wageneder.at/ontology/bpmn2.0#isImmediate">
        <rdfs:comment>An optional boolean value specifying whether Activities or Choreography Activities not in the model containing the Sequence Flow can occur between the elements connected by the Sequence Flow. 
If the value is true, they MAY NOT occur. If the value is false, they MAY occur. 
Also see the isClosed attribute on Process, Choreography, and Collaboration. 
When the attribute has no value, the default semantics depends on the kind of model containing Sequence Flows:

• For non-executable Processes (public Processes and non-executable private Processes) and Choreographies no value has the same semantics as if the value were false.

• For an executable Processes no value has the same semantics as if the value were true.

• For executable Processes, the attribute MUST NOT be false.</rdfs:comment>
    </owl:DatatypeProperty>
    


    <!-- http://www.wageneder.at/ontology/bpmn2.0#isInterrupting -->

    <owl:DatatypeProperty rdf:about="http://www.wageneder.at/ontology/bpmn2.0#isInterrupting"/>
    


    <!-- http://www.wageneder.at/ontology/bpmn2.0#isReference -->

    <owl:DatatypeProperty rdf:about="http://www.wageneder.at/ontology/bpmn2.0#isReference">
        <rdfs:comment>Indicates if the attribute value will be referenced or contained.

Default Value = false</rdfs:comment>
    </owl:DatatypeProperty>
    


    <!-- http://www.wageneder.at/ontology/bpmn2.0#isRequired -->

    <owl:DatatypeProperty rdf:about="http://www.wageneder.at/ontology/bpmn2.0#isRequired">
        <rdfs:comment>Specifies, if a parameter is optional or mandatory.</rdfs:comment>
    </owl:DatatypeProperty>
    


    <!-- http://www.wageneder.at/ontology/bpmn2.0#isSequential -->

    <owl:DatatypeProperty rdf:about="http://www.wageneder.at/ontology/bpmn2.0#isSequential"/>
    


    <!-- http://www.wageneder.at/ontology/bpmn2.0#isUnlimited -->

    <owl:DatatypeProperty rdf:about="http://www.wageneder.at/ontology/bpmn2.0#isUnlimited"/>
    


    <!-- http://www.wageneder.at/ontology/bpmn2.0#language -->

    <owl:DatatypeProperty rdf:about="http://www.wageneder.at/ontology/bpmn2.0#language">
        <rdfs:comment>Overrides the Expression language specified in the Definitions. The language MUST be specified in a URI format.</rdfs:comment>
    </owl:DatatypeProperty>
    


    <!-- http://www.wageneder.at/ontology/bpmn2.0#location -->

    <owl:DatatypeProperty rdf:about="http://www.wageneder.at/ontology/bpmn2.0#location">
        <rdfs:subPropertyOf rdf:resource="http://www.w3.org/2002/07/owl#topDataProperty"/>
        <rdfs:comment>Identifies the location of the imported element.</rdfs:comment>
    </owl:DatatypeProperty>
    


    <!-- http://www.wageneder.at/ontology/bpmn2.0#loopCounter -->

    <owl:DatatypeProperty rdf:about="http://www.wageneder.at/ontology/bpmn2.0#loopCounter"/>
    


    <!-- http://www.wageneder.at/ontology/bpmn2.0#loopMaximum -->

    <owl:DatatypeProperty rdf:about="http://www.wageneder.at/ontology/bpmn2.0#loopMaximum"/>
    


    <!-- http://www.wageneder.at/ontology/bpmn2.0#maximum -->

    <owl:DatatypeProperty rdf:about="http://www.wageneder.at/ontology/bpmn2.0#maximum"/>
    


    <!-- http://www.wageneder.at/ontology/bpmn2.0#minium -->

    <owl:DatatypeProperty rdf:about="http://www.wageneder.at/ontology/bpmn2.0#minium"/>
    


    <!-- http://www.wageneder.at/ontology/bpmn2.0#mustUnderstand -->

    <owl:DatatypeProperty rdf:about="http://www.wageneder.at/ontology/bpmn2.0#mustUnderstand">
        <rdfs:domain rdf:resource="http://www.wageneder.at/ontology/bpmn2.0#Extension"/>
        <rdfs:comment>This flag defines if the semantics defined by the extension definition and its attribute definition MUST be understood by the BPMN adopter in order to process the BPMN model correctly. 

Defaults to False</rdfs:comment>
    </owl:DatatypeProperty>
    


    <!-- http://www.wageneder.at/ontology/bpmn2.0#name -->

    <owl:DatatypeProperty rdf:about="http://www.wageneder.at/ontology/bpmn2.0#name">
        <rdfs:comment>1. ExtensionDefinition: The name of the extension. This is used as a namespace to uniquely identify the extension content.

2. ExtensionAttributeDefinition: The name of the extension attribute.

3. Category: The descriptive name of the element.

4. Error: The descriptive name of the Error.

5. Definition: The name of the Definition.

6. Message: Name is a text description of the Message.

7. Resource: This attribute specifies the name of the Resource.</rdfs:comment>
    </owl:DatatypeProperty>
    


    <!-- http://www.wageneder.at/ontology/bpmn2.0#namespace -->

    <owl:DatatypeProperty rdf:about="http://www.wageneder.at/ontology/bpmn2.0#namespace">
        <rdfs:subPropertyOf rdf:resource="http://www.w3.org/2002/07/owl#topDataProperty"/>
        <rdfs:comment>Identifies the namespace of the imported element.</rdfs:comment>
    </owl:DatatypeProperty>
    


    <!-- http://www.wageneder.at/ontology/bpmn2.0#numParticipants -->

    <owl:DatatypeProperty rdf:about="http://www.wageneder.at/ontology/bpmn2.0#numParticipants"/>
    


    <!-- http://www.wageneder.at/ontology/bpmn2.0#numberOfActiveInstances -->

    <owl:DatatypeProperty rdf:about="http://www.wageneder.at/ontology/bpmn2.0#numberOfActiveInstances"/>
    


    <!-- http://www.wageneder.at/ontology/bpmn2.0#numberOfCompletedInstances -->

    <owl:DatatypeProperty rdf:about="http://www.wageneder.at/ontology/bpmn2.0#numberOfCompletedInstances"/>
    


    <!-- http://www.wageneder.at/ontology/bpmn2.0#numberOfInstances -->

    <owl:DatatypeProperty rdf:about="http://www.wageneder.at/ontology/bpmn2.0#numberOfInstances"/>
    


    <!-- http://www.wageneder.at/ontology/bpmn2.0#numberOfTerminatedInstances -->

    <owl:DatatypeProperty rdf:about="http://www.wageneder.at/ontology/bpmn2.0#numberOfTerminatedInstances"/>
    


    <!-- http://www.wageneder.at/ontology/bpmn2.0#parallelMultiple -->

    <owl:DatatypeProperty rdf:about="http://www.wageneder.at/ontology/bpmn2.0#parallelMultiple"/>
    


    <!-- http://www.wageneder.at/ontology/bpmn2.0#processType -->

    <owl:DatatypeProperty rdf:about="http://www.wageneder.at/ontology/bpmn2.0#processType"/>
    


    <!-- http://www.wageneder.at/ontology/bpmn2.0#protocol -->

    <owl:DatatypeProperty rdf:about="http://www.wageneder.at/ontology/bpmn2.0#protocol"/>
    


    <!-- http://www.wageneder.at/ontology/bpmn2.0#script -->

    <owl:DatatypeProperty rdf:about="http://www.wageneder.at/ontology/bpmn2.0#script">
        <rdfs:subPropertyOf rdf:resource="http://www.w3.org/2002/07/owl#topDataProperty"/>
        <rdfs:comment>The modeler MAY include a script that can be run when the Task is per- formed. If a script is not included, then the Task will act as the equivalent of an Abstract Task.</rdfs:comment>
    </owl:DatatypeProperty>
    


    <!-- http://www.wageneder.at/ontology/bpmn2.0#scriptFormat -->

    <owl:DatatypeProperty rdf:about="http://www.wageneder.at/ontology/bpmn2.0#scriptFormat">
        <rdfs:subPropertyOf rdf:resource="http://www.w3.org/2002/07/owl#topDataProperty"/>
        <rdfs:comment>Defines the format of the script. This attribute value MUST be specified with a mime-type format. And it MUST be specified if a script is provided.</rdfs:comment>
    </owl:DatatypeProperty>
    


    <!-- http://www.wageneder.at/ontology/bpmn2.0#startQuantity -->

    <owl:DatatypeProperty rdf:about="http://www.wageneder.at/ontology/bpmn2.0#startQuantity">
        <rdfs:comment>The default value is 1. The value MUST NOT be less than 1. This attribute defines the number of tokens that MUST arrive before the Activity can begin. Note that any value for the attribute that is greater than 1 is an advanced type of modeling and should be used with caution.</rdfs:comment>
    </owl:DatatypeProperty>
    


    <!-- http://www.wageneder.at/ontology/bpmn2.0#state -->

    <owl:DatatypeProperty rdf:about="http://www.wageneder.at/ontology/bpmn2.0#state"/>
    


    <!-- http://www.wageneder.at/ontology/bpmn2.0#targetNamespace -->

    <owl:DatatypeProperty rdf:about="http://www.wageneder.at/ontology/bpmn2.0#targetNamespace">
        <rdfs:subPropertyOf rdf:resource="http://www.w3.org/2002/07/owl#topDataProperty"/>
        <rdfs:comment>This attribute identifies the namespace associated with the Definition and follows the convention established by XML Schema.</rdfs:comment>
    </owl:DatatypeProperty>
    


    <!-- http://www.wageneder.at/ontology/bpmn2.0#taskPriority -->

    <owl:DatatypeProperty rdf:about="http://www.wageneder.at/ontology/bpmn2.0#taskPriority"/>
    


    <!-- http://www.wageneder.at/ontology/bpmn2.0#testBefore -->

    <owl:DatatypeProperty rdf:about="http://www.wageneder.at/ontology/bpmn2.0#testBefore"/>
    


    <!-- http://www.wageneder.at/ontology/bpmn2.0#text -->

    <owl:DatatypeProperty rdf:about="http://www.wageneder.at/ontology/bpmn2.0#text">
        <rdfs:comment>This attribute is used to capture the text descriptions of a BPMN element.</rdfs:comment>
    </owl:DatatypeProperty>
    


    <!-- http://www.wageneder.at/ontology/bpmn2.0#textFormat -->

    <owl:DatatypeProperty rdf:about="http://www.wageneder.at/ontology/bpmn2.0#textFormat">
        <rdfs:comment>This attribute identifies the format of the text. It MUST follow the mime-type format. The default is &quot;text/plain.&quot;</rdfs:comment>
    </owl:DatatypeProperty>
    


    <!-- http://www.wageneder.at/ontology/bpmn2.0#triggeredByEvent -->

    <owl:DatatypeProperty rdf:about="http://www.wageneder.at/ontology/bpmn2.0#triggeredByEvent">
        <rdfs:comment>A flag that identifies whether this Sub-Process is an Event Sub-Process.

• If false, then this Sub-Process is a normal Sub-Process.

• If true, then this Sub-Process is an Event Sub-Process and is subject to additional constraints (see page 176).</rdfs:comment>
    </owl:DatatypeProperty>
    


    <!-- http://www.wageneder.at/ontology/bpmn2.0#type -->

    <owl:DatatypeProperty rdf:about="http://www.wageneder.at/ontology/bpmn2.0#type">
        <rdfs:subPropertyOf rdf:resource="http://www.w3.org/2002/07/owl#topDataProperty"/>
        <rdfs:comment>The type that is associated with the attribute.</rdfs:comment>
    </owl:DatatypeProperty>
    


    <!-- http://www.wageneder.at/ontology/bpmn2.0#typeLanguage -->

    <owl:DatatypeProperty rdf:about="http://www.wageneder.at/ontology/bpmn2.0#typeLanguage">
        <rdfs:subPropertyOf rdf:resource="http://www.w3.org/2002/07/owl#topDataProperty"/>
        <rdfs:comment>This attribute identifies the type system used by the elements of this Definition. Defaults to http://www.w3.org/2001/XMLSchema. This value can be overridden on each individual ItemDefinition. The language MUST be specified in a URI format.</rdfs:comment>
    </owl:DatatypeProperty>
    


    <!-- http://www.wageneder.at/ontology/bpmn2.0#value -->

    <owl:DatatypeProperty rdf:about="http://www.wageneder.at/ontology/bpmn2.0#value">
        <rdfs:comment>This attribute provides the value of the CategoryValue element.</rdfs:comment>
    </owl:DatatypeProperty>
    


    <!-- http://www.wageneder.at/ontology/bpmn2.0#waitForCompletion -->

    <owl:DatatypeProperty rdf:about="http://www.wageneder.at/ontology/bpmn2.0#waitForCompletion"/>
    


    <!-- http://www.wageneder.at/ontology/bpmn2.0#waitingForStart -->

    <owl:DatatypeProperty rdf:about="http://www.wageneder.at/ontology/bpmn2.0#waitingForStart"/>
    


    <!-- 
    ///////////////////////////////////////////////////////////////////////////////////////
    //
    // Classes
    //
    ///////////////////////////////////////////////////////////////////////////////////////
     -->

    


    <!-- http://www.wageneder.at/ontology/bpmn2.0#Activity -->

    <owl:Class rdf:about="http://www.wageneder.at/ontology/bpmn2.0#Activity">
        <rdfs:subClassOf rdf:resource="http://www.wageneder.at/ontology/bpmn2.0#ActivityLevel"/>
        <rdfs:subClassOf rdf:resource="http://www.wageneder.at/ontology/bpmn2.0#FlowNode"/>
        <rdfs:subClassOf>
            <owl:Restriction>
                <owl:onProperty rdf:resource="http://www.wageneder.at/ontology/bpmn2.0#hasBoundaryEventRefs"/>
                <owl:minQualifiedCardinality rdf:datatype="http://www.w3.org/2001/XMLSchema#nonNegativeInteger">0</owl:minQualifiedCardinality>
                <owl:onClass rdf:resource="http://www.wageneder.at/ontology/bpmn2.0#BoundaryEvent"/>
            </owl:Restriction>
        </rdfs:subClassOf>
        <rdfs:subClassOf>
            <owl:Restriction>
                <owl:onProperty rdf:resource="http://www.wageneder.at/ontology/bpmn2.0#hasDataInputAssociations"/>
                <owl:minQualifiedCardinality rdf:datatype="http://www.w3.org/2001/XMLSchema#nonNegativeInteger">0</owl:minQualifiedCardinality>
                <owl:onClass rdf:resource="http://www.wageneder.at/ontology/bpmn2.0#DataInputAssociation"/>
            </owl:Restriction>
        </rdfs:subClassOf>
        <rdfs:subClassOf>
            <owl:Restriction>
                <owl:onProperty rdf:resource="http://www.wageneder.at/ontology/bpmn2.0#hasDataOutputAssociations"/>
                <owl:minQualifiedCardinality rdf:datatype="http://www.w3.org/2001/XMLSchema#nonNegativeInteger">0</owl:minQualifiedCardinality>
                <owl:onClass rdf:resource="http://www.wageneder.at/ontology/bpmn2.0#DataOutputAssociation"/>
            </owl:Restriction>
        </rdfs:subClassOf>
        <rdfs:subClassOf>
            <owl:Restriction>
                <owl:onProperty rdf:resource="http://www.wageneder.at/ontology/bpmn2.0#hasDefault"/>
                <owl:minQualifiedCardinality rdf:datatype="http://www.w3.org/2001/XMLSchema#nonNegativeInteger">0</owl:minQualifiedCardinality>
                <owl:onClass rdf:resource="http://www.wageneder.at/ontology/bpmn2.0#SequenceFlow"/>
            </owl:Restriction>
        </rdfs:subClassOf>
        <rdfs:subClassOf>
            <owl:Restriction>
                <owl:onProperty rdf:resource="http://www.wageneder.at/ontology/bpmn2.0#hasIOSpecification"/>
                <owl:minQualifiedCardinality rdf:datatype="http://www.w3.org/2001/XMLSchema#nonNegativeInteger">0</owl:minQualifiedCardinality>
                <owl:onClass rdf:resource="http://www.wageneder.at/ontology/bpmn2.0#InputOutputSpecification"/>
            </owl:Restriction>
        </rdfs:subClassOf>
        <rdfs:subClassOf>
            <owl:Restriction>
                <owl:onProperty rdf:resource="http://www.wageneder.at/ontology/bpmn2.0#hasLoopCharacteristics"/>
                <owl:minQualifiedCardinality rdf:datatype="http://www.w3.org/2001/XMLSchema#nonNegativeInteger">0</owl:minQualifiedCardinality>
                <owl:onClass rdf:resource="http://www.wageneder.at/ontology/bpmn2.0#LoopCharacteristics"/>
            </owl:Restriction>
        </rdfs:subClassOf>
        <rdfs:subClassOf>
            <owl:Restriction>
                <owl:onProperty rdf:resource="http://www.wageneder.at/ontology/bpmn2.0#hasProperties"/>
                <owl:minQualifiedCardinality rdf:datatype="http://www.w3.org/2001/XMLSchema#nonNegativeInteger">0</owl:minQualifiedCardinality>
                <owl:onClass rdf:resource="http://www.wageneder.at/ontology/bpmn2.0#Property"/>
            </owl:Restriction>
        </rdfs:subClassOf>
        <rdfs:subClassOf>
            <owl:Restriction>
                <owl:onProperty rdf:resource="http://www.wageneder.at/ontology/bpmn2.0#hasResources"/>
                <owl:minQualifiedCardinality rdf:datatype="http://www.w3.org/2001/XMLSchema#nonNegativeInteger">0</owl:minQualifiedCardinality>
                <owl:onClass rdf:resource="http://www.wageneder.at/ontology/bpmn2.0#ResourceRole"/>
            </owl:Restriction>
        </rdfs:subClassOf>
        <rdfs:subClassOf>
            <owl:Restriction>
                <owl:onProperty rdf:resource="http://www.wageneder.at/ontology/bpmn2.0#hasDefault"/>
                <owl:maxQualifiedCardinality rdf:datatype="http://www.w3.org/2001/XMLSchema#nonNegativeInteger">1</owl:maxQualifiedCardinality>
                <owl:onClass rdf:resource="http://www.wageneder.at/ontology/bpmn2.0#SequenceFlow"/>
            </owl:Restriction>
        </rdfs:subClassOf>
        <rdfs:subClassOf>
            <owl:Restriction>
                <owl:onProperty rdf:resource="http://www.wageneder.at/ontology/bpmn2.0#hasIOSpecification"/>
                <owl:maxQualifiedCardinality rdf:datatype="http://www.w3.org/2001/XMLSchema#nonNegativeInteger">1</owl:maxQualifiedCardinality>
                <owl:onClass rdf:resource="http://www.wageneder.at/ontology/bpmn2.0#InputOutputSpecification"/>
            </owl:Restriction>
        </rdfs:subClassOf>
        <rdfs:subClassOf>
            <owl:Restriction>
                <owl:onProperty rdf:resource="http://www.wageneder.at/ontology/bpmn2.0#hasLoopCharacteristics"/>
                <owl:maxQualifiedCardinality rdf:datatype="http://www.w3.org/2001/XMLSchema#nonNegativeInteger">1</owl:maxQualifiedCardinality>
                <owl:onClass rdf:resource="http://www.wageneder.at/ontology/bpmn2.0#LoopCharacteristics"/>
            </owl:Restriction>
        </rdfs:subClassOf>
        <rdfs:subClassOf>
            <owl:Restriction>
                <owl:onProperty rdf:resource="http://www.wageneder.at/ontology/bpmn2.0#completionQuantity"/>
                <owl:qualifiedCardinality rdf:datatype="http://www.w3.org/2001/XMLSchema#nonNegativeInteger">1</owl:qualifiedCardinality>
                <owl:onDataRange rdf:resource="http://www.w3.org/2001/XMLSchema#integer"/>
            </owl:Restriction>
        </rdfs:subClassOf>
        <rdfs:subClassOf>
            <owl:Restriction>
                <owl:onProperty rdf:resource="http://www.wageneder.at/ontology/bpmn2.0#isForCompensation"/>
                <owl:qualifiedCardinality rdf:datatype="http://www.w3.org/2001/XMLSchema#nonNegativeInteger">1</owl:qualifiedCardinality>
                <owl:onDataRange rdf:resource="http://www.w3.org/2001/XMLSchema#boolean"/>
            </owl:Restriction>
        </rdfs:subClassOf>
        <rdfs:subClassOf>
            <owl:Restriction>
                <owl:onProperty rdf:resource="http://www.wageneder.at/ontology/bpmn2.0#startQuantity"/>
                <owl:qualifiedCardinality rdf:datatype="http://www.w3.org/2001/XMLSchema#nonNegativeInteger">1</owl:qualifiedCardinality>
                <owl:onDataRange rdf:resource="http://www.w3.org/2001/XMLSchema#integer"/>
            </owl:Restriction>
        </rdfs:subClassOf>
        <rdfs:subClassOf>
            <owl:Restriction>
                <owl:onProperty rdf:resource="http://www.wageneder.at/ontology/bpmn2.0#state"/>
                <owl:qualifiedCardinality rdf:datatype="http://www.w3.org/2001/XMLSchema#nonNegativeInteger">1</owl:qualifiedCardinality>
                <owl:onDataRange rdf:resource="http://www.w3.org/2001/XMLSchema#string"/>
            </owl:Restriction>
        </rdfs:subClassOf>
        <rdfs:comment>An Activity is work that is performed within a Business Process.

The Activity class is the abstract super class for all concrete Activity types.
The Activity element inherits the attributes and model associations of FlowElement (see Table 8.44). Table 10.3 presents the additional attributes and model associations of the Activity element.</rdfs:comment>
    </owl:Class>
    


    <!-- http://www.wageneder.at/ontology/bpmn2.0#ActivityLevel -->

    <owl:Class rdf:about="http://www.wageneder.at/ontology/bpmn2.0#ActivityLevel">
        <rdfs:subClassOf rdf:resource="http://www.wageneder.at/ontology/bpmn2.0#ProcessLevel"/>
        <rdfs:subClassOf>
            <owl:Restriction>
                <owl:onProperty rdf:resource="http://www.wageneder.at/ontology/bpmn2.0#hasCondition"/>
                <owl:qualifiedCardinality rdf:datatype="http://www.w3.org/2001/XMLSchema#nonNegativeInteger">1</owl:qualifiedCardinality>
                <owl:onClass rdf:resource="http://www.wageneder.at/ontology/bpmn2.0#FormalExpression"/>
            </owl:Restriction>
        </rdfs:subClassOf>
        <rdfs:comment>This is just a hierarchical element for organisational purposes.
It presents the Activity Folder</rdfs:comment>
    </owl:Class>
    


    <!-- http://www.wageneder.at/ontology/bpmn2.0#AdHocOrdering -->

    <owl:Class rdf:about="http://www.wageneder.at/ontology/bpmn2.0#AdHocOrdering">
        <rdfs:subClassOf rdf:resource="http://www.wageneder.at/ontology/bpmn2.0#ActivityLevel"/>
        <rdfs:subClassOf>
            <owl:Class>
                <owl:unionOf rdf:parseType="Collection">
                    <rdf:Description rdf:about="http://www.wageneder.at/ontology/bpmn2.0#Parallel"/>
                    <rdf:Description rdf:about="http://www.wageneder.at/ontology/bpmn2.0#Sequential"/>
                </owl:unionOf>
            </owl:Class>
        </rdfs:subClassOf>
        <rdfs:comment>This attribute defines if the Activities within the Process can be performed in
parallel or MUST be performed sequentially. The default setting is parallel
and the setting of sequential is a restriction on the performance that can be
needed due to shared resources. When the setting is sequential, then only
one Activity can be performed at a time. When the setting is parallel, then
zero (0) to all the Activities of the Sub-Process can be performed in parallel.</rdfs:comment>
    </owl:Class>
    


    <!-- http://www.wageneder.at/ontology/bpmn2.0#AdHocProcess -->

    <owl:Class rdf:about="http://www.wageneder.at/ontology/bpmn2.0#AdHocProcess">
        <rdfs:subClassOf rdf:resource="http://www.wageneder.at/ontology/bpmn2.0#SubProcess"/>
        <rdfs:subClassOf>
            <owl:Restriction>
                <owl:onProperty rdf:resource="http://www.wageneder.at/ontology/bpmn2.0#hasCompletionCondition"/>
                <owl:qualifiedCardinality rdf:datatype="http://www.w3.org/2001/XMLSchema#nonNegativeInteger">1</owl:qualifiedCardinality>
                <owl:onClass rdf:resource="http://www.wageneder.at/ontology/bpmn2.0#Expression"/>
            </owl:Restriction>
        </rdfs:subClassOf>
        <rdfs:subClassOf>
            <owl:Restriction>
                <owl:onProperty rdf:resource="http://www.wageneder.at/ontology/bpmn2.0#hasOrdering"/>
                <owl:qualifiedCardinality rdf:datatype="http://www.w3.org/2001/XMLSchema#nonNegativeInteger">1</owl:qualifiedCardinality>
                <owl:onClass rdf:resource="http://www.wageneder.at/ontology/bpmn2.0#AdHocOrdering"/>
            </owl:Restriction>
        </rdfs:subClassOf>
        <rdfs:subClassOf>
            <owl:Restriction>
                <owl:onProperty rdf:resource="http://www.wageneder.at/ontology/bpmn2.0#cancelRemainingInstances"/>
                <owl:qualifiedCardinality rdf:datatype="http://www.w3.org/2001/XMLSchema#nonNegativeInteger">1</owl:qualifiedCardinality>
                <owl:onDataRange rdf:resource="http://www.w3.org/2001/XMLSchema#boolean"/>
            </owl:Restriction>
        </rdfs:subClassOf>
        <owl:disjointWith rdf:resource="http://www.wageneder.at/ontology/bpmn2.0#Transaction"/>
        <rdfs:comment>An Ad-Hoc Sub-Process is a specialized type of Sub-Process that is a group of Activities that have no REQUIRED sequence relationships. A set of Activities can be defined for the Process, but the sequence and number of performances for the Activities is determined by the performers of the Activities.</rdfs:comment>
    </owl:Class>
    


    <!-- http://www.wageneder.at/ontology/bpmn2.0#All -->

    <owl:Class rdf:about="http://www.wageneder.at/ontology/bpmn2.0#All">
        <rdfs:subClassOf rdf:resource="http://www.wageneder.at/ontology/bpmn2.0#MultiInstanceBehaviour"/>
    </owl:Class>
    


    <!-- http://www.wageneder.at/ontology/bpmn2.0#Artifact -->

    <owl:Class rdf:about="http://www.wageneder.at/ontology/bpmn2.0#Artifact">
        <rdfs:subClassOf rdf:resource="http://www.wageneder.at/ontology/bpmn2.0#ArtifactLevel"/>
        <rdfs:subClassOf rdf:resource="http://www.wageneder.at/ontology/bpmn2.0#BaseElement"/>
        <rdfs:comment>BPMN provides modelers with the capability of showing additional information about a Process that is not directly related to the Sequence Flows or Message Flows of the Process.
At this point, BPMN provides three standard Artifacts: Associations, Groups, and Text Annotations.</rdfs:comment>
    </owl:Class>
    


    <!-- http://www.wageneder.at/ontology/bpmn2.0#ArtifactLevel -->

    <owl:Class rdf:about="http://www.wageneder.at/ontology/bpmn2.0#ArtifactLevel">
        <rdfs:subClassOf rdf:resource="http://www.wageneder.at/ontology/bpmn2.0#Common"/>
        <rdfs:comment>This is just a hierarchical element for organisational purposes.
It presents the Artifacts Folder</rdfs:comment>
    </owl:Class>
    


    <!-- http://www.wageneder.at/ontology/bpmn2.0#Assignment -->

    <owl:Class rdf:about="http://www.wageneder.at/ontology/bpmn2.0#Assignment">
        <rdfs:subClassOf rdf:resource="http://www.wageneder.at/ontology/bpmn2.0#BaseElement"/>
        <rdfs:subClassOf rdf:resource="http://www.wageneder.at/ontology/bpmn2.0#DataLevel"/>
        <rdfs:subClassOf>
            <owl:Restriction>
                <owl:onProperty rdf:resource="http://www.wageneder.at/ontology/bpmn2.0#hasFrom"/>
                <owl:qualifiedCardinality rdf:datatype="http://www.w3.org/2001/XMLSchema#nonNegativeInteger">1</owl:qualifiedCardinality>
                <owl:onClass rdf:resource="http://www.wageneder.at/ontology/bpmn2.0#Expression"/>
            </owl:Restriction>
        </rdfs:subClassOf>
        <rdfs:subClassOf>
            <owl:Restriction>
                <owl:onProperty rdf:resource="http://www.wageneder.at/ontology/bpmn2.0#hasTo"/>
                <owl:qualifiedCardinality rdf:datatype="http://www.w3.org/2001/XMLSchema#nonNegativeInteger">1</owl:qualifiedCardinality>
                <owl:onClass rdf:resource="http://www.wageneder.at/ontology/bpmn2.0#Expression"/>
            </owl:Restriction>
        </rdfs:subClassOf>
        <rdfs:comment>The Assignment element inherits the attributes and model associations of BaseElement (see Table 8.5). Table 10.64 presents the additional attributes of the Assignment element.</rdfs:comment>
    </owl:Class>
    


    <!-- http://www.wageneder.at/ontology/bpmn2.0#Association -->

    <owl:Class rdf:about="http://www.wageneder.at/ontology/bpmn2.0#Association">
        <rdfs:subClassOf rdf:resource="http://www.wageneder.at/ontology/bpmn2.0#Artifact"/>
        <rdfs:subClassOf>
            <owl:Restriction>
                <owl:onProperty rdf:resource="http://www.wageneder.at/ontology/bpmn2.0#hasAssociationDirection"/>
                <owl:qualifiedCardinality rdf:datatype="http://www.w3.org/2001/XMLSchema#nonNegativeInteger">1</owl:qualifiedCardinality>
                <owl:onClass rdf:resource="http://www.wageneder.at/ontology/bpmn2.0#AssociationDirection"/>
            </owl:Restriction>
        </rdfs:subClassOf>
        <rdfs:subClassOf>
            <owl:Restriction>
                <owl:onProperty rdf:resource="http://www.wageneder.at/ontology/bpmn2.0#hasSourceRef"/>
                <owl:qualifiedCardinality rdf:datatype="http://www.w3.org/2001/XMLSchema#nonNegativeInteger">1</owl:qualifiedCardinality>
                <owl:onClass rdf:resource="http://www.wageneder.at/ontology/bpmn2.0#BaseElement"/>
            </owl:Restriction>
        </rdfs:subClassOf>
        <rdfs:subClassOf>
            <owl:Restriction>
                <owl:onProperty rdf:resource="http://www.wageneder.at/ontology/bpmn2.0#hasTargetRef"/>
                <owl:qualifiedCardinality rdf:datatype="http://www.w3.org/2001/XMLSchema#nonNegativeInteger">1</owl:qualifiedCardinality>
                <owl:onClass rdf:resource="http://www.wageneder.at/ontology/bpmn2.0#BaseElement"/>
            </owl:Restriction>
        </rdfs:subClassOf>
        <rdfs:comment>An Association is used to associate information and Artifacts with Flow Objects. Text and graphical non-Flow Objects can be associated with the Flow Objects and Flow. An Association is also used to show the Activity used for compensation.</rdfs:comment>
    </owl:Class>
    


    <!-- http://www.wageneder.at/ontology/bpmn2.0#AssociationDirection -->

    <owl:Class rdf:about="http://www.wageneder.at/ontology/bpmn2.0#AssociationDirection">
        <rdfs:subClassOf rdf:resource="http://www.wageneder.at/ontology/bpmn2.0#ArtifactLevel"/>
        <rdfs:subClassOf>
            <owl:Class>
                <owl:unionOf rdf:parseType="Collection">
                    <rdf:Description rdf:about="http://www.wageneder.at/ontology/bpmn2.0#Both"/>
                    <rdf:Description rdf:about="http://www.wageneder.at/ontology/bpmn2.0#None"/>
                    <rdf:Description rdf:about="http://www.wageneder.at/ontology/bpmn2.0#One"/>
                </owl:unionOf>
            </owl:Class>
        </rdfs:subClassOf>
        <rdfs:comment>associationDirection is an attribute that defines whether or not the Association shows any directionality with an arrowhead. The default is None (no arrowhead). A value of One means that the arrowhead SHALL be at the Target Object. A value of Both means that there SHALL be an arrowhead at both ends of the Association line.</rdfs:comment>
    </owl:Class>
    


    <!-- http://www.wageneder.at/ontology/bpmn2.0#Auditing -->

    <owl:Class rdf:about="http://www.wageneder.at/ontology/bpmn2.0#Auditing">
        <rdfs:subClassOf rdf:resource="http://www.wageneder.at/ontology/bpmn2.0#BaseElement"/>
        <rdfs:subClassOf rdf:resource="http://www.wageneder.at/ontology/bpmn2.0#ProcessLevel"/>
        <rdfs:comment>The Auditing element and its model associations allow defining attributes related to auditing. It leverages the BPMN extensibility mechanism. This element is used by FlowElements and Process. The actual definition of auditing attributes is out of scope of this specification. BPMN 2.0 implementations can define their own set of attributes and their intended semantics.</rdfs:comment>
    </owl:Class>
    


    <!-- http://www.wageneder.at/ontology/bpmn2.0#BPMNCore -->

    <owl:Class rdf:about="http://www.wageneder.at/ontology/bpmn2.0#BPMNCore"/>
    


    <!-- http://www.wageneder.at/ontology/bpmn2.0#BPMNDI -->

    <owl:Class rdf:about="http://www.wageneder.at/ontology/bpmn2.0#BPMNDI">
        <rdfs:comment>This is just a hierarchical element for organisational purposes.
It presents the BPMNDI Folder</rdfs:comment>
    </owl:Class>
    


    <!-- http://www.wageneder.at/ontology/bpmn2.0#BPMNDiagram -->

    <owl:Class rdf:about="http://www.wageneder.at/ontology/bpmn2.0#BPMNDiagram">
        <rdfs:subClassOf rdf:resource="http://www.wageneder.at/ontology/bpmn2.0#BPMNDI"/>
        <rdfs:subClassOf rdf:resource="http://www.wageneder.at/ontology/bpmn2.0#BaseElement"/>
        <rdfs:comment>BPMNDiagram represents a depiction of all or part of a BPMN model.</rdfs:comment>
    </owl:Class>
    


    <!-- http://www.wageneder.at/ontology/bpmn2.0#Backward -->

    <owl:Class rdf:about="http://www.wageneder.at/ontology/bpmn2.0#Backward">
        <rdfs:subClassOf rdf:resource="http://www.wageneder.at/ontology/bpmn2.0#RelationshipDirection"/>
    </owl:Class>
    


    <!-- http://www.wageneder.at/ontology/bpmn2.0#BaseElement -->

    <owl:Class rdf:about="http://www.wageneder.at/ontology/bpmn2.0#BaseElement">
        <rdfs:subClassOf rdf:resource="http://www.wageneder.at/ontology/bpmn2.0#Foundation"/>
        <rdfs:subClassOf>
            <owl:Restriction>
                <owl:onProperty rdf:resource="http://www.wageneder.at/ontology/bpmn2.0#hasDocumentation"/>
                <owl:minQualifiedCardinality rdf:datatype="http://www.w3.org/2001/XMLSchema#nonNegativeInteger">0</owl:minQualifiedCardinality>
                <owl:onClass rdf:resource="http://www.wageneder.at/ontology/bpmn2.0#Documentation"/>
            </owl:Restriction>
        </rdfs:subClassOf>
        <rdfs:subClassOf>
            <owl:Restriction>
                <owl:onProperty rdf:resource="http://www.wageneder.at/ontology/bpmn2.0#hasExtensionDefinitions"/>
                <owl:minQualifiedCardinality rdf:datatype="http://www.w3.org/2001/XMLSchema#nonNegativeInteger">0</owl:minQualifiedCardinality>
                <owl:onClass rdf:resource="http://www.wageneder.at/ontology/bpmn2.0#ExtensionDefinition"/>
            </owl:Restriction>
        </rdfs:subClassOf>
        <rdfs:subClassOf>
            <owl:Restriction>
                <owl:onProperty rdf:resource="http://www.wageneder.at/ontology/bpmn2.0#hasExtensionValues"/>
                <owl:minQualifiedCardinality rdf:datatype="http://www.w3.org/2001/XMLSchema#nonNegativeInteger">0</owl:minQualifiedCardinality>
                <owl:onClass rdf:resource="http://www.wageneder.at/ontology/bpmn2.0#ExtensionAttributeValue"/>
            </owl:Restriction>
        </rdfs:subClassOf>
        <rdfs:subClassOf>
            <owl:Restriction>
                <owl:onProperty rdf:resource="http://www.wageneder.at/ontology/bpmn2.0#id"/>
                <owl:qualifiedCardinality rdf:datatype="http://www.w3.org/2001/XMLSchema#nonNegativeInteger">1</owl:qualifiedCardinality>
                <owl:onDataRange rdf:resource="http://www.w3.org/2001/XMLSchema#string"/>
            </owl:Restriction>
        </rdfs:subClassOf>
        <rdfs:comment rdf:datatype="http://www.w3.org/2001/XMLSchema#string">BaseElement is the abstract super class for most BPMN elements. It provides the attributes id and documentation, which other elements will inherit.</rdfs:comment>
        <rdfs:label xml:lang="de">BaseElement</rdfs:label>
    </owl:Class>
    


    <!-- http://www.wageneder.at/ontology/bpmn2.0#Both -->

    <owl:Class rdf:about="http://www.wageneder.at/ontology/bpmn2.0#Both">
        <rdfs:subClassOf rdf:resource="http://www.wageneder.at/ontology/bpmn2.0#AssociationDirection"/>
        <rdfs:subClassOf rdf:resource="http://www.wageneder.at/ontology/bpmn2.0#RelationshipDirection"/>
    </owl:Class>
    


    <!-- http://www.wageneder.at/ontology/bpmn2.0#BoundaryEvent -->

    <owl:Class rdf:about="http://www.wageneder.at/ontology/bpmn2.0#BoundaryEvent">
        <rdfs:subClassOf rdf:resource="http://www.wageneder.at/ontology/bpmn2.0#CatchEvent"/>
        <rdfs:subClassOf>
            <owl:Restriction>
                <owl:onProperty rdf:resource="http://www.wageneder.at/ontology/bpmn2.0#hasAttachedToRef"/>
                <owl:qualifiedCardinality rdf:datatype="http://www.w3.org/2001/XMLSchema#nonNegativeInteger">1</owl:qualifiedCardinality>
                <owl:onClass rdf:resource="http://www.wageneder.at/ontology/bpmn2.0#Activity"/>
            </owl:Restriction>
        </rdfs:subClassOf>
        <rdfs:subClassOf>
            <owl:Restriction>
                <owl:onProperty rdf:resource="http://www.wageneder.at/ontology/bpmn2.0#cancelActivity"/>
                <owl:qualifiedCardinality rdf:datatype="http://www.w3.org/2001/XMLSchema#nonNegativeInteger">1</owl:qualifiedCardinality>
                <owl:onDataRange rdf:resource="http://www.w3.org/2001/XMLSchema#boolean"/>
            </owl:Restriction>
        </rdfs:subClassOf>
    </owl:Class>
    


    <!-- http://www.wageneder.at/ontology/bpmn2.0#BusinessRuleTask -->

    <owl:Class rdf:about="http://www.wageneder.at/ontology/bpmn2.0#BusinessRuleTask">
        <rdfs:subClassOf rdf:resource="http://www.wageneder.at/ontology/bpmn2.0#Task"/>
        <rdfs:subClassOf>
            <owl:Restriction>
                <owl:onProperty rdf:resource="http://www.wageneder.at/ontology/bpmn2.0#implementation"/>
                <owl:qualifiedCardinality rdf:datatype="http://www.w3.org/2001/XMLSchema#nonNegativeInteger">1</owl:qualifiedCardinality>
                <owl:onDataRange rdf:resource="http://www.w3.org/2001/XMLSchema#string"/>
            </owl:Restriction>
        </rdfs:subClassOf>
        <rdfs:comment>A Business Rule Task provides a mechanism for the Process to provide input to a Business Rules Engine and to get the output of calculations that the Business Rules Engine might provide. The InputOutputSpecification of the Task (see page 211) will allow the Process to send data to and receive data from the Business Rules Engine.</rdfs:comment>
    </owl:Class>
    


    <!-- http://www.wageneder.at/ontology/bpmn2.0#CMOF -->

    <owl:Class rdf:about="http://www.wageneder.at/ontology/bpmn2.0#CMOF">
        <rdfs:comment>This is just a hierarchical element for organisational purposes.
It presents the CMOF Folder</rdfs:comment>
    </owl:Class>
    


    <!-- http://www.wageneder.at/ontology/bpmn2.0#CallActivity -->

    <owl:Class rdf:about="http://www.wageneder.at/ontology/bpmn2.0#CallActivity">
        <rdfs:subClassOf rdf:resource="http://www.wageneder.at/ontology/bpmn2.0#SubProcess"/>
        <rdfs:subClassOf>
            <owl:Restriction>
                <owl:onProperty rdf:resource="http://www.wageneder.at/ontology/bpmn2.0#hasCalledElement"/>
                <owl:minQualifiedCardinality rdf:datatype="http://www.w3.org/2001/XMLSchema#nonNegativeInteger">0</owl:minQualifiedCardinality>
                <owl:onClass rdf:resource="http://www.wageneder.at/ontology/bpmn2.0#CallableElement"/>
            </owl:Restriction>
        </rdfs:subClassOf>
        <rdfs:subClassOf>
            <owl:Restriction>
                <owl:onProperty rdf:resource="http://www.wageneder.at/ontology/bpmn2.0#hasCalledElement"/>
                <owl:maxQualifiedCardinality rdf:datatype="http://www.w3.org/2001/XMLSchema#nonNegativeInteger">1</owl:maxQualifiedCardinality>
                <owl:onClass rdf:resource="http://www.wageneder.at/ontology/bpmn2.0#CallableElement"/>
            </owl:Restriction>
        </rdfs:subClassOf>
        <rdfs:comment>A Call Activity identifies a point in the Process where a global Process or a Global Task is used. The Call Activity acts as a ‘wrapper’ for the invocation of a global Process or Global Task within the execution. The activation of a call Activity results in the transfer of control to the called global Process or Global Task.</rdfs:comment>
    </owl:Class>
    


    <!-- http://www.wageneder.at/ontology/bpmn2.0#CallConversation -->

    <owl:Class rdf:about="http://www.wageneder.at/ontology/bpmn2.0#CallConversation">
        <rdfs:subClassOf rdf:resource="http://www.wageneder.at/ontology/bpmn2.0#ConversationNode"/>
        <rdfs:subClassOf>
            <owl:Restriction>
                <owl:onProperty rdf:resource="http://www.wageneder.at/ontology/bpmn2.0#hasCalledCollaborationRef"/>
                <owl:minQualifiedCardinality rdf:datatype="http://www.w3.org/2001/XMLSchema#nonNegativeInteger">0</owl:minQualifiedCardinality>
                <owl:onClass rdf:resource="http://www.wageneder.at/ontology/bpmn2.0#Collaboration"/>
            </owl:Restriction>
        </rdfs:subClassOf>
        <rdfs:subClassOf>
            <owl:Restriction>
                <owl:onProperty rdf:resource="http://www.wageneder.at/ontology/bpmn2.0#hasParticipantAssociations"/>
                <owl:minQualifiedCardinality rdf:datatype="http://www.w3.org/2001/XMLSchema#nonNegativeInteger">0</owl:minQualifiedCardinality>
                <owl:onClass rdf:resource="http://www.wageneder.at/ontology/bpmn2.0#ParticipantAssociation"/>
            </owl:Restriction>
        </rdfs:subClassOf>
        <rdfs:subClassOf>
            <owl:Restriction>
                <owl:onProperty rdf:resource="http://www.wageneder.at/ontology/bpmn2.0#hasCalledCollaborationRef"/>
                <owl:maxQualifiedCardinality rdf:datatype="http://www.w3.org/2001/XMLSchema#nonNegativeInteger">1</owl:maxQualifiedCardinality>
                <owl:onClass rdf:resource="http://www.wageneder.at/ontology/bpmn2.0#Collaboration"/>
            </owl:Restriction>
        </rdfs:subClassOf>
        <rdfs:comment>The Call Conversation element inherits the attributes and model associations of ConversationNode (see Table 9.10). Table 9.12 presents the additional model associations for the Call Conversation element.</rdfs:comment>
    </owl:Class>
    


    <!-- http://www.wageneder.at/ontology/bpmn2.0#CallableElement -->

    <owl:Class rdf:about="http://www.wageneder.at/ontology/bpmn2.0#CallableElement">
        <rdfs:subClassOf rdf:resource="http://www.wageneder.at/ontology/bpmn2.0#Common"/>
        <rdfs:subClassOf rdf:resource="http://www.wageneder.at/ontology/bpmn2.0#RootElement"/>
        <rdfs:subClassOf>
            <owl:Restriction>
                <owl:onProperty rdf:resource="http://www.wageneder.at/ontology/bpmn2.0#hasIOBinding"/>
                <owl:minQualifiedCardinality rdf:datatype="http://www.w3.org/2001/XMLSchema#nonNegativeInteger">0</owl:minQualifiedCardinality>
                <owl:onClass rdf:resource="http://www.wageneder.at/ontology/bpmn2.0#InputOutputBinding"/>
            </owl:Restriction>
        </rdfs:subClassOf>
        <rdfs:subClassOf>
            <owl:Restriction>
                <owl:onProperty rdf:resource="http://www.wageneder.at/ontology/bpmn2.0#hasIOSpecification"/>
                <owl:minQualifiedCardinality rdf:datatype="http://www.w3.org/2001/XMLSchema#nonNegativeInteger">0</owl:minQualifiedCardinality>
                <owl:onClass rdf:resource="http://www.wageneder.at/ontology/bpmn2.0#InputOutputSpecification"/>
            </owl:Restriction>
        </rdfs:subClassOf>
        <rdfs:subClassOf>
            <owl:Restriction>
                <owl:onProperty rdf:resource="http://www.wageneder.at/ontology/bpmn2.0#hasSupportedInterfaceRefs"/>
                <owl:minQualifiedCardinality rdf:datatype="http://www.w3.org/2001/XMLSchema#nonNegativeInteger">0</owl:minQualifiedCardinality>
                <owl:onClass rdf:resource="http://www.wageneder.at/ontology/bpmn2.0#EndPoint"/>
            </owl:Restriction>
        </rdfs:subClassOf>
        <rdfs:subClassOf>
            <owl:Restriction>
                <owl:onProperty rdf:resource="http://www.wageneder.at/ontology/bpmn2.0#hasIOSpecification"/>
                <owl:maxQualifiedCardinality rdf:datatype="http://www.w3.org/2001/XMLSchema#nonNegativeInteger">1</owl:maxQualifiedCardinality>
                <owl:onClass rdf:resource="http://www.wageneder.at/ontology/bpmn2.0#InputOutputSpecification"/>
            </owl:Restriction>
        </rdfs:subClassOf>
        <rdfs:subClassOf>
            <owl:Restriction>
                <owl:onProperty rdf:resource="http://www.wageneder.at/ontology/bpmn2.0#name"/>
                <owl:minQualifiedCardinality rdf:datatype="http://www.w3.org/2001/XMLSchema#nonNegativeInteger">0</owl:minQualifiedCardinality>
                <owl:onDataRange rdf:resource="http://www.w3.org/2001/XMLSchema#string"/>
            </owl:Restriction>
        </rdfs:subClassOf>
        <rdfs:subClassOf>
            <owl:Restriction>
                <owl:onProperty rdf:resource="http://www.wageneder.at/ontology/bpmn2.0#name"/>
                <owl:maxQualifiedCardinality rdf:datatype="http://www.w3.org/2001/XMLSchema#nonNegativeInteger">1</owl:maxQualifiedCardinality>
                <owl:onDataRange rdf:resource="http://www.w3.org/2001/XMLSchema#string"/>
            </owl:Restriction>
        </rdfs:subClassOf>
        <rdfs:comment>CallableElement is the abstract super class of all Activities that have been defined outside of a Process or
Choreography but which can be called (or reused), by a Call Activity, from within a Process or Choreography. It
MAY reference Interfaces that define the service operations that it provides. The BPMN elements that can be called
by Call Activities (i.e., are CallableElements) are: Process and GlobalTask (see Figure 10.43).
CallableElements are RootElements, which can be imported and used in other Definitions. When
CallableElements (e.g., Process) are defined, they are contained within Definitions.
Figure 10.43</rdfs:comment>
    </owl:Class>
    


    <!-- http://www.wageneder.at/ontology/bpmn2.0#CancelEventDefinition -->

    <owl:Class rdf:about="http://www.wageneder.at/ontology/bpmn2.0#CancelEventDefinition">
        <rdfs:subClassOf rdf:resource="http://www.wageneder.at/ontology/bpmn2.0#EventDefinition"/>
        <rdfs:comment>Cancel Events are only used in the context of modeling Transaction Sub-Processes (see page 178 for more details
on Transactions). There are two variations: a catch Intermediate Event and an End Event.</rdfs:comment>
    </owl:Class>
    


    <!-- http://www.wageneder.at/ontology/bpmn2.0#CatchEvent -->

    <owl:Class rdf:about="http://www.wageneder.at/ontology/bpmn2.0#CatchEvent">
        <rdfs:subClassOf rdf:resource="http://www.wageneder.at/ontology/bpmn2.0#Event"/>
        <rdfs:subClassOf>
            <owl:Restriction>
                <owl:onProperty rdf:resource="http://www.wageneder.at/ontology/bpmn2.0#hasDataOutputAssociations"/>
                <owl:minQualifiedCardinality rdf:datatype="http://www.w3.org/2001/XMLSchema#nonNegativeInteger">0</owl:minQualifiedCardinality>
                <owl:onClass rdf:resource="http://www.wageneder.at/ontology/bpmn2.0#DataOutputAssociation"/>
            </owl:Restriction>
        </rdfs:subClassOf>
        <rdfs:subClassOf>
            <owl:Restriction>
                <owl:onProperty rdf:resource="http://www.wageneder.at/ontology/bpmn2.0#hasDataOutputs"/>
                <owl:minQualifiedCardinality rdf:datatype="http://www.w3.org/2001/XMLSchema#nonNegativeInteger">0</owl:minQualifiedCardinality>
                <owl:onClass rdf:resource="http://www.wageneder.at/ontology/bpmn2.0#DataOutput"/>
            </owl:Restriction>
        </rdfs:subClassOf>
        <rdfs:subClassOf>
            <owl:Restriction>
                <owl:onProperty rdf:resource="http://www.wageneder.at/ontology/bpmn2.0#hasEventDefinitionRefs"/>
                <owl:minQualifiedCardinality rdf:datatype="http://www.w3.org/2001/XMLSchema#nonNegativeInteger">0</owl:minQualifiedCardinality>
                <owl:onClass rdf:resource="http://www.wageneder.at/ontology/bpmn2.0#EventDefinition"/>
            </owl:Restriction>
        </rdfs:subClassOf>
        <rdfs:subClassOf>
            <owl:Restriction>
                <owl:onProperty rdf:resource="http://www.wageneder.at/ontology/bpmn2.0#hasEventDefinitions"/>
                <owl:minQualifiedCardinality rdf:datatype="http://www.w3.org/2001/XMLSchema#nonNegativeInteger">0</owl:minQualifiedCardinality>
                <owl:onClass rdf:resource="http://www.wageneder.at/ontology/bpmn2.0#EventDefinition"/>
            </owl:Restriction>
        </rdfs:subClassOf>
        <rdfs:subClassOf>
            <owl:Restriction>
                <owl:onProperty rdf:resource="http://www.wageneder.at/ontology/bpmn2.0#hasOutputSet"/>
                <owl:minQualifiedCardinality rdf:datatype="http://www.w3.org/2001/XMLSchema#nonNegativeInteger">0</owl:minQualifiedCardinality>
                <owl:onClass rdf:resource="http://www.wageneder.at/ontology/bpmn2.0#OutputSet"/>
            </owl:Restriction>
        </rdfs:subClassOf>
        <rdfs:subClassOf>
            <owl:Restriction>
                <owl:onProperty rdf:resource="http://www.wageneder.at/ontology/bpmn2.0#hasEventDefinitions"/>
                <owl:maxQualifiedCardinality rdf:datatype="http://www.w3.org/2001/XMLSchema#nonNegativeInteger">1</owl:maxQualifiedCardinality>
                <owl:onClass rdf:resource="http://www.wageneder.at/ontology/bpmn2.0#EventDefinition"/>
            </owl:Restriction>
        </rdfs:subClassOf>
        <rdfs:subClassOf>
            <owl:Restriction>
                <owl:onProperty rdf:resource="http://www.wageneder.at/ontology/bpmn2.0#hasOutputSet"/>
                <owl:maxQualifiedCardinality rdf:datatype="http://www.w3.org/2001/XMLSchema#nonNegativeInteger">1</owl:maxQualifiedCardinality>
                <owl:onClass rdf:resource="http://www.wageneder.at/ontology/bpmn2.0#OutputSet"/>
            </owl:Restriction>
        </rdfs:subClassOf>
        <rdfs:subClassOf>
            <owl:Restriction>
                <owl:onProperty rdf:resource="http://www.wageneder.at/ontology/bpmn2.0#parallelMultiple"/>
                <owl:qualifiedCardinality rdf:datatype="http://www.w3.org/2001/XMLSchema#nonNegativeInteger">1</owl:qualifiedCardinality>
                <owl:onDataRange rdf:resource="http://www.w3.org/2001/XMLSchema#boolean"/>
            </owl:Restriction>
        </rdfs:subClassOf>
        <owl:disjointWith rdf:resource="http://www.wageneder.at/ontology/bpmn2.0#ThrowEvent"/>
        <rdfs:comment>The CatchEvent element inherits the attributes and model associations of Event element</rdfs:comment>
    </owl:Class>
    


    <!-- http://www.wageneder.at/ontology/bpmn2.0#Category -->

    <owl:Class rdf:about="http://www.wageneder.at/ontology/bpmn2.0#Category">
        <rdfs:subClassOf rdf:resource="http://www.wageneder.at/ontology/bpmn2.0#ArtifactLevel"/>
        <rdfs:subClassOf rdf:resource="http://www.wageneder.at/ontology/bpmn2.0#RootElement"/>
        <rdfs:subClassOf>
            <owl:Restriction>
                <owl:onProperty rdf:resource="http://www.wageneder.at/ontology/bpmn2.0#hasCategoryValue"/>
                <owl:minQualifiedCardinality rdf:datatype="http://www.w3.org/2001/XMLSchema#nonNegativeInteger">0</owl:minQualifiedCardinality>
                <owl:onClass rdf:resource="http://www.wageneder.at/ontology/bpmn2.0#CategoryValue"/>
            </owl:Restriction>
        </rdfs:subClassOf>
        <rdfs:subClassOf>
            <owl:Restriction>
                <owl:onProperty rdf:resource="http://www.wageneder.at/ontology/bpmn2.0#name"/>
                <owl:qualifiedCardinality rdf:datatype="http://www.w3.org/2001/XMLSchema#nonNegativeInteger">1</owl:qualifiedCardinality>
                <owl:onDataRange rdf:resource="http://www.w3.org/2001/XMLSchema#string"/>
            </owl:Restriction>
        </rdfs:subClassOf>
        <rdfs:comment>Categories, which have user-defined semantics, can be used for documentation or analysis purposes. For example, FlowElements can be categorized as being customer oriented vs. support oriented. Furthermore, the cost and time of Activities per Category can be calculated.</rdfs:comment>
        <rdfs:comment>The Category element inherits the attributes and model associations of BaseElement (see Table 8.5) through its relationship to RootElement. Table 8.22 displays the additional model associations of the Category element.</rdfs:comment>
    </owl:Class>
    


    <!-- http://www.wageneder.at/ontology/bpmn2.0#CategoryValue -->

    <owl:Class rdf:about="http://www.wageneder.at/ontology/bpmn2.0#CategoryValue">
        <rdfs:subClassOf rdf:resource="http://www.wageneder.at/ontology/bpmn2.0#ArtifactLevel"/>
        <rdfs:subClassOf rdf:resource="http://www.wageneder.at/ontology/bpmn2.0#BaseElement"/>
        <rdfs:subClassOf>
            <owl:Restriction>
                <owl:onProperty rdf:resource="http://www.wageneder.at/ontology/bpmn2.0#hasCategorizedFlowElements"/>
                <owl:minQualifiedCardinality rdf:datatype="http://www.w3.org/2001/XMLSchema#nonNegativeInteger">0</owl:minQualifiedCardinality>
                <owl:onClass rdf:resource="http://www.wageneder.at/ontology/bpmn2.0#FlowElement"/>
            </owl:Restriction>
        </rdfs:subClassOf>
        <rdfs:subClassOf>
            <owl:Restriction>
                <owl:onProperty rdf:resource="http://www.wageneder.at/ontology/bpmn2.0#hasCategory"/>
                <owl:minQualifiedCardinality rdf:datatype="http://www.w3.org/2001/XMLSchema#nonNegativeInteger">0</owl:minQualifiedCardinality>
                <owl:onClass rdf:resource="http://www.wageneder.at/ontology/bpmn2.0#Category"/>
            </owl:Restriction>
        </rdfs:subClassOf>
        <rdfs:subClassOf>
            <owl:Restriction>
                <owl:onProperty rdf:resource="http://www.wageneder.at/ontology/bpmn2.0#hasCategory"/>
                <owl:maxQualifiedCardinality rdf:datatype="http://www.w3.org/2001/XMLSchema#nonNegativeInteger">1</owl:maxQualifiedCardinality>
                <owl:onClass rdf:resource="http://www.wageneder.at/ontology/bpmn2.0#Category"/>
            </owl:Restriction>
        </rdfs:subClassOf>
        <rdfs:subClassOf>
            <owl:Restriction>
                <owl:onProperty rdf:resource="http://www.wageneder.at/ontology/bpmn2.0#value"/>
                <owl:qualifiedCardinality rdf:datatype="http://www.w3.org/2001/XMLSchema#nonNegativeInteger">1</owl:qualifiedCardinality>
                <owl:onDataRange rdf:resource="http://www.w3.org/2001/XMLSchema#string"/>
            </owl:Restriction>
        </rdfs:subClassOf>
        <rdfs:comment>Categories, which have user-defined semantics, can be used for documentation or analysis purposes. For example, FlowElements can be categorized as being customer oriented vs. support oriented. Furthermore, the cost and time of Activities per Category can be calculated.
Groups are one way in which Categories of objects can be visually displayed on the diagram. That is, a Group is a visual depiction of a single CategoryValue.</rdfs:comment>
    </owl:Class>
    


    <!-- http://www.wageneder.at/ontology/bpmn2.0#Choreography -->

    <owl:Class rdf:about="http://www.wageneder.at/ontology/bpmn2.0#Choreography">
        <rdfs:subClassOf rdf:resource="http://www.wageneder.at/ontology/bpmn2.0#ChoreographyLevel"/>
        <rdfs:subClassOf rdf:resource="http://www.wageneder.at/ontology/bpmn2.0#Collaboration"/>
        <rdfs:subClassOf rdf:resource="http://www.wageneder.at/ontology/bpmn2.0#FlowElementsContainer"/>
        <rdfs:subClassOf>
            <owl:Restriction>
                <owl:onProperty rdf:resource="http://www.wageneder.at/ontology/bpmn2.0#hasCollaboration"/>
                <owl:minQualifiedCardinality rdf:datatype="http://www.w3.org/2001/XMLSchema#nonNegativeInteger">0</owl:minQualifiedCardinality>
                <owl:onClass rdf:resource="http://www.wageneder.at/ontology/bpmn2.0#Collaboration"/>
            </owl:Restriction>
        </rdfs:subClassOf>
        <rdfs:comment>The Choreography element inherits the attributes and model associations of Collaboration (see Table 9.1) and of FlowElementContainer (see Table 8.45), but does not have any additional attributes or model associations.</rdfs:comment>
    </owl:Class>
    


    <!-- http://www.wageneder.at/ontology/bpmn2.0#ChoreographyActivity -->

    <owl:Class rdf:about="http://www.wageneder.at/ontology/bpmn2.0#ChoreographyActivity">
        <rdfs:subClassOf rdf:resource="http://www.wageneder.at/ontology/bpmn2.0#FlowNode"/>
        <rdfs:comment>A Choreography Activity represents a point in a Choreography flow where an interaction occurs between two or more Participants.</rdfs:comment>
    </owl:Class>
    


    <!-- http://www.wageneder.at/ontology/bpmn2.0#ChoreographyLevel -->

    <owl:Class rdf:about="http://www.wageneder.at/ontology/bpmn2.0#ChoreographyLevel">
        <rdfs:subClassOf rdf:resource="http://www.wageneder.at/ontology/bpmn2.0#Common"/>
        <rdfs:comment>This is just a hierarchical element for organisational purposes.
It presents the Choreography Folder</rdfs:comment>
    </owl:Class>
    


    <!-- http://www.wageneder.at/ontology/bpmn2.0#Collaboration -->

    <owl:Class rdf:about="http://www.wageneder.at/ontology/bpmn2.0#Collaboration">
        <rdfs:subClassOf rdf:resource="http://www.wageneder.at/ontology/bpmn2.0#CollaborationLevel"/>
        <rdfs:subClassOf rdf:resource="http://www.wageneder.at/ontology/bpmn2.0#RootElement"/>
        <rdfs:subClassOf>
            <owl:Restriction>
                <owl:onProperty rdf:resource="http://www.wageneder.at/ontology/bpmn2.0#hasArtifacts"/>
                <owl:minQualifiedCardinality rdf:datatype="http://www.w3.org/2001/XMLSchema#nonNegativeInteger">0</owl:minQualifiedCardinality>
                <owl:onClass rdf:resource="http://www.wageneder.at/ontology/bpmn2.0#Artifact"/>
            </owl:Restriction>
        </rdfs:subClassOf>
        <rdfs:subClassOf>
            <owl:Restriction>
                <owl:onProperty rdf:resource="http://www.wageneder.at/ontology/bpmn2.0#hasChoreographyRef"/>
                <owl:minQualifiedCardinality rdf:datatype="http://www.w3.org/2001/XMLSchema#nonNegativeInteger">0</owl:minQualifiedCardinality>
                <owl:onClass rdf:resource="http://www.wageneder.at/ontology/bpmn2.0#Choreography"/>
            </owl:Restriction>
        </rdfs:subClassOf>
        <rdfs:subClassOf>
            <owl:Restriction>
                <owl:onProperty rdf:resource="http://www.wageneder.at/ontology/bpmn2.0#hasConversationLinks"/>
                <owl:minQualifiedCardinality rdf:datatype="http://www.w3.org/2001/XMLSchema#nonNegativeInteger">0</owl:minQualifiedCardinality>
                <owl:onClass rdf:resource="http://www.wageneder.at/ontology/bpmn2.0#ConversationLink"/>
            </owl:Restriction>
        </rdfs:subClassOf>
        <rdfs:subClassOf>
            <owl:Restriction>
                <owl:onProperty rdf:resource="http://www.wageneder.at/ontology/bpmn2.0#hasConversations"/>
                <owl:minQualifiedCardinality rdf:datatype="http://www.w3.org/2001/XMLSchema#nonNegativeInteger">0</owl:minQualifiedCardinality>
                <owl:onClass rdf:resource="http://www.wageneder.at/ontology/bpmn2.0#ConversationNode"/>
            </owl:Restriction>
        </rdfs:subClassOf>
        <rdfs:subClassOf>
            <owl:Restriction>
                <owl:onProperty rdf:resource="http://www.wageneder.at/ontology/bpmn2.0#hasCorrelationKeys"/>
                <owl:minQualifiedCardinality rdf:datatype="http://www.w3.org/2001/XMLSchema#nonNegativeInteger">0</owl:minQualifiedCardinality>
                <owl:onClass rdf:resource="http://www.wageneder.at/ontology/bpmn2.0#CorrelationKey"/>
            </owl:Restriction>
        </rdfs:subClassOf>
        <rdfs:subClassOf>
            <owl:Restriction>
                <owl:onProperty rdf:resource="http://www.wageneder.at/ontology/bpmn2.0#hasMessageFlow"/>
                <owl:minQualifiedCardinality rdf:datatype="http://www.w3.org/2001/XMLSchema#nonNegativeInteger">0</owl:minQualifiedCardinality>
                <owl:onClass rdf:resource="http://www.wageneder.at/ontology/bpmn2.0#MessageFlow"/>
            </owl:Restriction>
        </rdfs:subClassOf>
        <rdfs:subClassOf>
            <owl:Restriction>
                <owl:onProperty rdf:resource="http://www.wageneder.at/ontology/bpmn2.0#hasMessageFlowAssociations"/>
                <owl:minQualifiedCardinality rdf:datatype="http://www.w3.org/2001/XMLSchema#nonNegativeInteger">0</owl:minQualifiedCardinality>
                <owl:onClass rdf:resource="http://www.wageneder.at/ontology/bpmn2.0#MessageFlowAssociation"/>
            </owl:Restriction>
        </rdfs:subClassOf>
        <rdfs:subClassOf>
            <owl:Restriction>
                <owl:onProperty rdf:resource="http://www.wageneder.at/ontology/bpmn2.0#hasParticipantAssociations"/>
                <owl:minQualifiedCardinality rdf:datatype="http://www.w3.org/2001/XMLSchema#nonNegativeInteger">0</owl:minQualifiedCardinality>
                <owl:onClass rdf:resource="http://www.wageneder.at/ontology/bpmn2.0#ParticipantAssociation"/>
            </owl:Restriction>
        </rdfs:subClassOf>
        <rdfs:subClassOf>
            <owl:Restriction>
                <owl:onProperty rdf:resource="http://www.wageneder.at/ontology/bpmn2.0#hasParticipants"/>
                <owl:minQualifiedCardinality rdf:datatype="http://www.w3.org/2001/XMLSchema#nonNegativeInteger">0</owl:minQualifiedCardinality>
                <owl:onClass rdf:resource="http://www.wageneder.at/ontology/bpmn2.0#Participant"/>
            </owl:Restriction>
        </rdfs:subClassOf>
        <rdfs:subClassOf>
            <owl:Restriction>
                <owl:onProperty rdf:resource="http://www.wageneder.at/ontology/bpmn2.0#hasConversationAssociations"/>
                <owl:qualifiedCardinality rdf:datatype="http://www.w3.org/2001/XMLSchema#nonNegativeInteger">1</owl:qualifiedCardinality>
                <owl:onClass rdf:resource="http://www.wageneder.at/ontology/bpmn2.0#ConversationAssociation"/>
            </owl:Restriction>
        </rdfs:subClassOf>
        <rdfs:subClassOf>
            <owl:Restriction>
                <owl:onProperty rdf:resource="http://www.wageneder.at/ontology/bpmn2.0#isClosed"/>
                <owl:qualifiedCardinality rdf:datatype="http://www.w3.org/2001/XMLSchema#nonNegativeInteger">1</owl:qualifiedCardinality>
                <owl:onDataRange rdf:resource="http://www.w3.org/2001/XMLSchema#boolean"/>
            </owl:Restriction>
        </rdfs:subClassOf>
        <rdfs:subClassOf>
            <owl:Restriction>
                <owl:onProperty rdf:resource="http://www.wageneder.at/ontology/bpmn2.0#name"/>
                <owl:qualifiedCardinality rdf:datatype="http://www.w3.org/2001/XMLSchema#nonNegativeInteger">1</owl:qualifiedCardinality>
                <owl:onDataRange rdf:resource="http://www.w3.org/2001/XMLSchema#string"/>
            </owl:Restriction>
        </rdfs:subClassOf>
        <rdfs:comment>The Collaboration element inherits the attributes and model associations of BaseElement (see Table 8.5) through its relationship to RootElement. Table 9.1 presents the additional attributes and model associations for the Collaboration element.</rdfs:comment>
    </owl:Class>
    


    <!-- http://www.wageneder.at/ontology/bpmn2.0#CollaborationLevel -->

    <owl:Class rdf:about="http://www.wageneder.at/ontology/bpmn2.0#CollaborationLevel">
        <rdfs:subClassOf rdf:resource="http://www.wageneder.at/ontology/bpmn2.0#Common"/>
        <rdfs:comment>This is just a hierarchical element for organisational purposes.
It presents the Collaboration Folder</rdfs:comment>
    </owl:Class>
    


    <!-- http://www.wageneder.at/ontology/bpmn2.0#Common -->

    <owl:Class rdf:about="http://www.wageneder.at/ontology/bpmn2.0#Common">
        <rdfs:subClassOf rdf:resource="http://www.wageneder.at/ontology/bpmn2.0#BPMNCore"/>
        <rdfs:comment>This is just a hierarchical element for organisational purposes.</rdfs:comment>
    </owl:Class>
    


    <!-- http://www.wageneder.at/ontology/bpmn2.0#CompensationEventDefinition -->

    <owl:Class rdf:about="http://www.wageneder.at/ontology/bpmn2.0#CompensationEventDefinition">
        <rdfs:subClassOf rdf:resource="http://www.wageneder.at/ontology/bpmn2.0#EventDefinition"/>
        <rdfs:subClassOf>
            <owl:Restriction>
                <owl:onProperty rdf:resource="http://www.wageneder.at/ontology/bpmn2.0#hasActivityRef"/>
                <owl:minQualifiedCardinality rdf:datatype="http://www.w3.org/2001/XMLSchema#nonNegativeInteger">0</owl:minQualifiedCardinality>
                <owl:onClass rdf:resource="http://www.wageneder.at/ontology/bpmn2.0#Activity"/>
            </owl:Restriction>
        </rdfs:subClassOf>
        <rdfs:subClassOf>
            <owl:Restriction>
                <owl:onProperty rdf:resource="http://www.wageneder.at/ontology/bpmn2.0#hasActivityRef"/>
                <owl:maxQualifiedCardinality rdf:datatype="http://www.w3.org/2001/XMLSchema#nonNegativeInteger">1</owl:maxQualifiedCardinality>
                <owl:onClass rdf:resource="http://www.wageneder.at/ontology/bpmn2.0#Activity"/>
            </owl:Restriction>
        </rdfs:subClassOf>
        <rdfs:subClassOf>
            <owl:Restriction>
                <owl:onProperty rdf:resource="http://www.wageneder.at/ontology/bpmn2.0#waitForCompletion"/>
                <owl:qualifiedCardinality rdf:datatype="http://www.w3.org/2001/XMLSchema#nonNegativeInteger">1</owl:qualifiedCardinality>
                <owl:onDataRange rdf:resource="http://www.w3.org/2001/XMLSchema#boolean"/>
            </owl:Restriction>
        </rdfs:subClassOf>
        <rdfs:comment>Compensation Events are used in the context of triggering or handling compensation (see page 302 for more details on compensation). There are four variations: a Start Event, both a catch and throw Intermediate Event, and an End Event.</rdfs:comment>
    </owl:Class>
    


    <!-- http://www.wageneder.at/ontology/bpmn2.0#Complex -->

    <owl:Class rdf:about="http://www.wageneder.at/ontology/bpmn2.0#Complex">
        <rdfs:subClassOf rdf:resource="http://www.wageneder.at/ontology/bpmn2.0#MultiInstanceBehaviour"/>
    </owl:Class>
    


    <!-- http://www.wageneder.at/ontology/bpmn2.0#ComplexBehaviourDefinition -->

    <owl:Class rdf:about="http://www.wageneder.at/ontology/bpmn2.0#ComplexBehaviourDefinition">
        <rdfs:subClassOf rdf:resource="http://www.wageneder.at/ontology/bpmn2.0#ActivityLevel"/>
        <rdfs:subClassOf rdf:resource="http://www.wageneder.at/ontology/bpmn2.0#BaseElement"/>
        <rdfs:subClassOf>
            <owl:Restriction>
                <owl:onProperty rdf:resource="http://www.wageneder.at/ontology/bpmn2.0#hasEvent"/>
                <owl:minQualifiedCardinality rdf:datatype="http://www.w3.org/2001/XMLSchema#nonNegativeInteger">0</owl:minQualifiedCardinality>
                <owl:onClass rdf:resource="http://www.wageneder.at/ontology/bpmn2.0#ImplicitThrowEvent"/>
            </owl:Restriction>
        </rdfs:subClassOf>
        <rdfs:subClassOf>
            <owl:Restriction>
                <owl:onProperty rdf:resource="http://www.wageneder.at/ontology/bpmn2.0#hasEvent"/>
                <owl:maxQualifiedCardinality rdf:datatype="http://www.w3.org/2001/XMLSchema#nonNegativeInteger">1</owl:maxQualifiedCardinality>
                <owl:onClass rdf:resource="http://www.wageneder.at/ontology/bpmn2.0#ImplicitThrowEvent"/>
            </owl:Restriction>
        </rdfs:subClassOf>
        <rdfs:comment>The ComplexBehaviorDefinition element inherits the attributes and model associations of BaseElement (see Table 8.5). Table 10.31 presents the additional attributes and model associations for the ComplexBehaviorDefinition element.</rdfs:comment>
    </owl:Class>
    


    <!-- http://www.wageneder.at/ontology/bpmn2.0#ComplexGateway -->

    <owl:Class rdf:about="http://www.wageneder.at/ontology/bpmn2.0#ComplexGateway">
        <rdfs:subClassOf rdf:resource="http://www.wageneder.at/ontology/bpmn2.0#Gateway"/>
        <rdfs:subClassOf>
            <owl:Restriction>
                <owl:onProperty rdf:resource="http://www.wageneder.at/ontology/bpmn2.0#hasActivationCondition"/>
                <owl:minQualifiedCardinality rdf:datatype="http://www.w3.org/2001/XMLSchema#nonNegativeInteger">0</owl:minQualifiedCardinality>
                <owl:onClass rdf:resource="http://www.wageneder.at/ontology/bpmn2.0#Expression"/>
            </owl:Restriction>
        </rdfs:subClassOf>
        <rdfs:subClassOf>
            <owl:Restriction>
                <owl:onProperty rdf:resource="http://www.wageneder.at/ontology/bpmn2.0#hasDefault"/>
                <owl:minQualifiedCardinality rdf:datatype="http://www.w3.org/2001/XMLSchema#nonNegativeInteger">0</owl:minQualifiedCardinality>
                <owl:onClass rdf:resource="http://www.wageneder.at/ontology/bpmn2.0#SequenceFlow"/>
            </owl:Restriction>
        </rdfs:subClassOf>
        <rdfs:subClassOf>
            <owl:Restriction>
                <owl:onProperty rdf:resource="http://www.wageneder.at/ontology/bpmn2.0#hasActivationCondition"/>
                <owl:maxQualifiedCardinality rdf:datatype="http://www.w3.org/2001/XMLSchema#nonNegativeInteger">1</owl:maxQualifiedCardinality>
                <owl:onClass rdf:resource="http://www.wageneder.at/ontology/bpmn2.0#Expression"/>
            </owl:Restriction>
        </rdfs:subClassOf>
        <rdfs:subClassOf>
            <owl:Restriction>
                <owl:onProperty rdf:resource="http://www.wageneder.at/ontology/bpmn2.0#hasDefault"/>
                <owl:maxQualifiedCardinality rdf:datatype="http://www.w3.org/2001/XMLSchema#nonNegativeInteger">1</owl:maxQualifiedCardinality>
                <owl:onClass rdf:resource="http://www.wageneder.at/ontology/bpmn2.0#SequenceFlow"/>
            </owl:Restriction>
        </rdfs:subClassOf>
        <rdfs:subClassOf>
            <owl:Restriction>
                <owl:onProperty rdf:resource="http://www.wageneder.at/ontology/bpmn2.0#activationCount"/>
                <owl:qualifiedCardinality rdf:datatype="http://www.w3.org/2001/XMLSchema#nonNegativeInteger">1</owl:qualifiedCardinality>
                <owl:onDataRange rdf:resource="http://www.w3.org/2001/XMLSchema#integer"/>
            </owl:Restriction>
        </rdfs:subClassOf>
        <rdfs:subClassOf>
            <owl:Restriction>
                <owl:onProperty rdf:resource="http://www.wageneder.at/ontology/bpmn2.0#waitingForStart"/>
                <owl:qualifiedCardinality rdf:datatype="http://www.w3.org/2001/XMLSchema#nonNegativeInteger">1</owl:qualifiedCardinality>
                <owl:onDataRange rdf:resource="http://www.w3.org/2001/XMLSchema#boolean"/>
            </owl:Restriction>
        </rdfs:subClassOf>
        <rdfs:comment>The Complex Gateway can be used to model complex synchronization behavior. An Expression activationCondition is used to describe the precise behavior.</rdfs:comment>
    </owl:Class>
    


    <!-- http://www.wageneder.at/ontology/bpmn2.0#ConditionalEventDefinition -->

    <owl:Class rdf:about="http://www.wageneder.at/ontology/bpmn2.0#ConditionalEventDefinition">
        <rdfs:subClassOf rdf:resource="http://www.wageneder.at/ontology/bpmn2.0#EventDefinition"/>
        <rdfs:subClassOf>
            <owl:Restriction>
                <owl:onProperty rdf:resource="http://www.wageneder.at/ontology/bpmn2.0#hasCondition"/>
                <owl:qualifiedCardinality rdf:datatype="http://www.w3.org/2001/XMLSchema#nonNegativeInteger">1</owl:qualifiedCardinality>
                <owl:onClass rdf:resource="http://www.wageneder.at/ontology/bpmn2.0#Expression"/>
            </owl:Restriction>
        </rdfs:subClassOf>
        <rdfs:comment>The ConditionalEventDefinition element inherits the attributes and model associations of BaseElement through its relationship to the EventDefinition element</rdfs:comment>
    </owl:Class>
    


    <!-- http://www.wageneder.at/ontology/bpmn2.0#Converging -->

    <owl:Class rdf:about="http://www.wageneder.at/ontology/bpmn2.0#Converging">
        <rdfs:subClassOf rdf:resource="http://www.wageneder.at/ontology/bpmn2.0#GatewayDirection"/>
        <rdfs:comment>Converging: This Gateway MAY have multiple incoming Sequence Flows but MUST have no more than one (1) outgoing Sequence Flow.</rdfs:comment>
    </owl:Class>
    


    <!-- http://www.wageneder.at/ontology/bpmn2.0#Conversation -->

    <owl:Class rdf:about="http://www.wageneder.at/ontology/bpmn2.0#Conversation">
        <rdfs:subClassOf rdf:resource="http://www.wageneder.at/ontology/bpmn2.0#ConversationNode"/>
        <rdfs:comment>The Conversation element inherits the attributes and model associations of ConversationNode (see Table 9.10), but does not contain any additional attributes or model associations.</rdfs:comment>
    </owl:Class>
    


    <!-- http://www.wageneder.at/ontology/bpmn2.0#ConversationAssociation -->

    <owl:Class rdf:about="http://www.wageneder.at/ontology/bpmn2.0#ConversationAssociation">
        <rdfs:subClassOf rdf:resource="http://www.wageneder.at/ontology/bpmn2.0#BaseElement"/>
        <rdfs:subClassOf>
            <owl:Restriction>
                <owl:onProperty rdf:resource="http://www.wageneder.at/ontology/bpmn2.0#hasInnerConversationNodeRef"/>
                <owl:qualifiedCardinality rdf:datatype="http://www.w3.org/2001/XMLSchema#nonNegativeInteger">1</owl:qualifiedCardinality>
                <owl:onClass rdf:resource="http://www.wageneder.at/ontology/bpmn2.0#ConversationNode"/>
            </owl:Restriction>
        </rdfs:subClassOf>
        <rdfs:subClassOf>
            <owl:Restriction>
                <owl:onProperty rdf:resource="http://www.wageneder.at/ontology/bpmn2.0#hasOuterConversationNodeRef"/>
                <owl:qualifiedCardinality rdf:datatype="http://www.w3.org/2001/XMLSchema#nonNegativeInteger">1</owl:qualifiedCardinality>
                <owl:onClass rdf:resource="http://www.wageneder.at/ontology/bpmn2.0#ConversationNode"/>
            </owl:Restriction>
        </rdfs:subClassOf>
        <rdfs:comment>The ConversationAssociation element inherits the attributes and model associations of BaseElement (see Table 8.5). Table 9.14 presents the additional model associations for the ConversationAssociation element.</rdfs:comment>
    </owl:Class>
    


    <!-- http://www.wageneder.at/ontology/bpmn2.0#ConversationLevel -->

    <owl:Class rdf:about="http://www.wageneder.at/ontology/bpmn2.0#ConversationLevel">
        <rdfs:subClassOf rdf:resource="http://www.wageneder.at/ontology/bpmn2.0#CollaborationLevel"/>
        <rdfs:comment>This is just a hierarchical element for organisational purposes.
It presents the Conversations Folder</rdfs:comment>
    </owl:Class>
    


    <!-- http://www.wageneder.at/ontology/bpmn2.0#ConversationLink -->

    <owl:Class rdf:about="http://www.wageneder.at/ontology/bpmn2.0#ConversationLink">
        <rdfs:subClassOf rdf:resource="http://www.wageneder.at/ontology/bpmn2.0#BaseElement"/>
        <rdfs:subClassOf rdf:resource="http://www.wageneder.at/ontology/bpmn2.0#ConversationLevel"/>
        <rdfs:subClassOf>
            <owl:Restriction>
                <owl:onProperty rdf:resource="http://www.wageneder.at/ontology/bpmn2.0#hasCollaboration"/>
                <owl:qualifiedCardinality rdf:datatype="http://www.w3.org/2001/XMLSchema#nonNegativeInteger">1</owl:qualifiedCardinality>
                <owl:onClass rdf:resource="http://www.wageneder.at/ontology/bpmn2.0#Collaboration"/>
            </owl:Restriction>
        </rdfs:subClassOf>
        <rdfs:subClassOf>
            <owl:Restriction>
                <owl:onProperty rdf:resource="http://www.wageneder.at/ontology/bpmn2.0#hasSourceRef"/>
                <owl:qualifiedCardinality rdf:datatype="http://www.w3.org/2001/XMLSchema#nonNegativeInteger">1</owl:qualifiedCardinality>
                <owl:onClass rdf:resource="http://www.wageneder.at/ontology/bpmn2.0#InteractionNode"/>
            </owl:Restriction>
        </rdfs:subClassOf>
        <rdfs:subClassOf>
            <owl:Restriction>
                <owl:onProperty rdf:resource="http://www.wageneder.at/ontology/bpmn2.0#hasTargetRef"/>
                <owl:qualifiedCardinality rdf:datatype="http://www.w3.org/2001/XMLSchema#nonNegativeInteger">1</owl:qualifiedCardinality>
                <owl:onClass rdf:resource="http://www.wageneder.at/ontology/bpmn2.0#InteractionNode"/>
            </owl:Restriction>
        </rdfs:subClassOf>
        <rdfs:subClassOf>
            <owl:Restriction>
                <owl:onProperty rdf:resource="http://www.wageneder.at/ontology/bpmn2.0#name"/>
                <owl:minQualifiedCardinality rdf:datatype="http://www.w3.org/2001/XMLSchema#nonNegativeInteger">0</owl:minQualifiedCardinality>
                <owl:onDataRange rdf:resource="http://www.w3.org/2001/XMLSchema#string"/>
            </owl:Restriction>
        </rdfs:subClassOf>
        <rdfs:subClassOf>
            <owl:Restriction>
                <owl:onProperty rdf:resource="http://www.wageneder.at/ontology/bpmn2.0#name"/>
                <owl:maxQualifiedCardinality rdf:datatype="http://www.w3.org/2001/XMLSchema#nonNegativeInteger">1</owl:maxQualifiedCardinality>
                <owl:onDataRange rdf:resource="http://www.w3.org/2001/XMLSchema#string"/>
            </owl:Restriction>
        </rdfs:subClassOf>
        <rdfs:comment>The Conversation Link element inherits the attributes and model associations of BaseElement (see Table 8.5). Table 9.13 presents the additional attributes and model associations for the Conversation Link element.</rdfs:comment>
    </owl:Class>
    


    <!-- http://www.wageneder.at/ontology/bpmn2.0#ConversationNode -->

    <owl:Class rdf:about="http://www.wageneder.at/ontology/bpmn2.0#ConversationNode">
        <rdfs:subClassOf rdf:resource="http://www.wageneder.at/ontology/bpmn2.0#BaseElement"/>
        <rdfs:subClassOf rdf:resource="http://www.wageneder.at/ontology/bpmn2.0#ConversationLevel"/>
        <rdfs:subClassOf rdf:resource="http://www.wageneder.at/ontology/bpmn2.0#InteractionNode"/>
        <rdfs:subClassOf>
            <owl:Restriction>
                <owl:onProperty rdf:resource="http://www.wageneder.at/ontology/bpmn2.0#hasCollaboration"/>
                <owl:minQualifiedCardinality rdf:datatype="http://www.w3.org/2001/XMLSchema#nonNegativeInteger">0</owl:minQualifiedCardinality>
                <owl:onClass rdf:resource="http://www.wageneder.at/ontology/bpmn2.0#ConversationLink"/>
            </owl:Restriction>
        </rdfs:subClassOf>
        <rdfs:subClassOf>
            <owl:Restriction>
                <owl:onProperty rdf:resource="http://www.wageneder.at/ontology/bpmn2.0#hasConversationAssociation"/>
                <owl:minQualifiedCardinality rdf:datatype="http://www.w3.org/2001/XMLSchema#nonNegativeInteger">0</owl:minQualifiedCardinality>
                <owl:onClass rdf:resource="http://www.wageneder.at/ontology/bpmn2.0#ConversationAssociation"/>
            </owl:Restriction>
        </rdfs:subClassOf>
        <rdfs:subClassOf>
            <owl:Restriction>
                <owl:onProperty rdf:resource="http://www.wageneder.at/ontology/bpmn2.0#hasCorrelationKeys"/>
                <owl:minQualifiedCardinality rdf:datatype="http://www.w3.org/2001/XMLSchema#nonNegativeInteger">0</owl:minQualifiedCardinality>
                <owl:onClass rdf:resource="http://www.wageneder.at/ontology/bpmn2.0#CorrelationKey"/>
            </owl:Restriction>
        </rdfs:subClassOf>
        <rdfs:subClassOf>
            <owl:Restriction>
                <owl:onProperty rdf:resource="http://www.wageneder.at/ontology/bpmn2.0#hasMessageFlowRefs"/>
                <owl:minQualifiedCardinality rdf:datatype="http://www.w3.org/2001/XMLSchema#nonNegativeInteger">0</owl:minQualifiedCardinality>
                <owl:onClass rdf:resource="http://www.wageneder.at/ontology/bpmn2.0#MessageFlow"/>
            </owl:Restriction>
        </rdfs:subClassOf>
        <rdfs:subClassOf>
            <owl:Restriction>
                <owl:onProperty rdf:resource="http://www.wageneder.at/ontology/bpmn2.0#hasParticipantRefs"/>
                <owl:minQualifiedCardinality rdf:datatype="http://www.w3.org/2001/XMLSchema#nonNegativeInteger">2</owl:minQualifiedCardinality>
                <owl:onClass rdf:resource="http://www.wageneder.at/ontology/bpmn2.0#Participant"/>
            </owl:Restriction>
        </rdfs:subClassOf>
        <rdfs:subClassOf>
            <owl:Restriction>
                <owl:onProperty rdf:resource="http://www.wageneder.at/ontology/bpmn2.0#hasSubConversation"/>
                <owl:minQualifiedCardinality rdf:datatype="http://www.w3.org/2001/XMLSchema#nonNegativeInteger">0</owl:minQualifiedCardinality>
                <owl:onClass rdf:resource="http://www.wageneder.at/ontology/bpmn2.0#SubConversation"/>
            </owl:Restriction>
        </rdfs:subClassOf>
        <rdfs:subClassOf>
            <owl:Restriction>
                <owl:onProperty rdf:resource="http://www.wageneder.at/ontology/bpmn2.0#hasCollaboration"/>
                <owl:maxQualifiedCardinality rdf:datatype="http://www.w3.org/2001/XMLSchema#nonNegativeInteger">1</owl:maxQualifiedCardinality>
                <owl:onClass rdf:resource="http://www.wageneder.at/ontology/bpmn2.0#ConversationLink"/>
            </owl:Restriction>
        </rdfs:subClassOf>
        <rdfs:subClassOf>
            <owl:Restriction>
                <owl:onProperty rdf:resource="http://www.wageneder.at/ontology/bpmn2.0#hasSubConversation"/>
                <owl:maxQualifiedCardinality rdf:datatype="http://www.w3.org/2001/XMLSchema#nonNegativeInteger">1</owl:maxQualifiedCardinality>
                <owl:onClass rdf:resource="http://www.wageneder.at/ontology/bpmn2.0#SubConversation"/>
            </owl:Restriction>
        </rdfs:subClassOf>
        <rdfs:subClassOf>
            <owl:Restriction>
                <owl:onProperty rdf:resource="http://www.wageneder.at/ontology/bpmn2.0#name"/>
                <owl:minQualifiedCardinality rdf:datatype="http://www.w3.org/2001/XMLSchema#nonNegativeInteger">0</owl:minQualifiedCardinality>
                <owl:onDataRange rdf:resource="http://www.w3.org/2001/XMLSchema#string"/>
            </owl:Restriction>
        </rdfs:subClassOf>
        <rdfs:subClassOf>
            <owl:Restriction>
                <owl:onProperty rdf:resource="http://www.wageneder.at/ontology/bpmn2.0#name"/>
                <owl:maxQualifiedCardinality rdf:datatype="http://www.w3.org/2001/XMLSchema#nonNegativeInteger">1</owl:maxQualifiedCardinality>
                <owl:onDataRange rdf:resource="http://www.w3.org/2001/XMLSchema#string"/>
            </owl:Restriction>
        </rdfs:subClassOf>
        <rdfs:comment>ConversationNode is the abstract super class for all elements that can comprise the Conversation elements of a Collaboration diagram, which are Conversation (see page 129), Sub-Conversation (see page 129), and Call Conversation (see page 130).</rdfs:comment>
    </owl:Class>
    


    <!-- http://www.wageneder.at/ontology/bpmn2.0#Correlation -->

    <owl:Class rdf:about="http://www.wageneder.at/ontology/bpmn2.0#Correlation">
        <rdfs:subClassOf rdf:resource="http://www.wageneder.at/ontology/bpmn2.0#Common"/>
        <rdfs:comment>The CorrelationKey element inherits the attributes and model associations of BaseElement (see Table 8.5). Table 8.31 displays the additional model associations of the CorrelationKey element.</rdfs:comment>
    </owl:Class>
    


    <!-- http://www.wageneder.at/ontology/bpmn2.0#CorrelationKey -->

    <owl:Class rdf:about="http://www.wageneder.at/ontology/bpmn2.0#CorrelationKey">
        <rdfs:subClassOf rdf:resource="http://www.wageneder.at/ontology/bpmn2.0#Common"/>
        <rdfs:subClassOf>
            <owl:Restriction>
                <owl:onProperty rdf:resource="http://www.wageneder.at/ontology/bpmn2.0#hasCollaboration"/>
                <owl:minQualifiedCardinality rdf:datatype="http://www.w3.org/2001/XMLSchema#nonNegativeInteger">0</owl:minQualifiedCardinality>
                <owl:onClass rdf:resource="http://www.wageneder.at/ontology/bpmn2.0#Collaboration"/>
            </owl:Restriction>
        </rdfs:subClassOf>
        <rdfs:subClassOf>
            <owl:Restriction>
                <owl:onProperty rdf:resource="http://www.wageneder.at/ontology/bpmn2.0#hasConversationNode"/>
                <owl:minQualifiedCardinality rdf:datatype="http://www.w3.org/2001/XMLSchema#nonNegativeInteger">0</owl:minQualifiedCardinality>
                <owl:onClass rdf:resource="http://www.wageneder.at/ontology/bpmn2.0#ConversationNode"/>
            </owl:Restriction>
        </rdfs:subClassOf>
        <rdfs:subClassOf>
            <owl:Restriction>
                <owl:onProperty rdf:resource="http://www.wageneder.at/ontology/bpmn2.0#hasCorrelationPropertyRef"/>
                <owl:minQualifiedCardinality rdf:datatype="http://www.w3.org/2001/XMLSchema#nonNegativeInteger">0</owl:minQualifiedCardinality>
                <owl:onClass rdf:resource="http://www.wageneder.at/ontology/bpmn2.0#CorrelationProperty"/>
            </owl:Restriction>
        </rdfs:subClassOf>
        <rdfs:subClassOf>
            <owl:Restriction>
                <owl:onProperty rdf:resource="http://www.wageneder.at/ontology/bpmn2.0#hasCollaboration"/>
                <owl:maxQualifiedCardinality rdf:datatype="http://www.w3.org/2001/XMLSchema#nonNegativeInteger">1</owl:maxQualifiedCardinality>
                <owl:onClass rdf:resource="http://www.wageneder.at/ontology/bpmn2.0#Collaboration"/>
            </owl:Restriction>
        </rdfs:subClassOf>
        <rdfs:subClassOf>
            <owl:Restriction>
                <owl:onProperty rdf:resource="http://www.wageneder.at/ontology/bpmn2.0#hasConversationNode"/>
                <owl:maxQualifiedCardinality rdf:datatype="http://www.w3.org/2001/XMLSchema#nonNegativeInteger">1</owl:maxQualifiedCardinality>
                <owl:onClass rdf:resource="http://www.wageneder.at/ontology/bpmn2.0#ConversationNode"/>
            </owl:Restriction>
        </rdfs:subClassOf>
        <rdfs:subClassOf>
            <owl:Restriction>
                <owl:onProperty rdf:resource="http://www.wageneder.at/ontology/bpmn2.0#name"/>
                <owl:minQualifiedCardinality rdf:datatype="http://www.w3.org/2001/XMLSchema#nonNegativeInteger">0</owl:minQualifiedCardinality>
                <owl:onDataRange rdf:resource="http://www.w3.org/2001/XMLSchema#string"/>
            </owl:Restriction>
        </rdfs:subClassOf>
        <rdfs:subClassOf>
            <owl:Restriction>
                <owl:onProperty rdf:resource="http://www.wageneder.at/ontology/bpmn2.0#name"/>
                <owl:maxQualifiedCardinality rdf:datatype="http://www.w3.org/2001/XMLSchema#nonNegativeInteger">1</owl:maxQualifiedCardinality>
                <owl:onDataRange rdf:resource="http://www.w3.org/2001/XMLSchema#string"/>
            </owl:Restriction>
        </rdfs:subClassOf>
        <rdfs:comment>The CorrelationKey element inherits the attributes and model associations of BaseElement (see Table 8.5). Table 8.31 displays the additional model associations of the CorrelationKey element.</rdfs:comment>
    </owl:Class>
    


    <!-- http://www.wageneder.at/ontology/bpmn2.0#CorrelationProperty -->

    <owl:Class rdf:about="http://www.wageneder.at/ontology/bpmn2.0#CorrelationProperty">
        <rdfs:subClassOf rdf:resource="http://www.wageneder.at/ontology/bpmn2.0#Common"/>
        <rdfs:subClassOf>
            <owl:Restriction>
                <owl:onProperty rdf:resource="http://www.wageneder.at/ontology/bpmn2.0#hasCorrelationPropertyRetrievalExpression"/>
                <owl:minQualifiedCardinality rdf:datatype="http://www.w3.org/2001/XMLSchema#nonNegativeInteger">1</owl:minQualifiedCardinality>
                <owl:onClass rdf:resource="http://www.wageneder.at/ontology/bpmn2.0#CorrelationPropertyRetrievalExpression"/>
            </owl:Restriction>
        </rdfs:subClassOf>
        <rdfs:subClassOf>
            <owl:Restriction>
                <owl:onProperty rdf:resource="http://www.wageneder.at/ontology/bpmn2.0#hasType"/>
                <owl:minQualifiedCardinality rdf:datatype="http://www.w3.org/2001/XMLSchema#nonNegativeInteger">0</owl:minQualifiedCardinality>
                <owl:onClass rdf:resource="http://www.wageneder.at/ontology/bpmn2.0#ItemDefinition"/>
            </owl:Restriction>
        </rdfs:subClassOf>
        <rdfs:subClassOf>
            <owl:Restriction>
                <owl:onProperty rdf:resource="http://www.wageneder.at/ontology/bpmn2.0#hasType"/>
                <owl:maxQualifiedCardinality rdf:datatype="http://www.w3.org/2001/XMLSchema#nonNegativeInteger">1</owl:maxQualifiedCardinality>
                <owl:onClass rdf:resource="http://www.wageneder.at/ontology/bpmn2.0#ItemDefinition"/>
            </owl:Restriction>
        </rdfs:subClassOf>
        <rdfs:subClassOf>
            <owl:Restriction>
                <owl:onProperty rdf:resource="http://www.wageneder.at/ontology/bpmn2.0#name"/>
                <owl:minQualifiedCardinality rdf:datatype="http://www.w3.org/2001/XMLSchema#nonNegativeInteger">0</owl:minQualifiedCardinality>
                <owl:onDataRange rdf:resource="http://www.w3.org/2001/XMLSchema#string"/>
            </owl:Restriction>
        </rdfs:subClassOf>
        <rdfs:subClassOf>
            <owl:Restriction>
                <owl:onProperty rdf:resource="http://www.wageneder.at/ontology/bpmn2.0#name"/>
                <owl:maxQualifiedCardinality rdf:datatype="http://www.w3.org/2001/XMLSchema#nonNegativeInteger">1</owl:maxQualifiedCardinality>
                <owl:onDataRange rdf:resource="http://www.w3.org/2001/XMLSchema#string"/>
            </owl:Restriction>
        </rdfs:subClassOf>
        <rdfs:comment>The CorrelationProperty element inherits the attributes and model associations of BaseElement (see Table 8.5) through its relationship to RootElement. Table 8.32 displays the additional model associations of the CorrelationProperty element.</rdfs:comment>
    </owl:Class>
    


    <!-- http://www.wageneder.at/ontology/bpmn2.0#CorrelationPropertyBinding -->

    <owl:Class rdf:about="http://www.wageneder.at/ontology/bpmn2.0#CorrelationPropertyBinding">
        <rdfs:subClassOf rdf:resource="http://www.wageneder.at/ontology/bpmn2.0#Common"/>
        <rdfs:subClassOf>
            <owl:Restriction>
                <owl:onProperty rdf:resource="http://www.wageneder.at/ontology/bpmn2.0#hasDataPath"/>
                <owl:qualifiedCardinality rdf:datatype="http://www.w3.org/2001/XMLSchema#nonNegativeInteger">1</owl:qualifiedCardinality>
                <owl:onClass rdf:resource="http://www.wageneder.at/ontology/bpmn2.0#FormalExpression"/>
            </owl:Restriction>
        </rdfs:subClassOf>
        <rdfs:subClassOf>
            <owl:Restriction>
                <owl:onProperty rdf:resource="http://www.wageneder.at/ontology/bpmn2.0#hasCorrelationPropertyRef"/>
                <owl:maxQualifiedCardinality rdf:datatype="http://www.w3.org/2001/XMLSchema#nonNegativeInteger">1</owl:maxQualifiedCardinality>
                <owl:onClass rdf:resource="http://www.wageneder.at/ontology/bpmn2.0#CorrelationProperty"/>
            </owl:Restriction>
        </rdfs:subClassOf>
        <rdfs:comment>The CorrelationPropertyBinding element inherits the attributes and model associations of BaseElement (see Table 8.5). Table 8.35 displays the additional model associations of the CorrelationPropertyBinding element.</rdfs:comment>
    </owl:Class>
    


    <!-- http://www.wageneder.at/ontology/bpmn2.0#CorrelationPropertyRetrievalExpression -->

    <owl:Class rdf:about="http://www.wageneder.at/ontology/bpmn2.0#CorrelationPropertyRetrievalExpression">
        <rdfs:subClassOf rdf:resource="http://www.wageneder.at/ontology/bpmn2.0#Common"/>
        <rdfs:subClassOf>
            <owl:Restriction>
                <owl:onProperty rdf:resource="http://www.wageneder.at/ontology/bpmn2.0#hasCorrelationProperty"/>
                <owl:qualifiedCardinality rdf:datatype="http://www.w3.org/2001/XMLSchema#nonNegativeInteger">1</owl:qualifiedCardinality>
                <owl:onClass rdf:resource="http://www.wageneder.at/ontology/bpmn2.0#CorrelationProperty"/>
            </owl:Restriction>
        </rdfs:subClassOf>
        <rdfs:subClassOf>
            <owl:Restriction>
                <owl:onProperty rdf:resource="http://www.wageneder.at/ontology/bpmn2.0#hasMessagePath"/>
                <owl:qualifiedCardinality rdf:datatype="http://www.w3.org/2001/XMLSchema#nonNegativeInteger">1</owl:qualifiedCardinality>
                <owl:onClass rdf:resource="http://www.wageneder.at/ontology/bpmn2.0#FormalExpression"/>
            </owl:Restriction>
        </rdfs:subClassOf>
        <rdfs:subClassOf>
            <owl:Restriction>
                <owl:onProperty rdf:resource="http://www.wageneder.at/ontology/bpmn2.0#hasMessageRef"/>
                <owl:qualifiedCardinality rdf:datatype="http://www.w3.org/2001/XMLSchema#nonNegativeInteger">1</owl:qualifiedCardinality>
                <owl:onClass rdf:resource="http://www.wageneder.at/ontology/bpmn2.0#Message"/>
            </owl:Restriction>
        </rdfs:subClassOf>
        <rdfs:comment>The CorrelationPropertyRetrievalExpression element inherits the attributes and model associations of BaseElement (see Table 8.5). Table 8.33 displays the additional model associations of the CorrelationPropertyRetrievalExpression element.</rdfs:comment>
    </owl:Class>
    


    <!-- http://www.wageneder.at/ontology/bpmn2.0#CorrelationSubscription -->

    <owl:Class rdf:about="http://www.wageneder.at/ontology/bpmn2.0#CorrelationSubscription">
        <rdfs:subClassOf rdf:resource="http://www.wageneder.at/ontology/bpmn2.0#Common"/>
        <rdfs:subClassOf>
            <owl:Restriction>
                <owl:onProperty rdf:resource="http://www.wageneder.at/ontology/bpmn2.0#hasCorrelationPropertyBinding"/>
                <owl:minQualifiedCardinality rdf:datatype="http://www.w3.org/2001/XMLSchema#nonNegativeInteger">0</owl:minQualifiedCardinality>
                <owl:onClass rdf:resource="http://www.wageneder.at/ontology/bpmn2.0#CorrelationPropertyBinding"/>
            </owl:Restriction>
        </rdfs:subClassOf>
        <rdfs:subClassOf>
            <owl:Restriction>
                <owl:onProperty rdf:resource="http://www.wageneder.at/ontology/bpmn2.0#hasCorrelationKeyRef"/>
                <owl:qualifiedCardinality rdf:datatype="http://www.w3.org/2001/XMLSchema#nonNegativeInteger">1</owl:qualifiedCardinality>
                <owl:onClass rdf:resource="http://www.wageneder.at/ontology/bpmn2.0#CorrelationKey"/>
            </owl:Restriction>
        </rdfs:subClassOf>
        <rdfs:comment>The CorrelationSubscription element inherits the attributes and model associations of BaseElement (see Table 8.5). Table 8.34 displays the additional model associations of the CorrelationSubscription element.</rdfs:comment>
    </owl:Class>
    


    <!-- http://www.wageneder.at/ontology/bpmn2.0#DataAssociation -->

    <owl:Class rdf:about="http://www.wageneder.at/ontology/bpmn2.0#DataAssociation">
        <rdfs:subClassOf rdf:resource="http://www.wageneder.at/ontology/bpmn2.0#BaseElement"/>
        <rdfs:subClassOf rdf:resource="http://www.wageneder.at/ontology/bpmn2.0#DataLevel"/>
        <rdfs:subClassOf>
            <owl:Restriction>
                <owl:onProperty rdf:resource="http://www.wageneder.at/ontology/bpmn2.0#hasAssignment"/>
                <owl:minQualifiedCardinality rdf:datatype="http://www.w3.org/2001/XMLSchema#nonNegativeInteger">0</owl:minQualifiedCardinality>
                <owl:onClass rdf:resource="http://www.wageneder.at/ontology/bpmn2.0#Assignment"/>
            </owl:Restriction>
        </rdfs:subClassOf>
        <rdfs:subClassOf>
            <owl:Restriction>
                <owl:onProperty rdf:resource="http://www.wageneder.at/ontology/bpmn2.0#hasSourceRef"/>
                <owl:minQualifiedCardinality rdf:datatype="http://www.w3.org/2001/XMLSchema#nonNegativeInteger">0</owl:minQualifiedCardinality>
                <owl:onClass rdf:resource="http://www.wageneder.at/ontology/bpmn2.0#ItemAwareElement"/>
            </owl:Restriction>
        </rdfs:subClassOf>
        <rdfs:subClassOf>
            <owl:Restriction>
                <owl:onProperty rdf:resource="http://www.wageneder.at/ontology/bpmn2.0#hasTargetRef"/>
                <owl:minQualifiedCardinality rdf:datatype="http://www.w3.org/2001/XMLSchema#nonNegativeInteger">1</owl:minQualifiedCardinality>
                <owl:onClass rdf:resource="http://www.wageneder.at/ontology/bpmn2.0#ItemAwareElement"/>
            </owl:Restriction>
        </rdfs:subClassOf>
        <rdfs:subClassOf>
            <owl:Restriction>
                <owl:onProperty rdf:resource="http://www.wageneder.at/ontology/bpmn2.0#hasTransformation"/>
                <owl:minQualifiedCardinality rdf:datatype="http://www.w3.org/2001/XMLSchema#nonNegativeInteger">0</owl:minQualifiedCardinality>
                <owl:onClass rdf:resource="http://www.wageneder.at/ontology/bpmn2.0#FormalExpression"/>
            </owl:Restriction>
        </rdfs:subClassOf>
        <rdfs:subClassOf>
            <owl:Restriction>
                <owl:onProperty rdf:resource="http://www.wageneder.at/ontology/bpmn2.0#hasTransformation"/>
                <owl:maxQualifiedCardinality rdf:datatype="http://www.w3.org/2001/XMLSchema#nonNegativeInteger">1</owl:maxQualifiedCardinality>
                <owl:onClass rdf:resource="http://www.wageneder.at/ontology/bpmn2.0#FormalExpression"/>
            </owl:Restriction>
        </rdfs:subClassOf>
        <rdfs:comment>The DataAssociation element inherits the attributes and model associations of BaseElement (see Table 8.5). Table 10.63 presents the additional model associations of the DataAssociation element.</rdfs:comment>
    </owl:Class>
    


    <!-- http://www.wageneder.at/ontology/bpmn2.0#DataInput -->

    <owl:Class rdf:about="http://www.wageneder.at/ontology/bpmn2.0#DataInput">
        <rdfs:subClassOf rdf:resource="http://www.wageneder.at/ontology/bpmn2.0#ItemAwareElement"/>
        <rdfs:subClassOf>
            <owl:Restriction>
                <owl:onProperty rdf:resource="http://www.wageneder.at/ontology/bpmn2.0#hasInputSetRefs"/>
                <owl:minQualifiedCardinality rdf:datatype="http://www.w3.org/2001/XMLSchema#nonNegativeInteger">1</owl:minQualifiedCardinality>
                <owl:onClass rdf:resource="http://www.wageneder.at/ontology/bpmn2.0#InputSet"/>
            </owl:Restriction>
        </rdfs:subClassOf>
        <rdfs:subClassOf>
            <owl:Restriction>
                <owl:onProperty rdf:resource="http://www.wageneder.at/ontology/bpmn2.0#hasInputSetWithOptional"/>
                <owl:minQualifiedCardinality rdf:datatype="http://www.w3.org/2001/XMLSchema#nonNegativeInteger">0</owl:minQualifiedCardinality>
                <owl:onClass rdf:resource="http://www.wageneder.at/ontology/bpmn2.0#InputSet"/>
            </owl:Restriction>
        </rdfs:subClassOf>
        <rdfs:subClassOf>
            <owl:Restriction>
                <owl:onProperty rdf:resource="http://www.wageneder.at/ontology/bpmn2.0#hasInputSetWithWhileExecuting"/>
                <owl:minQualifiedCardinality rdf:datatype="http://www.w3.org/2001/XMLSchema#nonNegativeInteger">0</owl:minQualifiedCardinality>
                <owl:onClass rdf:resource="http://www.wageneder.at/ontology/bpmn2.0#InputSet"/>
            </owl:Restriction>
        </rdfs:subClassOf>
        <rdfs:subClassOf>
            <owl:Restriction>
                <owl:onProperty rdf:resource="http://www.wageneder.at/ontology/bpmn2.0#name"/>
                <owl:minQualifiedCardinality rdf:datatype="http://www.w3.org/2001/XMLSchema#nonNegativeInteger">0</owl:minQualifiedCardinality>
                <owl:onDataRange rdf:resource="http://www.w3.org/2001/XMLSchema#string"/>
            </owl:Restriction>
        </rdfs:subClassOf>
        <rdfs:subClassOf>
            <owl:Restriction>
                <owl:onProperty rdf:resource="http://www.wageneder.at/ontology/bpmn2.0#isCollection"/>
                <owl:qualifiedCardinality rdf:datatype="http://www.w3.org/2001/XMLSchema#nonNegativeInteger">1</owl:qualifiedCardinality>
                <owl:onDataRange rdf:resource="http://www.w3.org/2001/XMLSchema#boolean"/>
            </owl:Restriction>
        </rdfs:subClassOf>
        <rdfs:subClassOf>
            <owl:Restriction>
                <owl:onProperty rdf:resource="http://www.wageneder.at/ontology/bpmn2.0#name"/>
                <owl:maxQualifiedCardinality rdf:datatype="http://www.w3.org/2001/XMLSchema#nonNegativeInteger">1</owl:maxQualifiedCardinality>
                <owl:onDataRange rdf:resource="http://www.w3.org/2001/XMLSchema#string"/>
            </owl:Restriction>
        </rdfs:subClassOf>
        <rdfs:comment>The DataInput element inherits the attributes and model associations of BaseElement (see Table 8.5) and ItemAwareElement (Table 10.52). Table 10.59 presents the additional attributes and model associations of the DataInput element.</rdfs:comment>
    </owl:Class>
    


    <!-- http://www.wageneder.at/ontology/bpmn2.0#DataInputAssociation -->

    <owl:Class rdf:about="http://www.wageneder.at/ontology/bpmn2.0#DataInputAssociation">
        <rdfs:subClassOf rdf:resource="http://www.wageneder.at/ontology/bpmn2.0#BaseElement"/>
        <rdfs:subClassOf rdf:resource="http://www.wageneder.at/ontology/bpmn2.0#DataAssociation"/>
        <rdfs:comment>A Data Input is a declaration that a particular kind of data will be used as input of the InputOutputSpecification.

Data Inputs MAY have incoming Data Associations</rdfs:comment>
    </owl:Class>
    


    <!-- http://www.wageneder.at/ontology/bpmn2.0#DataLevel -->

    <owl:Class rdf:about="http://www.wageneder.at/ontology/bpmn2.0#DataLevel">
        <rdfs:subClassOf rdf:resource="http://www.wageneder.at/ontology/bpmn2.0#ProcessLevel"/>
        <rdfs:comment>This is just a hierarchical element for organisational purposes.
It presents the Data Folder</rdfs:comment>
    </owl:Class>
    


    <!-- http://www.wageneder.at/ontology/bpmn2.0#DataObject -->

    <owl:Class rdf:about="http://www.wageneder.at/ontology/bpmn2.0#DataObject">
        <rdfs:subClassOf rdf:resource="http://www.wageneder.at/ontology/bpmn2.0#FlowElement"/>
        <rdfs:subClassOf rdf:resource="http://www.wageneder.at/ontology/bpmn2.0#ItemAwareElement"/>
        <rdfs:subClassOf>
            <owl:Restriction>
                <owl:onProperty rdf:resource="http://www.wageneder.at/ontology/bpmn2.0#isCollection"/>
                <owl:qualifiedCardinality rdf:datatype="http://www.w3.org/2001/XMLSchema#nonNegativeInteger">1</owl:qualifiedCardinality>
                <owl:onDataRange rdf:resource="http://www.w3.org/2001/XMLSchema#boolean"/>
            </owl:Restriction>
        </rdfs:subClassOf>
        <owl:disjointWith rdf:resource="http://www.wageneder.at/ontology/bpmn2.0#Property"/>
        <rdfs:comment>The Data Object class is an item-aware element. Data Object elements MUST be contained within Process or Sub- Process elements. Data Object elements are visually displayed on a Process diagram. Data Object References are a way to reuse Data Objects in the same diagram</rdfs:comment>
    </owl:Class>
    


    <!-- http://www.wageneder.at/ontology/bpmn2.0#DataObjectReference -->

    <owl:Class rdf:about="http://www.wageneder.at/ontology/bpmn2.0#DataObjectReference">
        <rdfs:subClassOf rdf:resource="http://www.wageneder.at/ontology/bpmn2.0#FlowElement"/>
        <rdfs:subClassOf rdf:resource="http://www.wageneder.at/ontology/bpmn2.0#ItemAwareElement"/>
        <rdfs:subClassOf>
            <owl:Restriction>
                <owl:onProperty rdf:resource="http://www.wageneder.at/ontology/bpmn2.0#hasDataObjectRef"/>
                <owl:qualifiedCardinality rdf:datatype="http://www.w3.org/2001/XMLSchema#nonNegativeInteger">1</owl:qualifiedCardinality>
                <owl:onClass rdf:resource="http://www.wageneder.at/ontology/bpmn2.0#DataObject"/>
            </owl:Restriction>
        </rdfs:subClassOf>
        <rdfs:comment>The Data Object Reference element inherits the attributes and model associations of ItemAwareElement (Table 10.52) and FlowElement (see Table 8.44). Table 10.53 presents the additional attributes of the Data Object Reference element.</rdfs:comment>
    </owl:Class>
    


    <!-- http://www.wageneder.at/ontology/bpmn2.0#DataOutput -->

    <owl:Class rdf:about="http://www.wageneder.at/ontology/bpmn2.0#DataOutput">
        <rdfs:subClassOf rdf:resource="http://www.wageneder.at/ontology/bpmn2.0#ItemAwareElement"/>
        <rdfs:subClassOf>
            <owl:Restriction>
                <owl:onProperty rdf:resource="http://www.wageneder.at/ontology/bpmn2.0#hasOutputSetRefs"/>
                <owl:minQualifiedCardinality rdf:datatype="http://www.w3.org/2001/XMLSchema#nonNegativeInteger">1</owl:minQualifiedCardinality>
                <owl:onClass rdf:resource="http://www.wageneder.at/ontology/bpmn2.0#OutputSet"/>
            </owl:Restriction>
        </rdfs:subClassOf>
        <rdfs:subClassOf>
            <owl:Restriction>
                <owl:onProperty rdf:resource="http://www.wageneder.at/ontology/bpmn2.0#hasOutputSetWithOptional"/>
                <owl:minQualifiedCardinality rdf:datatype="http://www.w3.org/2001/XMLSchema#nonNegativeInteger">0</owl:minQualifiedCardinality>
                <owl:onClass rdf:resource="http://www.wageneder.at/ontology/bpmn2.0#OutputSet"/>
            </owl:Restriction>
        </rdfs:subClassOf>
        <rdfs:subClassOf>
            <owl:Restriction>
                <owl:onProperty rdf:resource="http://www.wageneder.at/ontology/bpmn2.0#hasOutputSetWithWhileExecuting"/>
                <owl:minQualifiedCardinality rdf:datatype="http://www.w3.org/2001/XMLSchema#nonNegativeInteger">0</owl:minQualifiedCardinality>
                <owl:onClass rdf:resource="http://www.wageneder.at/ontology/bpmn2.0#OutputSet"/>
            </owl:Restriction>
        </rdfs:subClassOf>
        <rdfs:subClassOf>
            <owl:Restriction>
                <owl:onProperty rdf:resource="http://www.wageneder.at/ontology/bpmn2.0#name"/>
                <owl:minQualifiedCardinality rdf:datatype="http://www.w3.org/2001/XMLSchema#nonNegativeInteger">0</owl:minQualifiedCardinality>
                <owl:onDataRange rdf:resource="http://www.w3.org/2001/XMLSchema#string"/>
            </owl:Restriction>
        </rdfs:subClassOf>
        <rdfs:subClassOf>
            <owl:Restriction>
                <owl:onProperty rdf:resource="http://www.wageneder.at/ontology/bpmn2.0#isCollection"/>
                <owl:qualifiedCardinality rdf:datatype="http://www.w3.org/2001/XMLSchema#nonNegativeInteger">1</owl:qualifiedCardinality>
                <owl:onDataRange rdf:resource="http://www.w3.org/2001/XMLSchema#boolean"/>
            </owl:Restriction>
        </rdfs:subClassOf>
        <rdfs:subClassOf>
            <owl:Restriction>
                <owl:onProperty rdf:resource="http://www.wageneder.at/ontology/bpmn2.0#name"/>
                <owl:maxQualifiedCardinality rdf:datatype="http://www.w3.org/2001/XMLSchema#nonNegativeInteger">1</owl:maxQualifiedCardinality>
                <owl:onDataRange rdf:resource="http://www.w3.org/2001/XMLSchema#string"/>
            </owl:Restriction>
        </rdfs:subClassOf>
        <rdfs:comment>The DataOutput element inherits the attributes and model associations of BaseElement (see Table 8.5) and ItemAwareElement (Table 10.52). Table 10.60 presents the additional attributes and model associations of the DataInput element.</rdfs:comment>
    </owl:Class>
    


    <!-- http://www.wageneder.at/ontology/bpmn2.0#DataOutputAssociation -->

    <owl:Class rdf:about="http://www.wageneder.at/ontology/bpmn2.0#DataOutputAssociation">
        <rdfs:subClassOf rdf:resource="http://www.wageneder.at/ontology/bpmn2.0#BaseElement"/>
        <rdfs:subClassOf rdf:resource="http://www.wageneder.at/ontology/bpmn2.0#DataAssociation"/>
        <rdfs:comment>A Data Output is a declaration that a particular kind of data can be produced as output of the InputOutputSpecification.

Data Outputs MAY have outgoing DataAssociations.</rdfs:comment>
    </owl:Class>
    


    <!-- http://www.wageneder.at/ontology/bpmn2.0#DataState -->

    <owl:Class rdf:about="http://www.wageneder.at/ontology/bpmn2.0#DataState">
        <rdfs:subClassOf rdf:resource="http://www.wageneder.at/ontology/bpmn2.0#BaseElement"/>
        <rdfs:subClassOf rdf:resource="http://www.wageneder.at/ontology/bpmn2.0#DataLevel"/>
        <rdfs:subClassOf>
            <owl:Restriction>
                <owl:onProperty rdf:resource="http://www.wageneder.at/ontology/bpmn2.0#name"/>
                <owl:qualifiedCardinality rdf:datatype="http://www.w3.org/2001/XMLSchema#nonNegativeInteger">1</owl:qualifiedCardinality>
                <owl:onDataRange rdf:resource="http://www.w3.org/2001/XMLSchema#string"/>
            </owl:Restriction>
        </rdfs:subClassOf>
        <rdfs:comment>The DataState element inherits the attributes and model associations of BaseElement (see Table 8.5). Table 10.54 presents the additional attributes and model associations of the DataObject element.</rdfs:comment>
    </owl:Class>
    


    <!-- http://www.wageneder.at/ontology/bpmn2.0#DataStore -->

    <owl:Class rdf:about="http://www.wageneder.at/ontology/bpmn2.0#DataStore">
        <rdfs:subClassOf rdf:resource="http://www.wageneder.at/ontology/bpmn2.0#ItemAwareElement"/>
        <rdfs:subClassOf rdf:resource="http://www.wageneder.at/ontology/bpmn2.0#RootElement"/>
        <rdfs:subClassOf>
            <owl:Restriction>
                <owl:onProperty rdf:resource="http://www.wageneder.at/ontology/bpmn2.0#capacity"/>
                <owl:minQualifiedCardinality rdf:datatype="http://www.w3.org/2001/XMLSchema#nonNegativeInteger">0</owl:minQualifiedCardinality>
                <owl:onDataRange rdf:resource="http://www.w3.org/2001/XMLSchema#integer"/>
            </owl:Restriction>
        </rdfs:subClassOf>
        <rdfs:subClassOf>
            <owl:Restriction>
                <owl:onProperty rdf:resource="http://www.wageneder.at/ontology/bpmn2.0#isUnlimited"/>
                <owl:qualifiedCardinality rdf:datatype="http://www.w3.org/2001/XMLSchema#nonNegativeInteger">1</owl:qualifiedCardinality>
                <owl:onDataRange rdf:resource="http://www.w3.org/2001/XMLSchema#boolean"/>
            </owl:Restriction>
        </rdfs:subClassOf>
        <rdfs:subClassOf>
            <owl:Restriction>
                <owl:onProperty rdf:resource="http://www.wageneder.at/ontology/bpmn2.0#name"/>
                <owl:qualifiedCardinality rdf:datatype="http://www.w3.org/2001/XMLSchema#nonNegativeInteger">1</owl:qualifiedCardinality>
                <owl:onDataRange rdf:resource="http://www.w3.org/2001/XMLSchema#string"/>
            </owl:Restriction>
        </rdfs:subClassOf>
        <rdfs:subClassOf>
            <owl:Restriction>
                <owl:onProperty rdf:resource="http://www.wageneder.at/ontology/bpmn2.0#capacity"/>
                <owl:maxQualifiedCardinality rdf:datatype="http://www.w3.org/2001/XMLSchema#nonNegativeInteger">1</owl:maxQualifiedCardinality>
                <owl:onDataRange rdf:resource="http://www.w3.org/2001/XMLSchema#integer"/>
            </owl:Restriction>
        </rdfs:subClassOf>
        <rdfs:comment>The DataStore element inherits the attributes and model associations of FlowElement (see Table 8.44) through its relationship to RootElement, and ItemAwareElement (see Table 10.51). Table 10.55 presents the additional attributes of the DataStore element.</rdfs:comment>
    </owl:Class>
    


    <!-- http://www.wageneder.at/ontology/bpmn2.0#DataStoreReference -->

    <owl:Class rdf:about="http://www.wageneder.at/ontology/bpmn2.0#DataStoreReference">
        <rdfs:subClassOf rdf:resource="http://www.wageneder.at/ontology/bpmn2.0#FlowElement"/>
        <rdfs:subClassOf rdf:resource="http://www.wageneder.at/ontology/bpmn2.0#ItemAwareElement"/>
        <rdfs:subClassOf>
            <owl:Restriction>
                <owl:onProperty rdf:resource="http://www.wageneder.at/ontology/bpmn2.0#hasDataStoreRef"/>
                <owl:minQualifiedCardinality rdf:datatype="http://www.w3.org/2001/XMLSchema#nonNegativeInteger">0</owl:minQualifiedCardinality>
                <owl:onClass rdf:resource="http://www.wageneder.at/ontology/bpmn2.0#DataStore"/>
            </owl:Restriction>
        </rdfs:subClassOf>
        <rdfs:subClassOf>
            <owl:Restriction>
                <owl:onProperty rdf:resource="http://www.wageneder.at/ontology/bpmn2.0#hasDataStoreRef"/>
                <owl:maxQualifiedCardinality rdf:datatype="http://www.w3.org/2001/XMLSchema#nonNegativeInteger">1</owl:maxQualifiedCardinality>
                <owl:onClass rdf:resource="http://www.wageneder.at/ontology/bpmn2.0#DataStore"/>
            </owl:Restriction>
        </rdfs:subClassOf>
        <rdfs:subClassOf>
            <owl:Restriction>
                <owl:onProperty rdf:resource="http://www.wageneder.at/ontology/bpmn2.0#name"/>
                <owl:minQualifiedCardinality rdf:datatype="http://www.w3.org/2001/XMLSchema#nonNegativeInteger">0</owl:minQualifiedCardinality>
                <owl:onDataRange rdf:resource="http://www.w3.org/2001/XMLSchema#string"/>
            </owl:Restriction>
        </rdfs:subClassOf>
        <rdfs:subClassOf>
            <owl:Restriction>
                <owl:onProperty rdf:resource="http://www.wageneder.at/ontology/bpmn2.0#id"/>
                <owl:qualifiedCardinality rdf:datatype="http://www.w3.org/2001/XMLSchema#nonNegativeInteger">1</owl:qualifiedCardinality>
                <owl:onDataRange rdf:resource="http://www.w3.org/2001/XMLSchema#string"/>
            </owl:Restriction>
        </rdfs:subClassOf>
        <rdfs:subClassOf>
            <owl:Restriction>
                <owl:onProperty rdf:resource="http://www.wageneder.at/ontology/bpmn2.0#name"/>
                <owl:maxQualifiedCardinality rdf:datatype="http://www.w3.org/2001/XMLSchema#nonNegativeInteger">1</owl:maxQualifiedCardinality>
                <owl:onDataRange rdf:resource="http://www.w3.org/2001/XMLSchema#string"/>
            </owl:Restriction>
        </rdfs:subClassOf>
        <rdfs:comment>The Data Store Reference element inherits the attributes and model associations of FlowElement (see Table 8.44) and ItemAwareElement (see Table 10.51). Table 10.56 presents the additional model associations of the Data Store Reference element.</rdfs:comment>
    </owl:Class>
    


    <!-- http://www.wageneder.at/ontology/bpmn2.0#Definitions -->

    <owl:Class rdf:about="http://www.wageneder.at/ontology/bpmn2.0#Definitions">
        <rdfs:subClassOf rdf:resource="http://www.wageneder.at/ontology/bpmn2.0#BaseElement"/>
        <rdfs:subClassOf rdf:resource="http://www.wageneder.at/ontology/bpmn2.0#Infrastructure"/>
        <rdfs:subClassOf>
            <owl:Restriction>
                <owl:onProperty rdf:resource="http://www.wageneder.at/ontology/bpmn2.0#hasDiagrams"/>
                <owl:minQualifiedCardinality rdf:datatype="http://www.w3.org/2001/XMLSchema#nonNegativeInteger">0</owl:minQualifiedCardinality>
                <owl:onClass rdf:resource="http://www.wageneder.at/ontology/bpmn2.0#BPMNDiagram"/>
            </owl:Restriction>
        </rdfs:subClassOf>
        <rdfs:subClassOf>
            <owl:Restriction>
                <owl:onProperty rdf:resource="http://www.wageneder.at/ontology/bpmn2.0#hasExtensions"/>
                <owl:minQualifiedCardinality rdf:datatype="http://www.w3.org/2001/XMLSchema#nonNegativeInteger">0</owl:minQualifiedCardinality>
                <owl:onClass rdf:resource="http://www.wageneder.at/ontology/bpmn2.0#Extension"/>
            </owl:Restriction>
        </rdfs:subClassOf>
        <rdfs:subClassOf>
            <owl:Restriction>
                <owl:onProperty rdf:resource="http://www.wageneder.at/ontology/bpmn2.0#hasImports"/>
                <owl:minQualifiedCardinality rdf:datatype="http://www.w3.org/2001/XMLSchema#nonNegativeInteger">0</owl:minQualifiedCardinality>
                <owl:onClass rdf:resource="http://www.wageneder.at/ontology/bpmn2.0#Import"/>
            </owl:Restriction>
        </rdfs:subClassOf>
        <rdfs:subClassOf>
            <owl:Restriction>
                <owl:onProperty rdf:resource="http://www.wageneder.at/ontology/bpmn2.0#hasRelationships"/>
                <owl:minQualifiedCardinality rdf:datatype="http://www.w3.org/2001/XMLSchema#nonNegativeInteger">0</owl:minQualifiedCardinality>
                <owl:onClass rdf:resource="http://www.wageneder.at/ontology/bpmn2.0#Relationship"/>
            </owl:Restriction>
        </rdfs:subClassOf>
        <rdfs:subClassOf>
            <owl:Restriction>
                <owl:onProperty rdf:resource="http://www.wageneder.at/ontology/bpmn2.0#hasRootElements"/>
                <owl:minQualifiedCardinality rdf:datatype="http://www.w3.org/2001/XMLSchema#nonNegativeInteger">0</owl:minQualifiedCardinality>
                <owl:onClass rdf:resource="http://www.wageneder.at/ontology/bpmn2.0#RootElement"/>
            </owl:Restriction>
        </rdfs:subClassOf>
        <rdfs:subClassOf>
            <owl:Restriction>
                <owl:onProperty rdf:resource="http://www.wageneder.at/ontology/bpmn2.0#exporter"/>
                <owl:minQualifiedCardinality rdf:datatype="http://www.w3.org/2001/XMLSchema#nonNegativeInteger">0</owl:minQualifiedCardinality>
                <owl:onDataRange rdf:resource="http://www.w3.org/2001/XMLSchema#string"/>
            </owl:Restriction>
        </rdfs:subClassOf>
        <rdfs:subClassOf>
            <owl:Restriction>
                <owl:onProperty rdf:resource="http://www.wageneder.at/ontology/bpmn2.0#exporterVersion"/>
                <owl:minQualifiedCardinality rdf:datatype="http://www.w3.org/2001/XMLSchema#nonNegativeInteger">0</owl:minQualifiedCardinality>
                <owl:onDataRange rdf:resource="http://www.w3.org/2001/XMLSchema#string"/>
            </owl:Restriction>
        </rdfs:subClassOf>
        <rdfs:subClassOf>
            <owl:Restriction>
                <owl:onProperty rdf:resource="http://www.wageneder.at/ontology/bpmn2.0#expressionLanguage"/>
                <owl:minQualifiedCardinality rdf:datatype="http://www.w3.org/2001/XMLSchema#nonNegativeInteger">0</owl:minQualifiedCardinality>
                <owl:onDataRange rdf:resource="http://www.w3.org/2001/XMLSchema#string"/>
            </owl:Restriction>
        </rdfs:subClassOf>
        <rdfs:subClassOf>
            <owl:Restriction>
                <owl:onProperty rdf:resource="http://www.wageneder.at/ontology/bpmn2.0#typeLanguage"/>
                <owl:minQualifiedCardinality rdf:datatype="http://www.w3.org/2001/XMLSchema#nonNegativeInteger">0</owl:minQualifiedCardinality>
                <owl:onDataRange rdf:resource="http://www.w3.org/2001/XMLSchema#string"/>
            </owl:Restriction>
        </rdfs:subClassOf>
        <rdfs:subClassOf>
            <owl:Restriction>
                <owl:onProperty rdf:resource="http://www.wageneder.at/ontology/bpmn2.0#name"/>
                <owl:qualifiedCardinality rdf:datatype="http://www.w3.org/2001/XMLSchema#nonNegativeInteger">1</owl:qualifiedCardinality>
                <owl:onDataRange rdf:resource="http://www.w3.org/2001/XMLSchema#string"/>
            </owl:Restriction>
        </rdfs:subClassOf>
        <rdfs:subClassOf>
            <owl:Restriction>
                <owl:onProperty rdf:resource="http://www.wageneder.at/ontology/bpmn2.0#targetNamespace"/>
                <owl:qualifiedCardinality rdf:datatype="http://www.w3.org/2001/XMLSchema#nonNegativeInteger">1</owl:qualifiedCardinality>
                <owl:onDataRange rdf:resource="http://www.w3.org/2001/XMLSchema#string"/>
            </owl:Restriction>
        </rdfs:subClassOf>
        <rdfs:subClassOf>
            <owl:Restriction>
                <owl:onProperty rdf:resource="http://www.wageneder.at/ontology/bpmn2.0#exporter"/>
                <owl:maxQualifiedCardinality rdf:datatype="http://www.w3.org/2001/XMLSchema#nonNegativeInteger">1</owl:maxQualifiedCardinality>
                <owl:onDataRange rdf:resource="http://www.w3.org/2001/XMLSchema#string"/>
            </owl:Restriction>
        </rdfs:subClassOf>
        <rdfs:subClassOf>
            <owl:Restriction>
                <owl:onProperty rdf:resource="http://www.wageneder.at/ontology/bpmn2.0#exporterVersion"/>
                <owl:maxQualifiedCardinality rdf:datatype="http://www.w3.org/2001/XMLSchema#nonNegativeInteger">1</owl:maxQualifiedCardinality>
                <owl:onDataRange rdf:resource="http://www.w3.org/2001/XMLSchema#string"/>
            </owl:Restriction>
        </rdfs:subClassOf>
        <rdfs:subClassOf>
            <owl:Restriction>
                <owl:onProperty rdf:resource="http://www.wageneder.at/ontology/bpmn2.0#expressionLanguage"/>
                <owl:maxQualifiedCardinality rdf:datatype="http://www.w3.org/2001/XMLSchema#nonNegativeInteger">1</owl:maxQualifiedCardinality>
                <owl:onDataRange rdf:resource="http://www.w3.org/2001/XMLSchema#string"/>
            </owl:Restriction>
        </rdfs:subClassOf>
        <rdfs:subClassOf>
            <owl:Restriction>
                <owl:onProperty rdf:resource="http://www.wageneder.at/ontology/bpmn2.0#typeLanguage"/>
                <owl:maxQualifiedCardinality rdf:datatype="http://www.w3.org/2001/XMLSchema#nonNegativeInteger">1</owl:maxQualifiedCardinality>
                <owl:onDataRange rdf:resource="http://www.w3.org/2001/XMLSchema#string"/>
            </owl:Restriction>
        </rdfs:subClassOf>
        <rdfs:comment>The Definitions class is the outermost containing object for all BPMN elements. It defines the scope of visibility and the namespace for all contained elements. The interchange of BPMN files will always be through one or more Definitions.

The Definitions element inherits the attributes and model associations of BaseElement (see Table 8.5). Table 8.1 presents the additional attributes and model associations of the Definitions element.</rdfs:comment>
    </owl:Class>
    


    <!-- http://www.wageneder.at/ontology/bpmn2.0#Diverging -->

    <owl:Class rdf:about="http://www.wageneder.at/ontology/bpmn2.0#Diverging">
        <rdfs:subClassOf rdf:resource="http://www.wageneder.at/ontology/bpmn2.0#GatewayDirection"/>
        <rdfs:comment>Diverging: This Gateway MAY have multiple outgoing Sequence Flows but MUST have no more than one (1) incoming Sequence Flow.</rdfs:comment>
    </owl:Class>
    


    <!-- http://www.wageneder.at/ontology/bpmn2.0#Documentation -->

    <owl:Class rdf:about="http://www.wageneder.at/ontology/bpmn2.0#Documentation">
        <rdfs:subClassOf rdf:resource="http://www.wageneder.at/ontology/bpmn2.0#BaseElement"/>
        <rdfs:subClassOf>
            <owl:Restriction>
                <owl:onProperty rdf:resource="http://www.wageneder.at/ontology/bpmn2.0#text"/>
                <owl:qualifiedCardinality rdf:datatype="http://www.w3.org/2001/XMLSchema#nonNegativeInteger">1</owl:qualifiedCardinality>
                <owl:onDataRange rdf:resource="http://www.w3.org/2001/XMLSchema#string"/>
            </owl:Restriction>
        </rdfs:subClassOf>
        <rdfs:subClassOf>
            <owl:Restriction>
                <owl:onProperty rdf:resource="http://www.wageneder.at/ontology/bpmn2.0#textFormat"/>
                <owl:qualifiedCardinality rdf:datatype="http://www.w3.org/2001/XMLSchema#nonNegativeInteger">1</owl:qualifiedCardinality>
                <owl:onDataRange rdf:resource="http://www.w3.org/2001/XMLSchema#string"/>
            </owl:Restriction>
        </rdfs:subClassOf>
        <rdfs:comment>All BPMN elements that inherit from the BaseElement will have the capability, through the Documentation
element, to have one (1) or more text descriptions of that element.

The Documentation element inherits the attributes and model associations of BaseElement</rdfs:comment>
    </owl:Class>
    


    <!-- http://www.wageneder.at/ontology/bpmn2.0#Element -->

    <owl:Class rdf:about="http://www.wageneder.at/ontology/bpmn2.0#Element">
        <rdfs:subClassOf rdf:resource="http://www.wageneder.at/ontology/bpmn2.0#BaseElement"/>
        <rdfs:subClassOf rdf:resource="http://www.wageneder.at/ontology/bpmn2.0#CMOF"/>
        <rdfs:subClassOf>
            <owl:Restriction>
                <owl:onProperty rdf:resource="http://www.wageneder.at/ontology/bpmn2.0#hasImplementationRef"/>
                <owl:minQualifiedCardinality rdf:datatype="http://www.w3.org/2001/XMLSchema#nonNegativeInteger">0</owl:minQualifiedCardinality>
                <owl:onClass rdf:resource="http://www.wageneder.at/ontology/bpmn2.0#Element"/>
            </owl:Restriction>
        </rdfs:subClassOf>
        <rdfs:subClassOf>
            <owl:Restriction>
                <owl:onProperty rdf:resource="http://www.wageneder.at/ontology/bpmn2.0#hasImplementationRef"/>
                <owl:maxQualifiedCardinality rdf:datatype="http://www.w3.org/2001/XMLSchema#nonNegativeInteger">1</owl:maxQualifiedCardinality>
                <owl:onClass rdf:resource="http://www.wageneder.at/ontology/bpmn2.0#Element"/>
            </owl:Restriction>
        </rdfs:subClassOf>
        <rdfs:comment>Abstract Definiton of an Element</rdfs:comment>
    </owl:Class>
    


    <!-- http://www.wageneder.at/ontology/bpmn2.0#EndEvent -->

    <owl:Class rdf:about="http://www.wageneder.at/ontology/bpmn2.0#EndEvent">
        <rdfs:subClassOf rdf:resource="http://www.wageneder.at/ontology/bpmn2.0#ThrowEvent"/>
        <rdfs:comment>As the name implies, the End Event indicates where a Process will end. In terms of Sequence Flows, the End Event ends the flow of the Process, and thus, will not have any outgoing Sequence Flows—no Sequence Flow can connect from an End Event.</rdfs:comment>
    </owl:Class>
    


    <!-- http://www.wageneder.at/ontology/bpmn2.0#EndPoint -->

    <owl:Class rdf:about="http://www.wageneder.at/ontology/bpmn2.0#EndPoint">
        <rdfs:subClassOf rdf:resource="http://www.wageneder.at/ontology/bpmn2.0#RootElement"/>
        <rdfs:subClassOf rdf:resource="http://www.wageneder.at/ontology/bpmn2.0#Service"/>
    </owl:Class>
    


    <!-- http://www.wageneder.at/ontology/bpmn2.0#Error -->

    <owl:Class rdf:about="http://www.wageneder.at/ontology/bpmn2.0#Error">
        <rdfs:subClassOf rdf:resource="http://www.wageneder.at/ontology/bpmn2.0#Common"/>
        <rdfs:subClassOf rdf:resource="http://www.wageneder.at/ontology/bpmn2.0#RootElement"/>
        <rdfs:subClassOf>
            <owl:Restriction>
                <owl:onProperty rdf:resource="http://www.wageneder.at/ontology/bpmn2.0#hasStructureRef"/>
                <owl:minQualifiedCardinality rdf:datatype="http://www.w3.org/2001/XMLSchema#nonNegativeInteger">0</owl:minQualifiedCardinality>
                <owl:onClass rdf:resource="http://www.wageneder.at/ontology/bpmn2.0#ItemDefinition"/>
            </owl:Restriction>
        </rdfs:subClassOf>
        <rdfs:subClassOf>
            <owl:Restriction>
                <owl:onProperty rdf:resource="http://www.wageneder.at/ontology/bpmn2.0#hasStructureRef"/>
                <owl:maxQualifiedCardinality rdf:datatype="http://www.w3.org/2001/XMLSchema#nonNegativeInteger">1</owl:maxQualifiedCardinality>
                <owl:onClass rdf:resource="http://www.wageneder.at/ontology/bpmn2.0#ItemDefinition"/>
            </owl:Restriction>
        </rdfs:subClassOf>
        <rdfs:subClassOf>
            <owl:Restriction>
                <owl:onProperty rdf:resource="http://www.wageneder.at/ontology/bpmn2.0#errorCode"/>
                <owl:qualifiedCardinality rdf:datatype="http://www.w3.org/2001/XMLSchema#nonNegativeInteger">1</owl:qualifiedCardinality>
                <owl:onDataRange rdf:resource="http://www.w3.org/2001/XMLSchema#string"/>
            </owl:Restriction>
        </rdfs:subClassOf>
        <rdfs:subClassOf>
            <owl:Restriction>
                <owl:onProperty rdf:resource="http://www.wageneder.at/ontology/bpmn2.0#name"/>
                <owl:qualifiedCardinality rdf:datatype="http://www.w3.org/2001/XMLSchema#nonNegativeInteger">1</owl:qualifiedCardinality>
                <owl:onDataRange rdf:resource="http://www.w3.org/2001/XMLSchema#string"/>
            </owl:Restriction>
        </rdfs:subClassOf>
        <rdfs:comment>An Error represents the content of an Error Event or the Fault of a failed Operation. An ItemDefinition is used to specify the structure of the Error. An Error is generated when there is a critical problem in the processing of an Activity or when the execution of an Operation failed.</rdfs:comment>
    </owl:Class>
    


    <!-- http://www.wageneder.at/ontology/bpmn2.0#ErrorEventDefinition -->

    <owl:Class rdf:about="http://www.wageneder.at/ontology/bpmn2.0#ErrorEventDefinition">
        <rdfs:subClassOf rdf:resource="http://www.wageneder.at/ontology/bpmn2.0#EventDefinition"/>
        <rdfs:subClassOf>
            <owl:Restriction>
                <owl:onProperty rdf:resource="http://www.wageneder.at/ontology/bpmn2.0#hasError"/>
                <owl:minQualifiedCardinality rdf:datatype="http://www.w3.org/2001/XMLSchema#nonNegativeInteger">0</owl:minQualifiedCardinality>
                <owl:onClass rdf:resource="http://www.wageneder.at/ontology/bpmn2.0#Error"/>
            </owl:Restriction>
        </rdfs:subClassOf>
        <rdfs:subClassOf>
            <owl:Restriction>
                <owl:onProperty rdf:resource="http://www.wageneder.at/ontology/bpmn2.0#hasError"/>
                <owl:maxQualifiedCardinality rdf:datatype="http://www.w3.org/2001/XMLSchema#nonNegativeInteger">1</owl:maxQualifiedCardinality>
                <owl:onClass rdf:resource="http://www.wageneder.at/ontology/bpmn2.0#Error"/>
            </owl:Restriction>
        </rdfs:subClassOf>
        <rdfs:comment>The ErrorEventDefinition element inherits the attributes and model associations of BaseElement through its relationship to the EventDefinition element</rdfs:comment>
    </owl:Class>
    


    <!-- http://www.wageneder.at/ontology/bpmn2.0#Escalation -->

    <owl:Class rdf:about="http://www.wageneder.at/ontology/bpmn2.0#Escalation">
        <rdfs:subClassOf rdf:resource="http://www.wageneder.at/ontology/bpmn2.0#EventLevel"/>
        <rdfs:subClassOf rdf:resource="http://www.wageneder.at/ontology/bpmn2.0#RootElement"/>
        <rdfs:subClassOf>
            <owl:Restriction>
                <owl:onProperty rdf:resource="http://www.wageneder.at/ontology/bpmn2.0#hasStructureRef"/>
                <owl:minQualifiedCardinality rdf:datatype="http://www.w3.org/2001/XMLSchema#nonNegativeInteger">0</owl:minQualifiedCardinality>
                <owl:onClass rdf:resource="http://www.wageneder.at/ontology/bpmn2.0#ItemDefinition"/>
            </owl:Restriction>
        </rdfs:subClassOf>
        <rdfs:subClassOf>
            <owl:Restriction>
                <owl:onProperty rdf:resource="http://www.wageneder.at/ontology/bpmn2.0#hasStructureRef"/>
                <owl:maxQualifiedCardinality rdf:datatype="http://www.w3.org/2001/XMLSchema#nonNegativeInteger">1</owl:maxQualifiedCardinality>
                <owl:onClass rdf:resource="http://www.wageneder.at/ontology/bpmn2.0#ItemDefinition"/>
            </owl:Restriction>
        </rdfs:subClassOf>
        <rdfs:subClassOf>
            <owl:Restriction>
                <owl:onProperty rdf:resource="http://www.wageneder.at/ontology/bpmn2.0#escalationCode"/>
                <owl:qualifiedCardinality rdf:datatype="http://www.w3.org/2001/XMLSchema#nonNegativeInteger">1</owl:qualifiedCardinality>
                <owl:onDataRange rdf:resource="http://www.w3.org/2001/XMLSchema#string"/>
            </owl:Restriction>
        </rdfs:subClassOf>
        <rdfs:subClassOf>
            <owl:Restriction>
                <owl:onProperty rdf:resource="http://www.wageneder.at/ontology/bpmn2.0#name"/>
                <owl:qualifiedCardinality rdf:datatype="http://www.w3.org/2001/XMLSchema#nonNegativeInteger">1</owl:qualifiedCardinality>
                <owl:onDataRange rdf:resource="http://www.w3.org/2001/XMLSchema#string"/>
            </owl:Restriction>
        </rdfs:subClassOf>
        <rdfs:comment>An Escalation identifies a business situation that a Process might need to react to. An ItemDefinition is used
to specify the structure of the Escalation.</rdfs:comment>
    </owl:Class>
    


    <!-- http://www.wageneder.at/ontology/bpmn2.0#EscalationEventDefinition -->

    <owl:Class rdf:about="http://www.wageneder.at/ontology/bpmn2.0#EscalationEventDefinition">
        <rdfs:subClassOf rdf:resource="http://www.wageneder.at/ontology/bpmn2.0#EventDefinition"/>
        <rdfs:subClassOf>
            <owl:Restriction>
                <owl:onProperty rdf:resource="http://www.wageneder.at/ontology/bpmn2.0#hasEscalationRef"/>
                <owl:minQualifiedCardinality rdf:datatype="http://www.w3.org/2001/XMLSchema#nonNegativeInteger">0</owl:minQualifiedCardinality>
                <owl:onClass rdf:resource="http://www.wageneder.at/ontology/bpmn2.0#Escalation"/>
            </owl:Restriction>
        </rdfs:subClassOf>
        <rdfs:subClassOf>
            <owl:Restriction>
                <owl:onProperty rdf:resource="http://www.wageneder.at/ontology/bpmn2.0#hasEscalationRef"/>
                <owl:maxQualifiedCardinality rdf:datatype="http://www.w3.org/2001/XMLSchema#nonNegativeInteger">1</owl:maxQualifiedCardinality>
                <owl:onClass rdf:resource="http://www.wageneder.at/ontology/bpmn2.0#Escalation"/>
            </owl:Restriction>
        </rdfs:subClassOf>
        <rdfs:comment>The EscalationEventDefinition element inherits the attributes and model associations of BaseElement through its relationship to the EventDefinition element</rdfs:comment>
    </owl:Class>
    


    <!-- http://www.wageneder.at/ontology/bpmn2.0#Event -->

    <owl:Class rdf:about="http://www.wageneder.at/ontology/bpmn2.0#Event">
        <rdfs:subClassOf rdf:resource="http://www.wageneder.at/ontology/bpmn2.0#EventLevel"/>
        <rdfs:subClassOf rdf:resource="http://www.wageneder.at/ontology/bpmn2.0#FlowNode"/>
        <rdfs:subClassOf rdf:resource="http://www.wageneder.at/ontology/bpmn2.0#InteractionNode"/>
        <rdfs:subClassOf>
            <owl:Restriction>
                <owl:onProperty rdf:resource="http://www.wageneder.at/ontology/bpmn2.0#hasProperties"/>
                <owl:minQualifiedCardinality rdf:datatype="http://www.w3.org/2001/XMLSchema#nonNegativeInteger">0</owl:minQualifiedCardinality>
                <owl:onClass rdf:resource="http://www.wageneder.at/ontology/bpmn2.0#Property"/>
            </owl:Restriction>
        </rdfs:subClassOf>
        <rdfs:comment>An Event is something that “happens” during the course of a Process. These Events affect the flow of the Process and usually have a cause or an impact. The term “event” is general enough to cover many things in a Process. The start of an Activity, the end of an Activity, the change of state of a document, a Message that arrives, etc., all could be considered Events. However, BPMN has restricted the use of Events to include only those types of Events that will affect the sequence or timing of Activities of a Process.</rdfs:comment>
    </owl:Class>
    


    <!-- http://www.wageneder.at/ontology/bpmn2.0#EventBasedGateway -->

    <owl:Class rdf:about="http://www.wageneder.at/ontology/bpmn2.0#EventBasedGateway">
        <rdfs:subClassOf rdf:resource="http://www.wageneder.at/ontology/bpmn2.0#Gateway"/>
        <rdfs:subClassOf>
            <owl:Restriction>
                <owl:onProperty rdf:resource="http://www.wageneder.at/ontology/bpmn2.0#hasEventGatewayType"/>
                <owl:qualifiedCardinality rdf:datatype="http://www.w3.org/2001/XMLSchema#nonNegativeInteger">1</owl:qualifiedCardinality>
                <owl:onClass rdf:resource="http://www.wageneder.at/ontology/bpmn2.0#EventBasedGatewayType"/>
            </owl:Restriction>
        </rdfs:subClassOf>
        <rdfs:subClassOf>
            <owl:Restriction>
                <owl:onProperty rdf:resource="http://www.wageneder.at/ontology/bpmn2.0#hasConditionExpression"/>
                <owl:maxQualifiedCardinality rdf:datatype="http://www.w3.org/2001/XMLSchema#nonNegativeInteger">0</owl:maxQualifiedCardinality>
                <owl:onClass rdf:resource="http://www.wageneder.at/ontology/bpmn2.0#Expression"/>
            </owl:Restriction>
        </rdfs:subClassOf>
        <rdfs:subClassOf>
            <owl:Restriction>
                <owl:onProperty rdf:resource="http://www.wageneder.at/ontology/bpmn2.0#instantiate"/>
                <owl:qualifiedCardinality rdf:datatype="http://www.w3.org/2001/XMLSchema#nonNegativeInteger">1</owl:qualifiedCardinality>
                <owl:onDataRange rdf:resource="http://www.w3.org/2001/XMLSchema#boolean"/>
            </owl:Restriction>
        </rdfs:subClassOf>
        <rdfs:comment>The Event-Based Gateway represents a branching point in the Process where the alternative paths that follow the Gateway are based on Events that occur, rather than the evaluation of Expressions using Process data (as with an Exclusive or Inclusive Gateway). A specific Event, usually the receipt of a Message, determines the path that will be taken. Basically, the decision is made by another Participant, based on data that is not visible to Process, thus, requiring the use of the Event-Based Gateway.</rdfs:comment>
    </owl:Class>
    


    <!-- http://www.wageneder.at/ontology/bpmn2.0#EventBasedGatewayType -->

    <owl:Class rdf:about="http://www.wageneder.at/ontology/bpmn2.0#EventBasedGatewayType">
        <rdfs:subClassOf rdf:resource="http://www.wageneder.at/ontology/bpmn2.0#GatewayLevel"/>
        <rdfs:subClassOf>
            <owl:Class>
                <owl:unionOf rdf:parseType="Collection">
                    <rdf:Description rdf:about="http://www.wageneder.at/ontology/bpmn2.0#Exclusive"/>
                    <rdf:Description rdf:about="http://www.wageneder.at/ontology/bpmn2.0#Parallel"/>
                </owl:unionOf>
            </owl:Class>
        </rdfs:subClassOf>
    </owl:Class>
    


    <!-- http://www.wageneder.at/ontology/bpmn2.0#EventDefinition -->

    <owl:Class rdf:about="http://www.wageneder.at/ontology/bpmn2.0#EventDefinition">
        <rdfs:subClassOf rdf:resource="http://www.wageneder.at/ontology/bpmn2.0#EventLevel"/>
        <rdfs:subClassOf rdf:resource="http://www.wageneder.at/ontology/bpmn2.0#RootElement"/>
        <rdfs:comment>Event Definitions refers to the triggers of Catch Events (Start and receive Intermediate Events) and the Results of Throw Events (End Events and send Intermediate Events).</rdfs:comment>
    </owl:Class>
    


    <!-- http://www.wageneder.at/ontology/bpmn2.0#EventLevel -->

    <owl:Class rdf:about="http://www.wageneder.at/ontology/bpmn2.0#EventLevel">
        <rdfs:subClassOf rdf:resource="http://www.wageneder.at/ontology/bpmn2.0#Common"/>
        <rdfs:comment>This is just a hierarchical element for organisational purposes.
It presents the Events Folder</rdfs:comment>
    </owl:Class>
    


    <!-- http://www.wageneder.at/ontology/bpmn2.0#Exclusive -->

    <owl:Class rdf:about="http://www.wageneder.at/ontology/bpmn2.0#Exclusive">
        <rdfs:subClassOf rdf:resource="http://www.wageneder.at/ontology/bpmn2.0#EventBasedGatewayType"/>
    </owl:Class>
    


    <!-- http://www.wageneder.at/ontology/bpmn2.0#ExclusiveGateway -->

    <owl:Class rdf:about="http://www.wageneder.at/ontology/bpmn2.0#ExclusiveGateway">
        <rdfs:subClassOf rdf:resource="http://www.wageneder.at/ontology/bpmn2.0#Gateway"/>
        <rdfs:subClassOf>
            <owl:Restriction>
                <owl:onProperty rdf:resource="http://www.wageneder.at/ontology/bpmn2.0#hasDefault"/>
                <owl:minQualifiedCardinality rdf:datatype="http://www.w3.org/2001/XMLSchema#nonNegativeInteger">0</owl:minQualifiedCardinality>
                <owl:onClass rdf:resource="http://www.wageneder.at/ontology/bpmn2.0#SequenceFlow"/>
            </owl:Restriction>
        </rdfs:subClassOf>
        <rdfs:subClassOf>
            <owl:Restriction>
                <owl:onProperty rdf:resource="http://www.wageneder.at/ontology/bpmn2.0#hasDefault"/>
                <owl:maxQualifiedCardinality rdf:datatype="http://www.w3.org/2001/XMLSchema#nonNegativeInteger">1</owl:maxQualifiedCardinality>
                <owl:onClass rdf:resource="http://www.wageneder.at/ontology/bpmn2.0#SequenceFlow"/>
            </owl:Restriction>
        </rdfs:subClassOf>
        <rdfs:comment>A diverging Exclusive Gateway (Decision) is used to create alternative paths within a Process flow. This is basically
the “diversion point in the road” for a Process. For a given instance of the Process, only one of the paths can be taken.</rdfs:comment>
    </owl:Class>
    


    <!-- http://www.wageneder.at/ontology/bpmn2.0#Expression -->

    <owl:Class rdf:about="http://www.wageneder.at/ontology/bpmn2.0#Expression">
        <rdfs:subClassOf rdf:resource="http://www.wageneder.at/ontology/bpmn2.0#BaseElement"/>
        <rdfs:subClassOf rdf:resource="http://www.wageneder.at/ontology/bpmn2.0#Common"/>
        <rdfs:subClassOf>
            <owl:Restriction>
                <owl:onProperty rdf:resource="http://www.wageneder.at/ontology/bpmn2.0#hasAssignment"/>
                <owl:minQualifiedCardinality rdf:datatype="http://www.w3.org/2001/XMLSchema#nonNegativeInteger">0</owl:minQualifiedCardinality>
                <owl:onClass rdf:resource="http://www.wageneder.at/ontology/bpmn2.0#Assignment"/>
            </owl:Restriction>
        </rdfs:subClassOf>
        <rdfs:subClassOf>
            <owl:Restriction>
                <owl:onProperty rdf:resource="http://www.wageneder.at/ontology/bpmn2.0#hasComplexGateway"/>
                <owl:minQualifiedCardinality rdf:datatype="http://www.w3.org/2001/XMLSchema#nonNegativeInteger">0</owl:minQualifiedCardinality>
                <owl:onClass rdf:resource="http://www.wageneder.at/ontology/bpmn2.0#ComplexGateway"/>
            </owl:Restriction>
        </rdfs:subClassOf>
        <rdfs:subClassOf>
            <owl:Restriction>
                <owl:onProperty rdf:resource="http://www.wageneder.at/ontology/bpmn2.0#hasAssignment"/>
                <owl:maxQualifiedCardinality rdf:datatype="http://www.w3.org/2001/XMLSchema#nonNegativeInteger">1</owl:maxQualifiedCardinality>
                <owl:onClass rdf:resource="http://www.wageneder.at/ontology/bpmn2.0#Assignment"/>
            </owl:Restriction>
        </rdfs:subClassOf>
        <rdfs:subClassOf>
            <owl:Restriction>
                <owl:onProperty rdf:resource="http://www.wageneder.at/ontology/bpmn2.0#hasComplexGateway"/>
                <owl:maxQualifiedCardinality rdf:datatype="http://www.w3.org/2001/XMLSchema#nonNegativeInteger">1</owl:maxQualifiedCardinality>
                <owl:onClass rdf:resource="http://www.wageneder.at/ontology/bpmn2.0#ComplexGateway"/>
            </owl:Restriction>
        </rdfs:subClassOf>
        <rdfs:comment>The Expression class is used to specify an Expression using natural-language text. These Expressions are not executable. The natural language text is captured using the documentation attribute, inherited from BaseElement.
Expression inherits the attributes and model associations of BaseElement (see Table 8.5), but adds no additional attributes or model associations.</rdfs:comment>
    </owl:Class>
    


    <!-- http://www.wageneder.at/ontology/bpmn2.0#Extensibility -->

    <owl:Class rdf:about="http://www.wageneder.at/ontology/bpmn2.0#Extensibility">
        <rdfs:subClassOf rdf:resource="http://www.wageneder.at/ontology/bpmn2.0#Foundation"/>
    </owl:Class>
    


    <!-- http://www.wageneder.at/ontology/bpmn2.0#Extension -->

    <owl:Class rdf:about="http://www.wageneder.at/ontology/bpmn2.0#Extension">
        <rdfs:subClassOf rdf:resource="http://www.wageneder.at/ontology/bpmn2.0#ExtensionLevel"/>
        <rdfs:subClassOf>
            <owl:Restriction>
                <owl:onProperty rdf:resource="http://www.wageneder.at/ontology/bpmn2.0#hasDefinition"/>
                <owl:qualifiedCardinality rdf:datatype="http://www.w3.org/2001/XMLSchema#nonNegativeInteger">1</owl:qualifiedCardinality>
                <owl:onClass rdf:resource="http://www.wageneder.at/ontology/bpmn2.0#ExtensionDefinition"/>
            </owl:Restriction>
        </rdfs:subClassOf>
        <rdfs:subClassOf>
            <owl:Restriction>
                <owl:onProperty rdf:resource="http://www.wageneder.at/ontology/bpmn2.0#mustUnderstand"/>
                <owl:qualifiedCardinality rdf:datatype="http://www.w3.org/2001/XMLSchema#nonNegativeInteger">1</owl:qualifiedCardinality>
                <owl:onDataRange rdf:resource="http://www.w3.org/2001/XMLSchema#boolean"/>
            </owl:Restriction>
        </rdfs:subClassOf>
        <rdfs:comment>The Extension element binds/imports an ExtensionDefinition and its attributes to a BPMN model definition.</rdfs:comment>
    </owl:Class>
    


    <!-- http://www.wageneder.at/ontology/bpmn2.0#ExtensionAttributeDefinition -->

    <owl:Class rdf:about="http://www.wageneder.at/ontology/bpmn2.0#ExtensionAttributeDefinition">
        <rdfs:subClassOf rdf:resource="http://www.wageneder.at/ontology/bpmn2.0#ExtensionLevel"/>
        <rdfs:subClassOf>
            <owl:Restriction>
                <owl:onProperty rdf:resource="http://www.wageneder.at/ontology/bpmn2.0#isReference"/>
                <owl:qualifiedCardinality rdf:datatype="http://www.w3.org/2001/XMLSchema#nonNegativeInteger">1</owl:qualifiedCardinality>
                <owl:onDataRange rdf:resource="http://www.w3.org/2001/XMLSchema#boolean"/>
            </owl:Restriction>
        </rdfs:subClassOf>
        <rdfs:subClassOf>
            <owl:Restriction>
                <owl:onProperty rdf:resource="http://www.wageneder.at/ontology/bpmn2.0#name"/>
                <owl:qualifiedCardinality rdf:datatype="http://www.w3.org/2001/XMLSchema#nonNegativeInteger">1</owl:qualifiedCardinality>
                <owl:onDataRange rdf:resource="http://www.w3.org/2001/XMLSchema#string"/>
            </owl:Restriction>
        </rdfs:subClassOf>
        <rdfs:subClassOf>
            <owl:Restriction>
                <owl:onProperty rdf:resource="http://www.wageneder.at/ontology/bpmn2.0#type"/>
                <owl:qualifiedCardinality rdf:datatype="http://www.w3.org/2001/XMLSchema#nonNegativeInteger">1</owl:qualifiedCardinality>
                <owl:onDataRange rdf:resource="http://www.w3.org/2001/XMLSchema#string"/>
            </owl:Restriction>
        </rdfs:subClassOf>
        <rdfs:comment>The ExtensionAttributeDefinition defines new attributes. This type is not applicable when the XML schema interchange is used; since the XSD mechanisms for supporting “AnyAttribute” and “Any” type already satisfy this requirement.</rdfs:comment>
    </owl:Class>
    


    <!-- http://www.wageneder.at/ontology/bpmn2.0#ExtensionAttributeValue -->

    <owl:Class rdf:about="http://www.wageneder.at/ontology/bpmn2.0#ExtensionAttributeValue">
        <rdfs:subClassOf rdf:resource="http://www.wageneder.at/ontology/bpmn2.0#ExtensionLevel"/>
        <rdfs:subClassOf>
            <owl:Restriction>
                <owl:onProperty rdf:resource="http://www.wageneder.at/ontology/bpmn2.0#hasValue"/>
                <owl:minQualifiedCardinality rdf:datatype="http://www.w3.org/2001/XMLSchema#nonNegativeInteger">0</owl:minQualifiedCardinality>
                <owl:onClass rdf:resource="http://www.wageneder.at/ontology/bpmn2.0#Element"/>
            </owl:Restriction>
        </rdfs:subClassOf>
        <rdfs:subClassOf>
            <owl:Restriction>
                <owl:onProperty rdf:resource="http://www.wageneder.at/ontology/bpmn2.0#hasValueRef"/>
                <owl:minQualifiedCardinality rdf:datatype="http://www.w3.org/2001/XMLSchema#nonNegativeInteger">0</owl:minQualifiedCardinality>
                <owl:onClass rdf:resource="http://www.wageneder.at/ontology/bpmn2.0#Element"/>
            </owl:Restriction>
        </rdfs:subClassOf>
        <rdfs:subClassOf>
            <owl:Restriction>
                <owl:onProperty rdf:resource="http://www.wageneder.at/ontology/bpmn2.0#hasExtensionAttributeDefinition"/>
                <owl:qualifiedCardinality rdf:datatype="http://www.w3.org/2001/XMLSchema#nonNegativeInteger">1</owl:qualifiedCardinality>
                <owl:onClass rdf:resource="http://www.wageneder.at/ontology/bpmn2.0#ExtensionAttributeDefinition"/>
            </owl:Restriction>
        </rdfs:subClassOf>
        <rdfs:subClassOf>
            <owl:Restriction>
                <owl:onProperty rdf:resource="http://www.wageneder.at/ontology/bpmn2.0#hasValue"/>
                <owl:maxQualifiedCardinality rdf:datatype="http://www.w3.org/2001/XMLSchema#nonNegativeInteger">1</owl:maxQualifiedCardinality>
                <owl:onClass rdf:resource="http://www.wageneder.at/ontology/bpmn2.0#Element"/>
            </owl:Restriction>
        </rdfs:subClassOf>
        <rdfs:subClassOf>
            <owl:Restriction>
                <owl:onProperty rdf:resource="http://www.wageneder.at/ontology/bpmn2.0#hasValueRef"/>
                <owl:maxQualifiedCardinality rdf:datatype="http://www.w3.org/2001/XMLSchema#nonNegativeInteger">1</owl:maxQualifiedCardinality>
                <owl:onClass rdf:resource="http://www.wageneder.at/ontology/bpmn2.0#Element"/>
            </owl:Restriction>
        </rdfs:subClassOf>
        <rdfs:comment>The ExtensionAttributeValue contains the attribute value. This type is not applicable when the XML schema interchange is used; since the XSD mechanisms for supporting “AnyAttribute” and “Any” type already satisfy this requirement.</rdfs:comment>
    </owl:Class>
    


    <!-- http://www.wageneder.at/ontology/bpmn2.0#ExtensionDefinition -->

    <owl:Class rdf:about="http://www.wageneder.at/ontology/bpmn2.0#ExtensionDefinition">
        <rdfs:subClassOf rdf:resource="http://www.wageneder.at/ontology/bpmn2.0#ExtensionLevel"/>
        <rdfs:subClassOf>
            <owl:Restriction>
                <owl:onProperty rdf:resource="http://www.wageneder.at/ontology/bpmn2.0#hasExtensionAttributeDefinitions"/>
                <owl:minQualifiedCardinality rdf:datatype="http://www.w3.org/2001/XMLSchema#nonNegativeInteger">0</owl:minQualifiedCardinality>
                <owl:onClass rdf:resource="http://www.wageneder.at/ontology/bpmn2.0#ExtensionAttributeDefinition"/>
            </owl:Restriction>
        </rdfs:subClassOf>
        <rdfs:subClassOf>
            <owl:Restriction>
                <owl:onProperty rdf:resource="http://www.wageneder.at/ontology/bpmn2.0#name"/>
                <owl:qualifiedCardinality rdf:datatype="http://www.w3.org/2001/XMLSchema#nonNegativeInteger">1</owl:qualifiedCardinality>
                <owl:onDataRange rdf:resource="http://www.w3.org/2001/XMLSchema#string"/>
            </owl:Restriction>
        </rdfs:subClassOf>
        <rdfs:comment>The ExtensionDefinition class defines and groups additional attributes. This type is not applicable when the XML schema interchange is used, since XSD Complex Types already satisfy this requirement.</rdfs:comment>
    </owl:Class>
    


    <!-- http://www.wageneder.at/ontology/bpmn2.0#ExtensionLevel -->

    <owl:Class rdf:about="http://www.wageneder.at/ontology/bpmn2.0#ExtensionLevel">
        <rdfs:subClassOf rdf:resource="http://www.wageneder.at/ontology/bpmn2.0#Foundation"/>
        <rdfs:comment>This is just a hierarchical element for organisational purposes.
It presents the Extension Folder

A BPMN Extension basically consists of four different elements:
1. Extension
2. ExtensionDefinition
3. ExtensionAttributeDefinition
4. ExtensionAttributeValue</rdfs:comment>
    </owl:Class>
    


    <!-- http://www.wageneder.at/ontology/bpmn2.0#ExternalRelationships -->

    <owl:Class rdf:about="http://www.wageneder.at/ontology/bpmn2.0#ExternalRelationships">
        <rdfs:subClassOf rdf:resource="http://www.wageneder.at/ontology/bpmn2.0#RootElement"/>
    </owl:Class>
    


    <!-- http://www.wageneder.at/ontology/bpmn2.0#FlowElement -->

    <owl:Class rdf:about="http://www.wageneder.at/ontology/bpmn2.0#FlowElement">
        <rdfs:subClassOf rdf:resource="http://www.wageneder.at/ontology/bpmn2.0#BaseElement"/>
        <rdfs:subClassOf rdf:resource="http://www.wageneder.at/ontology/bpmn2.0#Common"/>
        <rdfs:subClassOf>
            <owl:Restriction>
                <owl:onProperty rdf:resource="http://www.wageneder.at/ontology/bpmn2.0#hasAuditing"/>
                <owl:minQualifiedCardinality rdf:datatype="http://www.w3.org/2001/XMLSchema#nonNegativeInteger">0</owl:minQualifiedCardinality>
                <owl:onClass rdf:resource="http://www.wageneder.at/ontology/bpmn2.0#Auditing"/>
            </owl:Restriction>
        </rdfs:subClassOf>
        <rdfs:subClassOf>
            <owl:Restriction>
                <owl:onProperty rdf:resource="http://www.wageneder.at/ontology/bpmn2.0#hasCategoryValueRef"/>
                <owl:minQualifiedCardinality rdf:datatype="http://www.w3.org/2001/XMLSchema#nonNegativeInteger">0</owl:minQualifiedCardinality>
                <owl:onClass rdf:resource="http://www.wageneder.at/ontology/bpmn2.0#CategoryValue"/>
            </owl:Restriction>
        </rdfs:subClassOf>
        <rdfs:subClassOf>
            <owl:Restriction>
                <owl:onProperty rdf:resource="http://www.wageneder.at/ontology/bpmn2.0#hasMonitoring"/>
                <owl:minQualifiedCardinality rdf:datatype="http://www.w3.org/2001/XMLSchema#nonNegativeInteger">0</owl:minQualifiedCardinality>
                <owl:onClass rdf:resource="http://www.wageneder.at/ontology/bpmn2.0#Monitoring"/>
            </owl:Restriction>
        </rdfs:subClassOf>
        <rdfs:subClassOf>
            <owl:Restriction>
                <owl:onProperty rdf:resource="http://www.wageneder.at/ontology/bpmn2.0#hasContainer"/>
                <owl:qualifiedCardinality rdf:datatype="http://www.w3.org/2001/XMLSchema#nonNegativeInteger">1</owl:qualifiedCardinality>
                <owl:onClass rdf:resource="http://www.wageneder.at/ontology/bpmn2.0#FlowElementsContainer"/>
            </owl:Restriction>
        </rdfs:subClassOf>
        <rdfs:subClassOf>
            <owl:Restriction>
                <owl:onProperty rdf:resource="http://www.wageneder.at/ontology/bpmn2.0#hasAuditing"/>
                <owl:maxQualifiedCardinality rdf:datatype="http://www.w3.org/2001/XMLSchema#nonNegativeInteger">1</owl:maxQualifiedCardinality>
                <owl:onClass rdf:resource="http://www.wageneder.at/ontology/bpmn2.0#Auditing"/>
            </owl:Restriction>
        </rdfs:subClassOf>
        <rdfs:subClassOf>
            <owl:Restriction>
                <owl:onProperty rdf:resource="http://www.wageneder.at/ontology/bpmn2.0#hasMonitoring"/>
                <owl:maxQualifiedCardinality rdf:datatype="http://www.w3.org/2001/XMLSchema#nonNegativeInteger">1</owl:maxQualifiedCardinality>
                <owl:onClass rdf:resource="http://www.wageneder.at/ontology/bpmn2.0#Monitoring"/>
            </owl:Restriction>
        </rdfs:subClassOf>
        <rdfs:subClassOf>
            <owl:Restriction>
                <owl:onProperty rdf:resource="http://www.wageneder.at/ontology/bpmn2.0#name"/>
                <owl:minQualifiedCardinality rdf:datatype="http://www.w3.org/2001/XMLSchema#nonNegativeInteger">0</owl:minQualifiedCardinality>
                <owl:onDataRange rdf:resource="http://www.w3.org/2001/XMLSchema#string"/>
            </owl:Restriction>
        </rdfs:subClassOf>
        <rdfs:subClassOf>
            <owl:Restriction>
                <owl:onProperty rdf:resource="http://www.wageneder.at/ontology/bpmn2.0#name"/>
                <owl:maxQualifiedCardinality rdf:datatype="http://www.w3.org/2001/XMLSchema#nonNegativeInteger">1</owl:maxQualifiedCardinality>
                <owl:onDataRange rdf:resource="http://www.w3.org/2001/XMLSchema#string"/>
            </owl:Restriction>
        </rdfs:subClassOf>
        <rdfs:comment rdf:datatype="http://www.w3.org/2001/XMLSchema#string">FlowElement is the abstract super class for all elements that can appear in a Process flow, which are FlowNodes</rdfs:comment>
        <rdfs:label xml:lang="de">FlowElement</rdfs:label>
    </owl:Class>
    


    <!-- http://www.wageneder.at/ontology/bpmn2.0#FlowElementsContainer -->

    <owl:Class rdf:about="http://www.wageneder.at/ontology/bpmn2.0#FlowElementsContainer">
        <rdfs:subClassOf rdf:resource="http://www.wageneder.at/ontology/bpmn2.0#BaseElement"/>
        <rdfs:subClassOf rdf:resource="http://www.wageneder.at/ontology/bpmn2.0#Common"/>
        <rdfs:subClassOf>
            <owl:Restriction>
                <owl:onProperty rdf:resource="http://www.wageneder.at/ontology/bpmn2.0#hasFlowElements"/>
                <owl:minQualifiedCardinality rdf:datatype="http://www.w3.org/2001/XMLSchema#nonNegativeInteger">0</owl:minQualifiedCardinality>
                <owl:onClass rdf:resource="http://www.wageneder.at/ontology/bpmn2.0#FlowElement"/>
            </owl:Restriction>
        </rdfs:subClassOf>
        <rdfs:subClassOf>
            <owl:Restriction>
                <owl:onProperty rdf:resource="http://www.wageneder.at/ontology/bpmn2.0#hasLaneSets"/>
                <owl:minQualifiedCardinality rdf:datatype="http://www.w3.org/2001/XMLSchema#nonNegativeInteger">0</owl:minQualifiedCardinality>
                <owl:onClass rdf:resource="http://www.wageneder.at/ontology/bpmn2.0#LaneSet"/>
            </owl:Restriction>
        </rdfs:subClassOf>
        <rdfs:comment>FlowElementsContainer is an abstract super class for BPMN diagrams (or views) and defines the superset of elements that are contained in those diagrams.</rdfs:comment>
        <rdfs:label xml:lang="de">FlowElementsContainer</rdfs:label>
    </owl:Class>
    


    <!-- http://www.wageneder.at/ontology/bpmn2.0#FlowNode -->

    <owl:Class rdf:about="http://www.wageneder.at/ontology/bpmn2.0#FlowNode">
        <rdfs:subClassOf rdf:resource="http://www.wageneder.at/ontology/bpmn2.0#FlowElement"/>
        <rdfs:subClassOf>
            <owl:Restriction>
                <owl:onProperty rdf:resource="http://www.wageneder.at/ontology/bpmn2.0#hasIncoming"/>
                <owl:minQualifiedCardinality rdf:datatype="http://www.w3.org/2001/XMLSchema#nonNegativeInteger">0</owl:minQualifiedCardinality>
                <owl:onClass rdf:resource="http://www.wageneder.at/ontology/bpmn2.0#SequenceFlow"/>
            </owl:Restriction>
        </rdfs:subClassOf>
        <rdfs:subClassOf>
            <owl:Restriction>
                <owl:onProperty rdf:resource="http://www.wageneder.at/ontology/bpmn2.0#hasLanes"/>
                <owl:minQualifiedCardinality rdf:datatype="http://www.w3.org/2001/XMLSchema#nonNegativeInteger">0</owl:minQualifiedCardinality>
                <owl:onClass rdf:resource="http://www.wageneder.at/ontology/bpmn2.0#Lane"/>
            </owl:Restriction>
        </rdfs:subClassOf>
        <rdfs:subClassOf>
            <owl:Restriction>
                <owl:onProperty rdf:resource="http://www.wageneder.at/ontology/bpmn2.0#hasOutgoing"/>
                <owl:minQualifiedCardinality rdf:datatype="http://www.w3.org/2001/XMLSchema#nonNegativeInteger">0</owl:minQualifiedCardinality>
                <owl:onClass rdf:resource="http://www.wageneder.at/ontology/bpmn2.0#SequenceFlow"/>
            </owl:Restriction>
        </rdfs:subClassOf>
        <rdfs:comment>The FlowNode element is used to provide a single element as the source and target Sequence Flow associations (see Figure 8.35) instead of the individual associations of the elements that can connect to Sequence Flows.</rdfs:comment>
    </owl:Class>
    


    <!-- http://www.wageneder.at/ontology/bpmn2.0#FormalExpression -->

    <owl:Class rdf:about="http://www.wageneder.at/ontology/bpmn2.0#FormalExpression">
        <rdfs:subClassOf rdf:resource="http://www.wageneder.at/ontology/bpmn2.0#Expression"/>
        <rdfs:subClassOf>
            <owl:Restriction>
                <owl:onProperty rdf:resource="http://www.wageneder.at/ontology/bpmn2.0#hasCorrelationSet"/>
                <owl:minQualifiedCardinality rdf:datatype="http://www.w3.org/2001/XMLSchema#nonNegativeInteger">0</owl:minQualifiedCardinality>
                <owl:onClass rdf:resource="http://www.wageneder.at/ontology/bpmn2.0#CorrelationPropertyRetrievalExpression"/>
            </owl:Restriction>
        </rdfs:subClassOf>
        <rdfs:subClassOf>
            <owl:Restriction>
                <owl:onProperty rdf:resource="http://www.wageneder.at/ontology/bpmn2.0#hasBody"/>
                <owl:qualifiedCardinality rdf:datatype="http://www.w3.org/2001/XMLSchema#nonNegativeInteger">1</owl:qualifiedCardinality>
                <owl:onClass rdf:resource="http://www.wageneder.at/ontology/bpmn2.0#Element"/>
            </owl:Restriction>
        </rdfs:subClassOf>
        <rdfs:subClassOf>
            <owl:Restriction>
                <owl:onProperty rdf:resource="http://www.wageneder.at/ontology/bpmn2.0#hasEvaluatesToTypeRef"/>
                <owl:qualifiedCardinality rdf:datatype="http://www.w3.org/2001/XMLSchema#nonNegativeInteger">1</owl:qualifiedCardinality>
                <owl:onClass rdf:resource="http://www.wageneder.at/ontology/bpmn2.0#ItemDefinition"/>
            </owl:Restriction>
        </rdfs:subClassOf>
        <rdfs:subClassOf>
            <owl:Restriction>
                <owl:onProperty rdf:resource="http://www.wageneder.at/ontology/bpmn2.0#hasCorrelationSet"/>
                <owl:maxQualifiedCardinality rdf:datatype="http://www.w3.org/2001/XMLSchema#nonNegativeInteger">1</owl:maxQualifiedCardinality>
                <owl:onClass rdf:resource="http://www.wageneder.at/ontology/bpmn2.0#CorrelationPropertyRetrievalExpression"/>
            </owl:Restriction>
        </rdfs:subClassOf>
        <rdfs:subClassOf>
            <owl:Restriction>
                <owl:onProperty rdf:resource="http://www.wageneder.at/ontology/bpmn2.0#language"/>
                <owl:minQualifiedCardinality rdf:datatype="http://www.w3.org/2001/XMLSchema#nonNegativeInteger">0</owl:minQualifiedCardinality>
                <owl:onDataRange rdf:resource="http://www.w3.org/2001/XMLSchema#string"/>
            </owl:Restriction>
        </rdfs:subClassOf>
        <rdfs:subClassOf>
            <owl:Restriction>
                <owl:onProperty rdf:resource="http://www.wageneder.at/ontology/bpmn2.0#language"/>
                <owl:maxQualifiedCardinality rdf:datatype="http://www.w3.org/2001/XMLSchema#nonNegativeInteger">1</owl:maxQualifiedCardinality>
                <owl:onDataRange rdf:resource="http://www.w3.org/2001/XMLSchema#string"/>
            </owl:Restriction>
        </rdfs:subClassOf>
        <rdfs:comment>The FormalExpression class is used to specify an executable Expression using a specified Expression language. A natural-language description of the Expression can also be specified, in addition to the formal specification.</rdfs:comment>
    </owl:Class>
    


    <!-- http://www.wageneder.at/ontology/bpmn2.0#Forward -->

    <owl:Class rdf:about="http://www.wageneder.at/ontology/bpmn2.0#Forward">
        <rdfs:subClassOf rdf:resource="http://www.wageneder.at/ontology/bpmn2.0#RelationshipDirection"/>
    </owl:Class>
    


    <!-- http://www.wageneder.at/ontology/bpmn2.0#Foundation -->

    <owl:Class rdf:about="http://www.wageneder.at/ontology/bpmn2.0#Foundation">
        <rdfs:subClassOf rdf:resource="http://www.wageneder.at/ontology/bpmn2.0#BPMNCore"/>
        <rdfs:comment>This is just a hierarchical element for organisational purposes.</rdfs:comment>
    </owl:Class>
    


    <!-- http://www.wageneder.at/ontology/bpmn2.0#Gateway -->

    <owl:Class rdf:about="http://www.wageneder.at/ontology/bpmn2.0#Gateway">
        <rdfs:subClassOf rdf:resource="http://www.wageneder.at/ontology/bpmn2.0#FlowNode"/>
        <rdfs:subClassOf rdf:resource="http://www.wageneder.at/ontology/bpmn2.0#GatewayLevel"/>
        <rdfs:subClassOf>
            <owl:Restriction>
                <owl:onProperty rdf:resource="http://www.wageneder.at/ontology/bpmn2.0#hasGatewayDirection"/>
                <owl:qualifiedCardinality rdf:datatype="http://www.w3.org/2001/XMLSchema#nonNegativeInteger">1</owl:qualifiedCardinality>
                <owl:onClass rdf:resource="http://www.wageneder.at/ontology/bpmn2.0#GatewayDirection"/>
            </owl:Restriction>
        </rdfs:subClassOf>
        <rdfs:comment>Gateways are used to control how the Process flows (how Tokens flow) through Sequence Flows as they converge and diverge within a Process. If the flow does not need to be controlled, then a Gateway is not needed. The term “gateway” implies that there is a gating mechanism that either allows or disallows passage through the Gateway--that is, as tokens arrive at a Gateway, they can be merged together on input and/or split apart on output as the Gateway mechanisms are invoked.</rdfs:comment>
    </owl:Class>
    


    <!-- http://www.wageneder.at/ontology/bpmn2.0#GatewayDirection -->

    <owl:Class rdf:about="http://www.wageneder.at/ontology/bpmn2.0#GatewayDirection">
        <rdfs:subClassOf rdf:resource="http://www.wageneder.at/ontology/bpmn2.0#GatewayLevel"/>
        <rdfs:subClassOf>
            <owl:Class>
                <owl:unionOf rdf:parseType="Collection">
                    <rdf:Description rdf:about="http://www.wageneder.at/ontology/bpmn2.0#Converging"/>
                    <rdf:Description rdf:about="http://www.wageneder.at/ontology/bpmn2.0#Diverging"/>
                    <rdf:Description rdf:about="http://www.wageneder.at/ontology/bpmn2.0#Mixed"/>
                    <rdf:Description rdf:about="http://www.wageneder.at/ontology/bpmn2.0#Unspecified"/>
                </owl:unionOf>
            </owl:Class>
        </rdfs:subClassOf>
        <rdfs:comment>An attribute that adds constraints on how the Gateway MAY be used.</rdfs:comment>
    </owl:Class>
    


    <!-- http://www.wageneder.at/ontology/bpmn2.0#GatewayLevel -->

    <owl:Class rdf:about="http://www.wageneder.at/ontology/bpmn2.0#GatewayLevel">
        <rdfs:subClassOf rdf:resource="http://www.wageneder.at/ontology/bpmn2.0#Common"/>
        <rdfs:comment>This is just a hierarchical element for organisational purposes.
It presents the Gateways Folder</rdfs:comment>
    </owl:Class>
    


    <!-- http://www.wageneder.at/ontology/bpmn2.0#GlobalBusinessRuleTask -->

    <owl:Class rdf:about="http://www.wageneder.at/ontology/bpmn2.0#GlobalBusinessRuleTask">
        <rdfs:subClassOf rdf:resource="http://www.wageneder.at/ontology/bpmn2.0#GlobalTask"/>
        <rdfs:subClassOf>
            <owl:Restriction>
                <owl:onProperty rdf:resource="http://www.wageneder.at/ontology/bpmn2.0#implementation"/>
                <owl:qualifiedCardinality rdf:datatype="http://www.w3.org/2001/XMLSchema#nonNegativeInteger">1</owl:qualifiedCardinality>
                <owl:onDataRange rdf:resource="http://www.w3.org/2001/XMLSchema#string"/>
            </owl:Restriction>
        </rdfs:subClassOf>
        <rdfs:comment>For further Information see BusinessRuleTask p.154ff.</rdfs:comment>
    </owl:Class>
    


    <!-- http://www.wageneder.at/ontology/bpmn2.0#GlobalConversation -->

    <owl:Class rdf:about="http://www.wageneder.at/ontology/bpmn2.0#GlobalConversation">
        <rdfs:subClassOf rdf:resource="http://www.wageneder.at/ontology/bpmn2.0#Collaboration"/>
        <rdfs:subClassOf rdf:resource="http://www.wageneder.at/ontology/bpmn2.0#ConversationLevel"/>
        <rdfs:comment>The GlobalConversation element inherits the attributes and model associations and Collaboration (see Table 9.1), but does not have any additional attributes or model associations.</rdfs:comment>
    </owl:Class>
    


    <!-- http://www.wageneder.at/ontology/bpmn2.0#GlobalManualTask -->

    <owl:Class rdf:about="http://www.wageneder.at/ontology/bpmn2.0#GlobalManualTask">
        <rdfs:subClassOf rdf:resource="http://www.wageneder.at/ontology/bpmn2.0#GlobalTask"/>
        <rdfs:subClassOf rdf:resource="http://www.wageneder.at/ontology/bpmn2.0#HumanInteractionLevel"/>
        <rdfs:comment>For further Information see ManualTask p.154ff.</rdfs:comment>
    </owl:Class>
    


    <!-- http://www.wageneder.at/ontology/bpmn2.0#GlobalScriptTask -->

    <owl:Class rdf:about="http://www.wageneder.at/ontology/bpmn2.0#GlobalScriptTask">
        <rdfs:subClassOf rdf:resource="http://www.wageneder.at/ontology/bpmn2.0#ActivityLevel"/>
        <rdfs:subClassOf rdf:resource="http://www.wageneder.at/ontology/bpmn2.0#GlobalTask"/>
        <rdfs:subClassOf>
            <owl:Restriction>
                <owl:onProperty rdf:resource="http://www.wageneder.at/ontology/bpmn2.0#script"/>
                <owl:minQualifiedCardinality rdf:datatype="http://www.w3.org/2001/XMLSchema#nonNegativeInteger">0</owl:minQualifiedCardinality>
                <owl:onDataRange rdf:resource="http://www.w3.org/2001/XMLSchema#string"/>
            </owl:Restriction>
        </rdfs:subClassOf>
        <rdfs:subClassOf>
            <owl:Restriction>
                <owl:onProperty rdf:resource="http://www.wageneder.at/ontology/bpmn2.0#scriptFormat"/>
                <owl:minQualifiedCardinality rdf:datatype="http://www.w3.org/2001/XMLSchema#nonNegativeInteger">0</owl:minQualifiedCardinality>
                <owl:onDataRange rdf:resource="http://www.w3.org/2001/XMLSchema#string"/>
            </owl:Restriction>
        </rdfs:subClassOf>
        <rdfs:subClassOf>
            <owl:Restriction>
                <owl:onProperty rdf:resource="http://www.wageneder.at/ontology/bpmn2.0#script"/>
                <owl:maxQualifiedCardinality rdf:datatype="http://www.w3.org/2001/XMLSchema#nonNegativeInteger">1</owl:maxQualifiedCardinality>
                <owl:onDataRange rdf:resource="http://www.w3.org/2001/XMLSchema#string"/>
            </owl:Restriction>
        </rdfs:subClassOf>
        <rdfs:subClassOf>
            <owl:Restriction>
                <owl:onProperty rdf:resource="http://www.wageneder.at/ontology/bpmn2.0#scriptFormat"/>
                <owl:maxQualifiedCardinality rdf:datatype="http://www.w3.org/2001/XMLSchema#nonNegativeInteger">1</owl:maxQualifiedCardinality>
                <owl:onDataRange rdf:resource="http://www.w3.org/2001/XMLSchema#string"/>
            </owl:Restriction>
        </rdfs:subClassOf>
        <rdfs:comment>For further Information see ScriptTask p.154ff.</rdfs:comment>
    </owl:Class>
    


    <!-- http://www.wageneder.at/ontology/bpmn2.0#GlobalTask -->

    <owl:Class rdf:about="http://www.wageneder.at/ontology/bpmn2.0#GlobalTask">
        <rdfs:subClassOf rdf:resource="http://www.wageneder.at/ontology/bpmn2.0#CallableElement"/>
        <rdfs:subClassOf rdf:resource="http://www.wageneder.at/ontology/bpmn2.0#ProcessLevel"/>
        <rdfs:subClassOf>
            <owl:Restriction>
                <owl:onProperty rdf:resource="http://www.wageneder.at/ontology/bpmn2.0#hasResources"/>
                <owl:minQualifiedCardinality rdf:datatype="http://www.w3.org/2001/XMLSchema#nonNegativeInteger">0</owl:minQualifiedCardinality>
                <owl:onClass rdf:resource="http://www.wageneder.at/ontology/bpmn2.0#ResourceRole"/>
            </owl:Restriction>
        </rdfs:subClassOf>
        <rdfs:comment>The GlobalTask inherits the attributes and model associations of Callable Element (see Table 10.24). Table 10.26 presents the additional model associations of the GlobalTask.</rdfs:comment>
    </owl:Class>
    


    <!-- http://www.wageneder.at/ontology/bpmn2.0#GlobalUserTask -->

    <owl:Class rdf:about="http://www.wageneder.at/ontology/bpmn2.0#GlobalUserTask">
        <rdfs:subClassOf rdf:resource="http://www.wageneder.at/ontology/bpmn2.0#GlobalTask"/>
        <rdfs:subClassOf rdf:resource="http://www.wageneder.at/ontology/bpmn2.0#HumanInteractionLevel"/>
        <rdfs:subClassOf>
            <owl:Restriction>
                <owl:onProperty rdf:resource="http://www.wageneder.at/ontology/bpmn2.0#hasRenderings"/>
                <owl:minQualifiedCardinality rdf:datatype="http://www.w3.org/2001/XMLSchema#nonNegativeInteger">0</owl:minQualifiedCardinality>
                <owl:onClass rdf:resource="http://www.wageneder.at/ontology/bpmn2.0#Rendering"/>
            </owl:Restriction>
        </rdfs:subClassOf>
        <rdfs:subClassOf>
            <owl:Restriction>
                <owl:onProperty rdf:resource="http://www.wageneder.at/ontology/bpmn2.0#actualOwner"/>
                <owl:qualifiedCardinality rdf:datatype="http://www.w3.org/2001/XMLSchema#nonNegativeInteger">1</owl:qualifiedCardinality>
                <owl:onDataRange rdf:resource="http://www.w3.org/2001/XMLSchema#string"/>
            </owl:Restriction>
        </rdfs:subClassOf>
        <rdfs:subClassOf>
            <owl:Restriction>
                <owl:onProperty rdf:resource="http://www.wageneder.at/ontology/bpmn2.0#implementation"/>
                <owl:qualifiedCardinality rdf:datatype="http://www.w3.org/2001/XMLSchema#nonNegativeInteger">1</owl:qualifiedCardinality>
                <owl:onDataRange rdf:resource="http://www.w3.org/2001/XMLSchema#string"/>
            </owl:Restriction>
        </rdfs:subClassOf>
        <rdfs:subClassOf>
            <owl:Restriction>
                <owl:onProperty rdf:resource="http://www.wageneder.at/ontology/bpmn2.0#taskPriority"/>
                <owl:qualifiedCardinality rdf:datatype="http://www.w3.org/2001/XMLSchema#nonNegativeInteger">1</owl:qualifiedCardinality>
                <owl:onDataRange rdf:resource="http://www.w3.org/2001/XMLSchema#string"/>
            </owl:Restriction>
        </rdfs:subClassOf>
        <rdfs:comment>For further Information see UserTask p.154ff.</rdfs:comment>
    </owl:Class>
    


    <!-- http://www.wageneder.at/ontology/bpmn2.0#Group -->

    <owl:Class rdf:about="http://www.wageneder.at/ontology/bpmn2.0#Group">
        <rdfs:subClassOf rdf:resource="http://www.wageneder.at/ontology/bpmn2.0#Artifact"/>
        <rdfs:subClassOf>
            <owl:Restriction>
                <owl:onProperty rdf:resource="http://www.wageneder.at/ontology/bpmn2.0#hasCategoryValueRef"/>
                <owl:minQualifiedCardinality rdf:datatype="http://www.w3.org/2001/XMLSchema#nonNegativeInteger">0</owl:minQualifiedCardinality>
                <owl:onClass rdf:resource="http://www.wageneder.at/ontology/bpmn2.0#CategoryValue"/>
            </owl:Restriction>
        </rdfs:subClassOf>
        <rdfs:subClassOf>
            <owl:Restriction>
                <owl:onProperty rdf:resource="http://www.wageneder.at/ontology/bpmn2.0#hasCategoryValueRef"/>
                <owl:maxQualifiedCardinality rdf:datatype="http://www.w3.org/2001/XMLSchema#nonNegativeInteger">1</owl:maxQualifiedCardinality>
                <owl:onClass rdf:resource="http://www.wageneder.at/ontology/bpmn2.0#CategoryValue"/>
            </owl:Restriction>
        </rdfs:subClassOf>
        <rdfs:comment>The Group object is an Artifact that provides a visual mechanism to group elements of a diagram informally. The grouping is tied to the CategoryValue supporting element. That is, a Group is a visual depiction of a single CategoryValue. The graphical elements within the Group will be assigned the CategoryValue of the Group.</rdfs:comment>
    </owl:Class>
    


    <!-- http://www.wageneder.at/ontology/bpmn2.0#HumanInteractionLevel -->

    <owl:Class rdf:about="http://www.wageneder.at/ontology/bpmn2.0#HumanInteractionLevel">
        <rdfs:subClassOf rdf:resource="http://www.wageneder.at/ontology/bpmn2.0#ActivityLevel"/>
        <rdfs:comment>This is just a hierarchical element for organisational purposes.
It presents the Human Interactions Folder</rdfs:comment>
    </owl:Class>
    


    <!-- http://www.wageneder.at/ontology/bpmn2.0#HumanPerformer -->

    <owl:Class rdf:about="http://www.wageneder.at/ontology/bpmn2.0#HumanPerformer">
        <rdfs:subClassOf rdf:resource="http://www.wageneder.at/ontology/bpmn2.0#HumanInteractionLevel"/>
        <rdfs:subClassOf rdf:resource="http://www.wageneder.at/ontology/bpmn2.0#Performer"/>
        <rdfs:comment>The HumanPerformer element inherits the attributes and model associations of ResourceRole (see Table 10.5), through its relationship to Performer, but does not have any additional attributes or model associations.</rdfs:comment>
    </owl:Class>
    


    <!-- http://www.wageneder.at/ontology/bpmn2.0#ImplicitThrowEvent -->

    <owl:Class rdf:about="http://www.wageneder.at/ontology/bpmn2.0#ImplicitThrowEvent">
        <rdfs:subClassOf rdf:resource="http://www.wageneder.at/ontology/bpmn2.0#ThrowEvent"/>
    </owl:Class>
    


    <!-- http://www.wageneder.at/ontology/bpmn2.0#Import -->

    <owl:Class rdf:about="http://www.wageneder.at/ontology/bpmn2.0#Import">
        <rdfs:subClassOf rdf:resource="http://www.wageneder.at/ontology/bpmn2.0#Infrastructure"/>
        <rdfs:subClassOf>
            <owl:Restriction>
                <owl:onProperty rdf:resource="http://www.wageneder.at/ontology/bpmn2.0#hasDefinition"/>
                <owl:qualifiedCardinality rdf:datatype="http://www.w3.org/2001/XMLSchema#nonNegativeInteger">1</owl:qualifiedCardinality>
                <owl:onClass rdf:resource="http://www.wageneder.at/ontology/bpmn2.0#Definitions"/>
            </owl:Restriction>
        </rdfs:subClassOf>
        <rdfs:subClassOf>
            <owl:Restriction>
                <owl:onProperty rdf:resource="http://www.wageneder.at/ontology/bpmn2.0#location"/>
                <owl:minQualifiedCardinality rdf:datatype="http://www.w3.org/2001/XMLSchema#nonNegativeInteger">0</owl:minQualifiedCardinality>
                <owl:onDataRange rdf:resource="http://www.w3.org/2001/XMLSchema#string"/>
            </owl:Restriction>
        </rdfs:subClassOf>
        <rdfs:subClassOf>
            <owl:Restriction>
                <owl:onProperty rdf:resource="http://www.wageneder.at/ontology/bpmn2.0#importType"/>
                <owl:qualifiedCardinality rdf:datatype="http://www.w3.org/2001/XMLSchema#nonNegativeInteger">1</owl:qualifiedCardinality>
                <owl:onDataRange rdf:resource="http://www.w3.org/2001/XMLSchema#string"/>
            </owl:Restriction>
        </rdfs:subClassOf>
        <rdfs:subClassOf>
            <owl:Restriction>
                <owl:onProperty rdf:resource="http://www.wageneder.at/ontology/bpmn2.0#namespace"/>
                <owl:qualifiedCardinality rdf:datatype="http://www.w3.org/2001/XMLSchema#nonNegativeInteger">1</owl:qualifiedCardinality>
                <owl:onDataRange rdf:resource="http://www.w3.org/2001/XMLSchema#string"/>
            </owl:Restriction>
        </rdfs:subClassOf>
        <rdfs:subClassOf>
            <owl:Restriction>
                <owl:onProperty rdf:resource="http://www.wageneder.at/ontology/bpmn2.0#location"/>
                <owl:maxQualifiedCardinality rdf:datatype="http://www.w3.org/2001/XMLSchema#nonNegativeInteger">1</owl:maxQualifiedCardinality>
                <owl:onDataRange rdf:resource="http://www.w3.org/2001/XMLSchema#string"/>
            </owl:Restriction>
        </rdfs:subClassOf>
        <rdfs:comment>The Import class is used when referencing external element, either BPMN elements contained in other BPMN
Definitions or non-BPMN elements. Imports MUST be explicitly defined.</rdfs:comment>
    </owl:Class>
    


    <!-- http://www.wageneder.at/ontology/bpmn2.0#InclusiveGateway -->

    <owl:Class rdf:about="http://www.wageneder.at/ontology/bpmn2.0#InclusiveGateway">
        <rdfs:subClassOf rdf:resource="http://www.wageneder.at/ontology/bpmn2.0#Gateway"/>
        <rdfs:subClassOf>
            <owl:Restriction>
                <owl:onProperty rdf:resource="http://www.wageneder.at/ontology/bpmn2.0#hasDefault"/>
                <owl:minQualifiedCardinality rdf:datatype="http://www.w3.org/2001/XMLSchema#nonNegativeInteger">0</owl:minQualifiedCardinality>
                <owl:onClass rdf:resource="http://www.wageneder.at/ontology/bpmn2.0#SequenceFlow"/>
            </owl:Restriction>
        </rdfs:subClassOf>
        <rdfs:subClassOf>
            <owl:Restriction>
                <owl:onProperty rdf:resource="http://www.wageneder.at/ontology/bpmn2.0#hasDefault"/>
                <owl:maxQualifiedCardinality rdf:datatype="http://www.w3.org/2001/XMLSchema#nonNegativeInteger">1</owl:maxQualifiedCardinality>
                <owl:onClass rdf:resource="http://www.wageneder.at/ontology/bpmn2.0#SequenceFlow"/>
            </owl:Restriction>
        </rdfs:subClassOf>
        <rdfs:comment>A diverging Inclusive Gateway (Inclusive Decision) can be used to create alternative but also parallel paths within a Process flow. Unlike the Exclusive Gateway, all condition Expressions are evaluated. The true evaluation of one condition Expression does not exclude the evaluation of other condition Expressions. All Sequence Flows with a true evaluation will be traversed by a token. Since each path is considered to be independent, all combinations of the paths MAY be taken, from zero to all. However, it should be designed so that at least one path is taken.</rdfs:comment>
    </owl:Class>
    


    <!-- http://www.wageneder.at/ontology/bpmn2.0#Information -->

    <owl:Class rdf:about="http://www.wageneder.at/ontology/bpmn2.0#Information">
        <rdfs:subClassOf rdf:resource="http://www.wageneder.at/ontology/bpmn2.0#ItemKind"/>
        <owl:disjointWith rdf:resource="http://www.wageneder.at/ontology/bpmn2.0#Physical"/>
    </owl:Class>
    


    <!-- http://www.wageneder.at/ontology/bpmn2.0#Infrastructure -->

    <owl:Class rdf:about="http://www.wageneder.at/ontology/bpmn2.0#Infrastructure">
        <rdfs:subClassOf rdf:resource="http://www.wageneder.at/ontology/bpmn2.0#BPMNCore"/>
        <rdfs:comment>This is just a hierarchical element for organisational purposes.</rdfs:comment>
    </owl:Class>
    


    <!-- http://www.wageneder.at/ontology/bpmn2.0#InputOutputBinding -->

    <owl:Class rdf:about="http://www.wageneder.at/ontology/bpmn2.0#InputOutputBinding">
        <rdfs:subClassOf rdf:resource="http://www.wageneder.at/ontology/bpmn2.0#DataLevel"/>
        <rdfs:subClassOf>
            <owl:Restriction>
                <owl:onProperty rdf:resource="http://www.wageneder.at/ontology/bpmn2.0#hasInputDataRef"/>
                <owl:qualifiedCardinality rdf:datatype="http://www.w3.org/2001/XMLSchema#nonNegativeInteger">1</owl:qualifiedCardinality>
                <owl:onClass rdf:resource="http://www.wageneder.at/ontology/bpmn2.0#InputSet"/>
            </owl:Restriction>
        </rdfs:subClassOf>
        <rdfs:subClassOf>
            <owl:Restriction>
                <owl:onProperty rdf:resource="http://www.wageneder.at/ontology/bpmn2.0#hasOperationRef"/>
                <owl:qualifiedCardinality rdf:datatype="http://www.w3.org/2001/XMLSchema#nonNegativeInteger">1</owl:qualifiedCardinality>
                <owl:onClass rdf:resource="http://www.wageneder.at/ontology/bpmn2.0#Operation"/>
            </owl:Restriction>
        </rdfs:subClassOf>
        <rdfs:subClassOf>
            <owl:Restriction>
                <owl:onProperty rdf:resource="http://www.wageneder.at/ontology/bpmn2.0#hasOutputDataRef"/>
                <owl:qualifiedCardinality rdf:datatype="http://www.w3.org/2001/XMLSchema#nonNegativeInteger">1</owl:qualifiedCardinality>
                <owl:onClass rdf:resource="http://www.wageneder.at/ontology/bpmn2.0#OutputSet"/>
            </owl:Restriction>
        </rdfs:subClassOf>
        <rdfs:comment>When a CallableElement is exposed as a Service, it has to define one or more InputOutputBinding
elements. An InputOutputBinding element binds one Input and one Output of the
InputOutputSpecification to an Operation of a Service Interface. Table 10.25 presents the additional
model associations of the InputOutputBinding.</rdfs:comment>
    </owl:Class>
    


    <!-- http://www.wageneder.at/ontology/bpmn2.0#InputOutputSpecification -->

    <owl:Class rdf:about="http://www.wageneder.at/ontology/bpmn2.0#InputOutputSpecification">
        <rdfs:subClassOf rdf:resource="http://www.wageneder.at/ontology/bpmn2.0#BaseElement"/>
        <rdfs:subClassOf rdf:resource="http://www.wageneder.at/ontology/bpmn2.0#DataLevel"/>
        <rdfs:subClassOf>
            <owl:Restriction>
                <owl:onProperty rdf:resource="http://www.wageneder.at/ontology/bpmn2.0#hasDataInputs"/>
                <owl:minQualifiedCardinality rdf:datatype="http://www.w3.org/2001/XMLSchema#nonNegativeInteger">0</owl:minQualifiedCardinality>
                <owl:onClass rdf:resource="http://www.wageneder.at/ontology/bpmn2.0#DataInput"/>
            </owl:Restriction>
        </rdfs:subClassOf>
        <rdfs:subClassOf>
            <owl:Restriction>
                <owl:onProperty rdf:resource="http://www.wageneder.at/ontology/bpmn2.0#hasDataOutputs"/>
                <owl:minQualifiedCardinality rdf:datatype="http://www.w3.org/2001/XMLSchema#nonNegativeInteger">0</owl:minQualifiedCardinality>
                <owl:onClass rdf:resource="http://www.wageneder.at/ontology/bpmn2.0#DataOutput"/>
            </owl:Restriction>
        </rdfs:subClassOf>
        <rdfs:subClassOf>
            <owl:Restriction>
                <owl:onProperty rdf:resource="http://www.wageneder.at/ontology/bpmn2.0#hasInputSets"/>
                <owl:minQualifiedCardinality rdf:datatype="http://www.w3.org/2001/XMLSchema#nonNegativeInteger">1</owl:minQualifiedCardinality>
                <owl:onClass rdf:resource="http://www.wageneder.at/ontology/bpmn2.0#InputSet"/>
            </owl:Restriction>
        </rdfs:subClassOf>
        <rdfs:subClassOf>
            <owl:Restriction>
                <owl:onProperty rdf:resource="http://www.wageneder.at/ontology/bpmn2.0#hasOutputSets"/>
                <owl:minQualifiedCardinality rdf:datatype="http://www.w3.org/2001/XMLSchema#nonNegativeInteger">1</owl:minQualifiedCardinality>
                <owl:onClass rdf:resource="http://www.wageneder.at/ontology/bpmn2.0#OutputSet"/>
            </owl:Restriction>
        </rdfs:subClassOf>
        <rdfs:comment>Activities and Processes often need data in order to execute. In addition they can produce data during or as a result of execution. Data requirements are captured as Data Inputs and InputSets. Data that is produced is captured using Data Outputs and OutputSets. These elements are aggregated in a InputOutputSpecification class.</rdfs:comment>
    </owl:Class>
    


    <!-- http://www.wageneder.at/ontology/bpmn2.0#InputSet -->

    <owl:Class rdf:about="http://www.wageneder.at/ontology/bpmn2.0#InputSet">
        <rdfs:subClassOf rdf:resource="http://www.wageneder.at/ontology/bpmn2.0#BaseElement"/>
        <rdfs:subClassOf rdf:resource="http://www.wageneder.at/ontology/bpmn2.0#DataLevel"/>
        <rdfs:subClassOf>
            <owl:Restriction>
                <owl:onProperty rdf:resource="http://www.wageneder.at/ontology/bpmn2.0#hasDataInputRefs"/>
                <owl:minQualifiedCardinality rdf:datatype="http://www.w3.org/2001/XMLSchema#nonNegativeInteger">0</owl:minQualifiedCardinality>
                <owl:onClass rdf:resource="http://www.wageneder.at/ontology/bpmn2.0#DataInput"/>
            </owl:Restriction>
        </rdfs:subClassOf>
        <rdfs:subClassOf>
            <owl:Restriction>
                <owl:onProperty rdf:resource="http://www.wageneder.at/ontology/bpmn2.0#hasOptionalInputRefs"/>
                <owl:minQualifiedCardinality rdf:datatype="http://www.w3.org/2001/XMLSchema#nonNegativeInteger">0</owl:minQualifiedCardinality>
                <owl:onClass rdf:resource="http://www.wageneder.at/ontology/bpmn2.0#DataInput"/>
            </owl:Restriction>
        </rdfs:subClassOf>
        <rdfs:subClassOf>
            <owl:Restriction>
                <owl:onProperty rdf:resource="http://www.wageneder.at/ontology/bpmn2.0#hasOutputSetRefs"/>
                <owl:minQualifiedCardinality rdf:datatype="http://www.w3.org/2001/XMLSchema#nonNegativeInteger">0</owl:minQualifiedCardinality>
                <owl:onClass rdf:resource="http://www.wageneder.at/ontology/bpmn2.0#OutputSet"/>
            </owl:Restriction>
        </rdfs:subClassOf>
        <rdfs:subClassOf>
            <owl:Restriction>
                <owl:onProperty rdf:resource="http://www.wageneder.at/ontology/bpmn2.0#hasWhileExecutingInputRefs"/>
                <owl:minQualifiedCardinality rdf:datatype="http://www.w3.org/2001/XMLSchema#nonNegativeInteger">0</owl:minQualifiedCardinality>
                <owl:onClass rdf:resource="http://www.wageneder.at/ontology/bpmn2.0#DataInput"/>
            </owl:Restriction>
        </rdfs:subClassOf>
        <rdfs:subClassOf>
            <owl:Restriction>
                <owl:onProperty rdf:resource="http://www.wageneder.at/ontology/bpmn2.0#name"/>
                <owl:minQualifiedCardinality rdf:datatype="http://www.w3.org/2001/XMLSchema#nonNegativeInteger">0</owl:minQualifiedCardinality>
                <owl:onDataRange rdf:resource="http://www.w3.org/2001/XMLSchema#string"/>
            </owl:Restriction>
        </rdfs:subClassOf>
        <rdfs:subClassOf>
            <owl:Restriction>
                <owl:onProperty rdf:resource="http://www.wageneder.at/ontology/bpmn2.0#name"/>
                <owl:maxQualifiedCardinality rdf:datatype="http://www.w3.org/2001/XMLSchema#nonNegativeInteger">1</owl:maxQualifiedCardinality>
                <owl:onDataRange rdf:resource="http://www.w3.org/2001/XMLSchema#string"/>
            </owl:Restriction>
        </rdfs:subClassOf>
        <rdfs:comment>The InputSet element inherits the attributes and model associations of BaseElement (see Table 8.5). Table 10.61 presents the additional attributes and model associations of the InputSet element.</rdfs:comment>
    </owl:Class>
    


    <!-- http://www.wageneder.at/ontology/bpmn2.0#InteractionNode -->

    <owl:Class rdf:about="http://www.wageneder.at/ontology/bpmn2.0#InteractionNode">
        <rdfs:subClassOf rdf:resource="http://www.wageneder.at/ontology/bpmn2.0#CollaborationLevel"/>
        <rdfs:subClassOf>
            <owl:Restriction>
                <owl:onProperty rdf:resource="http://www.wageneder.at/ontology/bpmn2.0#hasIncomingConversationLinks"/>
                <owl:minQualifiedCardinality rdf:datatype="http://www.w3.org/2001/XMLSchema#nonNegativeInteger">0</owl:minQualifiedCardinality>
                <owl:onClass rdf:resource="http://www.wageneder.at/ontology/bpmn2.0#ConversationLink"/>
            </owl:Restriction>
        </rdfs:subClassOf>
        <rdfs:subClassOf>
            <owl:Restriction>
                <owl:onProperty rdf:resource="http://www.wageneder.at/ontology/bpmn2.0#hasOutgoingConversationLinks"/>
                <owl:minQualifiedCardinality rdf:datatype="http://www.w3.org/2001/XMLSchema#nonNegativeInteger">0</owl:minQualifiedCardinality>
                <owl:onClass rdf:resource="http://www.wageneder.at/ontology/bpmn2.0#ConversationLink"/>
            </owl:Restriction>
        </rdfs:subClassOf>
        <rdfs:comment>The InteractionNode element is used to provide a single element as the source and target Message Flow associations instead of the individual associations of the elements that can connect to Message Flows</rdfs:comment>
    </owl:Class>
    


    <!-- http://www.wageneder.at/ontology/bpmn2.0#Interface -->

    <owl:Class rdf:about="http://www.wageneder.at/ontology/bpmn2.0#Interface">
        <rdfs:subClassOf rdf:resource="http://www.wageneder.at/ontology/bpmn2.0#RootElement"/>
        <rdfs:subClassOf rdf:resource="http://www.wageneder.at/ontology/bpmn2.0#Service"/>
        <rdfs:subClassOf>
            <owl:Restriction>
                <owl:onProperty rdf:resource="http://www.wageneder.at/ontology/bpmn2.0#hasCallableElements"/>
                <owl:minQualifiedCardinality rdf:datatype="http://www.w3.org/2001/XMLSchema#nonNegativeInteger">0</owl:minQualifiedCardinality>
                <owl:onClass rdf:resource="http://www.wageneder.at/ontology/bpmn2.0#CallableElement"/>
            </owl:Restriction>
        </rdfs:subClassOf>
        <rdfs:subClassOf>
            <owl:Restriction>
                <owl:onProperty rdf:resource="http://www.wageneder.at/ontology/bpmn2.0#hasImplementationRef"/>
                <owl:minQualifiedCardinality rdf:datatype="http://www.w3.org/2001/XMLSchema#nonNegativeInteger">0</owl:minQualifiedCardinality>
                <owl:onClass rdf:resource="http://www.wageneder.at/ontology/bpmn2.0#Element"/>
            </owl:Restriction>
        </rdfs:subClassOf>
        <rdfs:subClassOf>
            <owl:Restriction>
                <owl:onProperty rdf:resource="http://www.wageneder.at/ontology/bpmn2.0#hasOperations"/>
                <owl:minQualifiedCardinality rdf:datatype="http://www.w3.org/2001/XMLSchema#nonNegativeInteger">1</owl:minQualifiedCardinality>
                <owl:onClass rdf:resource="http://www.wageneder.at/ontology/bpmn2.0#Operation"/>
            </owl:Restriction>
        </rdfs:subClassOf>
        <rdfs:subClassOf>
            <owl:Restriction>
                <owl:onProperty rdf:resource="http://www.wageneder.at/ontology/bpmn2.0#hasImplementationRef"/>
                <owl:maxQualifiedCardinality rdf:datatype="http://www.w3.org/2001/XMLSchema#nonNegativeInteger">1</owl:maxQualifiedCardinality>
                <owl:onClass rdf:resource="http://www.wageneder.at/ontology/bpmn2.0#Element"/>
            </owl:Restriction>
        </rdfs:subClassOf>
        <rdfs:subClassOf>
            <owl:Restriction>
                <owl:onProperty rdf:resource="http://www.wageneder.at/ontology/bpmn2.0#name"/>
                <owl:qualifiedCardinality rdf:datatype="http://www.w3.org/2001/XMLSchema#nonNegativeInteger">1</owl:qualifiedCardinality>
                <owl:onDataRange rdf:resource="http://www.w3.org/2001/XMLSchema#string"/>
            </owl:Restriction>
        </rdfs:subClassOf>
    </owl:Class>
    


    <!-- http://www.wageneder.at/ontology/bpmn2.0#IntermediateCatchEvent -->

    <owl:Class rdf:about="http://www.wageneder.at/ontology/bpmn2.0#IntermediateCatchEvent">
        <rdfs:subClassOf rdf:resource="http://www.wageneder.at/ontology/bpmn2.0#CatchEvent"/>
        <rdfs:comment>As the name implies, the Intermediate Event indicates where something happens (an Event) somewhere between the start and end of a Process.

An Intermediate Event that is placed within the normal flow of a Process can be used for one of two purposes. The Event can respond to (“catch”) the Event trigger or the Event can be used to set off (“throw”) the Event trigger.</rdfs:comment>
    </owl:Class>
    


    <!-- http://www.wageneder.at/ontology/bpmn2.0#IntermediateThrowEvent -->

    <owl:Class rdf:about="http://www.wageneder.at/ontology/bpmn2.0#IntermediateThrowEvent">
        <rdfs:subClassOf rdf:resource="http://www.wageneder.at/ontology/bpmn2.0#ThrowEvent"/>
        <rdfs:comment>As the name implies, the Intermediate Event indicates where something happens (an Event) somewhere between the start and end of a Process.

An Intermediate Event that is placed within the normal flow of a Process can be used for one of two purposes. The Event can respond to (“catch”) the Event trigger or the Event can be used to set off (“throw”) the Event trigger.</rdfs:comment>
    </owl:Class>
    


    <!-- http://www.wageneder.at/ontology/bpmn2.0#ItemAwareElement -->

    <owl:Class rdf:about="http://www.wageneder.at/ontology/bpmn2.0#ItemAwareElement">
        <rdfs:subClassOf rdf:resource="http://www.wageneder.at/ontology/bpmn2.0#BaseElement"/>
        <rdfs:subClassOf rdf:resource="http://www.wageneder.at/ontology/bpmn2.0#DataLevel"/>
        <rdfs:subClassOf>
            <owl:Restriction>
                <owl:onProperty rdf:resource="http://www.wageneder.at/ontology/bpmn2.0#hasDataState"/>
                <owl:minQualifiedCardinality rdf:datatype="http://www.w3.org/2001/XMLSchema#nonNegativeInteger">0</owl:minQualifiedCardinality>
                <owl:onClass rdf:resource="http://www.wageneder.at/ontology/bpmn2.0#DataState"/>
            </owl:Restriction>
        </rdfs:subClassOf>
        <rdfs:subClassOf>
            <owl:Restriction>
                <owl:onProperty rdf:resource="http://www.wageneder.at/ontology/bpmn2.0#hasItemSubjectRef"/>
                <owl:minQualifiedCardinality rdf:datatype="http://www.w3.org/2001/XMLSchema#nonNegativeInteger">0</owl:minQualifiedCardinality>
                <owl:onClass rdf:resource="http://www.wageneder.at/ontology/bpmn2.0#ItemDefinition"/>
            </owl:Restriction>
        </rdfs:subClassOf>
        <rdfs:subClassOf>
            <owl:Restriction>
                <owl:onProperty rdf:resource="http://www.wageneder.at/ontology/bpmn2.0#hasDataState"/>
                <owl:maxQualifiedCardinality rdf:datatype="http://www.w3.org/2001/XMLSchema#nonNegativeInteger">1</owl:maxQualifiedCardinality>
                <owl:onClass rdf:resource="http://www.wageneder.at/ontology/bpmn2.0#DataState"/>
            </owl:Restriction>
        </rdfs:subClassOf>
        <rdfs:subClassOf>
            <owl:Restriction>
                <owl:onProperty rdf:resource="http://www.wageneder.at/ontology/bpmn2.0#hasItemSubjectRef"/>
                <owl:maxQualifiedCardinality rdf:datatype="http://www.w3.org/2001/XMLSchema#nonNegativeInteger">1</owl:maxQualifiedCardinality>
                <owl:onClass rdf:resource="http://www.wageneder.at/ontology/bpmn2.0#ItemDefinition"/>
            </owl:Restriction>
        </rdfs:subClassOf>
        <rdfs:comment>Several elements in BPMN are subject to store or convey items during process execution. These elements are referenced generally as “item-aware elements.” This is similar to the variable construct common to many languages. As with variables, these elements have an ItemDefinition.</rdfs:comment>
    </owl:Class>
    


    <!-- http://www.wageneder.at/ontology/bpmn2.0#ItemDefinition -->

    <owl:Class rdf:about="http://www.wageneder.at/ontology/bpmn2.0#ItemDefinition">
        <rdfs:subClassOf rdf:resource="http://www.wageneder.at/ontology/bpmn2.0#Common"/>
        <rdfs:subClassOf rdf:resource="http://www.wageneder.at/ontology/bpmn2.0#RootElement"/>
        <rdfs:subClassOf>
            <owl:Restriction>
                <owl:onProperty rdf:resource="http://www.wageneder.at/ontology/bpmn2.0#hasCorrelationProperty"/>
                <owl:minQualifiedCardinality rdf:datatype="http://www.w3.org/2001/XMLSchema#nonNegativeInteger">0</owl:minQualifiedCardinality>
                <owl:onClass rdf:resource="http://www.wageneder.at/ontology/bpmn2.0#CorrelationProperty"/>
            </owl:Restriction>
        </rdfs:subClassOf>
        <rdfs:subClassOf>
            <owl:Restriction>
                <owl:onProperty rdf:resource="http://www.wageneder.at/ontology/bpmn2.0#hasImport"/>
                <owl:minQualifiedCardinality rdf:datatype="http://www.w3.org/2001/XMLSchema#nonNegativeInteger">0</owl:minQualifiedCardinality>
                <owl:onClass rdf:resource="http://www.wageneder.at/ontology/bpmn2.0#Import"/>
            </owl:Restriction>
        </rdfs:subClassOf>
        <rdfs:subClassOf>
            <owl:Restriction>
                <owl:onProperty rdf:resource="http://www.wageneder.at/ontology/bpmn2.0#hasMessage"/>
                <owl:minQualifiedCardinality rdf:datatype="http://www.w3.org/2001/XMLSchema#nonNegativeInteger">0</owl:minQualifiedCardinality>
                <owl:onClass rdf:resource="http://www.wageneder.at/ontology/bpmn2.0#Message"/>
            </owl:Restriction>
        </rdfs:subClassOf>
        <rdfs:subClassOf>
            <owl:Restriction>
                <owl:onProperty rdf:resource="http://www.wageneder.at/ontology/bpmn2.0#hasStructureRef"/>
                <owl:minQualifiedCardinality rdf:datatype="http://www.w3.org/2001/XMLSchema#nonNegativeInteger">0</owl:minQualifiedCardinality>
                <owl:onClass rdf:resource="http://www.wageneder.at/ontology/bpmn2.0#Element"/>
            </owl:Restriction>
        </rdfs:subClassOf>
        <rdfs:subClassOf>
            <owl:Restriction>
                <owl:onProperty rdf:resource="http://www.wageneder.at/ontology/bpmn2.0#hasItemKind"/>
                <owl:qualifiedCardinality rdf:datatype="http://www.w3.org/2001/XMLSchema#nonNegativeInteger">1</owl:qualifiedCardinality>
                <owl:onClass rdf:resource="http://www.wageneder.at/ontology/bpmn2.0#ItemKind"/>
            </owl:Restriction>
        </rdfs:subClassOf>
        <rdfs:subClassOf>
            <owl:Restriction>
                <owl:onProperty rdf:resource="http://www.wageneder.at/ontology/bpmn2.0#hasImport"/>
                <owl:maxQualifiedCardinality rdf:datatype="http://www.w3.org/2001/XMLSchema#nonNegativeInteger">1</owl:maxQualifiedCardinality>
                <owl:onClass rdf:resource="http://www.wageneder.at/ontology/bpmn2.0#Import"/>
            </owl:Restriction>
        </rdfs:subClassOf>
        <rdfs:subClassOf>
            <owl:Restriction>
                <owl:onProperty rdf:resource="http://www.wageneder.at/ontology/bpmn2.0#hasStructureRef"/>
                <owl:maxQualifiedCardinality rdf:datatype="http://www.w3.org/2001/XMLSchema#nonNegativeInteger">1</owl:maxQualifiedCardinality>
                <owl:onClass rdf:resource="http://www.wageneder.at/ontology/bpmn2.0#Element"/>
            </owl:Restriction>
        </rdfs:subClassOf>
        <rdfs:subClassOf>
            <owl:Restriction>
                <owl:onProperty rdf:resource="http://www.wageneder.at/ontology/bpmn2.0#isCollection"/>
                <owl:qualifiedCardinality rdf:datatype="http://www.w3.org/2001/XMLSchema#nonNegativeInteger">1</owl:qualifiedCardinality>
                <owl:onDataRange rdf:resource="http://www.w3.org/2001/XMLSchema#boolean"/>
            </owl:Restriction>
        </rdfs:subClassOf>
        <rdfs:comment>An ItemDefinition element can specify an import reference where the proper definition of the structure is defined.</rdfs:comment>
    </owl:Class>
    


    <!-- http://www.wageneder.at/ontology/bpmn2.0#ItemKind -->

    <owl:Class rdf:about="http://www.wageneder.at/ontology/bpmn2.0#ItemKind">
        <rdfs:subClassOf rdf:resource="http://www.wageneder.at/ontology/bpmn2.0#Common"/>
        <rdfs:subClassOf>
            <owl:Class>
                <owl:unionOf rdf:parseType="Collection">
                    <rdf:Description rdf:about="http://www.wageneder.at/ontology/bpmn2.0#Information"/>
                    <rdf:Description rdf:about="http://www.wageneder.at/ontology/bpmn2.0#Physical"/>
                </owl:unionOf>
            </owl:Class>
        </rdfs:subClassOf>
        <rdfs:comment>The itemKind attribute specifies the nature of an item which can be a physical or an information item.</rdfs:comment>
    </owl:Class>
    


    <!-- http://www.wageneder.at/ontology/bpmn2.0#Lane -->

    <owl:Class rdf:about="http://www.wageneder.at/ontology/bpmn2.0#Lane">
        <rdfs:subClassOf rdf:resource="http://www.wageneder.at/ontology/bpmn2.0#BaseElement"/>
        <rdfs:subClassOf rdf:resource="http://www.wageneder.at/ontology/bpmn2.0#ProcessLevel"/>
        <rdfs:subClassOf>
            <owl:Restriction>
                <owl:onProperty rdf:resource="http://www.wageneder.at/ontology/bpmn2.0#hasChildLaneSet"/>
                <owl:minQualifiedCardinality rdf:datatype="http://www.w3.org/2001/XMLSchema#nonNegativeInteger">0</owl:minQualifiedCardinality>
                <owl:onClass rdf:resource="http://www.wageneder.at/ontology/bpmn2.0#LaneSet"/>
            </owl:Restriction>
        </rdfs:subClassOf>
        <rdfs:subClassOf>
            <owl:Restriction>
                <owl:onProperty rdf:resource="http://www.wageneder.at/ontology/bpmn2.0#hasFlowNodeRefs"/>
                <owl:minQualifiedCardinality rdf:datatype="http://www.w3.org/2001/XMLSchema#nonNegativeInteger">0</owl:minQualifiedCardinality>
                <owl:onClass rdf:resource="http://www.wageneder.at/ontology/bpmn2.0#FlowNode"/>
            </owl:Restriction>
        </rdfs:subClassOf>
        <rdfs:subClassOf>
            <owl:Restriction>
                <owl:onProperty rdf:resource="http://www.wageneder.at/ontology/bpmn2.0#hasPartitionElement"/>
                <owl:minQualifiedCardinality rdf:datatype="http://www.w3.org/2001/XMLSchema#nonNegativeInteger">0</owl:minQualifiedCardinality>
                <owl:onClass rdf:resource="http://www.wageneder.at/ontology/bpmn2.0#BaseElement"/>
            </owl:Restriction>
        </rdfs:subClassOf>
        <rdfs:subClassOf>
            <owl:Restriction>
                <owl:onProperty rdf:resource="http://www.wageneder.at/ontology/bpmn2.0#hasPartitionElementRef"/>
                <owl:minQualifiedCardinality rdf:datatype="http://www.w3.org/2001/XMLSchema#nonNegativeInteger">0</owl:minQualifiedCardinality>
                <owl:onClass rdf:resource="http://www.wageneder.at/ontology/bpmn2.0#BaseElement"/>
            </owl:Restriction>
        </rdfs:subClassOf>
        <rdfs:subClassOf>
            <owl:Restriction>
                <owl:onProperty rdf:resource="http://www.wageneder.at/ontology/bpmn2.0#hasLaneSet"/>
                <owl:qualifiedCardinality rdf:datatype="http://www.w3.org/2001/XMLSchema#nonNegativeInteger">1</owl:qualifiedCardinality>
                <owl:onClass rdf:resource="http://www.wageneder.at/ontology/bpmn2.0#LaneSet"/>
            </owl:Restriction>
        </rdfs:subClassOf>
        <rdfs:subClassOf>
            <owl:Restriction>
                <owl:onProperty rdf:resource="http://www.wageneder.at/ontology/bpmn2.0#hasChildLaneSet"/>
                <owl:maxQualifiedCardinality rdf:datatype="http://www.w3.org/2001/XMLSchema#nonNegativeInteger">1</owl:maxQualifiedCardinality>
                <owl:onClass rdf:resource="http://www.wageneder.at/ontology/bpmn2.0#LaneSet"/>
            </owl:Restriction>
        </rdfs:subClassOf>
        <rdfs:subClassOf>
            <owl:Restriction>
                <owl:onProperty rdf:resource="http://www.wageneder.at/ontology/bpmn2.0#hasPartitionElement"/>
                <owl:maxQualifiedCardinality rdf:datatype="http://www.w3.org/2001/XMLSchema#nonNegativeInteger">1</owl:maxQualifiedCardinality>
                <owl:onClass rdf:resource="http://www.wageneder.at/ontology/bpmn2.0#BaseElement"/>
            </owl:Restriction>
        </rdfs:subClassOf>
        <rdfs:subClassOf>
            <owl:Restriction>
                <owl:onProperty rdf:resource="http://www.wageneder.at/ontology/bpmn2.0#hasPartitionElementRef"/>
                <owl:maxQualifiedCardinality rdf:datatype="http://www.w3.org/2001/XMLSchema#nonNegativeInteger">1</owl:maxQualifiedCardinality>
                <owl:onClass rdf:resource="http://www.wageneder.at/ontology/bpmn2.0#BaseElement"/>
            </owl:Restriction>
        </rdfs:subClassOf>
        <rdfs:subClassOf>
            <owl:Restriction>
                <owl:onProperty rdf:resource="http://www.wageneder.at/ontology/bpmn2.0#name"/>
                <owl:qualifiedCardinality rdf:datatype="http://www.w3.org/2001/XMLSchema#nonNegativeInteger">1</owl:qualifiedCardinality>
                <owl:onDataRange rdf:resource="http://www.w3.org/2001/XMLSchema#string"/>
            </owl:Restriction>
        </rdfs:subClassOf>
        <rdfs:comment>A Lane is a sub-partition within a Process (often within a Pool) and will extend the entire length of the Process level, either vertically or horizontally.</rdfs:comment>
    </owl:Class>
    


    <!-- http://www.wageneder.at/ontology/bpmn2.0#LaneSet -->

    <owl:Class rdf:about="http://www.wageneder.at/ontology/bpmn2.0#LaneSet">
        <rdfs:subClassOf rdf:resource="http://www.wageneder.at/ontology/bpmn2.0#BaseElement"/>
        <rdfs:subClassOf rdf:resource="http://www.wageneder.at/ontology/bpmn2.0#ProcessLevel"/>
        <rdfs:subClassOf>
            <owl:Restriction>
                <owl:onProperty rdf:resource="http://www.wageneder.at/ontology/bpmn2.0#hasFlowElementsContainer"/>
                <owl:minQualifiedCardinality rdf:datatype="http://www.w3.org/2001/XMLSchema#nonNegativeInteger">0</owl:minQualifiedCardinality>
                <owl:onClass rdf:resource="http://www.wageneder.at/ontology/bpmn2.0#FlowElementsContainer"/>
            </owl:Restriction>
        </rdfs:subClassOf>
        <rdfs:subClassOf>
            <owl:Restriction>
                <owl:onProperty rdf:resource="http://www.wageneder.at/ontology/bpmn2.0#hasLanes"/>
                <owl:minQualifiedCardinality rdf:datatype="http://www.w3.org/2001/XMLSchema#nonNegativeInteger">0</owl:minQualifiedCardinality>
                <owl:onClass rdf:resource="http://www.wageneder.at/ontology/bpmn2.0#Lane"/>
            </owl:Restriction>
        </rdfs:subClassOf>
        <rdfs:subClassOf>
            <owl:Restriction>
                <owl:onProperty rdf:resource="http://www.wageneder.at/ontology/bpmn2.0#hasParentLane"/>
                <owl:minQualifiedCardinality rdf:datatype="http://www.w3.org/2001/XMLSchema#nonNegativeInteger">0</owl:minQualifiedCardinality>
                <owl:onClass rdf:resource="http://www.wageneder.at/ontology/bpmn2.0#Lane"/>
            </owl:Restriction>
        </rdfs:subClassOf>
        <rdfs:subClassOf>
            <owl:Restriction>
                <owl:onProperty rdf:resource="http://www.wageneder.at/ontology/bpmn2.0#hasProcess"/>
                <owl:qualifiedCardinality rdf:datatype="http://www.w3.org/2001/XMLSchema#nonNegativeInteger">1</owl:qualifiedCardinality>
                <owl:onClass rdf:resource="http://www.wageneder.at/ontology/bpmn2.0#Process"/>
            </owl:Restriction>
        </rdfs:subClassOf>
        <rdfs:subClassOf>
            <owl:Restriction>
                <owl:onProperty rdf:resource="http://www.wageneder.at/ontology/bpmn2.0#hasFlowElementsContainer"/>
                <owl:maxQualifiedCardinality rdf:datatype="http://www.w3.org/2001/XMLSchema#nonNegativeInteger">1</owl:maxQualifiedCardinality>
                <owl:onClass rdf:resource="http://www.wageneder.at/ontology/bpmn2.0#FlowElementsContainer"/>
            </owl:Restriction>
        </rdfs:subClassOf>
        <rdfs:subClassOf>
            <owl:Restriction>
                <owl:onProperty rdf:resource="http://www.wageneder.at/ontology/bpmn2.0#hasParentLane"/>
                <owl:maxQualifiedCardinality rdf:datatype="http://www.w3.org/2001/XMLSchema#nonNegativeInteger">1</owl:maxQualifiedCardinality>
                <owl:onClass rdf:resource="http://www.wageneder.at/ontology/bpmn2.0#Lane"/>
            </owl:Restriction>
        </rdfs:subClassOf>
        <rdfs:subClassOf>
            <owl:Restriction>
                <owl:onProperty rdf:resource="http://www.wageneder.at/ontology/bpmn2.0#name"/>
                <owl:minQualifiedCardinality rdf:datatype="http://www.w3.org/2001/XMLSchema#nonNegativeInteger">0</owl:minQualifiedCardinality>
                <owl:onDataRange rdf:resource="http://www.w3.org/2001/XMLSchema#string"/>
            </owl:Restriction>
        </rdfs:subClassOf>
        <rdfs:subClassOf>
            <owl:Restriction>
                <owl:onProperty rdf:resource="http://www.wageneder.at/ontology/bpmn2.0#name"/>
                <owl:maxQualifiedCardinality rdf:datatype="http://www.w3.org/2001/XMLSchema#nonNegativeInteger">1</owl:maxQualifiedCardinality>
                <owl:onDataRange rdf:resource="http://www.w3.org/2001/XMLSchema#string"/>
            </owl:Restriction>
        </rdfs:subClassOf>
        <rdfs:comment>The LaneSet element defines the container for one or more Lanes. A Process can contain one or more LaneSets.
Each LaneSet and its Lanes can partition the Flow Nodes in a different way.</rdfs:comment>
    </owl:Class>
    


    <!-- http://www.wageneder.at/ontology/bpmn2.0#LinkEventDefinition -->

    <owl:Class rdf:about="http://www.wageneder.at/ontology/bpmn2.0#LinkEventDefinition">
        <rdfs:subClassOf rdf:resource="http://www.wageneder.at/ontology/bpmn2.0#EventDefinition"/>
        <rdfs:subClassOf>
            <owl:Restriction>
                <owl:onProperty rdf:resource="http://www.wageneder.at/ontology/bpmn2.0#hasSources"/>
                <owl:minQualifiedCardinality rdf:datatype="http://www.w3.org/2001/XMLSchema#nonNegativeInteger">1</owl:minQualifiedCardinality>
                <owl:onClass rdf:resource="http://www.wageneder.at/ontology/bpmn2.0#LinkEventDefinition"/>
            </owl:Restriction>
        </rdfs:subClassOf>
        <rdfs:subClassOf>
            <owl:Restriction>
                <owl:onProperty rdf:resource="http://www.wageneder.at/ontology/bpmn2.0#hasTarget"/>
                <owl:qualifiedCardinality rdf:datatype="http://www.w3.org/2001/XMLSchema#nonNegativeInteger">1</owl:qualifiedCardinality>
                <owl:onClass rdf:resource="http://www.wageneder.at/ontology/bpmn2.0#LinkEventDefinition"/>
            </owl:Restriction>
        </rdfs:subClassOf>
        <rdfs:subClassOf>
            <owl:Restriction>
                <owl:onProperty rdf:resource="http://www.wageneder.at/ontology/bpmn2.0#name"/>
                <owl:qualifiedCardinality rdf:datatype="http://www.w3.org/2001/XMLSchema#nonNegativeInteger">1</owl:qualifiedCardinality>
                <owl:onDataRange rdf:resource="http://www.w3.org/2001/XMLSchema#string"/>
            </owl:Restriction>
        </rdfs:subClassOf>
        <rdfs:comment>A Link Event is a mechanism for connecting two sections of a Process. Link Events can be used to create looping situations or to avoid long Sequence Flow lines. The use of Link Events is limited to a single Process level (i.e., they cannot link a parent Process with a Sub-Process).</rdfs:comment>
    </owl:Class>
    


    <!-- http://www.wageneder.at/ontology/bpmn2.0#LoopCharacteristics -->

    <owl:Class rdf:about="http://www.wageneder.at/ontology/bpmn2.0#LoopCharacteristics">
        <rdfs:subClassOf rdf:resource="http://www.wageneder.at/ontology/bpmn2.0#ActivityLevel"/>
        <rdfs:subClassOf rdf:resource="http://www.wageneder.at/ontology/bpmn2.0#BaseElement"/>
        <rdfs:subClassOf>
            <owl:Restriction>
                <owl:onProperty rdf:resource="http://www.wageneder.at/ontology/bpmn2.0#loopCounter"/>
                <owl:qualifiedCardinality rdf:datatype="http://www.w3.org/2001/XMLSchema#nonNegativeInteger">1</owl:qualifiedCardinality>
                <owl:onDataRange rdf:resource="http://www.w3.org/2001/XMLSchema#integer"/>
            </owl:Restriction>
        </rdfs:subClassOf>
        <rdfs:comment>Activities MAY be repeated sequentially, essentially behaving like a loop. The presence of LoopCharacteristics signifies that the Activity has looping behavior. LoopCharacteristics is an abstract class. Concrete subclasses define specific kinds of looping behavior.</rdfs:comment>
    </owl:Class>
    


    <!-- http://www.wageneder.at/ontology/bpmn2.0#ManualTask -->

    <owl:Class rdf:about="http://www.wageneder.at/ontology/bpmn2.0#ManualTask">
        <rdfs:subClassOf rdf:resource="http://www.wageneder.at/ontology/bpmn2.0#HumanInteractionLevel"/>
        <rdfs:subClassOf rdf:resource="http://www.wageneder.at/ontology/bpmn2.0#Task"/>
        <rdfs:comment>A Manual Task is a Task that is expected to be performed without the aid of any business process execution engine or
any application. An example of this could be a telephone technician installing a telephone at a customer location.</rdfs:comment>
    </owl:Class>
    


    <!-- http://www.wageneder.at/ontology/bpmn2.0#Message -->

    <owl:Class rdf:about="http://www.wageneder.at/ontology/bpmn2.0#Message">
        <rdfs:subClassOf rdf:resource="http://www.wageneder.at/ontology/bpmn2.0#Common"/>
        <rdfs:subClassOf rdf:resource="http://www.wageneder.at/ontology/bpmn2.0#RootElement"/>
        <rdfs:subClassOf>
            <owl:Restriction>
                <owl:onProperty rdf:resource="http://www.wageneder.at/ontology/bpmn2.0#hasItemRef"/>
                <owl:minQualifiedCardinality rdf:datatype="http://www.w3.org/2001/XMLSchema#nonNegativeInteger">0</owl:minQualifiedCardinality>
                <owl:onClass rdf:resource="http://www.wageneder.at/ontology/bpmn2.0#ItemDefinition"/>
            </owl:Restriction>
        </rdfs:subClassOf>
        <rdfs:subClassOf>
            <owl:Restriction>
                <owl:onProperty rdf:resource="http://www.wageneder.at/ontology/bpmn2.0#hasMessageFlow"/>
                <owl:minQualifiedCardinality rdf:datatype="http://www.w3.org/2001/XMLSchema#nonNegativeInteger">0</owl:minQualifiedCardinality>
                <owl:onClass rdf:resource="http://www.wageneder.at/ontology/bpmn2.0#MessageFlow"/>
            </owl:Restriction>
        </rdfs:subClassOf>
        <rdfs:subClassOf>
            <owl:Restriction>
                <owl:onProperty rdf:resource="http://www.wageneder.at/ontology/bpmn2.0#hasItemRef"/>
                <owl:maxQualifiedCardinality rdf:datatype="http://www.w3.org/2001/XMLSchema#nonNegativeInteger">1</owl:maxQualifiedCardinality>
                <owl:onClass rdf:resource="http://www.wageneder.at/ontology/bpmn2.0#ItemDefinition"/>
            </owl:Restriction>
        </rdfs:subClassOf>
        <rdfs:subClassOf>
            <owl:Restriction>
                <owl:onProperty rdf:resource="http://www.wageneder.at/ontology/bpmn2.0#name"/>
                <owl:qualifiedCardinality rdf:datatype="http://www.w3.org/2001/XMLSchema#nonNegativeInteger">1</owl:qualifiedCardinality>
                <owl:onDataRange rdf:resource="http://www.w3.org/2001/XMLSchema#string"/>
            </owl:Restriction>
        </rdfs:subClassOf>
        <rdfs:comment>A Message represents the content of a communication between two Participants. In BPMN 2.0, a Message is a graphical decorator (it was a supporting element in BPMN 1.2). An ItemDefinition is used to specify the Message structure.</rdfs:comment>
    </owl:Class>
    


    <!-- http://www.wageneder.at/ontology/bpmn2.0#MessageEventDefinition -->

    <owl:Class rdf:about="http://www.wageneder.at/ontology/bpmn2.0#MessageEventDefinition">
        <rdfs:subClassOf rdf:resource="http://www.wageneder.at/ontology/bpmn2.0#EventDefinition"/>
        <rdfs:subClassOf>
            <owl:Restriction>
                <owl:onProperty rdf:resource="http://www.wageneder.at/ontology/bpmn2.0#hasMessageRef"/>
                <owl:minQualifiedCardinality rdf:datatype="http://www.w3.org/2001/XMLSchema#nonNegativeInteger">0</owl:minQualifiedCardinality>
                <owl:onClass rdf:resource="http://www.wageneder.at/ontology/bpmn2.0#Message"/>
            </owl:Restriction>
        </rdfs:subClassOf>
        <rdfs:subClassOf>
            <owl:Restriction>
                <owl:onProperty rdf:resource="http://www.wageneder.at/ontology/bpmn2.0#hasOperationRef"/>
                <owl:minQualifiedCardinality rdf:datatype="http://www.w3.org/2001/XMLSchema#nonNegativeInteger">0</owl:minQualifiedCardinality>
                <owl:onClass rdf:resource="http://www.wageneder.at/ontology/bpmn2.0#Operation"/>
            </owl:Restriction>
        </rdfs:subClassOf>
        <rdfs:subClassOf>
            <owl:Restriction>
                <owl:onProperty rdf:resource="http://www.wageneder.at/ontology/bpmn2.0#hasMessageRef"/>
                <owl:maxQualifiedCardinality rdf:datatype="http://www.w3.org/2001/XMLSchema#nonNegativeInteger">1</owl:maxQualifiedCardinality>
                <owl:onClass rdf:resource="http://www.wageneder.at/ontology/bpmn2.0#Message"/>
            </owl:Restriction>
        </rdfs:subClassOf>
        <rdfs:subClassOf>
            <owl:Restriction>
                <owl:onProperty rdf:resource="http://www.wageneder.at/ontology/bpmn2.0#hasOperationRef"/>
                <owl:maxQualifiedCardinality rdf:datatype="http://www.w3.org/2001/XMLSchema#nonNegativeInteger">1</owl:maxQualifiedCardinality>
                <owl:onClass rdf:resource="http://www.wageneder.at/ontology/bpmn2.0#Operation"/>
            </owl:Restriction>
        </rdfs:subClassOf>
        <rdfs:comment>The MessageEventDefinition element inherits the attributes and model associations of BaseElement  through its relationship to the EventDefinition element</rdfs:comment>
    </owl:Class>
    


    <!-- http://www.wageneder.at/ontology/bpmn2.0#MessageFlow -->

    <owl:Class rdf:about="http://www.wageneder.at/ontology/bpmn2.0#MessageFlow">
        <rdfs:subClassOf rdf:resource="http://www.wageneder.at/ontology/bpmn2.0#BaseElement"/>
        <rdfs:subClassOf rdf:resource="http://www.wageneder.at/ontology/bpmn2.0#CollaborationLevel"/>
        <rdfs:subClassOf>
            <owl:Restriction>
                <owl:onProperty rdf:resource="http://www.wageneder.at/ontology/bpmn2.0#hasMessageFlowAssociation"/>
                <owl:minQualifiedCardinality rdf:datatype="http://www.w3.org/2001/XMLSchema#nonNegativeInteger">0</owl:minQualifiedCardinality>
                <owl:onClass rdf:resource="http://www.wageneder.at/ontology/bpmn2.0#MessageFlowAssociation"/>
            </owl:Restriction>
        </rdfs:subClassOf>
        <rdfs:subClassOf>
            <owl:Restriction>
                <owl:onProperty rdf:resource="http://www.wageneder.at/ontology/bpmn2.0#hasMessageRef"/>
                <owl:minQualifiedCardinality rdf:datatype="http://www.w3.org/2001/XMLSchema#nonNegativeInteger">0</owl:minQualifiedCardinality>
                <owl:onClass rdf:resource="http://www.wageneder.at/ontology/bpmn2.0#Message"/>
            </owl:Restriction>
        </rdfs:subClassOf>
        <rdfs:subClassOf>
            <owl:Restriction>
                <owl:onProperty rdf:resource="http://www.wageneder.at/ontology/bpmn2.0#hasCollaboration"/>
                <owl:qualifiedCardinality rdf:datatype="http://www.w3.org/2001/XMLSchema#nonNegativeInteger">1</owl:qualifiedCardinality>
                <owl:onClass rdf:resource="http://www.wageneder.at/ontology/bpmn2.0#Collaboration"/>
            </owl:Restriction>
        </rdfs:subClassOf>
        <rdfs:subClassOf>
            <owl:Restriction>
                <owl:onProperty rdf:resource="http://www.wageneder.at/ontology/bpmn2.0#hasSourceRef"/>
                <owl:qualifiedCardinality rdf:datatype="http://www.w3.org/2001/XMLSchema#nonNegativeInteger">1</owl:qualifiedCardinality>
                <owl:onClass rdf:resource="http://www.wageneder.at/ontology/bpmn2.0#InteractionNode"/>
            </owl:Restriction>
        </rdfs:subClassOf>
        <rdfs:subClassOf>
            <owl:Restriction>
                <owl:onProperty rdf:resource="http://www.wageneder.at/ontology/bpmn2.0#hasTargetRef"/>
                <owl:qualifiedCardinality rdf:datatype="http://www.w3.org/2001/XMLSchema#nonNegativeInteger">1</owl:qualifiedCardinality>
                <owl:onClass rdf:resource="http://www.wageneder.at/ontology/bpmn2.0#InteractionNode"/>
            </owl:Restriction>
        </rdfs:subClassOf>
        <rdfs:subClassOf>
            <owl:Restriction>
                <owl:onProperty rdf:resource="http://www.wageneder.at/ontology/bpmn2.0#hasMessageRef"/>
                <owl:maxQualifiedCardinality rdf:datatype="http://www.w3.org/2001/XMLSchema#nonNegativeInteger">1</owl:maxQualifiedCardinality>
                <owl:onClass rdf:resource="http://www.wageneder.at/ontology/bpmn2.0#Message"/>
            </owl:Restriction>
        </rdfs:subClassOf>
        <rdfs:subClassOf>
            <owl:Restriction>
                <owl:onProperty rdf:resource="http://www.wageneder.at/ontology/bpmn2.0#name"/>
                <owl:qualifiedCardinality rdf:datatype="http://www.w3.org/2001/XMLSchema#nonNegativeInteger">1</owl:qualifiedCardinality>
                <owl:onDataRange rdf:resource="http://www.w3.org/2001/XMLSchema#string"/>
            </owl:Restriction>
        </rdfs:subClassOf>
        <rdfs:comment>A Message Flow is used to show the flow of Messages between two Participants that are prepared to send and receive them.</rdfs:comment>
    </owl:Class>
    


    <!-- http://www.wageneder.at/ontology/bpmn2.0#MessageFlowAssociation -->

    <owl:Class rdf:about="http://www.wageneder.at/ontology/bpmn2.0#MessageFlowAssociation">
        <rdfs:subClassOf rdf:resource="http://www.wageneder.at/ontology/bpmn2.0#BaseElement"/>
        <rdfs:subClassOf rdf:resource="http://www.wageneder.at/ontology/bpmn2.0#CollaborationLevel"/>
        <rdfs:subClassOf>
            <owl:Restriction>
                <owl:onProperty rdf:resource="http://www.wageneder.at/ontology/bpmn2.0#hasCollaboration"/>
                <owl:qualifiedCardinality rdf:datatype="http://www.w3.org/2001/XMLSchema#nonNegativeInteger">1</owl:qualifiedCardinality>
                <owl:onClass rdf:resource="http://www.wageneder.at/ontology/bpmn2.0#Collaboration"/>
            </owl:Restriction>
        </rdfs:subClassOf>
        <rdfs:subClassOf>
            <owl:Restriction>
                <owl:onProperty rdf:resource="http://www.wageneder.at/ontology/bpmn2.0#hasInnerMessageFlowRef"/>
                <owl:qualifiedCardinality rdf:datatype="http://www.w3.org/2001/XMLSchema#nonNegativeInteger">1</owl:qualifiedCardinality>
                <owl:onClass rdf:resource="http://www.wageneder.at/ontology/bpmn2.0#MessageFlow"/>
            </owl:Restriction>
        </rdfs:subClassOf>
        <rdfs:subClassOf>
            <owl:Restriction>
                <owl:onProperty rdf:resource="http://www.wageneder.at/ontology/bpmn2.0#hasOuterMessageFlowRef"/>
                <owl:qualifiedCardinality rdf:datatype="http://www.w3.org/2001/XMLSchema#nonNegativeInteger">1</owl:qualifiedCardinality>
                <owl:onClass rdf:resource="http://www.wageneder.at/ontology/bpmn2.0#MessageFlow"/>
            </owl:Restriction>
        </rdfs:subClassOf>
        <rdfs:comment>The MessageFlowAssociation element inherits the attributes and model associations of BaseElement (see Table 8.5). Table 9.9 presents the additional model associations for the MessageFlowAssociation element.</rdfs:comment>
    </owl:Class>
    


    <!-- http://www.wageneder.at/ontology/bpmn2.0#Mixed -->

    <owl:Class rdf:about="http://www.wageneder.at/ontology/bpmn2.0#Mixed">
        <rdfs:subClassOf rdf:resource="http://www.wageneder.at/ontology/bpmn2.0#GatewayDirection"/>
        <rdfs:comment>Mixed: This Gateway contains multiple outgoing and multiple incoming Sequence Flows.</rdfs:comment>
    </owl:Class>
    


    <!-- http://www.wageneder.at/ontology/bpmn2.0#Monitoring -->

    <owl:Class rdf:about="http://www.wageneder.at/ontology/bpmn2.0#Monitoring">
        <rdfs:subClassOf rdf:resource="http://www.wageneder.at/ontology/bpmn2.0#BaseElement"/>
        <rdfs:subClassOf rdf:resource="http://www.wageneder.at/ontology/bpmn2.0#ProcessLevel"/>
        <rdfs:comment>The Monitoring and its model associations allow defining attributes related to monitoring. It leverages the BPMN extensibility mechanism. This element is used by FlowElements and Process. The actual definition of monitoring attributes is out of scope of this specification. BPMN 2.0 implementations can define their own set of attributes and their intended semantics.</rdfs:comment>
    </owl:Class>
    


    <!-- http://www.wageneder.at/ontology/bpmn2.0#MultiInstanceBehaviour -->

    <owl:Class rdf:about="http://www.wageneder.at/ontology/bpmn2.0#MultiInstanceBehaviour">
        <rdfs:subClassOf rdf:resource="http://www.wageneder.at/ontology/bpmn2.0#ActivityLevel"/>
        <rdfs:subClassOf>
            <owl:Class>
                <owl:unionOf rdf:parseType="Collection">
                    <rdf:Description rdf:about="http://www.wageneder.at/ontology/bpmn2.0#All"/>
                    <rdf:Description rdf:about="http://www.wageneder.at/ontology/bpmn2.0#Complex"/>
                    <rdf:Description rdf:about="http://www.wageneder.at/ontology/bpmn2.0#None"/>
                    <rdf:Description rdf:about="http://www.wageneder.at/ontology/bpmn2.0#One"/>
                </owl:unionOf>
            </owl:Class>
        </rdfs:subClassOf>
    </owl:Class>
    


    <!-- http://www.wageneder.at/ontology/bpmn2.0#MultiInstanceLoopCharacteristics -->

    <owl:Class rdf:about="http://www.wageneder.at/ontology/bpmn2.0#MultiInstanceLoopCharacteristics">
        <rdfs:subClassOf rdf:resource="http://www.wageneder.at/ontology/bpmn2.0#LoopCharacteristics"/>
        <rdfs:subClassOf>
            <owl:Restriction>
                <owl:onProperty rdf:resource="http://www.wageneder.at/ontology/bpmn2.0#hasCompletionCondition"/>
                <owl:minQualifiedCardinality rdf:datatype="http://www.w3.org/2001/XMLSchema#nonNegativeInteger">0</owl:minQualifiedCardinality>
                <owl:onClass rdf:resource="http://www.wageneder.at/ontology/bpmn2.0#Expression"/>
            </owl:Restriction>
        </rdfs:subClassOf>
        <rdfs:subClassOf>
            <owl:Restriction>
                <owl:onProperty rdf:resource="http://www.wageneder.at/ontology/bpmn2.0#hasComplexBehaviourDefinition"/>
                <owl:minQualifiedCardinality rdf:datatype="http://www.w3.org/2001/XMLSchema#nonNegativeInteger">0</owl:minQualifiedCardinality>
                <owl:onClass rdf:resource="http://www.wageneder.at/ontology/bpmn2.0#ComplexBehaviourDefinition"/>
            </owl:Restriction>
        </rdfs:subClassOf>
        <rdfs:subClassOf>
            <owl:Restriction>
                <owl:onProperty rdf:resource="http://www.wageneder.at/ontology/bpmn2.0#hasInputDataItem"/>
                <owl:minQualifiedCardinality rdf:datatype="http://www.w3.org/2001/XMLSchema#nonNegativeInteger">0</owl:minQualifiedCardinality>
                <owl:onClass rdf:resource="http://www.wageneder.at/ontology/bpmn2.0#DataInput"/>
            </owl:Restriction>
        </rdfs:subClassOf>
        <rdfs:subClassOf>
            <owl:Restriction>
                <owl:onProperty rdf:resource="http://www.wageneder.at/ontology/bpmn2.0#hasLoopCardinality"/>
                <owl:minQualifiedCardinality rdf:datatype="http://www.w3.org/2001/XMLSchema#nonNegativeInteger">0</owl:minQualifiedCardinality>
                <owl:onClass rdf:resource="http://www.wageneder.at/ontology/bpmn2.0#Expression"/>
            </owl:Restriction>
        </rdfs:subClassOf>
        <rdfs:subClassOf>
            <owl:Restriction>
                <owl:onProperty rdf:resource="http://www.wageneder.at/ontology/bpmn2.0#hasLoopDataInputRef"/>
                <owl:minQualifiedCardinality rdf:datatype="http://www.w3.org/2001/XMLSchema#nonNegativeInteger">0</owl:minQualifiedCardinality>
                <owl:onClass rdf:resource="http://www.wageneder.at/ontology/bpmn2.0#ItemAwareElement"/>
            </owl:Restriction>
        </rdfs:subClassOf>
        <rdfs:subClassOf>
            <owl:Restriction>
                <owl:onProperty rdf:resource="http://www.wageneder.at/ontology/bpmn2.0#hasLoopDataOutputRef"/>
                <owl:minQualifiedCardinality rdf:datatype="http://www.w3.org/2001/XMLSchema#nonNegativeInteger">0</owl:minQualifiedCardinality>
                <owl:onClass rdf:resource="http://www.wageneder.at/ontology/bpmn2.0#ItemAwareElement"/>
            </owl:Restriction>
        </rdfs:subClassOf>
        <rdfs:subClassOf>
            <owl:Restriction>
                <owl:onProperty rdf:resource="http://www.wageneder.at/ontology/bpmn2.0#hasNoneBehaviourEventRef"/>
                <owl:minQualifiedCardinality rdf:datatype="http://www.w3.org/2001/XMLSchema#nonNegativeInteger">0</owl:minQualifiedCardinality>
                <owl:onClass rdf:resource="http://www.wageneder.at/ontology/bpmn2.0#EventDefinition"/>
            </owl:Restriction>
        </rdfs:subClassOf>
        <rdfs:subClassOf>
            <owl:Restriction>
                <owl:onProperty rdf:resource="http://www.wageneder.at/ontology/bpmn2.0#hasOneBehaviourEventRef"/>
                <owl:minQualifiedCardinality rdf:datatype="http://www.w3.org/2001/XMLSchema#nonNegativeInteger">0</owl:minQualifiedCardinality>
                <owl:onClass rdf:resource="http://www.wageneder.at/ontology/bpmn2.0#EventDefinition"/>
            </owl:Restriction>
        </rdfs:subClassOf>
        <rdfs:subClassOf>
            <owl:Restriction>
                <owl:onProperty rdf:resource="http://www.wageneder.at/ontology/bpmn2.0#hasOutputDataItem"/>
                <owl:minQualifiedCardinality rdf:datatype="http://www.w3.org/2001/XMLSchema#nonNegativeInteger">0</owl:minQualifiedCardinality>
                <owl:onClass rdf:resource="http://www.wageneder.at/ontology/bpmn2.0#DataOutput"/>
            </owl:Restriction>
        </rdfs:subClassOf>
        <rdfs:subClassOf>
            <owl:Restriction>
                <owl:onProperty rdf:resource="http://www.wageneder.at/ontology/bpmn2.0#hasBehaviour"/>
                <owl:qualifiedCardinality rdf:datatype="http://www.w3.org/2001/XMLSchema#nonNegativeInteger">1</owl:qualifiedCardinality>
                <owl:onClass rdf:resource="http://www.wageneder.at/ontology/bpmn2.0#MultiInstanceBehaviour"/>
            </owl:Restriction>
        </rdfs:subClassOf>
        <rdfs:subClassOf>
            <owl:Restriction>
                <owl:onProperty rdf:resource="http://www.wageneder.at/ontology/bpmn2.0#hasCompletionCondition"/>
                <owl:maxQualifiedCardinality rdf:datatype="http://www.w3.org/2001/XMLSchema#nonNegativeInteger">1</owl:maxQualifiedCardinality>
                <owl:onClass rdf:resource="http://www.wageneder.at/ontology/bpmn2.0#Expression"/>
            </owl:Restriction>
        </rdfs:subClassOf>
        <rdfs:subClassOf>
            <owl:Restriction>
                <owl:onProperty rdf:resource="http://www.wageneder.at/ontology/bpmn2.0#hasInputDataItem"/>
                <owl:maxQualifiedCardinality rdf:datatype="http://www.w3.org/2001/XMLSchema#nonNegativeInteger">1</owl:maxQualifiedCardinality>
                <owl:onClass rdf:resource="http://www.wageneder.at/ontology/bpmn2.0#DataInput"/>
            </owl:Restriction>
        </rdfs:subClassOf>
        <rdfs:subClassOf>
            <owl:Restriction>
                <owl:onProperty rdf:resource="http://www.wageneder.at/ontology/bpmn2.0#hasLoopCardinality"/>
                <owl:maxQualifiedCardinality rdf:datatype="http://www.w3.org/2001/XMLSchema#nonNegativeInteger">1</owl:maxQualifiedCardinality>
                <owl:onClass rdf:resource="http://www.wageneder.at/ontology/bpmn2.0#Expression"/>
            </owl:Restriction>
        </rdfs:subClassOf>
        <rdfs:subClassOf>
            <owl:Restriction>
                <owl:onProperty rdf:resource="http://www.wageneder.at/ontology/bpmn2.0#hasLoopDataInputRef"/>
                <owl:maxQualifiedCardinality rdf:datatype="http://www.w3.org/2001/XMLSchema#nonNegativeInteger">1</owl:maxQualifiedCardinality>
                <owl:onClass rdf:resource="http://www.wageneder.at/ontology/bpmn2.0#ItemAwareElement"/>
            </owl:Restriction>
        </rdfs:subClassOf>
        <rdfs:subClassOf>
            <owl:Restriction>
                <owl:onProperty rdf:resource="http://www.wageneder.at/ontology/bpmn2.0#hasLoopDataOutputRef"/>
                <owl:maxQualifiedCardinality rdf:datatype="http://www.w3.org/2001/XMLSchema#nonNegativeInteger">1</owl:maxQualifiedCardinality>
                <owl:onClass rdf:resource="http://www.wageneder.at/ontology/bpmn2.0#ItemAwareElement"/>
            </owl:Restriction>
        </rdfs:subClassOf>
        <rdfs:subClassOf>
            <owl:Restriction>
                <owl:onProperty rdf:resource="http://www.wageneder.at/ontology/bpmn2.0#hasNoneBehaviourEventRef"/>
                <owl:maxQualifiedCardinality rdf:datatype="http://www.w3.org/2001/XMLSchema#nonNegativeInteger">1</owl:maxQualifiedCardinality>
                <owl:onClass rdf:resource="http://www.wageneder.at/ontology/bpmn2.0#EventDefinition"/>
            </owl:Restriction>
        </rdfs:subClassOf>
        <rdfs:subClassOf>
            <owl:Restriction>
                <owl:onProperty rdf:resource="http://www.wageneder.at/ontology/bpmn2.0#hasOneBehaviourEventRef"/>
                <owl:maxQualifiedCardinality rdf:datatype="http://www.w3.org/2001/XMLSchema#nonNegativeInteger">1</owl:maxQualifiedCardinality>
                <owl:onClass rdf:resource="http://www.wageneder.at/ontology/bpmn2.0#EventDefinition"/>
            </owl:Restriction>
        </rdfs:subClassOf>
        <rdfs:subClassOf>
            <owl:Restriction>
                <owl:onProperty rdf:resource="http://www.wageneder.at/ontology/bpmn2.0#hasOutputDataItem"/>
                <owl:maxQualifiedCardinality rdf:datatype="http://www.w3.org/2001/XMLSchema#nonNegativeInteger">1</owl:maxQualifiedCardinality>
                <owl:onClass rdf:resource="http://www.wageneder.at/ontology/bpmn2.0#DataOutput"/>
            </owl:Restriction>
        </rdfs:subClassOf>
        <rdfs:subClassOf>
            <owl:Restriction>
                <owl:onProperty rdf:resource="http://www.wageneder.at/ontology/bpmn2.0#isSequential"/>
                <owl:qualifiedCardinality rdf:datatype="http://www.w3.org/2001/XMLSchema#nonNegativeInteger">1</owl:qualifiedCardinality>
                <owl:onDataRange rdf:resource="http://www.w3.org/2001/XMLSchema#boolean"/>
            </owl:Restriction>
        </rdfs:subClassOf>
        <rdfs:subClassOf>
            <owl:Restriction>
                <owl:onProperty rdf:resource="http://www.wageneder.at/ontology/bpmn2.0#loopCounter"/>
                <owl:qualifiedCardinality rdf:datatype="http://www.w3.org/2001/XMLSchema#nonNegativeInteger">1</owl:qualifiedCardinality>
                <owl:onDataRange rdf:resource="http://www.w3.org/2001/XMLSchema#integer"/>
            </owl:Restriction>
        </rdfs:subClassOf>
        <rdfs:subClassOf>
            <owl:Restriction>
                <owl:onProperty rdf:resource="http://www.wageneder.at/ontology/bpmn2.0#numberOfActiveInstances"/>
                <owl:qualifiedCardinality rdf:datatype="http://www.w3.org/2001/XMLSchema#nonNegativeInteger">1</owl:qualifiedCardinality>
                <owl:onDataRange rdf:resource="http://www.w3.org/2001/XMLSchema#integer"/>
            </owl:Restriction>
        </rdfs:subClassOf>
        <rdfs:subClassOf>
            <owl:Restriction>
                <owl:onProperty rdf:resource="http://www.wageneder.at/ontology/bpmn2.0#numberOfCompletedInstances"/>
                <owl:qualifiedCardinality rdf:datatype="http://www.w3.org/2001/XMLSchema#nonNegativeInteger">1</owl:qualifiedCardinality>
                <owl:onDataRange rdf:resource="http://www.w3.org/2001/XMLSchema#integer"/>
            </owl:Restriction>
        </rdfs:subClassOf>
        <rdfs:subClassOf>
            <owl:Restriction>
                <owl:onProperty rdf:resource="http://www.wageneder.at/ontology/bpmn2.0#numberOfInstances"/>
                <owl:qualifiedCardinality rdf:datatype="http://www.w3.org/2001/XMLSchema#nonNegativeInteger">1</owl:qualifiedCardinality>
                <owl:onDataRange rdf:resource="http://www.w3.org/2001/XMLSchema#integer"/>
            </owl:Restriction>
        </rdfs:subClassOf>
        <rdfs:subClassOf>
            <owl:Restriction>
                <owl:onProperty rdf:resource="http://www.wageneder.at/ontology/bpmn2.0#numberOfTerminatedInstances"/>
                <owl:qualifiedCardinality rdf:datatype="http://www.w3.org/2001/XMLSchema#nonNegativeInteger">1</owl:qualifiedCardinality>
                <owl:onDataRange rdf:resource="http://www.w3.org/2001/XMLSchema#integer"/>
            </owl:Restriction>
        </rdfs:subClassOf>
        <rdfs:comment>The MultiInstanceLoopCharacteristics element inherits the attributes and model associations of BaseElement (see Table 8.5), through its relationship to LoopCharacteristics. Table 10.29 presents the additional attributes and model associations for the MultiInstanceLoopCharacteristics element.</rdfs:comment>
    </owl:Class>
    


    <!-- http://www.wageneder.at/ontology/bpmn2.0#None -->

    <owl:Class rdf:about="http://www.wageneder.at/ontology/bpmn2.0#None">
        <rdfs:subClassOf rdf:resource="http://www.wageneder.at/ontology/bpmn2.0#AssociationDirection"/>
        <rdfs:subClassOf rdf:resource="http://www.wageneder.at/ontology/bpmn2.0#RelationshipDirection"/>
    </owl:Class>
    


    <!-- http://www.wageneder.at/ontology/bpmn2.0#One -->

    <owl:Class rdf:about="http://www.wageneder.at/ontology/bpmn2.0#One">
        <rdfs:subClassOf rdf:resource="http://www.wageneder.at/ontology/bpmn2.0#AssociationDirection"/>
    </owl:Class>
    


    <!-- http://www.wageneder.at/ontology/bpmn2.0#Operation -->

    <owl:Class rdf:about="http://www.wageneder.at/ontology/bpmn2.0#Operation">
        <rdfs:subClassOf rdf:resource="http://www.wageneder.at/ontology/bpmn2.0#BaseElement"/>
        <rdfs:subClassOf rdf:resource="http://www.wageneder.at/ontology/bpmn2.0#Service"/>
        <rdfs:subClassOf>
            <owl:Restriction>
                <owl:onProperty rdf:resource="http://www.wageneder.at/ontology/bpmn2.0#hasErrorRef"/>
                <owl:minQualifiedCardinality rdf:datatype="http://www.w3.org/2001/XMLSchema#nonNegativeInteger">0</owl:minQualifiedCardinality>
                <owl:onClass rdf:resource="http://www.wageneder.at/ontology/bpmn2.0#Error"/>
            </owl:Restriction>
        </rdfs:subClassOf>
        <rdfs:subClassOf>
            <owl:Restriction>
                <owl:onProperty rdf:resource="http://www.wageneder.at/ontology/bpmn2.0#hasIOBinding"/>
                <owl:minQualifiedCardinality rdf:datatype="http://www.w3.org/2001/XMLSchema#nonNegativeInteger">0</owl:minQualifiedCardinality>
                <owl:onClass rdf:resource="http://www.wageneder.at/ontology/bpmn2.0#InputOutputBinding"/>
            </owl:Restriction>
        </rdfs:subClassOf>
        <rdfs:subClassOf>
            <owl:Restriction>
                <owl:onProperty rdf:resource="http://www.wageneder.at/ontology/bpmn2.0#hasImplementationRef"/>
                <owl:minQualifiedCardinality rdf:datatype="http://www.w3.org/2001/XMLSchema#nonNegativeInteger">0</owl:minQualifiedCardinality>
                <owl:onClass rdf:resource="http://www.wageneder.at/ontology/bpmn2.0#Element"/>
            </owl:Restriction>
        </rdfs:subClassOf>
        <rdfs:subClassOf>
            <owl:Restriction>
                <owl:onProperty rdf:resource="http://www.wageneder.at/ontology/bpmn2.0#hasOutMessageRef"/>
                <owl:minQualifiedCardinality rdf:datatype="http://www.w3.org/2001/XMLSchema#nonNegativeInteger">0</owl:minQualifiedCardinality>
                <owl:onClass rdf:resource="http://www.wageneder.at/ontology/bpmn2.0#Message"/>
            </owl:Restriction>
        </rdfs:subClassOf>
        <rdfs:subClassOf>
            <owl:Restriction>
                <owl:onProperty rdf:resource="http://www.wageneder.at/ontology/bpmn2.0#hasInMessageRef"/>
                <owl:qualifiedCardinality rdf:datatype="http://www.w3.org/2001/XMLSchema#nonNegativeInteger">1</owl:qualifiedCardinality>
                <owl:onClass rdf:resource="http://www.wageneder.at/ontology/bpmn2.0#Message"/>
            </owl:Restriction>
        </rdfs:subClassOf>
        <rdfs:subClassOf>
            <owl:Restriction>
                <owl:onProperty rdf:resource="http://www.wageneder.at/ontology/bpmn2.0#hasImplementationRef"/>
                <owl:maxQualifiedCardinality rdf:datatype="http://www.w3.org/2001/XMLSchema#nonNegativeInteger">1</owl:maxQualifiedCardinality>
                <owl:onClass rdf:resource="http://www.wageneder.at/ontology/bpmn2.0#Element"/>
            </owl:Restriction>
        </rdfs:subClassOf>
        <rdfs:subClassOf>
            <owl:Restriction>
                <owl:onProperty rdf:resource="http://www.wageneder.at/ontology/bpmn2.0#hasOutMessageRef"/>
                <owl:maxQualifiedCardinality rdf:datatype="http://www.w3.org/2001/XMLSchema#nonNegativeInteger">1</owl:maxQualifiedCardinality>
                <owl:onClass rdf:resource="http://www.wageneder.at/ontology/bpmn2.0#Message"/>
            </owl:Restriction>
        </rdfs:subClassOf>
        <rdfs:subClassOf>
            <owl:Restriction>
                <owl:onProperty rdf:resource="http://www.wageneder.at/ontology/bpmn2.0#name"/>
                <owl:qualifiedCardinality rdf:datatype="http://www.w3.org/2001/XMLSchema#nonNegativeInteger">1</owl:qualifiedCardinality>
                <owl:onDataRange rdf:resource="http://www.w3.org/2001/XMLSchema#string"/>
            </owl:Restriction>
        </rdfs:subClassOf>
        <rdfs:comment>An Operation defines Messages that are consumed and, optionally, produced when the Operation is called. It can also define zero or more errors that are returned when operation fails. The Operation inherits the attributes and model associations of BaseElement</rdfs:comment>
    </owl:Class>
    


    <!-- http://www.wageneder.at/ontology/bpmn2.0#OutputSet -->

    <owl:Class rdf:about="http://www.wageneder.at/ontology/bpmn2.0#OutputSet">
        <rdfs:subClassOf rdf:resource="http://www.wageneder.at/ontology/bpmn2.0#BaseElement"/>
        <rdfs:subClassOf rdf:resource="http://www.wageneder.at/ontology/bpmn2.0#DataLevel"/>
        <rdfs:subClassOf>
            <owl:Restriction>
                <owl:onProperty rdf:resource="http://www.wageneder.at/ontology/bpmn2.0#hasDataOutputRefs"/>
                <owl:minQualifiedCardinality rdf:datatype="http://www.w3.org/2001/XMLSchema#nonNegativeInteger">0</owl:minQualifiedCardinality>
                <owl:onClass rdf:resource="http://www.wageneder.at/ontology/bpmn2.0#DataOutput"/>
            </owl:Restriction>
        </rdfs:subClassOf>
        <rdfs:subClassOf>
            <owl:Restriction>
                <owl:onProperty rdf:resource="http://www.wageneder.at/ontology/bpmn2.0#hasInputSetRefs"/>
                <owl:minQualifiedCardinality rdf:datatype="http://www.w3.org/2001/XMLSchema#nonNegativeInteger">0</owl:minQualifiedCardinality>
                <owl:onClass rdf:resource="http://www.wageneder.at/ontology/bpmn2.0#OutputSet"/>
            </owl:Restriction>
        </rdfs:subClassOf>
        <rdfs:subClassOf>
            <owl:Restriction>
                <owl:onProperty rdf:resource="http://www.wageneder.at/ontology/bpmn2.0#hasOptionalOutputRefs"/>
                <owl:minQualifiedCardinality rdf:datatype="http://www.w3.org/2001/XMLSchema#nonNegativeInteger">0</owl:minQualifiedCardinality>
                <owl:onClass rdf:resource="http://www.wageneder.at/ontology/bpmn2.0#DataOutput"/>
            </owl:Restriction>
        </rdfs:subClassOf>
        <rdfs:subClassOf>
            <owl:Restriction>
                <owl:onProperty rdf:resource="http://www.wageneder.at/ontology/bpmn2.0#hasWhileExecutingOutputRefs"/>
                <owl:minQualifiedCardinality rdf:datatype="http://www.w3.org/2001/XMLSchema#nonNegativeInteger">0</owl:minQualifiedCardinality>
                <owl:onClass rdf:resource="http://www.wageneder.at/ontology/bpmn2.0#DataOutput"/>
            </owl:Restriction>
        </rdfs:subClassOf>
        <rdfs:subClassOf>
            <owl:Restriction>
                <owl:onProperty rdf:resource="http://www.wageneder.at/ontology/bpmn2.0#name"/>
                <owl:minQualifiedCardinality rdf:datatype="http://www.w3.org/2001/XMLSchema#nonNegativeInteger">0</owl:minQualifiedCardinality>
                <owl:onDataRange rdf:resource="http://www.w3.org/2001/XMLSchema#string"/>
            </owl:Restriction>
        </rdfs:subClassOf>
        <rdfs:subClassOf>
            <owl:Restriction>
                <owl:onProperty rdf:resource="http://www.wageneder.at/ontology/bpmn2.0#name"/>
                <owl:maxQualifiedCardinality rdf:datatype="http://www.w3.org/2001/XMLSchema#nonNegativeInteger">1</owl:maxQualifiedCardinality>
                <owl:onDataRange rdf:resource="http://www.w3.org/2001/XMLSchema#string"/>
            </owl:Restriction>
        </rdfs:subClassOf>
        <rdfs:comment>The OutputSet element inherits the attributes and model associations of BaseElement (see Table 8.5). Table 10.62 presents the additional attributes and model associations of the OutputSet element.</rdfs:comment>
    </owl:Class>
    


    <!-- http://www.wageneder.at/ontology/bpmn2.0#Parallel -->

    <owl:Class rdf:about="http://www.wageneder.at/ontology/bpmn2.0#Parallel">
        <rdfs:subClassOf rdf:resource="http://www.wageneder.at/ontology/bpmn2.0#EventBasedGatewayType"/>
    </owl:Class>
    


    <!-- http://www.wageneder.at/ontology/bpmn2.0#ParallelGateway -->

    <owl:Class rdf:about="http://www.wageneder.at/ontology/bpmn2.0#ParallelGateway">
        <rdfs:subClassOf rdf:resource="http://www.wageneder.at/ontology/bpmn2.0#Gateway"/>
        <rdfs:comment>A Parallel Gateway is used to synchronize (combine) parallel flows and to create parallel flows.

A Parallel Gateway creates parallel paths without checking any conditions; each outgoing Sequence Flow receives a token upon execution of this Gateway. For incoming flows, the Parallel Gateway will wait for all incoming flows before triggering the flow through its outgoing Sequence Flows.</rdfs:comment>
    </owl:Class>
    


    <!-- http://www.wageneder.at/ontology/bpmn2.0#Participant -->

    <owl:Class rdf:about="http://www.wageneder.at/ontology/bpmn2.0#Participant">
        <rdfs:subClassOf rdf:resource="http://www.wageneder.at/ontology/bpmn2.0#BaseElement"/>
        <rdfs:subClassOf rdf:resource="http://www.wageneder.at/ontology/bpmn2.0#InteractionNode"/>
        <rdfs:subClassOf>
            <owl:Restriction>
                <owl:onProperty rdf:resource="http://www.wageneder.at/ontology/bpmn2.0#hasConversationNode"/>
                <owl:minQualifiedCardinality rdf:datatype="http://www.w3.org/2001/XMLSchema#nonNegativeInteger">0</owl:minQualifiedCardinality>
                <owl:onClass rdf:resource="http://www.wageneder.at/ontology/bpmn2.0#ConversationNode"/>
            </owl:Restriction>
        </rdfs:subClassOf>
        <rdfs:subClassOf>
            <owl:Restriction>
                <owl:onProperty rdf:resource="http://www.wageneder.at/ontology/bpmn2.0#hasEndPointRefs"/>
                <owl:minQualifiedCardinality rdf:datatype="http://www.w3.org/2001/XMLSchema#nonNegativeInteger">0</owl:minQualifiedCardinality>
                <owl:onClass rdf:resource="http://www.wageneder.at/ontology/bpmn2.0#EndPoint"/>
            </owl:Restriction>
        </rdfs:subClassOf>
        <rdfs:subClassOf>
            <owl:Restriction>
                <owl:onProperty rdf:resource="http://www.wageneder.at/ontology/bpmn2.0#hasInterfaceRef"/>
                <owl:minQualifiedCardinality rdf:datatype="http://www.w3.org/2001/XMLSchema#nonNegativeInteger">0</owl:minQualifiedCardinality>
                <owl:onClass rdf:resource="http://www.wageneder.at/ontology/bpmn2.0#Interface"/>
            </owl:Restriction>
        </rdfs:subClassOf>
        <rdfs:subClassOf>
            <owl:Restriction>
                <owl:onProperty rdf:resource="http://www.wageneder.at/ontology/bpmn2.0#hasParticipantAssociation"/>
                <owl:minQualifiedCardinality rdf:datatype="http://www.w3.org/2001/XMLSchema#nonNegativeInteger">0</owl:minQualifiedCardinality>
                <owl:onClass rdf:resource="http://www.wageneder.at/ontology/bpmn2.0#ParticipantAssociation"/>
            </owl:Restriction>
        </rdfs:subClassOf>
        <rdfs:subClassOf>
            <owl:Restriction>
                <owl:onProperty rdf:resource="http://www.wageneder.at/ontology/bpmn2.0#hasParticipantMultiplicity"/>
                <owl:minQualifiedCardinality rdf:datatype="http://www.w3.org/2001/XMLSchema#nonNegativeInteger">0</owl:minQualifiedCardinality>
                <owl:onClass rdf:resource="http://www.wageneder.at/ontology/bpmn2.0#ParticipantMultiplicity"/>
            </owl:Restriction>
        </rdfs:subClassOf>
        <rdfs:subClassOf>
            <owl:Restriction>
                <owl:onProperty rdf:resource="http://www.wageneder.at/ontology/bpmn2.0#hasPartnerEntityRef"/>
                <owl:minQualifiedCardinality rdf:datatype="http://www.w3.org/2001/XMLSchema#nonNegativeInteger">0</owl:minQualifiedCardinality>
                <owl:onClass rdf:resource="http://www.wageneder.at/ontology/bpmn2.0#PartnerEntity"/>
            </owl:Restriction>
        </rdfs:subClassOf>
        <rdfs:subClassOf>
            <owl:Restriction>
                <owl:onProperty rdf:resource="http://www.wageneder.at/ontology/bpmn2.0#hasPartnerRoleRef"/>
                <owl:minQualifiedCardinality rdf:datatype="http://www.w3.org/2001/XMLSchema#nonNegativeInteger">0</owl:minQualifiedCardinality>
                <owl:onClass rdf:resource="http://www.wageneder.at/ontology/bpmn2.0#PartnerRole"/>
            </owl:Restriction>
        </rdfs:subClassOf>
        <rdfs:subClassOf>
            <owl:Restriction>
                <owl:onProperty rdf:resource="http://www.wageneder.at/ontology/bpmn2.0#hasProcessRef"/>
                <owl:minQualifiedCardinality rdf:datatype="http://www.w3.org/2001/XMLSchema#nonNegativeInteger">0</owl:minQualifiedCardinality>
                <owl:onClass rdf:resource="http://www.wageneder.at/ontology/bpmn2.0#Process"/>
            </owl:Restriction>
        </rdfs:subClassOf>
        <rdfs:subClassOf>
            <owl:Restriction>
                <owl:onProperty rdf:resource="http://www.wageneder.at/ontology/bpmn2.0#hasCollaboration"/>
                <owl:qualifiedCardinality rdf:datatype="http://www.w3.org/2001/XMLSchema#nonNegativeInteger">1</owl:qualifiedCardinality>
                <owl:onClass rdf:resource="http://www.wageneder.at/ontology/bpmn2.0#Collaboration"/>
            </owl:Restriction>
        </rdfs:subClassOf>
        <rdfs:subClassOf>
            <owl:Restriction>
                <owl:onProperty rdf:resource="http://www.wageneder.at/ontology/bpmn2.0#hasParticipantMultiplicity"/>
                <owl:maxQualifiedCardinality rdf:datatype="http://www.w3.org/2001/XMLSchema#nonNegativeInteger">1</owl:maxQualifiedCardinality>
                <owl:onClass rdf:resource="http://www.wageneder.at/ontology/bpmn2.0#ParticipantMultiplicity"/>
            </owl:Restriction>
        </rdfs:subClassOf>
        <rdfs:subClassOf>
            <owl:Restriction>
                <owl:onProperty rdf:resource="http://www.wageneder.at/ontology/bpmn2.0#hasProcessRef"/>
                <owl:maxQualifiedCardinality rdf:datatype="http://www.w3.org/2001/XMLSchema#nonNegativeInteger">1</owl:maxQualifiedCardinality>
                <owl:onClass rdf:resource="http://www.wageneder.at/ontology/bpmn2.0#Process"/>
            </owl:Restriction>
        </rdfs:subClassOf>
        <rdfs:subClassOf>
            <owl:Restriction>
                <owl:onProperty rdf:resource="http://www.wageneder.at/ontology/bpmn2.0#name"/>
                <owl:minQualifiedCardinality rdf:datatype="http://www.w3.org/2001/XMLSchema#nonNegativeInteger">0</owl:minQualifiedCardinality>
                <owl:onDataRange rdf:resource="http://www.w3.org/2001/XMLSchema#string"/>
            </owl:Restriction>
        </rdfs:subClassOf>
        <rdfs:comment>A Participant represents a specific PartnerEntity (e.g., a company) and/or a more general PartnerRole (e.g., a buyer, seller, or manufacturer) that are Participants in a Collaboration. A Participant is often responsible for the execution of the Process enclosed in a Pool; however, a Pool MAY be defined without a Process.</rdfs:comment>
    </owl:Class>
    


    <!-- http://www.wageneder.at/ontology/bpmn2.0#ParticipantAssociation -->

    <owl:Class rdf:about="http://www.wageneder.at/ontology/bpmn2.0#ParticipantAssociation">
        <rdfs:subClassOf rdf:resource="http://www.wageneder.at/ontology/bpmn2.0#BaseElement"/>
        <rdfs:subClassOf rdf:resource="http://www.wageneder.at/ontology/bpmn2.0#CollaborationLevel"/>
        <rdfs:subClassOf>
            <owl:Restriction>
                <owl:onProperty rdf:resource="http://www.wageneder.at/ontology/bpmn2.0#hasCallConversation"/>
                <owl:minQualifiedCardinality rdf:datatype="http://www.w3.org/2001/XMLSchema#nonNegativeInteger">0</owl:minQualifiedCardinality>
                <owl:onClass rdf:resource="http://www.wageneder.at/ontology/bpmn2.0#CallConversation"/>
            </owl:Restriction>
        </rdfs:subClassOf>
        <rdfs:subClassOf>
            <owl:Restriction>
                <owl:onProperty rdf:resource="http://www.wageneder.at/ontology/bpmn2.0#hasCollaboration"/>
                <owl:minQualifiedCardinality rdf:datatype="http://www.w3.org/2001/XMLSchema#nonNegativeInteger">0</owl:minQualifiedCardinality>
                <owl:onClass rdf:resource="http://www.wageneder.at/ontology/bpmn2.0#Collaboration"/>
            </owl:Restriction>
        </rdfs:subClassOf>
        <rdfs:subClassOf>
            <owl:Restriction>
                <owl:onProperty rdf:resource="http://www.wageneder.at/ontology/bpmn2.0#hasInnerParticipantRef"/>
                <owl:qualifiedCardinality rdf:datatype="http://www.w3.org/2001/XMLSchema#nonNegativeInteger">1</owl:qualifiedCardinality>
                <owl:onClass rdf:resource="http://www.wageneder.at/ontology/bpmn2.0#Participant"/>
            </owl:Restriction>
        </rdfs:subClassOf>
        <rdfs:subClassOf>
            <owl:Restriction>
                <owl:onProperty rdf:resource="http://www.wageneder.at/ontology/bpmn2.0#hasOuterParticipantRef"/>
                <owl:qualifiedCardinality rdf:datatype="http://www.w3.org/2001/XMLSchema#nonNegativeInteger">1</owl:qualifiedCardinality>
                <owl:onClass rdf:resource="http://www.wageneder.at/ontology/bpmn2.0#Participant"/>
            </owl:Restriction>
        </rdfs:subClassOf>
        <rdfs:subClassOf>
            <owl:Restriction>
                <owl:onProperty rdf:resource="http://www.wageneder.at/ontology/bpmn2.0#hasCallConversation"/>
                <owl:maxQualifiedCardinality rdf:datatype="http://www.w3.org/2001/XMLSchema#nonNegativeInteger">1</owl:maxQualifiedCardinality>
                <owl:onClass rdf:resource="http://www.wageneder.at/ontology/bpmn2.0#CallConversation"/>
            </owl:Restriction>
        </rdfs:subClassOf>
        <rdfs:subClassOf>
            <owl:Restriction>
                <owl:onProperty rdf:resource="http://www.wageneder.at/ontology/bpmn2.0#hasCollaboration"/>
                <owl:maxQualifiedCardinality rdf:datatype="http://www.w3.org/2001/XMLSchema#nonNegativeInteger">1</owl:maxQualifiedCardinality>
                <owl:onClass rdf:resource="http://www.wageneder.at/ontology/bpmn2.0#Collaboration"/>
            </owl:Restriction>
        </rdfs:subClassOf>
        <rdfs:comment>The ParticipantAssociation element inherits the attributes and model associations of BaseElement (see Table 8.5). Table 9.7 presents the additional model associations for the ParticipantAssociation element.</rdfs:comment>
    </owl:Class>
    


    <!-- http://www.wageneder.at/ontology/bpmn2.0#ParticipantMultiplicity -->

    <owl:Class rdf:about="http://www.wageneder.at/ontology/bpmn2.0#ParticipantMultiplicity">
        <rdfs:subClassOf rdf:resource="http://www.wageneder.at/ontology/bpmn2.0#CollaborationLevel"/>
        <rdfs:subClassOf>
            <owl:Restriction>
                <owl:onProperty rdf:resource="http://www.wageneder.at/ontology/bpmn2.0#maximum"/>
                <owl:minQualifiedCardinality rdf:datatype="http://www.w3.org/2001/XMLSchema#nonNegativeInteger">0</owl:minQualifiedCardinality>
                <owl:onDataRange rdf:resource="http://www.w3.org/2001/XMLSchema#integer"/>
            </owl:Restriction>
        </rdfs:subClassOf>
        <rdfs:subClassOf>
            <owl:Restriction>
                <owl:onProperty rdf:resource="http://www.wageneder.at/ontology/bpmn2.0#numParticipants"/>
                <owl:minQualifiedCardinality rdf:datatype="http://www.w3.org/2001/XMLSchema#nonNegativeInteger">0</owl:minQualifiedCardinality>
                <owl:onDataRange rdf:resource="http://www.w3.org/2001/XMLSchema#integer"/>
            </owl:Restriction>
        </rdfs:subClassOf>
        <rdfs:subClassOf>
            <owl:Restriction>
                <owl:onProperty rdf:resource="http://www.wageneder.at/ontology/bpmn2.0#minium"/>
                <owl:qualifiedCardinality rdf:datatype="http://www.w3.org/2001/XMLSchema#nonNegativeInteger">1</owl:qualifiedCardinality>
                <owl:onDataRange rdf:resource="http://www.w3.org/2001/XMLSchema#integer"/>
            </owl:Restriction>
        </rdfs:subClassOf>
        <rdfs:subClassOf>
            <owl:Restriction>
                <owl:onProperty rdf:resource="http://www.wageneder.at/ontology/bpmn2.0#maximum"/>
                <owl:maxQualifiedCardinality rdf:datatype="http://www.w3.org/2001/XMLSchema#nonNegativeInteger">1</owl:maxQualifiedCardinality>
                <owl:onDataRange rdf:resource="http://www.w3.org/2001/XMLSchema#integer"/>
            </owl:Restriction>
        </rdfs:subClassOf>
        <rdfs:subClassOf>
            <owl:Restriction>
                <owl:onProperty rdf:resource="http://www.wageneder.at/ontology/bpmn2.0#numParticipants"/>
                <owl:maxQualifiedCardinality rdf:datatype="http://www.w3.org/2001/XMLSchema#nonNegativeInteger">1</owl:maxQualifiedCardinality>
                <owl:onDataRange rdf:resource="http://www.w3.org/2001/XMLSchema#integer"/>
            </owl:Restriction>
        </rdfs:subClassOf>
        <rdfs:comment>Table 9.5 presents the attributes for the ParticipantMultiplicity element.</rdfs:comment>
    </owl:Class>
    


    <!-- http://www.wageneder.at/ontology/bpmn2.0#PartnerEntity -->

    <owl:Class rdf:about="http://www.wageneder.at/ontology/bpmn2.0#PartnerEntity">
        <rdfs:subClassOf rdf:resource="http://www.wageneder.at/ontology/bpmn2.0#Common"/>
        <rdfs:subClassOf rdf:resource="http://www.wageneder.at/ontology/bpmn2.0#RootElement"/>
        <rdfs:subClassOf>
            <owl:Restriction>
                <owl:onProperty rdf:resource="http://www.wageneder.at/ontology/bpmn2.0#hasParticipantRef"/>
                <owl:minQualifiedCardinality rdf:datatype="http://www.w3.org/2001/XMLSchema#nonNegativeInteger">0</owl:minQualifiedCardinality>
                <owl:onClass rdf:resource="http://www.wageneder.at/ontology/bpmn2.0#Participant"/>
            </owl:Restriction>
        </rdfs:subClassOf>
        <rdfs:subClassOf>
            <owl:Restriction>
                <owl:onProperty rdf:resource="http://www.wageneder.at/ontology/bpmn2.0#name"/>
                <owl:qualifiedCardinality rdf:datatype="http://www.w3.org/2001/XMLSchema#nonNegativeInteger">1</owl:qualifiedCardinality>
                <owl:onDataRange rdf:resource="http://www.w3.org/2001/XMLSchema#string"/>
            </owl:Restriction>
        </rdfs:subClassOf>
        <rdfs:comment>The PartnerEntity element inherits the attributes and model associations of BaseElement (see Figure 8.5). Table 9.3 presents the additional attributes and model associations for the PartnerEntity element.</rdfs:comment>
    </owl:Class>
    


    <!-- http://www.wageneder.at/ontology/bpmn2.0#PartnerRole -->

    <owl:Class rdf:about="http://www.wageneder.at/ontology/bpmn2.0#PartnerRole">
        <rdfs:subClassOf rdf:resource="http://www.wageneder.at/ontology/bpmn2.0#Common"/>
        <rdfs:subClassOf rdf:resource="http://www.wageneder.at/ontology/bpmn2.0#RootElement"/>
        <rdfs:subClassOf>
            <owl:Restriction>
                <owl:onProperty rdf:resource="http://www.wageneder.at/ontology/bpmn2.0#hasParticipantRef"/>
                <owl:minQualifiedCardinality rdf:datatype="http://www.w3.org/2001/XMLSchema#nonNegativeInteger">0</owl:minQualifiedCardinality>
                <owl:onClass rdf:resource="http://www.wageneder.at/ontology/bpmn2.0#Participant"/>
            </owl:Restriction>
        </rdfs:subClassOf>
        <rdfs:subClassOf>
            <owl:Restriction>
                <owl:onProperty rdf:resource="http://www.wageneder.at/ontology/bpmn2.0#name"/>
                <owl:qualifiedCardinality rdf:datatype="http://www.w3.org/2001/XMLSchema#nonNegativeInteger">1</owl:qualifiedCardinality>
                <owl:onDataRange rdf:resource="http://www.w3.org/2001/XMLSchema#string"/>
            </owl:Restriction>
        </rdfs:subClassOf>
        <rdfs:comment>The PartnerRole element inherits the attributes and model associations of BaseElement (see Figure 8.5). Table 9.4 presents the additional attributes and model associations for the PartnerRole element.</rdfs:comment>
    </owl:Class>
    


    <!-- http://www.wageneder.at/ontology/bpmn2.0#Performer -->

    <owl:Class rdf:about="http://www.wageneder.at/ontology/bpmn2.0#Performer">
        <rdfs:subClassOf rdf:resource="http://www.wageneder.at/ontology/bpmn2.0#BaseElement"/>
        <rdfs:subClassOf rdf:resource="http://www.wageneder.at/ontology/bpmn2.0#ResourceRole"/>
        <rdfs:comment>The Performer element inherits the attributes and model associations of BaseElement (see Table 8.5) through its relationship to ResourceRole, but does not  ave any additional attributes or model associations.</rdfs:comment>
    </owl:Class>
    


    <!-- http://www.wageneder.at/ontology/bpmn2.0#Physical -->

    <owl:Class rdf:about="http://www.wageneder.at/ontology/bpmn2.0#Physical">
        <rdfs:subClassOf rdf:resource="http://www.wageneder.at/ontology/bpmn2.0#ItemKind"/>
    </owl:Class>
    


    <!-- http://www.wageneder.at/ontology/bpmn2.0#PotentialOwner -->

    <owl:Class rdf:about="http://www.wageneder.at/ontology/bpmn2.0#PotentialOwner">
        <rdfs:subClassOf rdf:resource="http://www.wageneder.at/ontology/bpmn2.0#HumanPerformer"/>
        <rdfs:comment>Potential owners of a User Task are persons who can claim and work on it. A potential owner becomes the actual ownerof a Task, usually by explicitly claiming it.</rdfs:comment>
    </owl:Class>
    


    <!-- http://www.wageneder.at/ontology/bpmn2.0#Private -->

    <owl:Class rdf:about="http://www.wageneder.at/ontology/bpmn2.0#Private">
        <rdfs:subClassOf rdf:resource="http://www.wageneder.at/ontology/bpmn2.0#ProcessType"/>
    </owl:Class>
    


    <!-- http://www.wageneder.at/ontology/bpmn2.0#Process -->

    <owl:Class rdf:about="http://www.wageneder.at/ontology/bpmn2.0#Process">
        <rdfs:subClassOf rdf:resource="http://www.wageneder.at/ontology/bpmn2.0#CallableElement"/>
        <rdfs:subClassOf rdf:resource="http://www.wageneder.at/ontology/bpmn2.0#FlowElementsContainer"/>
        <rdfs:subClassOf rdf:resource="http://www.wageneder.at/ontology/bpmn2.0#ProcessLevel"/>
        <rdfs:subClassOf>
            <owl:Restriction>
                <owl:onProperty rdf:resource="http://www.wageneder.at/ontology/bpmn2.0#hasArtifact"/>
                <owl:minQualifiedCardinality rdf:datatype="http://www.w3.org/2001/XMLSchema#nonNegativeInteger">0</owl:minQualifiedCardinality>
                <owl:onClass rdf:resource="http://www.wageneder.at/ontology/bpmn2.0#Artifact"/>
            </owl:Restriction>
        </rdfs:subClassOf>
        <rdfs:subClassOf>
            <owl:Restriction>
                <owl:onProperty rdf:resource="http://www.wageneder.at/ontology/bpmn2.0#hasAuditing"/>
                <owl:minQualifiedCardinality rdf:datatype="http://www.w3.org/2001/XMLSchema#nonNegativeInteger">0</owl:minQualifiedCardinality>
                <owl:onClass rdf:resource="http://www.wageneder.at/ontology/bpmn2.0#Auditing"/>
            </owl:Restriction>
        </rdfs:subClassOf>
        <rdfs:subClassOf>
            <owl:Restriction>
                <owl:onProperty rdf:resource="http://www.wageneder.at/ontology/bpmn2.0#hasCorrelationSubscriptions"/>
                <owl:minQualifiedCardinality rdf:datatype="http://www.w3.org/2001/XMLSchema#nonNegativeInteger">0</owl:minQualifiedCardinality>
                <owl:onClass rdf:resource="http://www.wageneder.at/ontology/bpmn2.0#CorrelationSubscription"/>
            </owl:Restriction>
        </rdfs:subClassOf>
        <rdfs:subClassOf>
            <owl:Restriction>
                <owl:onProperty rdf:resource="http://www.wageneder.at/ontology/bpmn2.0#hasDefinitionalCollaborationRef"/>
                <owl:minQualifiedCardinality rdf:datatype="http://www.w3.org/2001/XMLSchema#nonNegativeInteger">0</owl:minQualifiedCardinality>
                <owl:onClass rdf:resource="http://www.wageneder.at/ontology/bpmn2.0#Collaboration"/>
            </owl:Restriction>
        </rdfs:subClassOf>
        <rdfs:subClassOf>
            <owl:Restriction>
                <owl:onProperty rdf:resource="http://www.wageneder.at/ontology/bpmn2.0#hasMonitoring"/>
                <owl:minQualifiedCardinality rdf:datatype="http://www.w3.org/2001/XMLSchema#nonNegativeInteger">0</owl:minQualifiedCardinality>
                <owl:onClass rdf:resource="http://www.wageneder.at/ontology/bpmn2.0#Monitoring"/>
            </owl:Restriction>
        </rdfs:subClassOf>
        <rdfs:subClassOf>
            <owl:Restriction>
                <owl:onProperty rdf:resource="http://www.wageneder.at/ontology/bpmn2.0#hasParticipant"/>
                <owl:minQualifiedCardinality rdf:datatype="http://www.w3.org/2001/XMLSchema#nonNegativeInteger">0</owl:minQualifiedCardinality>
                <owl:onClass rdf:resource="http://www.wageneder.at/ontology/bpmn2.0#Participant"/>
            </owl:Restriction>
        </rdfs:subClassOf>
        <rdfs:subClassOf>
            <owl:Restriction>
                <owl:onProperty rdf:resource="http://www.wageneder.at/ontology/bpmn2.0#hasProperties"/>
                <owl:minQualifiedCardinality rdf:datatype="http://www.w3.org/2001/XMLSchema#nonNegativeInteger">0</owl:minQualifiedCardinality>
                <owl:onClass rdf:resource="http://www.wageneder.at/ontology/bpmn2.0#Property"/>
            </owl:Restriction>
        </rdfs:subClassOf>
        <rdfs:subClassOf>
            <owl:Restriction>
                <owl:onProperty rdf:resource="http://www.wageneder.at/ontology/bpmn2.0#hasResources"/>
                <owl:minQualifiedCardinality rdf:datatype="http://www.w3.org/2001/XMLSchema#nonNegativeInteger">0</owl:minQualifiedCardinality>
                <owl:onClass rdf:resource="http://www.wageneder.at/ontology/bpmn2.0#ResourceRole"/>
            </owl:Restriction>
        </rdfs:subClassOf>
        <rdfs:subClassOf>
            <owl:Restriction>
                <owl:onProperty rdf:resource="http://www.wageneder.at/ontology/bpmn2.0#hasSupports"/>
                <owl:minQualifiedCardinality rdf:datatype="http://www.w3.org/2001/XMLSchema#nonNegativeInteger">0</owl:minQualifiedCardinality>
                <owl:onClass rdf:resource="http://www.wageneder.at/ontology/bpmn2.0#Process"/>
            </owl:Restriction>
        </rdfs:subClassOf>
        <rdfs:subClassOf>
            <owl:Restriction>
                <owl:onProperty rdf:resource="http://www.wageneder.at/ontology/bpmn2.0#hasCollaboration"/>
                <owl:qualifiedCardinality rdf:datatype="http://www.w3.org/2001/XMLSchema#nonNegativeInteger">1</owl:qualifiedCardinality>
                <owl:onClass rdf:resource="http://www.wageneder.at/ontology/bpmn2.0#Collaboration"/>
            </owl:Restriction>
        </rdfs:subClassOf>
        <rdfs:subClassOf>
            <owl:Restriction>
                <owl:onProperty rdf:resource="http://www.wageneder.at/ontology/bpmn2.0#hasProcessType"/>
                <owl:qualifiedCardinality rdf:datatype="http://www.w3.org/2001/XMLSchema#nonNegativeInteger">1</owl:qualifiedCardinality>
                <owl:onClass rdf:resource="http://www.wageneder.at/ontology/bpmn2.0#ProcessType"/>
            </owl:Restriction>
        </rdfs:subClassOf>
        <rdfs:subClassOf>
            <owl:Restriction>
                <owl:onProperty rdf:resource="http://www.wageneder.at/ontology/bpmn2.0#hasArtifact"/>
                <owl:maxQualifiedCardinality rdf:datatype="http://www.w3.org/2001/XMLSchema#nonNegativeInteger">1</owl:maxQualifiedCardinality>
                <owl:onClass rdf:resource="http://www.wageneder.at/ontology/bpmn2.0#Artifact"/>
            </owl:Restriction>
        </rdfs:subClassOf>
        <rdfs:subClassOf>
            <owl:Restriction>
                <owl:onProperty rdf:resource="http://www.wageneder.at/ontology/bpmn2.0#hasAuditing"/>
                <owl:maxQualifiedCardinality rdf:datatype="http://www.w3.org/2001/XMLSchema#nonNegativeInteger">1</owl:maxQualifiedCardinality>
                <owl:onClass rdf:resource="http://www.wageneder.at/ontology/bpmn2.0#Auditing"/>
            </owl:Restriction>
        </rdfs:subClassOf>
        <rdfs:subClassOf>
            <owl:Restriction>
                <owl:onProperty rdf:resource="http://www.wageneder.at/ontology/bpmn2.0#hasDefinitionalCollaborationRef"/>
                <owl:maxQualifiedCardinality rdf:datatype="http://www.w3.org/2001/XMLSchema#nonNegativeInteger">1</owl:maxQualifiedCardinality>
                <owl:onClass rdf:resource="http://www.wageneder.at/ontology/bpmn2.0#Collaboration"/>
            </owl:Restriction>
        </rdfs:subClassOf>
        <rdfs:subClassOf>
            <owl:Restriction>
                <owl:onProperty rdf:resource="http://www.wageneder.at/ontology/bpmn2.0#hasMonitoring"/>
                <owl:maxQualifiedCardinality rdf:datatype="http://www.w3.org/2001/XMLSchema#nonNegativeInteger">1</owl:maxQualifiedCardinality>
                <owl:onClass rdf:resource="http://www.wageneder.at/ontology/bpmn2.0#Monitoring"/>
            </owl:Restriction>
        </rdfs:subClassOf>
        <rdfs:subClassOf>
            <owl:Restriction>
                <owl:onProperty rdf:resource="http://www.wageneder.at/ontology/bpmn2.0#isClosed"/>
                <owl:qualifiedCardinality rdf:datatype="http://www.w3.org/2001/XMLSchema#nonNegativeInteger">1</owl:qualifiedCardinality>
                <owl:onDataRange rdf:resource="http://www.w3.org/2001/XMLSchema#boolean"/>
            </owl:Restriction>
        </rdfs:subClassOf>
        <rdfs:subClassOf>
            <owl:Restriction>
                <owl:onProperty rdf:resource="http://www.wageneder.at/ontology/bpmn2.0#isExecutable"/>
                <owl:qualifiedCardinality rdf:datatype="http://www.w3.org/2001/XMLSchema#nonNegativeInteger">1</owl:qualifiedCardinality>
                <owl:onDataRange rdf:resource="http://www.w3.org/2001/XMLSchema#boolean"/>
            </owl:Restriction>
        </rdfs:subClassOf>
        <rdfs:subClassOf>
            <owl:Restriction>
                <owl:onProperty rdf:resource="http://www.wageneder.at/ontology/bpmn2.0#state"/>
                <owl:qualifiedCardinality rdf:datatype="http://www.w3.org/2001/XMLSchema#nonNegativeInteger">1</owl:qualifiedCardinality>
                <owl:onDataRange rdf:resource="http://www.w3.org/2001/XMLSchema#string"/>
            </owl:Restriction>
        </rdfs:subClassOf>
        <rdfs:comment>The Process element inherits the attributes and model associations of CallableElement (see Table 10.24) and of FlowElementContainer (see Table 8.45). Table 10.1 presents the additional attributes and model associations of the Process element.</rdfs:comment>
    </owl:Class>
    


    <!-- http://www.wageneder.at/ontology/bpmn2.0#ProcessLevel -->

    <owl:Class rdf:about="http://www.wageneder.at/ontology/bpmn2.0#ProcessLevel">
        <rdfs:subClassOf rdf:resource="http://www.wageneder.at/ontology/bpmn2.0#Common"/>
        <rdfs:comment>This is just a hierarchical element for organisational purposes.
It presents the Process Folder</rdfs:comment>
    </owl:Class>
    


    <!-- http://www.wageneder.at/ontology/bpmn2.0#ProcessType -->

    <owl:Class rdf:about="http://www.wageneder.at/ontology/bpmn2.0#ProcessType">
        <rdfs:subClassOf rdf:resource="http://www.wageneder.at/ontology/bpmn2.0#ProcessLevel"/>
        <rdfs:subClassOf>
            <owl:Class>
                <owl:unionOf rdf:parseType="Collection">
                    <rdf:Description rdf:about="http://www.wageneder.at/ontology/bpmn2.0#None"/>
                    <rdf:Description rdf:about="http://www.wageneder.at/ontology/bpmn2.0#Private"/>
                    <rdf:Description rdf:about="http://www.wageneder.at/ontology/bpmn2.0#Public"/>
                </owl:unionOf>
            </owl:Class>
        </rdfs:subClassOf>
    </owl:Class>
    


    <!-- http://www.wageneder.at/ontology/bpmn2.0#Property -->

    <owl:Class rdf:about="http://www.wageneder.at/ontology/bpmn2.0#Property">
        <rdfs:subClassOf rdf:resource="http://www.wageneder.at/ontology/bpmn2.0#ItemAwareElement"/>
        <rdfs:subClassOf>
            <owl:Restriction>
                <owl:onProperty rdf:resource="http://www.wageneder.at/ontology/bpmn2.0#hasEvent"/>
                <owl:minQualifiedCardinality rdf:datatype="http://www.w3.org/2001/XMLSchema#nonNegativeInteger">0</owl:minQualifiedCardinality>
                <owl:onClass rdf:resource="http://www.wageneder.at/ontology/bpmn2.0#Event"/>
            </owl:Restriction>
        </rdfs:subClassOf>
        <rdfs:subClassOf>
            <owl:Restriction>
                <owl:onProperty rdf:resource="http://www.wageneder.at/ontology/bpmn2.0#hasEvent"/>
                <owl:maxQualifiedCardinality rdf:datatype="http://www.w3.org/2001/XMLSchema#nonNegativeInteger">1</owl:maxQualifiedCardinality>
                <owl:onClass rdf:resource="http://www.wageneder.at/ontology/bpmn2.0#Event"/>
            </owl:Restriction>
        </rdfs:subClassOf>
        <rdfs:subClassOf>
            <owl:Restriction>
                <owl:onProperty rdf:resource="http://www.wageneder.at/ontology/bpmn2.0#name"/>
                <owl:qualifiedCardinality rdf:datatype="http://www.w3.org/2001/XMLSchema#nonNegativeInteger">1</owl:qualifiedCardinality>
                <owl:onDataRange rdf:resource="http://www.w3.org/2001/XMLSchema#string"/>
            </owl:Restriction>
        </rdfs:subClassOf>
        <rdfs:comment>Properties, like Data Objects, are item-aware elements. But, unlike Data Objects, they are not visually displayed on a Process diagram. Certain flow elements MAY contain properties, in particular only Processes, Activities, and Events MAY contain Properties.</rdfs:comment>
    </owl:Class>
    


    <!-- http://www.wageneder.at/ontology/bpmn2.0#Public -->

    <owl:Class rdf:about="http://www.wageneder.at/ontology/bpmn2.0#Public">
        <rdfs:subClassOf rdf:resource="http://www.wageneder.at/ontology/bpmn2.0#ProcessType"/>
    </owl:Class>
    


    <!-- http://www.wageneder.at/ontology/bpmn2.0#ReceiveTask -->

    <owl:Class rdf:about="http://www.wageneder.at/ontology/bpmn2.0#ReceiveTask">
        <rdfs:subClassOf rdf:resource="http://www.wageneder.at/ontology/bpmn2.0#Task"/>
        <rdfs:subClassOf>
            <owl:Restriction>
                <owl:onProperty rdf:resource="http://www.wageneder.at/ontology/bpmn2.0#hasMessageRef"/>
                <owl:minQualifiedCardinality rdf:datatype="http://www.w3.org/2001/XMLSchema#nonNegativeInteger">0</owl:minQualifiedCardinality>
                <owl:onClass rdf:resource="http://www.wageneder.at/ontology/bpmn2.0#Message"/>
            </owl:Restriction>
        </rdfs:subClassOf>
        <rdfs:subClassOf>
            <owl:Restriction>
                <owl:onProperty rdf:resource="http://www.wageneder.at/ontology/bpmn2.0#hasOperationRef"/>
                <owl:qualifiedCardinality rdf:datatype="http://www.w3.org/2001/XMLSchema#nonNegativeInteger">1</owl:qualifiedCardinality>
                <owl:onClass rdf:resource="http://www.wageneder.at/ontology/bpmn2.0#Operation"/>
            </owl:Restriction>
        </rdfs:subClassOf>
        <rdfs:subClassOf>
            <owl:Restriction>
                <owl:onProperty rdf:resource="http://www.wageneder.at/ontology/bpmn2.0#hasMessageRef"/>
                <owl:maxQualifiedCardinality rdf:datatype="http://www.w3.org/2001/XMLSchema#nonNegativeInteger">1</owl:maxQualifiedCardinality>
                <owl:onClass rdf:resource="http://www.wageneder.at/ontology/bpmn2.0#Message"/>
            </owl:Restriction>
        </rdfs:subClassOf>
        <rdfs:subClassOf>
            <owl:Restriction>
                <owl:onProperty rdf:resource="http://www.wageneder.at/ontology/bpmn2.0#implementation"/>
                <owl:qualifiedCardinality rdf:datatype="http://www.w3.org/2001/XMLSchema#nonNegativeInteger">1</owl:qualifiedCardinality>
                <owl:onDataRange rdf:resource="http://www.w3.org/2001/XMLSchema#string"/>
            </owl:Restriction>
        </rdfs:subClassOf>
        <rdfs:subClassOf>
            <owl:Restriction>
                <owl:onProperty rdf:resource="http://www.wageneder.at/ontology/bpmn2.0#instantiate"/>
                <owl:qualifiedCardinality rdf:datatype="http://www.w3.org/2001/XMLSchema#nonNegativeInteger">1</owl:qualifiedCardinality>
                <owl:onDataRange rdf:resource="http://www.w3.org/2001/XMLSchema#boolean"/>
            </owl:Restriction>
        </rdfs:subClassOf>
        <rdfs:comment>A Receive Task is a simple Task that is designed to wait for a Message to arrive from an external Participant
(relative to the Process). Once the Message has been received, the Task is completed.</rdfs:comment>
    </owl:Class>
    


    <!-- http://www.wageneder.at/ontology/bpmn2.0#Relationship -->

    <owl:Class rdf:about="http://www.wageneder.at/ontology/bpmn2.0#Relationship">
        <rdfs:subClassOf rdf:resource="http://www.wageneder.at/ontology/bpmn2.0#BaseElement"/>
        <rdfs:subClassOf>
            <owl:Restriction>
                <owl:onProperty rdf:resource="http://www.wageneder.at/ontology/bpmn2.0#hasSources"/>
                <owl:minQualifiedCardinality rdf:datatype="http://www.w3.org/2001/XMLSchema#nonNegativeInteger">1</owl:minQualifiedCardinality>
                <owl:onClass rdf:resource="http://www.wageneder.at/ontology/bpmn2.0#Element"/>
            </owl:Restriction>
        </rdfs:subClassOf>
        <rdfs:subClassOf>
            <owl:Restriction>
                <owl:onProperty rdf:resource="http://www.wageneder.at/ontology/bpmn2.0#hasTargets"/>
                <owl:minQualifiedCardinality rdf:datatype="http://www.w3.org/2001/XMLSchema#nonNegativeInteger">1</owl:minQualifiedCardinality>
                <owl:onClass rdf:resource="http://www.wageneder.at/ontology/bpmn2.0#Element"/>
            </owl:Restriction>
        </rdfs:subClassOf>
        <rdfs:subClassOf>
            <owl:Restriction>
                <owl:onProperty rdf:resource="http://www.wageneder.at/ontology/bpmn2.0#hasDefinition"/>
                <owl:qualifiedCardinality rdf:datatype="http://www.w3.org/2001/XMLSchema#nonNegativeInteger">1</owl:qualifiedCardinality>
                <owl:onClass rdf:resource="http://www.wageneder.at/ontology/bpmn2.0#Definitions"/>
            </owl:Restriction>
        </rdfs:subClassOf>
        <rdfs:subClassOf>
            <owl:Restriction>
                <owl:onProperty rdf:resource="http://www.wageneder.at/ontology/bpmn2.0#hasDirection"/>
                <owl:qualifiedCardinality rdf:datatype="http://www.w3.org/2001/XMLSchema#nonNegativeInteger">1</owl:qualifiedCardinality>
                <owl:onClass rdf:resource="http://www.wageneder.at/ontology/bpmn2.0#RelationshipDirection"/>
            </owl:Restriction>
        </rdfs:subClassOf>
        <rdfs:subClassOf>
            <owl:Restriction>
                <owl:onProperty rdf:resource="http://www.wageneder.at/ontology/bpmn2.0#type"/>
                <owl:qualifiedCardinality rdf:datatype="http://www.w3.org/2001/XMLSchema#nonNegativeInteger">1</owl:qualifiedCardinality>
                <owl:onDataRange rdf:resource="http://www.w3.org/2001/XMLSchema#string"/>
            </owl:Restriction>
        </rdfs:subClassOf>
        <rdfs:comment>The ‘identity/relationship’ model it is reduced to the creation of families of typed relationships that enable BPMN and non-BPMN Artifacts to be related in non intrusive manner.</rdfs:comment>
    </owl:Class>
    


    <!-- http://www.wageneder.at/ontology/bpmn2.0#RelationshipDirection -->

    <owl:Class rdf:about="http://www.wageneder.at/ontology/bpmn2.0#RelationshipDirection">
        <rdfs:subClassOf rdf:resource="http://www.wageneder.at/ontology/bpmn2.0#Foundation"/>
        <rdfs:subClassOf>
            <owl:Class>
                <owl:unionOf rdf:parseType="Collection">
                    <rdf:Description rdf:about="http://www.wageneder.at/ontology/bpmn2.0#Backward"/>
                    <rdf:Description rdf:about="http://www.wageneder.at/ontology/bpmn2.0#Both"/>
                    <rdf:Description rdf:about="http://www.wageneder.at/ontology/bpmn2.0#Forward"/>
                    <rdf:Description rdf:about="http://www.wageneder.at/ontology/bpmn2.0#None"/>
                </owl:unionOf>
            </owl:Class>
        </rdfs:subClassOf>
        <rdfs:comment>This attribute specifies the direction of the relationship.</rdfs:comment>
    </owl:Class>
    


    <!-- http://www.wageneder.at/ontology/bpmn2.0#Rendering -->

    <owl:Class rdf:about="http://www.wageneder.at/ontology/bpmn2.0#Rendering">
        <rdfs:subClassOf rdf:resource="http://www.wageneder.at/ontology/bpmn2.0#HumanInteractionLevel"/>
        <rdfs:subClassOf>
            <owl:Restriction>
                <owl:onProperty rdf:resource="http://www.wageneder.at/ontology/bpmn2.0#hasUserTask"/>
                <owl:minQualifiedCardinality rdf:datatype="http://www.w3.org/2001/XMLSchema#nonNegativeInteger">0</owl:minQualifiedCardinality>
                <owl:onClass rdf:resource="http://www.wageneder.at/ontology/bpmn2.0#UserTask"/>
            </owl:Restriction>
        </rdfs:subClassOf>
        <rdfs:subClassOf>
            <owl:Restriction>
                <owl:onProperty rdf:resource="http://www.wageneder.at/ontology/bpmn2.0#hasUserTask"/>
                <owl:maxQualifiedCardinality rdf:datatype="http://www.w3.org/2001/XMLSchema#nonNegativeInteger">1</owl:maxQualifiedCardinality>
                <owl:onClass rdf:resource="http://www.wageneder.at/ontology/bpmn2.0#UserTask"/>
            </owl:Restriction>
        </rdfs:subClassOf>
        <rdfs:comment>The Rendering element is the extension point for renderings. Things like language considerations are opaque for the Rendering element because the rendering applications typically provide Multilanguage support.</rdfs:comment>
    </owl:Class>
    


    <!-- http://www.wageneder.at/ontology/bpmn2.0#Resource -->

    <owl:Class rdf:about="http://www.wageneder.at/ontology/bpmn2.0#Resource">
        <rdfs:subClassOf rdf:resource="http://www.wageneder.at/ontology/bpmn2.0#Common"/>
        <rdfs:subClassOf rdf:resource="http://www.wageneder.at/ontology/bpmn2.0#RootElement"/>
        <rdfs:subClassOf>
            <owl:Restriction>
                <owl:onProperty rdf:resource="http://www.wageneder.at/ontology/bpmn2.0#hasResourceParameters"/>
                <owl:minQualifiedCardinality rdf:datatype="http://www.w3.org/2001/XMLSchema#nonNegativeInteger">0</owl:minQualifiedCardinality>
                <owl:onClass rdf:resource="http://www.wageneder.at/ontology/bpmn2.0#ResourceParameter"/>
            </owl:Restriction>
        </rdfs:subClassOf>
        <rdfs:subClassOf>
            <owl:Restriction>
                <owl:onProperty rdf:resource="http://www.wageneder.at/ontology/bpmn2.0#name"/>
                <owl:qualifiedCardinality rdf:datatype="http://www.w3.org/2001/XMLSchema#nonNegativeInteger">1</owl:qualifiedCardinality>
                <owl:onDataRange rdf:resource="http://www.w3.org/2001/XMLSchema#string"/>
            </owl:Restriction>
        </rdfs:subClassOf>
        <rdfs:comment>The Resource class is used to specify resources that can be referenced by Activities. These Resources can be
Human Resources as well as any other resource assigned to Activities during Process execution time.

The definition of a Resource is “abstract,” because it only defines the Resource, without detailing how e.g., actual
user IDs are associated at runtime. Multiple Activities can utilize the same Resource.

Every Resource can define a set of ResourceParameters. These parameters can be used at runtime to define query e.g., into an Organizational Directory. Every Activity referencing a parameterized Resource can bind values available in the scope of the Activity to these parameters.</rdfs:comment>
    </owl:Class>
    


    <!-- http://www.wageneder.at/ontology/bpmn2.0#ResourceAssignmentsExpression -->

    <owl:Class rdf:about="http://www.wageneder.at/ontology/bpmn2.0#ResourceAssignmentsExpression">
        <rdfs:subClassOf rdf:resource="http://www.wageneder.at/ontology/bpmn2.0#ActivityLevel"/>
        <rdfs:subClassOf rdf:resource="http://www.wageneder.at/ontology/bpmn2.0#BaseElement"/>
        <rdfs:subClassOf>
            <owl:Restriction>
                <owl:onProperty rdf:resource="http://www.wageneder.at/ontology/bpmn2.0#hasExpression"/>
                <owl:qualifiedCardinality rdf:datatype="http://www.w3.org/2001/XMLSchema#nonNegativeInteger">1</owl:qualifiedCardinality>
                <owl:onClass rdf:resource="http://www.wageneder.at/ontology/bpmn2.0#Expression"/>
            </owl:Restriction>
        </rdfs:subClassOf>
        <rdfs:comment>The ResourceAssignmentExpression element inherits the attributes and model associations of BaseElement (see Table 8.5). Table 10.6 presents the additional model associations of the ResourceAssignmentExpression element.</rdfs:comment>
    </owl:Class>
    


    <!-- http://www.wageneder.at/ontology/bpmn2.0#ResourceParameter -->

    <owl:Class rdf:about="http://www.wageneder.at/ontology/bpmn2.0#ResourceParameter">
        <rdfs:subClassOf rdf:resource="http://www.wageneder.at/ontology/bpmn2.0#Common"/>
        <rdfs:subClassOf rdf:resource="http://www.wageneder.at/ontology/bpmn2.0#RootElement"/>
        <rdfs:subClassOf>
            <owl:Restriction>
                <owl:onProperty rdf:resource="http://www.wageneder.at/ontology/bpmn2.0#hasType"/>
                <owl:qualifiedCardinality rdf:datatype="http://www.w3.org/2001/XMLSchema#nonNegativeInteger">1</owl:qualifiedCardinality>
                <owl:onClass rdf:resource="http://www.wageneder.at/ontology/bpmn2.0#ItemDefinition"/>
            </owl:Restriction>
        </rdfs:subClassOf>
        <rdfs:subClassOf>
            <owl:Restriction>
                <owl:onProperty rdf:resource="http://www.wageneder.at/ontology/bpmn2.0#isRequired"/>
                <owl:qualifiedCardinality rdf:datatype="http://www.w3.org/2001/XMLSchema#nonNegativeInteger">1</owl:qualifiedCardinality>
                <owl:onDataRange rdf:resource="http://www.w3.org/2001/XMLSchema#boolean"/>
            </owl:Restriction>
        </rdfs:subClassOf>
        <rdfs:subClassOf>
            <owl:Restriction>
                <owl:onProperty rdf:resource="http://www.wageneder.at/ontology/bpmn2.0#name"/>
                <owl:qualifiedCardinality rdf:datatype="http://www.w3.org/2001/XMLSchema#nonNegativeInteger">1</owl:qualifiedCardinality>
                <owl:onDataRange rdf:resource="http://www.w3.org/2001/XMLSchema#string"/>
            </owl:Restriction>
        </rdfs:subClassOf>
        <rdfs:comment>The ResourceParameter element inherits the attributes and model associations of BaseElement (see Table 8.5) through its relationship to RootElement. Table 8.51 presents the additional model associations for the ResourceParameter element.</rdfs:comment>
    </owl:Class>
    


    <!-- http://www.wageneder.at/ontology/bpmn2.0#ResourceParameterBinding -->

    <owl:Class rdf:about="http://www.wageneder.at/ontology/bpmn2.0#ResourceParameterBinding">
        <rdfs:subClassOf rdf:resource="http://www.wageneder.at/ontology/bpmn2.0#ActivityLevel"/>
        <rdfs:subClassOf rdf:resource="http://www.wageneder.at/ontology/bpmn2.0#BaseElement"/>
        <rdfs:subClassOf>
            <owl:Restriction>
                <owl:onProperty rdf:resource="http://www.wageneder.at/ontology/bpmn2.0#hasExpression"/>
                <owl:qualifiedCardinality rdf:datatype="http://www.w3.org/2001/XMLSchema#nonNegativeInteger">1</owl:qualifiedCardinality>
                <owl:onClass rdf:resource="http://www.wageneder.at/ontology/bpmn2.0#Expression"/>
            </owl:Restriction>
        </rdfs:subClassOf>
        <rdfs:subClassOf>
            <owl:Restriction>
                <owl:onProperty rdf:resource="http://www.wageneder.at/ontology/bpmn2.0#hasParameterRef"/>
                <owl:qualifiedCardinality rdf:datatype="http://www.w3.org/2001/XMLSchema#nonNegativeInteger">1</owl:qualifiedCardinality>
                <owl:onClass rdf:resource="http://www.wageneder.at/ontology/bpmn2.0#ResourceParameter"/>
            </owl:Restriction>
        </rdfs:subClassOf>
        <rdfs:comment>The ResourceParameterBinding element inherits the attributes and model associations of BaseElement (see Table 8.5). Table 10.7 presents the additional model associations of the ResourceParameterBinding element.</rdfs:comment>
    </owl:Class>
    


    <!-- http://www.wageneder.at/ontology/bpmn2.0#ResourceRole -->

    <owl:Class rdf:about="http://www.wageneder.at/ontology/bpmn2.0#ResourceRole">
        <rdfs:subClassOf rdf:resource="http://www.wageneder.at/ontology/bpmn2.0#ActivityLevel"/>
        <rdfs:subClassOf rdf:resource="http://www.wageneder.at/ontology/bpmn2.0#BaseElement"/>
        <rdfs:subClassOf>
            <owl:Restriction>
                <owl:onProperty rdf:resource="http://www.wageneder.at/ontology/bpmn2.0#hasResourceAssignmentExpression"/>
                <owl:minQualifiedCardinality rdf:datatype="http://www.w3.org/2001/XMLSchema#nonNegativeInteger">0</owl:minQualifiedCardinality>
                <owl:onClass rdf:resource="http://www.wageneder.at/ontology/bpmn2.0#ResourceAssignmentsExpression"/>
            </owl:Restriction>
        </rdfs:subClassOf>
        <rdfs:subClassOf>
            <owl:Restriction>
                <owl:onProperty rdf:resource="http://www.wageneder.at/ontology/bpmn2.0#hasResourceParameterBindings"/>
                <owl:minQualifiedCardinality rdf:datatype="http://www.w3.org/2001/XMLSchema#nonNegativeInteger">0</owl:minQualifiedCardinality>
                <owl:onClass rdf:resource="http://www.wageneder.at/ontology/bpmn2.0#ResourceParameterBinding"/>
            </owl:Restriction>
        </rdfs:subClassOf>
        <rdfs:subClassOf>
            <owl:Restriction>
                <owl:onProperty rdf:resource="http://www.wageneder.at/ontology/bpmn2.0#hasResourceRef"/>
                <owl:minQualifiedCardinality rdf:datatype="http://www.w3.org/2001/XMLSchema#nonNegativeInteger">0</owl:minQualifiedCardinality>
                <owl:onClass rdf:resource="http://www.wageneder.at/ontology/bpmn2.0#Resource"/>
            </owl:Restriction>
        </rdfs:subClassOf>
        <rdfs:subClassOf>
            <owl:Restriction>
                <owl:onProperty rdf:resource="http://www.wageneder.at/ontology/bpmn2.0#hasProcess"/>
                <owl:qualifiedCardinality rdf:datatype="http://www.w3.org/2001/XMLSchema#nonNegativeInteger">1</owl:qualifiedCardinality>
                <owl:onClass rdf:resource="http://www.wageneder.at/ontology/bpmn2.0#Process"/>
            </owl:Restriction>
        </rdfs:subClassOf>
        <rdfs:subClassOf>
            <owl:Restriction>
                <owl:onProperty rdf:resource="http://www.wageneder.at/ontology/bpmn2.0#hasResourceAssignmentExpression"/>
                <owl:maxQualifiedCardinality rdf:datatype="http://www.w3.org/2001/XMLSchema#nonNegativeInteger">1</owl:maxQualifiedCardinality>
                <owl:onClass rdf:resource="http://www.wageneder.at/ontology/bpmn2.0#ResourceAssignmentsExpression"/>
            </owl:Restriction>
        </rdfs:subClassOf>
        <rdfs:subClassOf>
            <owl:Restriction>
                <owl:onProperty rdf:resource="http://www.wageneder.at/ontology/bpmn2.0#hasResourceRef"/>
                <owl:maxQualifiedCardinality rdf:datatype="http://www.w3.org/2001/XMLSchema#nonNegativeInteger">1</owl:maxQualifiedCardinality>
                <owl:onClass rdf:resource="http://www.wageneder.at/ontology/bpmn2.0#Resource"/>
            </owl:Restriction>
        </rdfs:subClassOf>
        <rdfs:subClassOf>
            <owl:Restriction>
                <owl:onProperty rdf:resource="http://www.wageneder.at/ontology/bpmn2.0#name"/>
                <owl:minQualifiedCardinality rdf:datatype="http://www.w3.org/2001/XMLSchema#nonNegativeInteger">0</owl:minQualifiedCardinality>
                <owl:onDataRange rdf:resource="http://www.w3.org/2001/XMLSchema#string"/>
            </owl:Restriction>
        </rdfs:subClassOf>
        <rdfs:subClassOf>
            <owl:Restriction>
                <owl:onProperty rdf:resource="http://www.wageneder.at/ontology/bpmn2.0#name"/>
                <owl:maxQualifiedCardinality rdf:datatype="http://www.w3.org/2001/XMLSchema#nonNegativeInteger">1</owl:maxQualifiedCardinality>
                <owl:onDataRange rdf:resource="http://www.w3.org/2001/XMLSchema#string"/>
            </owl:Restriction>
        </rdfs:subClassOf>
        <rdfs:comment>The ResourceRole element inherits the attributes and model associations of BaseElement</rdfs:comment>
    </owl:Class>
    


    <!-- http://www.wageneder.at/ontology/bpmn2.0#RootElement -->

    <owl:Class rdf:about="http://www.wageneder.at/ontology/bpmn2.0#RootElement">
        <rdfs:subClassOf rdf:resource="http://www.wageneder.at/ontology/bpmn2.0#BaseElement"/>
        <rdfs:subClassOf>
            <owl:Restriction>
                <owl:onProperty rdf:resource="http://www.wageneder.at/ontology/bpmn2.0#hasDefinition"/>
                <owl:minQualifiedCardinality rdf:datatype="http://www.w3.org/2001/XMLSchema#nonNegativeInteger">0</owl:minQualifiedCardinality>
                <owl:onClass rdf:resource="http://www.wageneder.at/ontology/bpmn2.0#Definitions"/>
            </owl:Restriction>
        </rdfs:subClassOf>
        <rdfs:subClassOf>
            <owl:Restriction>
                <owl:onProperty rdf:resource="http://www.wageneder.at/ontology/bpmn2.0#hasDefinition"/>
                <owl:maxQualifiedCardinality rdf:datatype="http://www.w3.org/2001/XMLSchema#nonNegativeInteger">1</owl:maxQualifiedCardinality>
                <owl:onClass rdf:resource="http://www.wageneder.at/ontology/bpmn2.0#Definitions"/>
            </owl:Restriction>
        </rdfs:subClassOf>
        <rdfs:comment>RootElement is the abstract super class for all BPMN elements that are contained within Definitions.</rdfs:comment>
    </owl:Class>
    


    <!-- http://www.wageneder.at/ontology/bpmn2.0#ScriptTask -->

    <owl:Class rdf:about="http://www.wageneder.at/ontology/bpmn2.0#ScriptTask">
        <rdfs:subClassOf rdf:resource="http://www.wageneder.at/ontology/bpmn2.0#Task"/>
        <rdfs:subClassOf>
            <owl:Restriction>
                <owl:onProperty rdf:resource="http://www.wageneder.at/ontology/bpmn2.0#script"/>
                <owl:minQualifiedCardinality rdf:datatype="http://www.w3.org/2001/XMLSchema#nonNegativeInteger">0</owl:minQualifiedCardinality>
                <owl:onDataRange rdf:resource="http://www.w3.org/2001/XMLSchema#string"/>
            </owl:Restriction>
        </rdfs:subClassOf>
        <rdfs:subClassOf>
            <owl:Restriction>
                <owl:onProperty rdf:resource="http://www.wageneder.at/ontology/bpmn2.0#scriptFormat"/>
                <owl:minQualifiedCardinality rdf:datatype="http://www.w3.org/2001/XMLSchema#nonNegativeInteger">0</owl:minQualifiedCardinality>
                <owl:onDataRange rdf:resource="http://www.w3.org/2001/XMLSchema#string"/>
            </owl:Restriction>
        </rdfs:subClassOf>
        <rdfs:subClassOf>
            <owl:Restriction>
                <owl:onProperty rdf:resource="http://www.wageneder.at/ontology/bpmn2.0#script"/>
                <owl:maxQualifiedCardinality rdf:datatype="http://www.w3.org/2001/XMLSchema#nonNegativeInteger">1</owl:maxQualifiedCardinality>
                <owl:onDataRange rdf:resource="http://www.w3.org/2001/XMLSchema#string"/>
            </owl:Restriction>
        </rdfs:subClassOf>
        <rdfs:subClassOf>
            <owl:Restriction>
                <owl:onProperty rdf:resource="http://www.wageneder.at/ontology/bpmn2.0#scriptFormat"/>
                <owl:maxQualifiedCardinality rdf:datatype="http://www.w3.org/2001/XMLSchema#nonNegativeInteger">1</owl:maxQualifiedCardinality>
                <owl:onDataRange rdf:resource="http://www.w3.org/2001/XMLSchema#string"/>
            </owl:Restriction>
        </rdfs:subClassOf>
        <rdfs:comment>A Script Task is executed by a business process engine. The modeler or implementer defines a script in a language that the engine can interpret. When the Task is ready to start, the engine will execute the script. When the script is completed, the Task will also be completed.</rdfs:comment>
    </owl:Class>
    


    <!-- http://www.wageneder.at/ontology/bpmn2.0#SendTask -->

    <owl:Class rdf:about="http://www.wageneder.at/ontology/bpmn2.0#SendTask">
        <rdfs:subClassOf rdf:resource="http://www.wageneder.at/ontology/bpmn2.0#Task"/>
        <rdfs:subClassOf>
            <owl:Restriction>
                <owl:onProperty rdf:resource="http://www.wageneder.at/ontology/bpmn2.0#hasMessageRef"/>
                <owl:minQualifiedCardinality rdf:datatype="http://www.w3.org/2001/XMLSchema#nonNegativeInteger">0</owl:minQualifiedCardinality>
                <owl:onClass rdf:resource="http://www.wageneder.at/ontology/bpmn2.0#Message"/>
            </owl:Restriction>
        </rdfs:subClassOf>
        <rdfs:subClassOf>
            <owl:Restriction>
                <owl:onProperty rdf:resource="http://www.wageneder.at/ontology/bpmn2.0#hasOperationRef"/>
                <owl:qualifiedCardinality rdf:datatype="http://www.w3.org/2001/XMLSchema#nonNegativeInteger">1</owl:qualifiedCardinality>
                <owl:onClass rdf:resource="http://www.wageneder.at/ontology/bpmn2.0#Operation"/>
            </owl:Restriction>
        </rdfs:subClassOf>
        <rdfs:subClassOf>
            <owl:Restriction>
                <owl:onProperty rdf:resource="http://www.wageneder.at/ontology/bpmn2.0#hasMessageRef"/>
                <owl:maxQualifiedCardinality rdf:datatype="http://www.w3.org/2001/XMLSchema#nonNegativeInteger">1</owl:maxQualifiedCardinality>
                <owl:onClass rdf:resource="http://www.wageneder.at/ontology/bpmn2.0#Message"/>
            </owl:Restriction>
        </rdfs:subClassOf>
        <rdfs:subClassOf>
            <owl:Restriction>
                <owl:onProperty rdf:resource="http://www.wageneder.at/ontology/bpmn2.0#implementation"/>
                <owl:qualifiedCardinality rdf:datatype="http://www.w3.org/2001/XMLSchema#nonNegativeInteger">1</owl:qualifiedCardinality>
                <owl:onDataRange rdf:resource="http://www.w3.org/2001/XMLSchema#string"/>
            </owl:Restriction>
        </rdfs:subClassOf>
        <rdfs:comment>A Send Task is a simple Task that is designed to send a Message to an external Participant (relative to the
Process). Once the Message has been sent, the Task is completed.</rdfs:comment>
    </owl:Class>
    


    <!-- http://www.wageneder.at/ontology/bpmn2.0#SequenceFlow -->

    <owl:Class rdf:about="http://www.wageneder.at/ontology/bpmn2.0#SequenceFlow">
        <rdfs:subClassOf rdf:resource="http://www.wageneder.at/ontology/bpmn2.0#Common"/>
        <rdfs:subClassOf rdf:resource="http://www.wageneder.at/ontology/bpmn2.0#FlowElement"/>
        <rdfs:subClassOf>
            <owl:Restriction>
                <owl:onProperty rdf:resource="http://www.wageneder.at/ontology/bpmn2.0#hasComplexGateway"/>
                <owl:minQualifiedCardinality rdf:datatype="http://www.w3.org/2001/XMLSchema#nonNegativeInteger">0</owl:minQualifiedCardinality>
                <owl:onClass rdf:resource="http://www.wageneder.at/ontology/bpmn2.0#ComplexGateway"/>
            </owl:Restriction>
        </rdfs:subClassOf>
        <rdfs:subClassOf>
            <owl:Restriction>
                <owl:onProperty rdf:resource="http://www.wageneder.at/ontology/bpmn2.0#hasConditionExpression"/>
                <owl:minQualifiedCardinality rdf:datatype="http://www.w3.org/2001/XMLSchema#nonNegativeInteger">0</owl:minQualifiedCardinality>
                <owl:onClass rdf:resource="http://www.wageneder.at/ontology/bpmn2.0#Expression"/>
            </owl:Restriction>
        </rdfs:subClassOf>
        <rdfs:subClassOf>
            <owl:Restriction>
                <owl:onProperty rdf:resource="http://www.wageneder.at/ontology/bpmn2.0#hasExclusiceGateway"/>
                <owl:minQualifiedCardinality rdf:datatype="http://www.w3.org/2001/XMLSchema#nonNegativeInteger">0</owl:minQualifiedCardinality>
                <owl:onClass rdf:resource="http://www.wageneder.at/ontology/bpmn2.0#ExclusiveGateway"/>
            </owl:Restriction>
        </rdfs:subClassOf>
        <rdfs:subClassOf>
            <owl:Restriction>
                <owl:onProperty rdf:resource="http://www.wageneder.at/ontology/bpmn2.0#hasInclusiveGateway"/>
                <owl:minQualifiedCardinality rdf:datatype="http://www.w3.org/2001/XMLSchema#nonNegativeInteger">0</owl:minQualifiedCardinality>
                <owl:onClass rdf:resource="http://www.wageneder.at/ontology/bpmn2.0#InclusiveGateway"/>
            </owl:Restriction>
        </rdfs:subClassOf>
        <rdfs:subClassOf>
            <owl:Restriction>
                <owl:onProperty rdf:resource="http://www.wageneder.at/ontology/bpmn2.0#hasActivity"/>
                <owl:qualifiedCardinality rdf:datatype="http://www.w3.org/2001/XMLSchema#nonNegativeInteger">1</owl:qualifiedCardinality>
                <owl:onClass rdf:resource="http://www.wageneder.at/ontology/bpmn2.0#Activity"/>
            </owl:Restriction>
        </rdfs:subClassOf>
        <rdfs:subClassOf>
            <owl:Restriction>
                <owl:onProperty rdf:resource="http://www.wageneder.at/ontology/bpmn2.0#hasSourceRef"/>
                <owl:qualifiedCardinality rdf:datatype="http://www.w3.org/2001/XMLSchema#nonNegativeInteger">1</owl:qualifiedCardinality>
                <owl:onClass rdf:resource="http://www.wageneder.at/ontology/bpmn2.0#FlowNode"/>
            </owl:Restriction>
        </rdfs:subClassOf>
        <rdfs:subClassOf>
            <owl:Restriction>
                <owl:onProperty rdf:resource="http://www.wageneder.at/ontology/bpmn2.0#hasTargetRef"/>
                <owl:qualifiedCardinality rdf:datatype="http://www.w3.org/2001/XMLSchema#nonNegativeInteger">1</owl:qualifiedCardinality>
                <owl:onClass rdf:resource="http://www.wageneder.at/ontology/bpmn2.0#FlowNode"/>
            </owl:Restriction>
        </rdfs:subClassOf>
        <rdfs:subClassOf>
            <owl:Restriction>
                <owl:onProperty rdf:resource="http://www.wageneder.at/ontology/bpmn2.0#hasConditionExpression"/>
                <owl:maxQualifiedCardinality rdf:datatype="http://www.w3.org/2001/XMLSchema#nonNegativeInteger">1</owl:maxQualifiedCardinality>
                <owl:onClass rdf:resource="http://www.wageneder.at/ontology/bpmn2.0#Expression"/>
            </owl:Restriction>
        </rdfs:subClassOf>
        <rdfs:subClassOf>
            <owl:Restriction>
                <owl:onProperty rdf:resource="http://www.wageneder.at/ontology/bpmn2.0#isImmediate"/>
                <owl:minQualifiedCardinality rdf:datatype="http://www.w3.org/2001/XMLSchema#nonNegativeInteger">0</owl:minQualifiedCardinality>
                <owl:onDataRange rdf:resource="http://www.w3.org/2001/XMLSchema#boolean"/>
            </owl:Restriction>
        </rdfs:subClassOf>
        <rdfs:subClassOf>
            <owl:Restriction>
                <owl:onProperty rdf:resource="http://www.wageneder.at/ontology/bpmn2.0#isImmediate"/>
                <owl:maxQualifiedCardinality rdf:datatype="http://www.w3.org/2001/XMLSchema#nonNegativeInteger">1</owl:maxQualifiedCardinality>
                <owl:onDataRange rdf:resource="http://www.w3.org/2001/XMLSchema#boolean"/>
            </owl:Restriction>
        </rdfs:subClassOf>
        <rdfs:comment>A Sequence Flow is used to show the order of Flow Elements in a Process or a Choreography. Each Sequence Flow has only one source and only one target.</rdfs:comment>
    </owl:Class>
    


    <!-- http://www.wageneder.at/ontology/bpmn2.0#Sequential -->

    <owl:Class rdf:about="http://www.wageneder.at/ontology/bpmn2.0#Sequential">
        <rdfs:subClassOf rdf:resource="http://www.wageneder.at/ontology/bpmn2.0#AdHocOrdering"/>
    </owl:Class>
    


    <!-- http://www.wageneder.at/ontology/bpmn2.0#Service -->

    <owl:Class rdf:about="http://www.wageneder.at/ontology/bpmn2.0#Service">
        <rdfs:subClassOf rdf:resource="http://www.wageneder.at/ontology/bpmn2.0#BPMNCore"/>
        <rdfs:comment>This is just a hierarchical element for organisational purposes.</rdfs:comment>
    </owl:Class>
    


    <!-- http://www.wageneder.at/ontology/bpmn2.0#ServiceTask -->

    <owl:Class rdf:about="http://www.wageneder.at/ontology/bpmn2.0#ServiceTask">
        <rdfs:subClassOf rdf:resource="http://www.wageneder.at/ontology/bpmn2.0#Task"/>
        <rdfs:subClassOf>
            <owl:Restriction>
                <owl:onProperty rdf:resource="http://www.wageneder.at/ontology/bpmn2.0#hasOperationRef"/>
                <owl:minQualifiedCardinality rdf:datatype="http://www.w3.org/2001/XMLSchema#nonNegativeInteger">0</owl:minQualifiedCardinality>
                <owl:onClass rdf:resource="http://www.wageneder.at/ontology/bpmn2.0#Operation"/>
            </owl:Restriction>
        </rdfs:subClassOf>
        <rdfs:subClassOf>
            <owl:Restriction>
                <owl:onProperty rdf:resource="http://www.wageneder.at/ontology/bpmn2.0#hasOperationRef"/>
                <owl:maxQualifiedCardinality rdf:datatype="http://www.w3.org/2001/XMLSchema#nonNegativeInteger">1</owl:maxQualifiedCardinality>
                <owl:onClass rdf:resource="http://www.wageneder.at/ontology/bpmn2.0#Operation"/>
            </owl:Restriction>
        </rdfs:subClassOf>
        <rdfs:subClassOf>
            <owl:Restriction>
                <owl:onProperty rdf:resource="http://www.wageneder.at/ontology/bpmn2.0#implementation"/>
                <owl:qualifiedCardinality rdf:datatype="http://www.w3.org/2001/XMLSchema#nonNegativeInteger">1</owl:qualifiedCardinality>
                <owl:onDataRange rdf:resource="http://www.w3.org/2001/XMLSchema#string"/>
            </owl:Restriction>
        </rdfs:subClassOf>
        <rdfs:comment>A Service Task is a Task that uses some sort of service, which could be a Web service or an automated application.</rdfs:comment>
    </owl:Class>
    


    <!-- http://www.wageneder.at/ontology/bpmn2.0#Signal -->

    <owl:Class rdf:about="http://www.wageneder.at/ontology/bpmn2.0#Signal">
        <rdfs:subClassOf rdf:resource="http://www.wageneder.at/ontology/bpmn2.0#EventLevel"/>
        <rdfs:subClassOf>
            <owl:Restriction>
                <owl:onProperty rdf:resource="http://www.wageneder.at/ontology/bpmn2.0#hasStructureRef"/>
                <owl:minQualifiedCardinality rdf:datatype="http://www.w3.org/2001/XMLSchema#nonNegativeInteger">0</owl:minQualifiedCardinality>
                <owl:onClass rdf:resource="http://www.wageneder.at/ontology/bpmn2.0#ItemDefinition"/>
            </owl:Restriction>
        </rdfs:subClassOf>
        <rdfs:subClassOf>
            <owl:Restriction>
                <owl:onProperty rdf:resource="http://www.wageneder.at/ontology/bpmn2.0#hasStructureRef"/>
                <owl:maxQualifiedCardinality rdf:datatype="http://www.w3.org/2001/XMLSchema#nonNegativeInteger">1</owl:maxQualifiedCardinality>
                <owl:onClass rdf:resource="http://www.wageneder.at/ontology/bpmn2.0#ItemDefinition"/>
            </owl:Restriction>
        </rdfs:subClassOf>
        <rdfs:subClassOf>
            <owl:Restriction>
                <owl:onProperty rdf:resource="http://www.wageneder.at/ontology/bpmn2.0#name"/>
                <owl:minQualifiedCardinality rdf:datatype="http://www.w3.org/2001/XMLSchema#nonNegativeInteger">0</owl:minQualifiedCardinality>
                <owl:onDataRange rdf:resource="http://www.w3.org/2001/XMLSchema#string"/>
            </owl:Restriction>
        </rdfs:subClassOf>
        <rdfs:subClassOf>
            <owl:Restriction>
                <owl:onProperty rdf:resource="http://www.wageneder.at/ontology/bpmn2.0#name"/>
                <owl:maxQualifiedCardinality rdf:datatype="http://www.w3.org/2001/XMLSchema#nonNegativeInteger">1</owl:maxQualifiedCardinality>
                <owl:onDataRange rdf:resource="http://www.w3.org/2001/XMLSchema#string"/>
            </owl:Restriction>
        </rdfs:subClassOf>
    </owl:Class>
    


    <!-- http://www.wageneder.at/ontology/bpmn2.0#SignalEventDefinition -->

    <owl:Class rdf:about="http://www.wageneder.at/ontology/bpmn2.0#SignalEventDefinition">
        <rdfs:subClassOf rdf:resource="http://www.wageneder.at/ontology/bpmn2.0#EventDefinition"/>
        <rdfs:subClassOf>
            <owl:Restriction>
                <owl:onProperty rdf:resource="http://www.wageneder.at/ontology/bpmn2.0#hasSignalRef"/>
                <owl:minQualifiedCardinality rdf:datatype="http://www.w3.org/2001/XMLSchema#nonNegativeInteger">0</owl:minQualifiedCardinality>
                <owl:onClass rdf:resource="http://www.wageneder.at/ontology/bpmn2.0#Signal"/>
            </owl:Restriction>
        </rdfs:subClassOf>
        <rdfs:subClassOf>
            <owl:Restriction>
                <owl:onProperty rdf:resource="http://www.wageneder.at/ontology/bpmn2.0#hasSignalRef"/>
                <owl:maxQualifiedCardinality rdf:datatype="http://www.w3.org/2001/XMLSchema#nonNegativeInteger">1</owl:maxQualifiedCardinality>
                <owl:onClass rdf:resource="http://www.wageneder.at/ontology/bpmn2.0#Signal"/>
            </owl:Restriction>
        </rdfs:subClassOf>
        <rdfs:comment>The SignalEventDefinition element inherits the attributes and model associations of BaseElement through its relationship to the EventDefinition element</rdfs:comment>
    </owl:Class>
    


    <!-- http://www.wageneder.at/ontology/bpmn2.0#StandardLoopCharacteristics -->

    <owl:Class rdf:about="http://www.wageneder.at/ontology/bpmn2.0#StandardLoopCharacteristics">
        <rdfs:subClassOf rdf:resource="http://www.wageneder.at/ontology/bpmn2.0#LoopCharacteristics"/>
        <rdfs:subClassOf>
            <owl:Restriction>
                <owl:onProperty rdf:resource="http://www.wageneder.at/ontology/bpmn2.0#hasLoopCondition"/>
                <owl:minQualifiedCardinality rdf:datatype="http://www.w3.org/2001/XMLSchema#nonNegativeInteger">0</owl:minQualifiedCardinality>
                <owl:onClass rdf:resource="http://www.wageneder.at/ontology/bpmn2.0#Expression"/>
            </owl:Restriction>
        </rdfs:subClassOf>
        <rdfs:subClassOf>
            <owl:Restriction>
                <owl:onProperty rdf:resource="http://www.wageneder.at/ontology/bpmn2.0#hasLoopCondition"/>
                <owl:maxQualifiedCardinality rdf:datatype="http://www.w3.org/2001/XMLSchema#nonNegativeInteger">1</owl:maxQualifiedCardinality>
                <owl:onClass rdf:resource="http://www.wageneder.at/ontology/bpmn2.0#Expression"/>
            </owl:Restriction>
        </rdfs:subClassOf>
        <rdfs:subClassOf>
            <owl:Restriction>
                <owl:onProperty rdf:resource="http://www.wageneder.at/ontology/bpmn2.0#loopMaximum"/>
                <owl:minQualifiedCardinality rdf:datatype="http://www.w3.org/2001/XMLSchema#nonNegativeInteger">0</owl:minQualifiedCardinality>
                <owl:onDataRange rdf:resource="http://www.w3.org/2001/XMLSchema#integer"/>
            </owl:Restriction>
        </rdfs:subClassOf>
        <rdfs:subClassOf>
            <owl:Restriction>
                <owl:onProperty rdf:resource="http://www.wageneder.at/ontology/bpmn2.0#testBefore"/>
                <owl:qualifiedCardinality rdf:datatype="http://www.w3.org/2001/XMLSchema#nonNegativeInteger">1</owl:qualifiedCardinality>
                <owl:onDataRange rdf:resource="http://www.w3.org/2001/XMLSchema#boolean"/>
            </owl:Restriction>
        </rdfs:subClassOf>
        <rdfs:subClassOf>
            <owl:Restriction>
                <owl:onProperty rdf:resource="http://www.wageneder.at/ontology/bpmn2.0#loopMaximum"/>
                <owl:maxQualifiedCardinality rdf:datatype="http://www.w3.org/2001/XMLSchema#nonNegativeInteger">1</owl:maxQualifiedCardinality>
                <owl:onDataRange rdf:resource="http://www.w3.org/2001/XMLSchema#integer"/>
            </owl:Restriction>
        </rdfs:subClassOf>
        <rdfs:comment>The StandardLoopCharacteristics element inherits the attributes and model associations of BaseElement (see Figure 8.5), through its relationship to LoopCharacteristics. Table 10.28 presents the additional attributes and model associations for the StandardLoopCharacteristics element.</rdfs:comment>
    </owl:Class>
    


    <!-- http://www.wageneder.at/ontology/bpmn2.0#StartEvent -->

    <owl:Class rdf:about="http://www.wageneder.at/ontology/bpmn2.0#StartEvent">
        <rdfs:subClassOf rdf:resource="http://www.wageneder.at/ontology/bpmn2.0#CatchEvent"/>
        <rdfs:subClassOf>
            <owl:Restriction>
                <owl:onProperty rdf:resource="http://www.wageneder.at/ontology/bpmn2.0#isInterrupting"/>
                <owl:qualifiedCardinality rdf:datatype="http://www.w3.org/2001/XMLSchema#nonNegativeInteger">1</owl:qualifiedCardinality>
                <owl:onDataRange rdf:resource="http://www.w3.org/2001/XMLSchema#boolean"/>
            </owl:Restriction>
        </rdfs:subClassOf>
        <rdfs:comment>As the name implies, the Start Event indicates where a particular Process will start. In terms of Sequence Flows, the Start Event starts the flow of the Process, and thus, will not have any incoming Sequence Flows—no Sequence Flow can connect to a Start Event.</rdfs:comment>
    </owl:Class>
    


    <!-- http://www.wageneder.at/ontology/bpmn2.0#SubConversation -->

    <owl:Class rdf:about="http://www.wageneder.at/ontology/bpmn2.0#SubConversation">
        <rdfs:subClassOf rdf:resource="http://www.wageneder.at/ontology/bpmn2.0#ConversationNode"/>
        <rdfs:subClassOf>
            <owl:Restriction>
                <owl:onProperty rdf:resource="http://www.wageneder.at/ontology/bpmn2.0#hasConversationNodes"/>
                <owl:minQualifiedCardinality rdf:datatype="http://www.w3.org/2001/XMLSchema#nonNegativeInteger">0</owl:minQualifiedCardinality>
                <owl:onClass rdf:resource="http://www.wageneder.at/ontology/bpmn2.0#ConversationNode"/>
            </owl:Restriction>
        </rdfs:subClassOf>
        <rdfs:comment>The Sub-Conversation element inherits the attributes and model associations of ConversationNode (see Table 9.10). Table 9.11 presents the additional model associations for the Sub-Conversation element.</rdfs:comment>
    </owl:Class>
    


    <!-- http://www.wageneder.at/ontology/bpmn2.0#SubProcess -->

    <owl:Class rdf:about="http://www.wageneder.at/ontology/bpmn2.0#SubProcess">
        <rdfs:subClassOf rdf:resource="http://www.wageneder.at/ontology/bpmn2.0#Activity"/>
        <rdfs:subClassOf rdf:resource="http://www.wageneder.at/ontology/bpmn2.0#FlowElementsContainer"/>
        <rdfs:subClassOf>
            <owl:Restriction>
                <owl:onProperty rdf:resource="http://www.wageneder.at/ontology/bpmn2.0#hasArtifacts"/>
                <owl:minQualifiedCardinality rdf:datatype="http://www.w3.org/2001/XMLSchema#nonNegativeInteger">0</owl:minQualifiedCardinality>
                <owl:onClass rdf:resource="http://www.wageneder.at/ontology/bpmn2.0#Artifact"/>
            </owl:Restriction>
        </rdfs:subClassOf>
        <rdfs:subClassOf>
            <owl:Restriction>
                <owl:onProperty rdf:resource="http://www.wageneder.at/ontology/bpmn2.0#triggeredByEvent"/>
                <owl:qualifiedCardinality rdf:datatype="http://www.w3.org/2001/XMLSchema#nonNegativeInteger">1</owl:qualifiedCardinality>
                <owl:onDataRange rdf:resource="http://www.w3.org/2001/XMLSchema#boolean"/>
            </owl:Restriction>
        </rdfs:subClassOf>
        <rdfs:comment>A Sub-Process is an Activity whose internal details have been modeled using Activities, Gateways, Events, and Sequence Flows. A Sub-Process is a graphical object within a Process, but it also can be “opened up” to show a lower-level Process. Sub-Processes define a contextual scope that can be used for attribute visibility, transactional scope, for the handling of exceptions (see page 275 for more details), of Events, or for compensation (see page 302 for more details).</rdfs:comment>
    </owl:Class>
    


    <!-- http://www.wageneder.at/ontology/bpmn2.0#Task -->

    <owl:Class rdf:about="http://www.wageneder.at/ontology/bpmn2.0#Task">
        <rdfs:subClassOf rdf:resource="http://www.wageneder.at/ontology/bpmn2.0#Activity"/>
        <rdfs:subClassOf rdf:resource="http://www.wageneder.at/ontology/bpmn2.0#InteractionNode"/>
        <rdfs:comment>A Task is an atomic Activity within a Process flow. A Task is used when the work in the Process cannot be broken down to a finer level of detail. Generally, an end-user and/or applications are used to perform the Task when it is executed.</rdfs:comment>
    </owl:Class>
    


    <!-- http://www.wageneder.at/ontology/bpmn2.0#TerminateEventDefinition -->

    <owl:Class rdf:about="http://www.wageneder.at/ontology/bpmn2.0#TerminateEventDefinition">
        <rdfs:subClassOf rdf:resource="http://www.wageneder.at/ontology/bpmn2.0#EventDefinition"/>
        <rdfs:comment>The MessageEventDefinition element inherits the attributes and model associations of BaseElement  through its relationship to the EventDefinition element</rdfs:comment>
    </owl:Class>
    


    <!-- http://www.wageneder.at/ontology/bpmn2.0#TextAnnotation -->

    <owl:Class rdf:about="http://www.wageneder.at/ontology/bpmn2.0#TextAnnotation">
        <rdfs:subClassOf rdf:resource="http://www.wageneder.at/ontology/bpmn2.0#Artifact"/>
        <rdfs:subClassOf>
            <owl:Restriction>
                <owl:onProperty rdf:resource="http://www.wageneder.at/ontology/bpmn2.0#text"/>
                <owl:qualifiedCardinality rdf:datatype="http://www.w3.org/2001/XMLSchema#nonNegativeInteger">1</owl:qualifiedCardinality>
                <owl:onDataRange rdf:resource="http://www.w3.org/2001/XMLSchema#string"/>
            </owl:Restriction>
        </rdfs:subClassOf>
        <rdfs:subClassOf>
            <owl:Restriction>
                <owl:onProperty rdf:resource="http://www.wageneder.at/ontology/bpmn2.0#textFormat"/>
                <owl:qualifiedCardinality rdf:datatype="http://www.w3.org/2001/XMLSchema#nonNegativeInteger">1</owl:qualifiedCardinality>
                <owl:onDataRange rdf:resource="http://www.w3.org/2001/XMLSchema#string"/>
            </owl:Restriction>
        </rdfs:subClassOf>
        <rdfs:comment>Text Annotations are a mechanism for a modeler to provide additional information for the reader of a BPMN Diagram.</rdfs:comment>
    </owl:Class>
    


    <!-- http://www.wageneder.at/ontology/bpmn2.0#ThrowEvent -->

    <owl:Class rdf:about="http://www.wageneder.at/ontology/bpmn2.0#ThrowEvent">
        <rdfs:subClassOf rdf:resource="http://www.wageneder.at/ontology/bpmn2.0#Event"/>
        <rdfs:subClassOf>
            <owl:Restriction>
                <owl:onProperty rdf:resource="http://www.wageneder.at/ontology/bpmn2.0#hasDataInputAssociations"/>
                <owl:minQualifiedCardinality rdf:datatype="http://www.w3.org/2001/XMLSchema#nonNegativeInteger">0</owl:minQualifiedCardinality>
                <owl:onClass rdf:resource="http://www.wageneder.at/ontology/bpmn2.0#DataInputAssociation"/>
            </owl:Restriction>
        </rdfs:subClassOf>
        <rdfs:subClassOf>
            <owl:Restriction>
                <owl:onProperty rdf:resource="http://www.wageneder.at/ontology/bpmn2.0#hasDataInputs"/>
                <owl:minQualifiedCardinality rdf:datatype="http://www.w3.org/2001/XMLSchema#nonNegativeInteger">0</owl:minQualifiedCardinality>
                <owl:onClass rdf:resource="http://www.wageneder.at/ontology/bpmn2.0#DataInput"/>
            </owl:Restriction>
        </rdfs:subClassOf>
        <rdfs:subClassOf>
            <owl:Restriction>
                <owl:onProperty rdf:resource="http://www.wageneder.at/ontology/bpmn2.0#hasEventDefinitionRefs"/>
                <owl:minQualifiedCardinality rdf:datatype="http://www.w3.org/2001/XMLSchema#nonNegativeInteger">0</owl:minQualifiedCardinality>
                <owl:onClass rdf:resource="http://www.wageneder.at/ontology/bpmn2.0#EventDefinition"/>
            </owl:Restriction>
        </rdfs:subClassOf>
        <rdfs:subClassOf>
            <owl:Restriction>
                <owl:onProperty rdf:resource="http://www.wageneder.at/ontology/bpmn2.0#hasEventDefinitions"/>
                <owl:minQualifiedCardinality rdf:datatype="http://www.w3.org/2001/XMLSchema#nonNegativeInteger">0</owl:minQualifiedCardinality>
                <owl:onClass rdf:resource="http://www.wageneder.at/ontology/bpmn2.0#EventDefinition"/>
            </owl:Restriction>
        </rdfs:subClassOf>
        <rdfs:subClassOf>
            <owl:Restriction>
                <owl:onProperty rdf:resource="http://www.wageneder.at/ontology/bpmn2.0#hasInputSet"/>
                <owl:minQualifiedCardinality rdf:datatype="http://www.w3.org/2001/XMLSchema#nonNegativeInteger">0</owl:minQualifiedCardinality>
                <owl:onClass rdf:resource="http://www.wageneder.at/ontology/bpmn2.0#InputSet"/>
            </owl:Restriction>
        </rdfs:subClassOf>
        <rdfs:subClassOf>
            <owl:Restriction>
                <owl:onProperty rdf:resource="http://www.wageneder.at/ontology/bpmn2.0#hasEventDefinitions"/>
                <owl:maxQualifiedCardinality rdf:datatype="http://www.w3.org/2001/XMLSchema#nonNegativeInteger">1</owl:maxQualifiedCardinality>
                <owl:onClass rdf:resource="http://www.wageneder.at/ontology/bpmn2.0#EventDefinition"/>
            </owl:Restriction>
        </rdfs:subClassOf>
        <rdfs:subClassOf>
            <owl:Restriction>
                <owl:onProperty rdf:resource="http://www.wageneder.at/ontology/bpmn2.0#hasInputSet"/>
                <owl:maxQualifiedCardinality rdf:datatype="http://www.w3.org/2001/XMLSchema#nonNegativeInteger">1</owl:maxQualifiedCardinality>
                <owl:onClass rdf:resource="http://www.wageneder.at/ontology/bpmn2.0#InputSet"/>
            </owl:Restriction>
        </rdfs:subClassOf>
        <rdfs:comment>The ThrowEvent element inherits the attributes and model associations of Event element</rdfs:comment>
    </owl:Class>
    


    <!-- http://www.wageneder.at/ontology/bpmn2.0#TimerEventDefinition -->

    <owl:Class rdf:about="http://www.wageneder.at/ontology/bpmn2.0#TimerEventDefinition">
        <rdfs:subClassOf rdf:resource="http://www.wageneder.at/ontology/bpmn2.0#EventDefinition"/>
        <rdfs:subClassOf>
            <owl:Restriction>
                <owl:onProperty rdf:resource="http://www.wageneder.at/ontology/bpmn2.0#hasTimeCycle"/>
                <owl:minQualifiedCardinality rdf:datatype="http://www.w3.org/2001/XMLSchema#nonNegativeInteger">0</owl:minQualifiedCardinality>
                <owl:onClass rdf:resource="http://www.wageneder.at/ontology/bpmn2.0#Expression"/>
            </owl:Restriction>
        </rdfs:subClassOf>
        <rdfs:subClassOf>
            <owl:Restriction>
                <owl:onProperty rdf:resource="http://www.wageneder.at/ontology/bpmn2.0#hasTimeDate"/>
                <owl:minQualifiedCardinality rdf:datatype="http://www.w3.org/2001/XMLSchema#nonNegativeInteger">0</owl:minQualifiedCardinality>
                <owl:onClass rdf:resource="http://www.wageneder.at/ontology/bpmn2.0#Expression"/>
            </owl:Restriction>
        </rdfs:subClassOf>
        <rdfs:subClassOf>
            <owl:Restriction>
                <owl:onProperty rdf:resource="http://www.wageneder.at/ontology/bpmn2.0#hasTimeDuration"/>
                <owl:minQualifiedCardinality rdf:datatype="http://www.w3.org/2001/XMLSchema#nonNegativeInteger">0</owl:minQualifiedCardinality>
                <owl:onClass rdf:resource="http://www.wageneder.at/ontology/bpmn2.0#Expression"/>
            </owl:Restriction>
        </rdfs:subClassOf>
        <rdfs:subClassOf>
            <owl:Restriction>
                <owl:onProperty rdf:resource="http://www.wageneder.at/ontology/bpmn2.0#hasTimeCycle"/>
                <owl:maxQualifiedCardinality rdf:datatype="http://www.w3.org/2001/XMLSchema#nonNegativeInteger">1</owl:maxQualifiedCardinality>
                <owl:onClass rdf:resource="http://www.wageneder.at/ontology/bpmn2.0#Expression"/>
            </owl:Restriction>
        </rdfs:subClassOf>
        <rdfs:subClassOf>
            <owl:Restriction>
                <owl:onProperty rdf:resource="http://www.wageneder.at/ontology/bpmn2.0#hasTimeDate"/>
                <owl:maxQualifiedCardinality rdf:datatype="http://www.w3.org/2001/XMLSchema#nonNegativeInteger">1</owl:maxQualifiedCardinality>
                <owl:onClass rdf:resource="http://www.wageneder.at/ontology/bpmn2.0#Expression"/>
            </owl:Restriction>
        </rdfs:subClassOf>
        <rdfs:subClassOf>
            <owl:Restriction>
                <owl:onProperty rdf:resource="http://www.wageneder.at/ontology/bpmn2.0#hasTimeDuration"/>
                <owl:maxQualifiedCardinality rdf:datatype="http://www.w3.org/2001/XMLSchema#nonNegativeInteger">1</owl:maxQualifiedCardinality>
                <owl:onClass rdf:resource="http://www.wageneder.at/ontology/bpmn2.0#Expression"/>
            </owl:Restriction>
        </rdfs:subClassOf>
        <rdfs:comment>The TimerEventDefinition element inherits the attributes and model associations of BaseElement through its relationship to the EventDefinition element</rdfs:comment>
    </owl:Class>
    


    <!-- http://www.wageneder.at/ontology/bpmn2.0#Transaction -->

    <owl:Class rdf:about="http://www.wageneder.at/ontology/bpmn2.0#Transaction">
        <rdfs:subClassOf rdf:resource="http://www.wageneder.at/ontology/bpmn2.0#SubProcess"/>
        <rdfs:subClassOf>
            <owl:Restriction>
                <owl:onProperty rdf:resource="http://www.wageneder.at/ontology/bpmn2.0#hasMethod"/>
                <owl:qualifiedCardinality rdf:datatype="http://www.w3.org/2001/XMLSchema#nonNegativeInteger">1</owl:qualifiedCardinality>
                <owl:onClass rdf:resource="http://www.wageneder.at/ontology/bpmn2.0#Transaction"/>
            </owl:Restriction>
        </rdfs:subClassOf>
        <rdfs:subClassOf>
            <owl:Restriction>
                <owl:onProperty rdf:resource="http://www.wageneder.at/ontology/bpmn2.0#protocol"/>
                <owl:qualifiedCardinality rdf:datatype="http://www.w3.org/2001/XMLSchema#nonNegativeInteger">1</owl:qualifiedCardinality>
                <owl:onDataRange rdf:resource="http://www.w3.org/2001/XMLSchema#string"/>
            </owl:Restriction>
        </rdfs:subClassOf>
        <rdfs:comment>A Transaction is a specialized type of Sub-Process that will have a special behavior that is controlled through a transaction protocol (such as WS-Transaction).</rdfs:comment>
    </owl:Class>
    


    <!-- http://www.wageneder.at/ontology/bpmn2.0#Unspecified -->

    <owl:Class rdf:about="http://www.wageneder.at/ontology/bpmn2.0#Unspecified">
        <rdfs:subClassOf rdf:resource="http://www.wageneder.at/ontology/bpmn2.0#GatewayDirection"/>
        <rdfs:comment>Unspecified: There are no constraints. The Gateway MAY have any number of incoming and outgoing Sequence Flows.</rdfs:comment>
    </owl:Class>
    


    <!-- http://www.wageneder.at/ontology/bpmn2.0#UserTask -->

    <owl:Class rdf:about="http://www.wageneder.at/ontology/bpmn2.0#UserTask">
        <rdfs:subClassOf rdf:resource="http://www.wageneder.at/ontology/bpmn2.0#HumanInteractionLevel"/>
        <rdfs:subClassOf rdf:resource="http://www.wageneder.at/ontology/bpmn2.0#Task"/>
        <rdfs:subClassOf>
            <owl:Restriction>
                <owl:onProperty rdf:resource="http://www.wageneder.at/ontology/bpmn2.0#hasRenderings"/>
                <owl:minQualifiedCardinality rdf:datatype="http://www.w3.org/2001/XMLSchema#nonNegativeInteger">0</owl:minQualifiedCardinality>
                <owl:onClass rdf:resource="http://www.wageneder.at/ontology/bpmn2.0#UserTask"/>
            </owl:Restriction>
        </rdfs:subClassOf>
        <rdfs:subClassOf>
            <owl:Restriction>
                <owl:onProperty rdf:resource="http://www.wageneder.at/ontology/bpmn2.0#actualOwner"/>
                <owl:qualifiedCardinality rdf:datatype="http://www.w3.org/2001/XMLSchema#nonNegativeInteger">1</owl:qualifiedCardinality>
                <owl:onDataRange rdf:resource="http://www.w3.org/2001/XMLSchema#string"/>
            </owl:Restriction>
        </rdfs:subClassOf>
        <rdfs:subClassOf>
            <owl:Restriction>
                <owl:onProperty rdf:resource="http://www.wageneder.at/ontology/bpmn2.0#implementation"/>
                <owl:qualifiedCardinality rdf:datatype="http://www.w3.org/2001/XMLSchema#nonNegativeInteger">1</owl:qualifiedCardinality>
                <owl:onDataRange rdf:resource="http://www.w3.org/2001/XMLSchema#string"/>
            </owl:Restriction>
        </rdfs:subClassOf>
        <rdfs:subClassOf>
            <owl:Restriction>
                <owl:onProperty rdf:resource="http://www.wageneder.at/ontology/bpmn2.0#taskPriority"/>
                <owl:qualifiedCardinality rdf:datatype="http://www.w3.org/2001/XMLSchema#nonNegativeInteger">1</owl:qualifiedCardinality>
                <owl:onDataRange rdf:resource="http://www.w3.org/2001/XMLSchema#integer"/>
            </owl:Restriction>
        </rdfs:subClassOf>
        <rdfs:comment>A User Task is a typical “workflow” Task where a human performer performs the Task with the assistance of a
software application and is scheduled through a task list manager of some sort.</rdfs:comment>
    </owl:Class>
    


    <!-- 
    ///////////////////////////////////////////////////////////////////////////////////////
    //
    // General axioms
    //
    ///////////////////////////////////////////////////////////////////////////////////////
     -->

    <rdf:Description>
        <rdf:type rdf:resource="http://www.w3.org/2002/07/owl#AllDisjointClasses"/>
        <owl:members rdf:parseType="Collection">
            <rdf:Description rdf:about="http://www.wageneder.at/ontology/bpmn2.0#Association"/>
            <rdf:Description rdf:about="http://www.wageneder.at/ontology/bpmn2.0#Group"/>
            <rdf:Description rdf:about="http://www.wageneder.at/ontology/bpmn2.0#TextAnnotation"/>
        </owl:members>
    </rdf:Description>
    <rdf:Description>
        <rdf:type rdf:resource="http://www.w3.org/2002/07/owl#AllDisjointClasses"/>
        <owl:members rdf:parseType="Collection">
            <rdf:Description rdf:about="http://www.wageneder.at/ontology/bpmn2.0#Backward"/>
            <rdf:Description rdf:about="http://www.wageneder.at/ontology/bpmn2.0#Both"/>
            <rdf:Description rdf:about="http://www.wageneder.at/ontology/bpmn2.0#Forward"/>
            <rdf:Description rdf:about="http://www.wageneder.at/ontology/bpmn2.0#None"/>
        </owl:members>
    </rdf:Description>
    <rdf:Description>
        <rdf:type rdf:resource="http://www.w3.org/2002/07/owl#AllDisjointClasses"/>
        <owl:members rdf:parseType="Collection">
            <rdf:Description rdf:about="http://www.wageneder.at/ontology/bpmn2.0#Both"/>
            <rdf:Description rdf:about="http://www.wageneder.at/ontology/bpmn2.0#None"/>
            <rdf:Description rdf:about="http://www.wageneder.at/ontology/bpmn2.0#One"/>
        </owl:members>
    </rdf:Description>
    <rdf:Description>
        <rdf:type rdf:resource="http://www.w3.org/2002/07/owl#AllDisjointClasses"/>
        <owl:members rdf:parseType="Collection">
            <rdf:Description rdf:about="http://www.wageneder.at/ontology/bpmn2.0#BoundaryEvent"/>
            <rdf:Description rdf:about="http://www.wageneder.at/ontology/bpmn2.0#IntermediateCatchEvent"/>
            <rdf:Description rdf:about="http://www.wageneder.at/ontology/bpmn2.0#StartEvent"/>
        </owl:members>
    </rdf:Description>
    <rdf:Description>
        <rdf:type rdf:resource="http://www.w3.org/2002/07/owl#AllDisjointClasses"/>
        <owl:members rdf:parseType="Collection">
            <rdf:Description rdf:about="http://www.wageneder.at/ontology/bpmn2.0#BusinessRuleTask"/>
            <rdf:Description rdf:about="http://www.wageneder.at/ontology/bpmn2.0#ManualTask"/>
            <rdf:Description rdf:about="http://www.wageneder.at/ontology/bpmn2.0#ReceiveTask"/>
            <rdf:Description rdf:about="http://www.wageneder.at/ontology/bpmn2.0#ScriptTask"/>
            <rdf:Description rdf:about="http://www.wageneder.at/ontology/bpmn2.0#SendTask"/>
            <rdf:Description rdf:about="http://www.wageneder.at/ontology/bpmn2.0#ServiceTask"/>
            <rdf:Description rdf:about="http://www.wageneder.at/ontology/bpmn2.0#UserTask"/>
        </owl:members>
    </rdf:Description>
    <rdf:Description>
        <rdf:type rdf:resource="http://www.w3.org/2002/07/owl#AllDisjointClasses"/>
        <owl:members rdf:parseType="Collection">
            <rdf:Description rdf:about="http://www.wageneder.at/ontology/bpmn2.0#CallActivity"/>
            <rdf:Description rdf:about="http://www.wageneder.at/ontology/bpmn2.0#SubProcess"/>
            <rdf:Description rdf:about="http://www.wageneder.at/ontology/bpmn2.0#Task"/>
        </owl:members>
    </rdf:Description>
    <rdf:Description>
        <rdf:type rdf:resource="http://www.w3.org/2002/07/owl#AllDisjointClasses"/>
        <owl:members rdf:parseType="Collection">
            <rdf:Description rdf:about="http://www.wageneder.at/ontology/bpmn2.0#CancelEventDefinition"/>
            <rdf:Description rdf:about="http://www.wageneder.at/ontology/bpmn2.0#CompensationEventDefinition"/>
            <rdf:Description rdf:about="http://www.wageneder.at/ontology/bpmn2.0#ConditionalEventDefinition"/>
            <rdf:Description rdf:about="http://www.wageneder.at/ontology/bpmn2.0#ErrorEventDefinition"/>
            <rdf:Description rdf:about="http://www.wageneder.at/ontology/bpmn2.0#EscalationEventDefinition"/>
            <rdf:Description rdf:about="http://www.wageneder.at/ontology/bpmn2.0#LinkEventDefinition"/>
            <rdf:Description rdf:about="http://www.wageneder.at/ontology/bpmn2.0#MessageEventDefinition"/>
            <rdf:Description rdf:about="http://www.wageneder.at/ontology/bpmn2.0#SignalEventDefinition"/>
            <rdf:Description rdf:about="http://www.wageneder.at/ontology/bpmn2.0#TerminateEventDefinition"/>
            <rdf:Description rdf:about="http://www.wageneder.at/ontology/bpmn2.0#TimerEventDefinition"/>
        </owl:members>
    </rdf:Description>
    <rdf:Description>
        <rdf:type rdf:resource="http://www.w3.org/2002/07/owl#AllDisjointClasses"/>
        <owl:members rdf:parseType="Collection">
            <rdf:Description rdf:about="http://www.wageneder.at/ontology/bpmn2.0#ComplexGateway"/>
            <rdf:Description rdf:about="http://www.wageneder.at/ontology/bpmn2.0#ExclusiveGateway"/>
            <rdf:Description rdf:about="http://www.wageneder.at/ontology/bpmn2.0#InclusiveGateway"/>
            <rdf:Description rdf:about="http://www.wageneder.at/ontology/bpmn2.0#ParallelGateway"/>
        </owl:members>
    </rdf:Description>
    <rdf:Description>
        <rdf:type rdf:resource="http://www.w3.org/2002/07/owl#AllDisjointClasses"/>
        <owl:members rdf:parseType="Collection">
            <rdf:Description rdf:about="http://www.wageneder.at/ontology/bpmn2.0#Converging"/>
            <rdf:Description rdf:about="http://www.wageneder.at/ontology/bpmn2.0#Diverging"/>
            <rdf:Description rdf:about="http://www.wageneder.at/ontology/bpmn2.0#Mixed"/>
            <rdf:Description rdf:about="http://www.wageneder.at/ontology/bpmn2.0#Unspecified"/>
        </owl:members>
    </rdf:Description>
    <rdf:Description>
        <rdf:type rdf:resource="http://www.w3.org/2002/07/owl#AllDisjointClasses"/>
        <owl:members rdf:parseType="Collection">
            <rdf:Description rdf:about="http://www.wageneder.at/ontology/bpmn2.0#EndEvent"/>
            <rdf:Description rdf:about="http://www.wageneder.at/ontology/bpmn2.0#ImplicitThrowEvent"/>
            <rdf:Description rdf:about="http://www.wageneder.at/ontology/bpmn2.0#IntermediateThrowEvent"/>
        </owl:members>
    </rdf:Description>
</rdf:RDF>



<!-- Generated by the OWL API (version 4.2.8.20170104-2310) https://github.com/owlcs/owlapi -->

